# baseURI: https://w3id.org/con-tax/zones/aat-spaces
# prefix: aat-spaces

@prefix : <https://w3id.org/con-tax/zones/aat-spaces#> .
@prefix aat: <http://vocab.getty.edu/aat/> .
@prefix aat-spaces: <https://w3id.org/con-tax/zones/aat-spaces#> .
@prefix bot: <https://w3id.org/bot#> .
@prefix cc: <http://creativecommons.org/ns#> .
@prefix contax: <https://w3id.org/con-tax#> .
@prefix dbr: <http://dbpedia.org/resource/> .
@prefix dct: <http://purl.org/dc/terms/> .
@prefix dcterms: <http://purl.org/dc/terms/> .
@prefix gvp: <http://vocab.getty.edu/ontology#> .
@prefix iso-thes: <http://purl.org/iso25964/skos-thes#> .
@prefix owl: <http://www.w3.org/2002/07/owl#> .
@prefix rdf: <http://www.w3.org/1999/02/22-rdf-syntax-ns#> .
@prefix rdfs: <http://www.w3.org/2000/01/rdf-schema#> .
@prefix schema: <http://schema.org/> .
@prefix skos: <http://www.w3.org/2004/02/skos/core#> .
@prefix vann: <http://purl.org/vocab/vann/> .
@prefix vcard: <http://www.w3.org/2006/vcard/ns#> .
@prefix voaf: <http://purl.org/vocommons/voaf#> .
@prefix wd: <http://www.wikidata.org/entity/> .
@prefix xl: <http://www.w3.org/2008/05/skos-xl#> .
@prefix xsd: <http://www.w3.org/2001/XMLSchema#> .

bot:Space
  rdf:type owl:Class ;
.
<https://w3id.org/con-tax/zones/aat-spaces>
  rdf:type voaf:Vocabulary ;
  rdf:type owl:Ontology ;
  cc:license <https://opendatacommons.org/licenses/by/1-0/> ;
  dcterms:creator [
      rdf:type vcard:Individual ;
      vcard:family-name "Bonduel" ;
      vcard:fn "Mathias Bonduel" ;
      vcard:given-name "Mathias" ;
      vcard:hasOrganizationName [
          rdf:type vcard:Organization ;
          owl:sameAs dbr:Katholieke_Universiteit_Leuven ;
          vcard:hasURL <https://www.kuleuven.be> ;
          vcard:organization-name "KU Leuven" ;
        ] ;
      vcard:hasURL <https://orcid.org/0000-0002-3313-924X> ;
      vcard:hasURL <https://www.kuleuven.be/wieiswie/nl/person/00110827> ;
      vcard:hasURL <https://www.researchgate.net/profile/Mathias_Bonduel> ;
    ] ;
  dcterms:description """A taxonomy of building spaces (extending bot:Space) derived from the Getty Art & Architecture Thesaurus (Getty AAT: https://www.getty.edu/research/tools/vocabularies/aat/about.html), v2020-07-29.

Note: Contains information from the J. Paul Getty Trust, Getty Research Institute, the Art & Architecture Thesaurus, which is made available under the ODC Attribution License."""@en ;
  dcterms:issued "2020-11-29"^^xsd:date ;
  dcterms:title "AAT-SPACES taxonomy"@en ;
  vann:preferredNamespacePrefix "aat-spaces" ;
  vann:preferredNamespaceUri "https://w3id.org/con-tax/zones/aat-spaces#" ;
  rdfs:comment "- Version 0.0.1: initial version"@en ;
  owl:versionInfo "0.0.1" ;
.
<https://w3id.org/con-tax/zones/aat-spaces#300002222>
  rdf:type owl:Class ;
  rdfs:comment "Apertures in the center of roofs of atriums in Roman houses, sloping inward to discharge rainwater into a cistern or tank, called an impluvium."@en ;
  rdfs:comment "Openingen in het midden van daken van atriums in romeinse huizen, die naar binnen hellen om regenwater door te geven naar een waterreservoir of tank, dat een impluvium wordt genoemd."@nl ;
  rdfs:isDefinedBy <https://w3id.org/con-tax/zones/aat-spaces> ;
  rdfs:label "compluvia"@en ;
  rdfs:label "compluvia"@nl ;
  rdfs:label "compluvium"@nl ;
  rdfs:seeAlso <http://vocab.getty.edu/aat/300002222> ;
  rdfs:seeAlso wd:Q868614 ;
  rdfs:subClassOf <https://w3id.org/con-tax/zones/aat-spaces#300004097> ;
.
<https://w3id.org/con-tax/zones/aat-spaces#300002588>
  rdf:type owl:Class ;
  rdfs:comment "Railed platforms projecting from the exterior walls of buildings. Use also for similar interior features, when small. For larger platforms which extend the length of one side of a room or are recessed behind an arcade, use \"galleries (upper level spaces).\""@en ;
  rdfs:comment "Wordt gebruikt voor platforms met hekwerk die zich aan de buitenkant van een gebouw bevinden. gebruik ook voor dergelijke constructies binnen gebouwen, wanneer deze klein zijn. Gebruik voor dergelijke constructies binnen gebouwen die ruimten met elkaar verbinden 'galerijen'. Gebruik 'loggia's' voor overdekte ruimten die aan één tot drie zijden naar buiten toe geopend zijn."@nl ;
  rdfs:isDefinedBy <https://w3id.org/con-tax/zones/aat-spaces> ;
  rdfs:label "balconies"@en ;
  rdfs:label "balkon"@nl ;
  rdfs:label "balkons"@nl ;
  rdfs:seeAlso <http://vocab.getty.edu/aat/300002588> ;
  rdfs:seeAlso wd:Q170552 ;
  rdfs:subClassOf <https://w3id.org/con-tax/zones/aat-spaces#300133704> ;
.
<https://w3id.org/con-tax/zones/aat-spaces#300002589>
  rdf:type owl:Class ;
  rdfs:comment "Gebruikt voor kleine balkons, met naar binnen openslaande vensterdeuren, meestal niet groot genoeg om op te staan en weinig meer dan een beschermende reling."@nl ;
  rdfs:comment "Very small balconies, usually not large enough to stand on and consisting of little more than a protective railing."@en ;
  rdfs:isDefinedBy <https://w3id.org/con-tax/zones/aat-spaces> ;
  rdfs:label "Frans balkon"@nl ;
  rdfs:label "Franse balkons"@nl ;
  rdfs:label "balconets"@en ;
  rdfs:seeAlso <http://vocab.getty.edu/aat/300002589> ;
  rdfs:subClassOf <https://w3id.org/con-tax/zones/aat-spaces#300002588> ;
.
<https://w3id.org/con-tax/zones/aat-spaces#300003781>
  rdf:type owl:Class ;
  rdfs:comment "Afgescheiden ruimten of kapellen waarin belangrijke relieken staan opgesteld, vaak direct achter het altaar. Geen Nederlands equivalent. Zie 'kapellen'."@nl ;
  rdfs:comment "Refers to shrines, often in the form of small chapels, situated behind the altar, where saints' relics are kept."@en ;
  rdfs:isDefinedBy <https://w3id.org/con-tax/zones/aat-spaces> ;
  rdfs:label "feretories"@en ;
  rdfs:label "relikwieënkastje"@nl ;
  rdfs:label "relikwieënkastjes"@nl ;
  rdfs:seeAlso <http://vocab.getty.edu/aat/300003781> ;
  rdfs:subClassOf <https://w3id.org/con-tax/zones/aat-spaces#300004560> ;
.
<https://w3id.org/con-tax/zones/aat-spaces#300004011>
  rdf:type gvp:GuideTerm ;
  rdfs:isDefinedBy <https://w3id.org/con-tax/zones/aat-spaces> ;
  rdfs:label "<kamers en ruimten naar locatie of context>"@nl ;
  rdfs:label "<rooms and spaces by location or context>"@en ;
  rdfs:label "kamers en ruimten naar locatie of context"@nl ;
  rdfs:seeAlso <http://vocab.getty.edu/aat/300004011> ;
  contax:containsConcept <https://w3id.org/con-tax/zones/aat-spaces#300075459> ;
  contax:containsConcept <https://w3id.org/con-tax/zones/aat-spaces#300078790> ;
.
<https://w3id.org/con-tax/zones/aat-spaces#300004013>
  rdf:type owl:Class ;
  rdfs:comment "Kamers of delen van kamers die een halfrond oppervlak hebben."@nl ;
  rdfs:comment "Rooms or divisions of rooms that are semicircular in plan."@en ;
  rdfs:isDefinedBy <https://w3id.org/con-tax/zones/aat-spaces> ;
  rdfs:label "hemicycles"@en ;
  rdfs:label "hemicycli"@nl ;
  rdfs:label "hemicyclus"@nl ;
  rdfs:seeAlso <http://vocab.getty.edu/aat/300004013> ;
  rdfs:seeAlso wd:Q2528224 ;
  rdfs:subClassOf <https://w3id.org/con-tax/zones/aat-spaces#300078790> ;
.
<https://w3id.org/con-tax/zones/aat-spaces#300004014>
  rdf:type owl:Class ;
  rdfs:comment "Enigszins afgescheiden ruimten, die meestal halfcirkelvormig zijn en zitplaatsen hebben. Voornamelijk in Romeinse architectuur."@nl ;
  rdfs:comment "Niches, recesses, or other sheltered spaces, often semicircular and lined with seats; primarily in Roman architecture."@en ;
  rdfs:isDefinedBy <https://w3id.org/con-tax/zones/aat-spaces> ;
  rdfs:label "exedra"@nl ;
  rdfs:label "exedrae (binnenruimten)"@nl ;
  rdfs:label "exedrae (interior spaces)"@en ;
  rdfs:label "exedrae"@nl ;
  rdfs:seeAlso <http://vocab.getty.edu/aat/300004014> ;
  rdfs:seeAlso wd:Q594648 ;
  rdfs:subClassOf <https://w3id.org/con-tax/zones/aat-spaces#300078790> ;
.
<https://w3id.org/con-tax/zones/aat-spaces#300004021>
  rdf:type gvp:GuideTerm ;
  rdfs:isDefinedBy <https://w3id.org/con-tax/zones/aat-spaces> ;
  rdfs:label "<kamers en ruimten naar functie>"@nl ;
  rdfs:label "<rooms and spaces by function>"@en ;
  rdfs:label "kamers en ruimten naar functie"@nl ;
  rdfs:seeAlso <http://vocab.getty.edu/aat/300004021> ;
  contax:containsConcept <https://w3id.org/con-tax/zones/aat-spaces#300004241> ;
  contax:containsConcept <https://w3id.org/con-tax/zones/aat-spaces#300004259> ;
  contax:containsConcept <https://w3id.org/con-tax/zones/aat-spaces#300004362> ;
  contax:containsConcept <https://w3id.org/con-tax/zones/aat-spaces#300004465> ;
  contax:containsConcept <https://w3id.org/con-tax/zones/aat-spaces#300075880> ;
  contax:containsConcept <https://w3id.org/con-tax/zones/aat-spaces#300075881> ;
  contax:containsConcept <https://w3id.org/con-tax/zones/aat-spaces#300103935> ;
  contax:containsConcept <https://w3id.org/con-tax/zones/aat-spaces#300103941> ;
  contax:containsConcept <https://w3id.org/con-tax/zones/aat-spaces#300432409> ;
  contax:containsGuideTerm <https://w3id.org/con-tax/zones/aat-spaces#300004189> ;
  contax:containsGuideTerm <https://w3id.org/con-tax/zones/aat-spaces#300004328> ;
  contax:containsGuideTerm <https://w3id.org/con-tax/zones/aat-spaces#300004332> ;
  contax:containsGuideTerm <https://w3id.org/con-tax/zones/aat-spaces#300004388> ;
  contax:containsGuideTerm <https://w3id.org/con-tax/zones/aat-spaces#300004505> ;
  contax:containsGuideTerm <https://w3id.org/con-tax/zones/aat-spaces#300075769> ;
  contax:containsGuideTerm <https://w3id.org/con-tax/zones/aat-spaces#300075809> ;
  contax:containsGuideTerm <https://w3id.org/con-tax/zones/aat-spaces#300081780> ;
.
<https://w3id.org/con-tax/zones/aat-spaces#300004026>
  rdf:type owl:Class ;
  rdfs:comment "Eenpersoonskamers in gebouwen met vele soortgelijke kamers, zoals in een klooster of een gevangenis."@nl ;
  rdfs:comment "Single rooms usually housing only one person within a building having numerous similar rooms, as in a convent or in a prison."@en ;
  rdfs:isDefinedBy <https://w3id.org/con-tax/zones/aat-spaces> ;
  rdfs:label "cel"@nl ;
  rdfs:label "cellen"@nl ;
  rdfs:label "cells (interior spaces)"@en ;
  rdfs:seeAlso <http://vocab.getty.edu/aat/300004026> ;
  rdfs:subClassOf <https://w3id.org/con-tax/zones/aat-spaces#300078790> ;
.
<https://w3id.org/con-tax/zones/aat-spaces#300004031>
  rdf:type owl:Class ;
  rdfs:comment "Overdekte, naar één kant open gangen doorgaans met zuilen en bogen, die buiten langs of door een gebouw lopen. Voor ruimten boven de zijbeuken in kerken, die geopend zijn naar het schip wordt 'tribunes (verdiepingen)' of 'triforia' gebruikt."@nl ;
  rdfs:comment "Substantial interior spaces at the level of an upper story that overlook the level below and usually extend the full length or width of a room. For railed platforms projecting from the exterior walls of buildings or small, similar interior features, use \"balconies.\" For floor levels in a church above the aisles and open to the nave, use \"tribunes (stories)\" or \"triforiums.\""@en ;
  rdfs:isDefinedBy <https://w3id.org/con-tax/zones/aat-spaces> ;
  rdfs:label "galerij"@nl ;
  rdfs:label "galerijen"@nl ;
  rdfs:label "galleries (upper level spaces)"@en ;
  rdfs:seeAlso <http://vocab.getty.edu/aat/300004031> ;
  rdfs:subClassOf <https://w3id.org/con-tax/zones/aat-spaces#300133704> ;
.
<https://w3id.org/con-tax/zones/aat-spaces#300004034>
  rdf:type owl:Class ;
  rdfs:comment "Galerijen of balkons voor muzikanten, zowel in seculaire als in religieuze gebouwen."@nl ;
  rdfs:comment "Galleries or balconies for players of musical instruments, whether in secular or religious buildings."@en ;
  rdfs:isDefinedBy <https://w3id.org/con-tax/zones/aat-spaces> ;
  rdfs:label "minstrel galleries"@en ;
  rdfs:label "minstrel galleries"@nl ;
  rdfs:label "minstrel gallery"@nl ;
  rdfs:seeAlso <http://vocab.getty.edu/aat/300004034> ;
  rdfs:seeAlso wd:Q4921857 ;
  rdfs:subClassOf <https://w3id.org/con-tax/zones/aat-spaces#300004031> ;
.
<https://w3id.org/con-tax/zones/aat-spaces#300004035>
  rdf:type owl:Class ;
  rdfs:comment "Galleries appropriated to a choir."@en ;
  rdfs:comment "Gallerijen bedoelt voor zangkoren."@nl ;
  rdfs:isDefinedBy <https://w3id.org/con-tax/zones/aat-spaces> ;
  rdfs:label "choir lofts"@en ;
  rdfs:label "zangerstribune"@nl ;
  rdfs:label "zangerstribunes"@nl ;
  rdfs:label "zangtribune"@nl ;
  rdfs:label "zangtribunes"@nl ;
  rdfs:seeAlso <http://vocab.getty.edu/aat/300004035> ;
  rdfs:seeAlso wd:Q26213933 ;
  rdfs:subClassOf <https://w3id.org/con-tax/zones/aat-spaces#300004031> ;
.
<https://w3id.org/con-tax/zones/aat-spaces#300004039>
  rdf:type owl:Class ;
  rdfs:comment "Galerijen of tribunes voor een orgel, vaak in een kerk."@nl ;
  rdfs:comment "Galleries or lofts in which an organ is located, often in a church and intended mainly for use by the organist and choir. It is often connected to the organ, with which it may form a single architectural-decorative structure.  In some regions, the organ loft is very large, often consisting of several superimposed levels, and is reserved for men attending Mass. It is usually made of wood or stone, supported by ledges with a parapet and sometimes grilles that conceal the members of the choir. It is usually located in the western portion of the nave, above the main entrance to the church, sometimes supported by the inner door. It may also be located in other parts of the nave, in the arms of the transept, or along the walls of the choir."@en ;
  rdfs:isDefinedBy <https://w3id.org/con-tax/zones/aat-spaces> ;
  rdfs:label "organ lofts"@en ;
  rdfs:label "orgelgalerij"@nl ;
  rdfs:label "orgelgalerijen"@nl ;
  rdfs:label "orgeltribune"@nl ;
  rdfs:label "orgeltribunes"@nl ;
  rdfs:seeAlso <http://vocab.getty.edu/aat/300004039> ;
  rdfs:subClassOf <https://w3id.org/con-tax/zones/aat-spaces#300004031> ;
.
<https://w3id.org/con-tax/zones/aat-spaces#300004042>
  rdf:type owl:Class ;
  rdfs:comment "Opslagruimten voor hooi op de bovenverdieping van stallen of schuren."@nl ;
  rdfs:comment "Upper-story storage spaces for hay in stables or barns."@en ;
  rdfs:isDefinedBy <https://w3id.org/con-tax/zones/aat-spaces> ;
  rdfs:label "haylofts"@en ;
  rdfs:label "hooischelven"@nl ;
  rdfs:label "hooizolder"@nl ;
  rdfs:label "hooizolders"@nl ;
  rdfs:seeAlso <http://vocab.getty.edu/aat/300004042> ;
  rdfs:seeAlso wd:Q4416269 ;
  rdfs:subClassOf <https://w3id.org/con-tax/zones/aat-spaces#300133704> ;
.
<https://w3id.org/con-tax/zones/aat-spaces#300004044>
  rdf:type owl:Class ;
  rdfs:comment "Benaming voor ruimten in gebouwen of andere constructies, volledig afgescheiden van de andere delen door middel van een vloer, plafond en muren of tussenschotten."@nl ;
  rdfs:comment "Refers to the interior portions of buildings or other structures fully separated and divided off from the other portions by a floor, ceiling, and walls or partitions."@en ;
  rdfs:isDefinedBy <https://w3id.org/con-tax/zones/aat-spaces> ;
  rdfs:label "kamer"@nl ;
  rdfs:label "kamers"@nl ;
  rdfs:label "rooms (interior spaces)"@en ;
  rdfs:seeAlso <http://vocab.getty.edu/aat/300004044> ;
  rdfs:seeAlso wd:Q180516 ;
  rdfs:subClassOf <https://w3id.org/con-tax/zones/aat-spaces#300078790> ;
.
<https://w3id.org/con-tax/zones/aat-spaces#300004048>
  rdf:type owl:Class ;
  rdfs:comment "Generally refers to large round rooms."@en ;
  rdfs:comment "Grote ronde kamers."@nl ;
  rdfs:isDefinedBy <https://w3id.org/con-tax/zones/aat-spaces> ;
  rdfs:label "rotonde (binnenruimte)"@nl ;
  rdfs:label "rotonde"@nl ;
  rdfs:label "rotonden (binnenruimten)"@nl ;
  rdfs:label "rotonden"@nl ;
  rdfs:label "rotundas (interior spaces)"@en ;
  rdfs:seeAlso <http://vocab.getty.edu/aat/300004048> ;
  rdfs:subClassOf <https://w3id.org/con-tax/zones/aat-spaces#300078790> ;
.
<https://w3id.org/con-tax/zones/aat-spaces#300004050>
  rdf:type owl:Class ;
  rdfs:comment "Successions of connected rooms, generally on one floor, that are occupied as one unit."@en ;
  rdfs:comment "Twee of meer ineenlopende kamers, meestal op dezelfde verdieping, die als een eenheid worden bewoond. Toevoeging: meestal met grote vleugel- of schuifdeuren ertussen."@nl ;
  rdfs:isDefinedBy <https://w3id.org/con-tax/zones/aat-spaces> ;
  rdfs:label "kamers en suite"@nl ;
  rdfs:label "suite (samenstel van kamers)"@nl ;
  rdfs:label "suite"@nl ;
  rdfs:label "suites (rooms)"@en ;
  rdfs:label "suites (samenstel van kamers)"@nl ;
  rdfs:label "suites"@nl ;
  rdfs:seeAlso <http://vocab.getty.edu/aat/300004050> ;
  rdfs:subClassOf <https://w3id.org/con-tax/zones/aat-spaces#300075458> ;
.
<https://w3id.org/con-tax/zones/aat-spaces#300004053>
  rdf:type gvp:GuideTerm ;
  rdfs:isDefinedBy <https://w3id.org/con-tax/zones/aat-spaces> ;
  rdfs:label "<kamers en ruimten naar vorm>"@nl ;
  rdfs:label "<rooms and spaces by form>"@en ;
  rdfs:label "kamers en ruimten naar vorm"@nl ;
  rdfs:seeAlso <http://vocab.getty.edu/aat/300004053> ;
  contax:containsConcept <https://w3id.org/con-tax/zones/aat-spaces#300002588> ;
  contax:containsConcept <https://w3id.org/con-tax/zones/aat-spaces#300004031> ;
  contax:containsConcept <https://w3id.org/con-tax/zones/aat-spaces#300004054> ;
  contax:containsConcept <https://w3id.org/con-tax/zones/aat-spaces#300075460> ;
  contax:containsConcept <https://w3id.org/con-tax/zones/aat-spaces#300127475> ;
.
<https://w3id.org/con-tax/zones/aat-spaces#300004054>
  rdf:type owl:Class ;
  rdfs:comment "Use to designate small recessed spaces off of larger rooms."@en ;
  rdfs:comment "Wordt gebruikt voor kleine inspringende kleine ruimten van grotere kamers. Aanvulling: kleine vertrekjes grenzend aan een grotere kamer en daarvan met een deur of een gordijn afgescheiden, meestal zonder eigen uitgang en vensterlicht, gewoonlijk als slaapplaats ingericht. Gebruik 'nissen' voor uitsparingen in de dikte van muren, zodat het muurvlak op enige hoogte of breedte dieper ligt."@nl ;
  rdfs:isDefinedBy <https://w3id.org/con-tax/zones/aat-spaces> ;
  rdfs:label "alcoves"@en ;
  rdfs:label "alkoof"@nl ;
  rdfs:label "alkoven"@nl ;
  rdfs:seeAlso <http://vocab.getty.edu/aat/300004054> ;
  rdfs:subClassOf <https://w3id.org/con-tax/zones/aat-spaces#300133704> ;
.
<https://w3id.org/con-tax/zones/aat-spaces#300004055>
  rdf:type owl:Class ;
  rdfs:comment "Alcoves or small room openings off the atrium of an ancient Roman house."@en ;
  rdfs:comment "Alkoven of zijruimten van het atrium in antieke Romeinse huizen."@nl ;
  rdfs:isDefinedBy <https://w3id.org/con-tax/zones/aat-spaces> ;
  rdfs:label "ala"@nl ;
  rdfs:label "alae"@en ;
  rdfs:label "alae"@nl ;
  rdfs:seeAlso <http://vocab.getty.edu/aat/300004055> ;
  rdfs:subClassOf <https://w3id.org/con-tax/zones/aat-spaces#300004054> ;
.
<https://w3id.org/con-tax/zones/aat-spaces#300004058>
  rdf:type owl:Class ;
  rdfs:comment "Recessed seating areas by a fire or hearth."@en ;
  rdfs:comment "Ruimten met verzonken zitplaatsen bij een vuur of haard."@nl ;
  rdfs:isDefinedBy <https://w3id.org/con-tax/zones/aat-spaces> ;
  rdfs:label "haardplaats"@nl ;
  rdfs:label "haardplaatsen"@nl ;
  rdfs:label "inglenooks"@en ;
  rdfs:seeAlso <http://vocab.getty.edu/aat/300004058> ;
  rdfs:seeAlso wd:Q6032582 ;
  rdfs:subClassOf <https://w3id.org/con-tax/zones/aat-spaces#300004054> ;
.
<https://w3id.org/con-tax/zones/aat-spaces#300004063>
  rdf:type owl:Class ;
  rdfs:comment "Kamers of groepen kamers die als woning of als privé-woongedeelten worden gebruikt in huizen, hotels of in flatgebouwen."@nl ;
  rdfs:comment "Rooms or sets of rooms used as dwellings or private living quarters and located in houses, hotels, or within apartment houses."@en ;
  rdfs:isDefinedBy <https://w3id.org/con-tax/zones/aat-spaces> ;
  rdfs:label "apartments"@en ;
  rdfs:label "appartement"@nl ;
  rdfs:label "appartementen"@nl ;
  rdfs:seeAlso <http://vocab.getty.edu/aat/300004063> ;
  rdfs:seeAlso wd:Q188507 ;
  rdfs:subClassOf <https://w3id.org/con-tax/zones/aat-spaces#300075458> ;
.
<https://w3id.org/con-tax/zones/aat-spaces#300004064>
  rdf:type owl:Class ;
  rdfs:comment "One-floor apartments, usually modest, each having an outside entrance; may also be used for buildings having a small number of such units and usually dating from the late 19th or early 20th century. Generally American usage."@en ;
  rdfs:comment "Woningen, gewoonlijk bescheiden van omvang, waarvan alle vertrekken zich op één verdieping bevinden. Elke flat heeft een afzonderlijke buitendeur. De term kan ook worden gebruikt voor gebouwen met een zeker aantal van dergelijke woningen. De Engelse term dateert van het einde van de 19de of het begin van de 20ste eeuw."@nl ;
  rdfs:isDefinedBy <https://w3id.org/con-tax/zones/aat-spaces> ;
  rdfs:label "flat"@nl ;
  rdfs:label "flats (apartments)"@en ;
  rdfs:label "flats"@nl ;
  rdfs:seeAlso <http://vocab.getty.edu/aat/300004064> ;
  rdfs:seeAlso wd:Q188507 ;
  rdfs:subClassOf <https://w3id.org/con-tax/zones/aat-spaces#300004063> ;
.
<https://w3id.org/con-tax/zones/aat-spaces#300004071>
  rdf:type owl:Class ;
  rdfs:comment "Apartments containing one spacious room, often with large windows, which is or resembles an artist's studio, and serves as both a sitting area and a sleeping area, and with access to a separate bathroom and small kitchen."@en ;
  rdfs:comment "Eenkamerflats met keukentje en sanitaire voorzieningen."@nl ;
  rdfs:isDefinedBy <https://w3id.org/con-tax/zones/aat-spaces> ;
  rdfs:label "studio (appartement)"@nl ;
  rdfs:label "studio apartments"@en ;
  rdfs:label "studio"@nl ;
  rdfs:label "studio's (appartementen)"@nl ;
  rdfs:label "studio's"@nl ;
  rdfs:seeAlso <http://vocab.getty.edu/aat/300004071> ;
  rdfs:subClassOf <https://w3id.org/con-tax/zones/aat-spaces#300004063> ;
.
<https://w3id.org/con-tax/zones/aat-spaces#300004076>
  rdf:type owl:Class ;
  rdfs:comment "Enclosed spaces under sloping roofs, between the roof and the ceiling of the uppermost story, especially in houses, whether used for storage or habitation. For open platforms in houses set close to ceilings or for large spaces below the roofs of commercial buildings or warehouses, use \"lofts (upper level floors)\"."@en ;
  rdfs:comment "Wordt gebruikt voor afgesloten ruimten onder schuine daken, tussen het dak en het plafond van de bovenste verdieping, vooral in huizen. Ze kunnen zowel voor opslag als voor bewoning worden gebruikt. Voor open platforms in huizen, die zich dicht bij het plafond bevinden, of voor grote ruimten onder de daken van kantoren of pakhuizen wordt 'lofts' gebruikt."@nl ;
  rdfs:isDefinedBy <https://w3id.org/con-tax/zones/aat-spaces> ;
  rdfs:label "attics (interior spaces)"@en-us ;
  rdfs:label "zolder"@nl ;
  rdfs:label "zolders"@nl ;
  rdfs:seeAlso <http://vocab.getty.edu/aat/300004076> ;
  rdfs:subClassOf <https://w3id.org/con-tax/zones/aat-spaces#300078790> ;
.
<https://w3id.org/con-tax/zones/aat-spaces#300004086>
  rdf:type owl:Class ;
  rdfs:comment "Kleine ruimten bedoeld voor specifieke doeleinden. Zie voor handelsoptrekjes 'stalletjes'."@nl ;
  rdfs:comment "Small enclosures or stands, permanent or temporary, and freestanding or not, used for selling goods or to afford privacy to their occupants."@en ;
  rdfs:isDefinedBy <https://w3id.org/con-tax/zones/aat-spaces> ;
  rdfs:label "booths"@en ;
  rdfs:label "cabine"@nl ;
  rdfs:label "cabines (binnenruimten)"@nl ;
  rdfs:label "cabines"@nl ;
  rdfs:seeAlso <http://vocab.getty.edu/aat/300004086> ;
  rdfs:subClassOf <https://w3id.org/con-tax/zones/aat-spaces#300078790> ;
.
<https://w3id.org/con-tax/zones/aat-spaces#300004087>
  rdf:type owl:Class ;
  rdfs:comment "Booths where art works or goods are exhibited or sold."@en ;
  rdfs:isDefinedBy <https://w3id.org/con-tax/zones/aat-spaces> ;
  rdfs:label "exhibition booths"@en ;
  rdfs:label "verkoopstalletje"@nl ;
  rdfs:label "verkoopstalletjes"@nl ;
  rdfs:seeAlso <http://vocab.getty.edu/aat/300004087> ;
  rdfs:subClassOf <https://w3id.org/con-tax/zones/aat-spaces#300004086> ;
.
<https://w3id.org/con-tax/zones/aat-spaces#300004088>
  rdf:type owl:Class ;
  rdfs:comment "Rooms or other areas, above or below ground, that are reserved for burial, generally intended to accomodate one or a small number of bodies."@en ;
  rdfs:isDefinedBy <https://w3id.org/con-tax/zones/aat-spaces> ;
  rdfs:label "burial chambers"@en ;
  rdfs:label "grafkamer"@nl ;
  rdfs:label "grafkamers"@nl ;
  rdfs:seeAlso <http://vocab.getty.edu/aat/300004088> ;
  rdfs:seeAlso wd:Q358316 ;
  rdfs:subClassOf <https://w3id.org/con-tax/zones/aat-spaces#300075882> ;
.
<https://w3id.org/con-tax/zones/aat-spaces#300004090>
  rdf:type owl:Class ;
  rdfs:comment "Overdekte stallingen voor auto's, vaak zonder muren, is gewoonlijk in of aan een groter gebouw gekoppeld."@nl ;
  rdfs:comment "Roofed shelters for automobiles, often without walls; usually associated with or projecting from a separate building."@en ;
  rdfs:isDefinedBy <https://w3id.org/con-tax/zones/aat-spaces> ;
  rdfs:label "carport"@nl ;
  rdfs:label "carports"@en ;
  rdfs:label "carports"@nl ;
  rdfs:seeAlso <http://vocab.getty.edu/aat/300004090> ;
  rdfs:seeAlso wd:Q1044817 ;
  rdfs:subClassOf <https://w3id.org/con-tax/zones/aat-spaces#300075459> ;
.
<https://w3id.org/con-tax/zones/aat-spaces#300004095>
  rdf:type owl:Class ;
  rdfs:comment "Niet-overdekte ruimten, die geheel of gedeeltelijk worden omsloten door de muren van een gebouw."@nl ;
  rdfs:comment "Uncovered areas, surrounded or partially surrounded by the walls of a building."@en ;
  rdfs:isDefinedBy <https://w3id.org/con-tax/zones/aat-spaces> ;
  rdfs:label "binnenplaats"@nl ;
  rdfs:label "binnenplaatsen"@nl ;
  rdfs:label "courtyards"@en-us ;
  rdfs:seeAlso <http://vocab.getty.edu/aat/300004095> ;
  rdfs:subClassOf <https://w3id.org/con-tax/zones/aat-spaces#300075460> ;
.
<https://w3id.org/con-tax/zones/aat-spaces#300004097>
  rdf:type owl:Class ;
  rdfs:comment "De centrale ruimten in Romeinse huizen, met een compluvium (opening in het dak) voor doorlating van regenwater en een impluvium (rechthoekig bassin) om het regenwater in op te vangen."@nl ;
  rdfs:comment "The main inner halls of Roman houses having a compluvium (opening in the roof) for rainwater and an impluvium (rectangular basin) to collect the water."@en ;
  rdfs:isDefinedBy <https://w3id.org/con-tax/zones/aat-spaces> ;
  rdfs:label "atrium (Romeinse binnenplaats)"@nl ;
  rdfs:label "atrium"@nl ;
  rdfs:label "atriums (Roman halls)"@en ;
  rdfs:label "atriums (Romeinse binnenplaatsen)"@nl ;
  rdfs:label "atriums"@nl ;
  rdfs:seeAlso <http://vocab.getty.edu/aat/300004097> ;
  rdfs:seeAlso wd:Q189265 ;
  rdfs:subClassOf <https://w3id.org/con-tax/zones/aat-spaces#300075460> ;
.
<https://w3id.org/con-tax/zones/aat-spaces#300004101>
  rdf:type owl:Class ;
  rdfs:comment "Antieke Romeinse binnenplaatsen met zuilengangen aan alle vier de zijden."@nl ;
  rdfs:comment "Enclosed Roman courtyards with porticoes on all four sides."@en ;
  rdfs:isDefinedBy <https://w3id.org/con-tax/zones/aat-spaces> ;
  rdfs:label "quadriportici"@en ;
  rdfs:label "quadriportici"@nl ;
  rdfs:label "quadriporticus"@nl ;
  rdfs:seeAlso <http://vocab.getty.edu/aat/300004101> ;
  rdfs:subClassOf <https://w3id.org/con-tax/zones/aat-spaces#300004095> ;
.
<https://w3id.org/con-tax/zones/aat-spaces#300004104>
  rdf:type owl:Class ;
  rdfs:comment "Courts forming an entrance plaza for a single building or several buildings in a group."@en ;
  rdfs:comment "Open ruimten, pleinen voor de hoofdingangen van gebouwen en aan twee of drie zijden door vleugels of armen omvat. VWB"@nl ;
  rdfs:isDefinedBy <https://w3id.org/con-tax/zones/aat-spaces> ;
  rdfs:label "forecourts"@en-us ;
  rdfs:label "voorplein"@nl ;
  rdfs:label "voorpleinen"@nl ;
  rdfs:seeAlso <http://vocab.getty.edu/aat/300004104> ;
  rdfs:subClassOf <https://w3id.org/con-tax/zones/aat-spaces#300004095> ;
.
<https://w3id.org/con-tax/zones/aat-spaces#300004108>
  rdf:type owl:Class ;
  rdfs:comment "Binnenplaatsen die voornamelijk dienen om licht en lucht toe te laten. Gebruik 'luchtschachten' voor smallere binnenplaatsen die voornamelijk dienen voor ventilatie. Gebruik 'lichtkokers' voor kokers die licht doorlaten voor lager gelegen ruimten."@nl ;
  rdfs:comment "Courts or recesses serving primarily to provide light or ventilation to windows along the walls; for very small courts used primarily for ventilation, use \"air shafts.\""@en ;
  rdfs:isDefinedBy <https://w3id.org/con-tax/zones/aat-spaces> ;
  rdfs:label "lichtschacht"@nl ;
  rdfs:label "lichtschachten"@nl ;
  rdfs:label "light courts"@en ;
  rdfs:seeAlso <http://vocab.getty.edu/aat/300004108> ;
  rdfs:subClassOf <https://w3id.org/con-tax/zones/aat-spaces#300004095> ;
.
<https://w3id.org/con-tax/zones/aat-spaces#300004113>
  rdf:type owl:Class ;
  rdfs:comment "Platte daken belegd met hout of metaal om als buitenruimte te gebruiken."@nl ;
  rdfs:comment "Uncovered wood or metal platforms, usually attached to structures and often raised off the ground or on rooftops."@en ;
  rdfs:isDefinedBy <https://w3id.org/con-tax/zones/aat-spaces> ;
  rdfs:label "dakterras (niet-overdekte ruimte)"@nl ;
  rdfs:label "dakterras"@nl ;
  rdfs:label "dakterrassen (niet-overdekte ruimtes)"@nl ;
  rdfs:label "dakterrassen"@nl ;
  rdfs:label "decks (uncovered spaces)"@en ;
  rdfs:seeAlso <http://vocab.getty.edu/aat/300004113> ;
  rdfs:seeAlso wd:Q2637989 ;
  rdfs:subClassOf <https://w3id.org/con-tax/zones/aat-spaces#300075460> ;
.
<https://w3id.org/con-tax/zones/aat-spaces#300004114>
  rdf:type owl:Class ;
  rdfs:comment "Decks or flat roofs intended for sunbathing."@en ;
  rdfs:comment "Terrassen om te zonnebaden."@nl ;
  rdfs:isDefinedBy <https://w3id.org/con-tax/zones/aat-spaces> ;
  rdfs:label "sun decks"@en ;
  rdfs:label "zonneterras"@nl ;
  rdfs:label "zonneterrassen"@nl ;
  rdfs:seeAlso <http://vocab.getty.edu/aat/300004114> ;
  rdfs:subClassOf <https://w3id.org/con-tax/zones/aat-spaces#300004113> ;
.
<https://w3id.org/con-tax/zones/aat-spaces#300004120>
  rdf:type owl:Class ;
  rdfs:comment "Rooms equipped with lockers, often having showers and toilets and sometimes used as dressing rooms, as in clubhouses and gymnasiums."@en ;
  rdfs:comment "Ruimten die zijn uitgerust met kastjes en vaak met douche en toilet om zich om te kleden, met name in sportaccomodaties en clubhuizen. Gebruik in het Nederlands liever de algemene term 'kleedkamers'."@nl ;
  rdfs:isDefinedBy <https://w3id.org/con-tax/zones/aat-spaces> ;
  rdfs:label "kleedlokaal"@nl ;
  rdfs:label "kleedlokalen"@nl ;
  rdfs:label "locker rooms"@en ;
  rdfs:seeAlso <http://vocab.getty.edu/aat/300004120> ;
  rdfs:seeAlso wd:Q1070054 ;
  rdfs:subClassOf <https://w3id.org/con-tax/zones/aat-spaces#300133704> ;
.
<https://w3id.org/con-tax/zones/aat-spaces#300004132>
  rdf:type owl:Class ;
  rdfs:comment "Overdekte, open bouwconstructies aan een huis, meestal aan de zonzijde."@nl ;
  rdfs:comment "Use to designate roofed spaces, open along two or more sides and adjunct to a building, commonly serving either to shelter an entrance or used as living space."@en ;
  rdfs:isDefinedBy <https://w3id.org/con-tax/zones/aat-spaces> ;
  rdfs:label "porches"@en-us ;
  rdfs:label "veranda"@nl ;
  rdfs:label "veranda's"@nl ;
  rdfs:seeAlso <http://vocab.getty.edu/aat/300004132> ;
  rdfs:seeAlso wd:Q816741 ;
  rdfs:subClassOf <https://w3id.org/con-tax/zones/aat-spaces#300075459> ;
.
<https://w3id.org/con-tax/zones/aat-spaces#300004136>
  rdf:type owl:Class ;
  rdfs:comment "Living spaces open in part to the outdoors."@en ;
  rdfs:comment "Woonruimten die voor een deel naar buiten toe open zijn."@nl ;
  rdfs:isDefinedBy <https://w3id.org/con-tax/zones/aat-spaces> ;
  rdfs:label "lanai"@nl ;
  rdfs:label "lanais"@en ;
  rdfs:label "lanais"@nl ;
  rdfs:seeAlso <http://vocab.getty.edu/aat/300004136> ;
  rdfs:seeAlso wd:Q6482869 ;
  rdfs:subClassOf <https://w3id.org/con-tax/zones/aat-spaces#300004435> ;
.
<https://w3id.org/con-tax/zones/aat-spaces#300004137>
  rdf:type owl:Class ;
  rdfs:comment "Covered, roomlike spaces, open to the outdoors usually through arcades or colonnades; may be contained within or adjacent to buildings."@en ;
  rdfs:comment "Overdekte ruimten in of aan gebouwen, die aan één tot drie zijden open zijn, waarbij het dak wordt gedragen door arcaturen of zuilenrijen."@nl ;
  rdfs:isDefinedBy <https://w3id.org/con-tax/zones/aat-spaces> ;
  rdfs:label "loggia"@nl ;
  rdfs:label "loggia's"@nl ;
  rdfs:label "loggias"@en ;
  rdfs:seeAlso <http://vocab.getty.edu/aat/300004137> ;
  rdfs:seeAlso wd:Q466544 ;
  rdfs:subClassOf <https://w3id.org/con-tax/zones/aat-spaces#300075459> ;
.
<https://w3id.org/con-tax/zones/aat-spaces#300004143>
  rdf:type owl:Class ;
  rdfs:comment "Overdekte buitenruimten, die voertuigen en passagiers beschutten bij de ingang van gebouwen."@nl ;
  rdfs:comment "Projecting roofs or porchlike structures that shelter vehicles and passengers at the entrances to buildings; also for short vehicular tunnels through buildings, sheltering an entrance."@en ;
  rdfs:isDefinedBy <https://w3id.org/con-tax/zones/aat-spaces> ;
  rdfs:label "koetspoorten"@nl ;
  rdfs:label "overdekte ingang"@nl ;
  rdfs:label "overdekte ingangen"@nl ;
  rdfs:label "porte-cochère"@nl ;
  rdfs:label "porte-cochères"@en ;
  rdfs:label "porte-cochères"@nl ;
  rdfs:seeAlso <http://vocab.getty.edu/aat/300004143> ;
  rdfs:seeAlso wd:Q2719092 ;
  rdfs:subClassOf <https://w3id.org/con-tax/zones/aat-spaces#300075459> ;
.
<https://w3id.org/con-tax/zones/aat-spaces#300004145>
  rdf:type owl:Class ;
  rdfs:comment "In- of aangebouwde portalen, die aan de straatzijde geheel open zijn en leiden naar de deur van een huis."@nl ;
  rdfs:comment "Roofed porchlike spaces, open along at least one side and usually associated with an entrance, supported by columns and often surmounted by a pediment; porticoes may project from the main building mass or be recessed in it."@en ;
  rdfs:isDefinedBy <https://w3id.org/con-tax/zones/aat-spaces> ;
  rdfs:label "porticoes"@en-us ;
  rdfs:label "portiek"@nl ;
  rdfs:label "portieken"@nl ;
  rdfs:seeAlso <http://vocab.getty.edu/aat/300004145> ;
  rdfs:seeAlso wd:Q185600 ;
  rdfs:subClassOf <https://w3id.org/con-tax/zones/aat-spaces#300075459> ;
.
<https://w3id.org/con-tax/zones/aat-spaces#300004152>
  rdf:type owl:Class ;
  rdfs:comment "Circular, projecting porticoes."@en ;
  rdfs:comment "Ronde, vooruitspringende portieken."@nl ;
  rdfs:isDefinedBy <https://w3id.org/con-tax/zones/aat-spaces> ;
  rdfs:label "cyrtostyle"@nl ;
  rdfs:label "cyrtostyles"@en ;
  rdfs:label "cyrtostyles"@nl ;
  rdfs:seeAlso <http://vocab.getty.edu/aat/300004152> ;
  rdfs:subClassOf <https://w3id.org/con-tax/zones/aat-spaces#300004145> ;
.
<https://w3id.org/con-tax/zones/aat-spaces#300004160>
  rdf:type owl:Class ;
  rdfs:comment "Meestal geplaveide kleine verandas, platformen of tredes bij de toegangsdeuren van huizen. Soms met palen, stangen of kettingen afgezet. Gebruik bordessen (trappen) voor de grotere getrapte toegangen tot aanzienlijke gebouwen."@nl ;
  rdfs:comment "Porches, platforms, entrance stairways, or small verandas at house doors."@en ;
  rdfs:isDefinedBy <https://w3id.org/con-tax/zones/aat-spaces> ;
  rdfs:label "bordes (stoep)"@nl ;
  rdfs:label "bordes"@nl ;
  rdfs:label "bordessen (stoepen)"@nl ;
  rdfs:label "bordessen"@nl ;
  rdfs:label "stoep (niet-overdekte ruimte)"@nl ;
  rdfs:label "stoep"@nl ;
  rdfs:label "stoepen (niet-overdekte ruimten)"@nl ;
  rdfs:label "stoepen"@nl ;
  rdfs:label "stoops (uncovered spaces)"@en ;
  rdfs:seeAlso <http://vocab.getty.edu/aat/300004160> ;
  rdfs:seeAlso wd:Q814853 ;
  rdfs:subClassOf <https://w3id.org/con-tax/zones/aat-spaces#300075460> ;
.
<https://w3id.org/con-tax/zones/aat-spaces#300004161>
  rdf:type owl:Class ;
  rdfs:comment "Bordessen waarvan de trap haaks op de deur staat."@nl ;
  rdfs:comment "High stoops making a quarter turn, reached by a flight of stairs along a building front."@en ;
  rdfs:isDefinedBy <https://w3id.org/con-tax/zones/aat-spaces> ;
  rdfs:label "box stoops"@en ;
  rdfs:label "hoekbordes"@nl ;
  rdfs:label "hoekbordessen"@nl ;
  rdfs:seeAlso <http://vocab.getty.edu/aat/300004161> ;
  rdfs:subClassOf <https://w3id.org/con-tax/zones/aat-spaces#300004160> ;
.
<https://w3id.org/con-tax/zones/aat-spaces#300004172>
  rdf:type owl:Class ;
  rdfs:comment "Afgeschoten ruimten voor stalling van dieren."@nl ;
  rdfs:comment "Divisions of stables or barns, each accommodating one animal."@en ;
  rdfs:isDefinedBy <https://w3id.org/con-tax/zones/aat-spaces> ;
  rdfs:label "hok (stalruimte)"@nl ;
  rdfs:label "hok"@nl ;
  rdfs:label "hokken (stalruimten)"@nl ;
  rdfs:label "hokken"@nl ;
  rdfs:label "stalls (stable spaces)"@en ;
  rdfs:seeAlso <http://vocab.getty.edu/aat/300004172> ;
  rdfs:subClassOf <https://w3id.org/con-tax/zones/aat-spaces#300133704> ;
.
<https://w3id.org/con-tax/zones/aat-spaces#300004173>
  rdf:type owl:Class ;
  rdfs:comment "Kleine, afgescheiden compartimenten, met name in bibliotheken, die worden gebruikt voor studie in relatieve privacy."@nl ;
  rdfs:comment "Small rooms, cubicles, alcoves, or enclosed study desks, such as in libraries, used for individual or semiprivate study."@en ;
  rdfs:isDefinedBy <https://w3id.org/con-tax/zones/aat-spaces> ;
  rdfs:label "carrels"@en ;
  rdfs:label "studeercel"@nl ;
  rdfs:label "studeercellen"@nl ;
  rdfs:label "studiecel"@nl ;
  rdfs:label "studiecellen"@nl ;
  rdfs:label "studienis"@nl ;
  rdfs:label "studienissen"@nl ;
  rdfs:seeAlso <http://vocab.getty.edu/aat/300004173> ;
  rdfs:seeAlso wd:Q456042 ;
  rdfs:subClassOf <https://w3id.org/con-tax/zones/aat-spaces#300133704> ;
.
<https://w3id.org/con-tax/zones/aat-spaces#300004179>
  rdf:type owl:Class ;
  rdfs:comment "Ruimten, open, halfopen of met glas, bedoeld om een maximale hoeveelheid zonlicht op te vangen."@nl ;
  rdfs:comment "Sunny rooms or balconies designed for exposure to the rays of the sun. In ancient Greek and Roman houses, solariums were open sunporches or apartments on the roofs of buildings. In modern usage, may also refer to rooms having large windows, particularly rooms provided for patients in hospitals or clinics."@en ;
  rdfs:isDefinedBy <https://w3id.org/con-tax/zones/aat-spaces> ;
  rdfs:label "solarium"@nl ;
  rdfs:label "solariums (building spaces)"@en ;
  rdfs:label "solariums"@nl ;
  rdfs:seeAlso <http://vocab.getty.edu/aat/300004179> ;
  rdfs:seeAlso wd:Q1791429 ;
  rdfs:subClassOf <https://w3id.org/con-tax/zones/aat-spaces#300078790> ;
.
<https://w3id.org/con-tax/zones/aat-spaces#300004180>
  rdf:type owl:Class ;
  rdfs:comment "Kamers gelegen tussen het atrium en het peristylium in oude Romeinse huizen."@nl ;
  rdfs:comment "Rooms located at the far end of the atriums in ancient Roman houses."@en ;
  rdfs:isDefinedBy <https://w3id.org/con-tax/zones/aat-spaces> ;
  rdfs:label "tablina"@en ;
  rdfs:label "tablina"@nl ;
  rdfs:label "tablinum"@nl ;
  rdfs:seeAlso <http://vocab.getty.edu/aat/300004180> ;
  rdfs:subClassOf <https://w3id.org/con-tax/zones/aat-spaces#300078790> ;
.
<https://w3id.org/con-tax/zones/aat-spaces#300004184>
  rdf:type owl:Class ;
  rdfs:comment "Gebruik voor geplaveide recreatieruimtes aangrenzend eigentijdse huizen en de geplaveide binnenplaatsen van Spaanse of gebouwen in Spaanse stijl."@nl ;
  rdfs:comment "Paved roofless areas of relatively small or medium size associated with architecture, such as a roofless recreation area adjoining a house or a roofless inner courtyard open to the sky of Spanish or Spanish-style buildings."@en ;
  rdfs:isDefinedBy <https://w3id.org/con-tax/zones/aat-spaces> ;
  rdfs:label "patio"@nl ;
  rdfs:label "patio's (recreation area)"@nl ;
  rdfs:label "patio's"@nl ;
  rdfs:label "patios (recreation areas)"@en ;
  rdfs:seeAlso <http://vocab.getty.edu/aat/300004184> ;
  rdfs:seeAlso wd:Q737988 ;
  rdfs:subClassOf <https://w3id.org/con-tax/zones/aat-spaces#300075460> ;
.
<https://w3id.org/con-tax/zones/aat-spaces#300004189>
  rdf:type gvp:GuideTerm ;
  rdfs:isDefinedBy <https://w3id.org/con-tax/zones/aat-spaces> ;
  rdfs:label "<bad-, kleed- en sanitairruimten>"@nl ;
  rdfs:label "<spaces for bath, dressing and sanitary uses>"@en ;
  rdfs:label "bad-, kleed- en sanitairruimten"@nl ;
  rdfs:seeAlso <http://vocab.getty.edu/aat/300004189> ;
  contax:containsConcept <https://w3id.org/con-tax/zones/aat-spaces#300004120> ;
  contax:containsConcept <https://w3id.org/con-tax/zones/aat-spaces#300004197> ;
  contax:containsConcept <https://w3id.org/con-tax/zones/aat-spaces#300004202> ;
  contax:containsConcept <https://w3id.org/con-tax/zones/aat-spaces#300004235> ;
  contax:containsConcept <https://w3id.org/con-tax/zones/aat-spaces#300004239> ;
  contax:containsConcept <https://w3id.org/con-tax/zones/aat-spaces#300004240> ;
  contax:containsConcept <https://w3id.org/con-tax/zones/aat-spaces#300004369> ;
  contax:containsConcept <https://w3id.org/con-tax/zones/aat-spaces#300008006> ;
  contax:containsConcept <https://w3id.org/con-tax/zones/aat-spaces#300080054> ;
  contax:containsConcept <https://w3id.org/con-tax/zones/aat-spaces#300081124> ;
  contax:containsConcept <https://w3id.org/con-tax/zones/aat-spaces#300081126> ;
  contax:containsConcept <https://w3id.org/con-tax/zones/aat-spaces#300190936> ;
.
<https://w3id.org/con-tax/zones/aat-spaces#300004197>
  rdf:type owl:Class ;
  rdfs:comment "Rooms containing a bathtub or shower, and usually a toilet and lavatory; for rooms containing only a toilet and lavatory, use \"lavatories (rooms);\" for public facilities containing toilets and lavatories, use \"rest rooms.\""@en ;
  rdfs:comment "Wordt gebruikt voor kamers waarin zich een badkuip of douche bevindt, en meestal een toilet of wastafel. Voor ruimten met alleen een toilet en wastafel wordt 'toiletten' gebruikt; voor openbare faciliteiten met toiletten en wastafels wordt  'toiletruimten' gebruikt."@nl ;
  rdfs:isDefinedBy <https://w3id.org/con-tax/zones/aat-spaces> ;
  rdfs:label "badkamer"@nl ;
  rdfs:label "badkamers"@nl ;
  rdfs:label "bathrooms"@en ;
  rdfs:seeAlso <http://vocab.getty.edu/aat/300004197> ;
  rdfs:seeAlso wd:Q190771 ;
  rdfs:subClassOf <https://w3id.org/con-tax/zones/aat-spaces#300133704> ;
.
<https://w3id.org/con-tax/zones/aat-spaces#300004202>
  rdf:type owl:Class ;
  rdfs:comment "Public facilities containing toilets and lavatories, such as are found in office buildings, schools, transportation facilities, and other nonresidential locations."@en ;
  rdfs:comment "Wordt gebruikt voor ruimten met w.c.'s en wastafels in gebouwen met een openbaar karakter."@nl ;
  rdfs:isDefinedBy <https://w3id.org/con-tax/zones/aat-spaces> ;
  rdfs:label "openbaar toilet (sanitairruimte)"@nl ;
  rdfs:label "openbaar toilet"@nl ;
  rdfs:label "openbare toiletten (sanitairruimten)"@nl ;
  rdfs:label "openbare toiletten"@nl ;
  rdfs:label "rest rooms"@en-us ;
  rdfs:seeAlso <http://vocab.getty.edu/aat/300004202> ;
  rdfs:subClassOf <https://w3id.org/con-tax/zones/aat-spaces#300133704> ;
.
<https://w3id.org/con-tax/zones/aat-spaces#300004203>
  rdf:type owl:Class ;
  rdfs:comment "De ruimten voor warme baden in Romeinse badhuizen."@nl ;
  rdfs:comment "The vapor baths or hot plunges in Roman baths."@en ;
  rdfs:isDefinedBy <https://w3id.org/con-tax/zones/aat-spaces> ;
  rdfs:label "caldaria"@en ;
  rdfs:label "caldaria"@nl ;
  rdfs:label "caldarium"@nl ;
  rdfs:seeAlso <http://vocab.getty.edu/aat/300004203> ;
  rdfs:seeAlso wd:Q1026403 ;
  rdfs:subClassOf <https://w3id.org/con-tax/zones/aat-spaces#300080054> ;
.
<https://w3id.org/con-tax/zones/aat-spaces#300004219>
  rdf:type owl:Class ;
  rdfs:comment "Hot air baths for inducing sweating; also such rooms in Roman baths."@en ;
  rdfs:comment "Zweetkamers in Romeinse badhuizen."@nl ;
  rdfs:isDefinedBy <https://w3id.org/con-tax/zones/aat-spaces> ;
  rdfs:label "sudatoria"@en ;
  rdfs:label "sudatoria"@nl ;
  rdfs:label "sudatorium"@nl ;
  rdfs:seeAlso <http://vocab.getty.edu/aat/300004219> ;
  rdfs:seeAlso wd:Q914762 ;
  rdfs:subClassOf <https://w3id.org/con-tax/zones/aat-spaces#300080054> ;
.
<https://w3id.org/con-tax/zones/aat-spaces#300004223>
  rdf:type owl:Class ;
  rdfs:comment "Dressing rooms in ancient Greek and Roman baths and palaestrae."@en ;
  rdfs:comment "Kleedkamers in oude Griekse en Romeinse badhuizen en palaestra."@nl ;
  rdfs:isDefinedBy <https://w3id.org/con-tax/zones/aat-spaces> ;
  rdfs:label "apoditeria"@nl ;
  rdfs:label "apoditerium"@nl ;
  rdfs:label "apodyteria"@en ;
  rdfs:seeAlso <http://vocab.getty.edu/aat/300004223> ;
  rdfs:subClassOf <https://w3id.org/con-tax/zones/aat-spaces#300080054> ;
.
<https://w3id.org/con-tax/zones/aat-spaces#300004231>
  rdf:type owl:Class ;
  rdfs:comment "In ancient Roman baths, spaces containing water of intermediate temperatures between the caldarium and the frigidarium."@en ;
  rdfs:comment "Ruimten met baden met lauw water in Romeinse badhuizen."@nl ;
  rdfs:isDefinedBy <https://w3id.org/con-tax/zones/aat-spaces> ;
  rdfs:label "tepidaria"@en ;
  rdfs:label "tepidaria"@nl ;
  rdfs:label "tepidarium"@nl ;
  rdfs:seeAlso <http://vocab.getty.edu/aat/300004231> ;
  rdfs:seeAlso wd:Q601970 ;
  rdfs:subClassOf <https://w3id.org/con-tax/zones/aat-spaces#300080054> ;
.
<https://w3id.org/con-tax/zones/aat-spaces#300004233>
  rdf:type owl:Class ;
  rdfs:comment "De ruimten voor koude baden in Romeinse badhuizen, soms met een koud stortbad."@nl ;
  rdfs:comment "The cold rooms of Roman baths, sometimes including a cold plunge."@en ;
  rdfs:isDefinedBy <https://w3id.org/con-tax/zones/aat-spaces> ;
  rdfs:label "frigidaria"@en ;
  rdfs:label "frigidaria"@nl ;
  rdfs:label "frigidarium"@nl ;
  rdfs:seeAlso <http://vocab.getty.edu/aat/300004233> ;
  rdfs:seeAlso wd:Q1142866 ;
  rdfs:subClassOf <https://w3id.org/con-tax/zones/aat-spaces#300080054> ;
.
<https://w3id.org/con-tax/zones/aat-spaces#300004235>
  rdf:type owl:Class ;
  rdfs:comment "Rooms for bathing in which steam is produced from water thrown on heated stones or other similar materials."@en ;
  rdfs:comment "Ruimten, waarin men een hete luchtbad kan nemen."@nl ;
  rdfs:isDefinedBy <https://w3id.org/con-tax/zones/aat-spaces> ;
  rdfs:label "sauna"@nl ;
  rdfs:label "sauna's"@nl ;
  rdfs:label "saunabad"@nl ;
  rdfs:label "saunabaden"@nl ;
  rdfs:label "saunas (spaces)"@en-us ;
  rdfs:seeAlso <http://vocab.getty.edu/aat/300004235> ;
  rdfs:seeAlso wd:Q57036 ;
  rdfs:subClassOf <https://w3id.org/con-tax/zones/aat-spaces#300133704> ;
.
<https://w3id.org/con-tax/zones/aat-spaces#300004239>
  rdf:type owl:Class ;
  rdfs:comment "Individual compartments or self-contained units having a single overhead perforated nozzle and accommodating one person."@en ;
  rdfs:comment "Wordt gebruikt voor afzonderlijke compartimenten of onafhankelijke eenheden, bedoeld voor één persoon om te douchen."@nl ;
  rdfs:isDefinedBy <https://w3id.org/con-tax/zones/aat-spaces> ;
  rdfs:label "douchecel"@nl ;
  rdfs:label "douchecellen"@nl ;
  rdfs:label "douchehok"@nl ;
  rdfs:label "douchehokken"@nl ;
  rdfs:label "shower stalls"@en-us ;
  rdfs:seeAlso <http://vocab.getty.edu/aat/300004239> ;
  rdfs:subClassOf <https://w3id.org/con-tax/zones/aat-spaces#300133704> ;
.
<https://w3id.org/con-tax/zones/aat-spaces#300004240>
  rdf:type owl:Class ;
  rdfs:comment "Rooms designed for or used to induce sweating by the occupants through the introduction of hot steam into the space, which is often located in a bath, spa, or gym."@en ;
  rdfs:isDefinedBy <https://w3id.org/con-tax/zones/aat-spaces> ;
  rdfs:label "steam rooms"@en ;
  rdfs:label "stoombadruimte"@nl ;
  rdfs:label "stoombadruimten"@nl ;
  rdfs:seeAlso <http://vocab.getty.edu/aat/300004240> ;
  rdfs:seeAlso wd:Q7605381 ;
  rdfs:subClassOf <https://w3id.org/con-tax/zones/aat-spaces#300133704> ;
.
<https://w3id.org/con-tax/zones/aat-spaces#300004241>
  rdf:type owl:Class ;
  rdfs:comment "Open spaces in rooms that allow for unencumbered movement within them. Circulation spaces can occupy a percentage of a room, or be constructed for the singular purpose of allowing free circulation. For outdoor pedestrian circulation pathways see terms collocated under \"walkways\"."@en ;
  rdfs:comment "Voor paden en wegen die zich buiten bevinden wordt verwezen naar de termen die zijn ondergebracht onder 'wandelwegen'."@nl ;
  rdfs:isDefinedBy <https://w3id.org/con-tax/zones/aat-spaces> ;
  rdfs:label "circulation spaces"@en ;
  rdfs:label "verbindingsruimte"@nl ;
  rdfs:label "verbindingsruimten"@nl ;
  rdfs:seeAlso <http://vocab.getty.edu/aat/300004241> ;
  rdfs:subClassOf <https://w3id.org/con-tax/zones/aat-spaces#300133704> ;
.
<https://w3id.org/con-tax/zones/aat-spaces#300004245>
  rdf:type owl:Class ;
  rdfs:comment "Airtight spaces permitting passage between spaces of different air pressures or qualities, or between underwater and air-filled spaces."@en ;
  rdfs:comment "Luchtdichte ruimten die doorgang verschaffen tussen ruimten met verschillende luchtdruk of luchtkwaliteit, of tussen ruimten onder water en met lucht gevulde ruimten."@nl ;
  rdfs:isDefinedBy <https://w3id.org/con-tax/zones/aat-spaces> ;
  rdfs:label "air locks (airtight spaces)"@en ;
  rdfs:label "luchtslot"@nl ;
  rdfs:label "luchtsloten"@nl ;
  rdfs:label "luchtsluis"@nl ;
  rdfs:label "luchtsluizen"@nl ;
  rdfs:seeAlso <http://vocab.getty.edu/aat/300004245> ;
  rdfs:seeAlso wd:Q594958 ;
  rdfs:subClassOf <https://w3id.org/con-tax/zones/aat-spaces#300133704> ;
.
<https://w3id.org/con-tax/zones/aat-spaces#300004246>
  rdf:type owl:Class ;
  rdfs:comment "Continuous recesses or grooves built into walls to receive pipes, ducts, and other elements."@en ;
  rdfs:comment "Wordt gebruikt voor uitsparingen in muren bedoeld voor buizen voor nutsvoorzieningen."@nl ;
  rdfs:isDefinedBy <https://w3id.org/con-tax/zones/aat-spaces> ;
  rdfs:label "chases (wall spaces)"@en ;
  rdfs:label "leidingsleuf"@nl ;
  rdfs:label "leidingsleuven"@nl ;
  rdfs:label "uitkapping"@nl ;
  rdfs:label "uitkappingen"@nl ;
  rdfs:seeAlso <http://vocab.getty.edu/aat/300004246> ;
  rdfs:seeAlso wd:Q28739986 ;
  rdfs:subClassOf <https://w3id.org/con-tax/zones/aat-spaces#300133704> ;
.
<https://w3id.org/con-tax/zones/aat-spaces#300004249>
  rdf:type owl:Class ;
  rdfs:comment "Hellende of verticale goten of schachten om goederen of materialen naar een lager niveau te vervoeren."@nl ;
  rdfs:comment "Inclined or vertical troughs or shafts, for conveying materials of any kind to a lower level."@en ;
  rdfs:isDefinedBy <https://w3id.org/con-tax/zones/aat-spaces> ;
  rdfs:label "chutes"@en ;
  rdfs:label "stortkoker"@nl ;
  rdfs:label "stortkokers"@nl ;
  rdfs:seeAlso <http://vocab.getty.edu/aat/300004249> ;
  rdfs:subClassOf <https://w3id.org/con-tax/zones/aat-spaces#300133704> ;
.
<https://w3id.org/con-tax/zones/aat-spaces#300004250>
  rdf:type owl:Class ;
  rdfs:comment "Sloping channels through which coal can descend, either on a small scale into the basement of a home or on a large scale in an industrial facility."@en ;
  rdfs:isDefinedBy <https://w3id.org/con-tax/zones/aat-spaces> ;
  rdfs:label "coal chutes"@en ;
  rdfs:label "kolengoot"@nl ;
  rdfs:label "kolengoten"@nl ;
  rdfs:label "kolentrechter"@nl ;
  rdfs:label "kolentrechters"@nl ;
  rdfs:seeAlso <http://vocab.getty.edu/aat/300004250> ;
  rdfs:subClassOf <https://w3id.org/con-tax/zones/aat-spaces#300004249> ;
.
<https://w3id.org/con-tax/zones/aat-spaces#300004251>
  rdf:type owl:Class ;
  rdfs:comment "Sloping channels for the transfer of clothes and linens requiring laundering from upper floors to laundry rooms located on lower floors, either in a home or commercial hotel."@en ;
  rdfs:isDefinedBy <https://w3id.org/con-tax/zones/aat-spaces> ;
  rdfs:label "laundry chutes"@en ;
  rdfs:label "wasgoedtrechter"@nl ;
  rdfs:label "wasgoedtrechters"@nl ;
  rdfs:seeAlso <http://vocab.getty.edu/aat/300004251> ;
  rdfs:subClassOf <https://w3id.org/con-tax/zones/aat-spaces#300004249> ;
.
<https://w3id.org/con-tax/zones/aat-spaces#300004253>
  rdf:type owl:Class ;
  rdfs:comment "Sloping channels used for transporting trash from upper floors to a lower floor of a building, where it is stored or removed."@en ;
  rdfs:isDefinedBy <https://w3id.org/con-tax/zones/aat-spaces> ;
  rdfs:label "refuse chutes"@en ;
  rdfs:label "vuilniskoker"@nl ;
  rdfs:label "vuilniskokers"@nl ;
  rdfs:label "vuilnisstortkoker"@nl ;
  rdfs:label "vuilnisstortkokers"@nl ;
  rdfs:seeAlso <http://vocab.getty.edu/aat/300004253> ;
  rdfs:subClassOf <https://w3id.org/con-tax/zones/aat-spaces#300004249> ;
.
<https://w3id.org/con-tax/zones/aat-spaces#300004254>
  rdf:type owl:Class ;
  rdfs:comment "Open ruimten of hallen waar menigten hoofdzakelijk bij toeval samenkomen, zoals pleinen, promenades en grote stationshallen."@nl ;
  rdfs:comment "Open spaces or halls where crowds may gather, especially by chance coming together, as in a large railroad station."@en ;
  rdfs:isDefinedBy <https://w3id.org/con-tax/zones/aat-spaces> ;
  rdfs:label "concourse"@nl ;
  rdfs:label "concourses"@en ;
  rdfs:label "concourses"@nl ;
  rdfs:seeAlso <http://vocab.getty.edu/aat/300004254> ;
  rdfs:subClassOf <https://w3id.org/con-tax/zones/aat-spaces#300004241> ;
.
<https://w3id.org/con-tax/zones/aat-spaces#300004257>
  rdf:type owl:Class ;
  rdfs:comment "Lage ruimten onder vloeren van gebouwen die toegang geven tot riolering, leidingen, bedrading en andere voorzieningen."@nl ;
  rdfs:comment "Small spaces provided in a building in order to be able to gain access to plumbing, wiring, and other equipment."@en ;
  rdfs:isDefinedBy <https://w3id.org/con-tax/zones/aat-spaces> ;
  rdfs:label "crawl spaces"@en ;
  rdfs:label "kruipruimte"@nl ;
  rdfs:label "kruipruimten"@nl ;
  rdfs:seeAlso <http://vocab.getty.edu/aat/300004257> ;
  rdfs:subClassOf <https://w3id.org/con-tax/zones/aat-spaces#300133704> ;
.
<https://w3id.org/con-tax/zones/aat-spaces#300004259>
  rdf:type owl:Class ;
  rdfs:comment "Components of structures used for entering. "@en ;
  rdfs:isDefinedBy <https://w3id.org/con-tax/zones/aat-spaces> ;
  rdfs:label "entrance spaces"@en ;
  rdfs:label "ingangsruimten"@nl ;
  rdfs:seeAlso <http://vocab.getty.edu/aat/300004259> ;
  rdfs:subClassOf <https://w3id.org/con-tax/zones/aat-spaces#300133704> ;
.
<https://w3id.org/con-tax/zones/aat-spaces#300004263>
  rdf:type owl:Class ;
  rdfs:comment "Passages or rooms just inside the entrance of a residence, but sometimes with a vestibule between it and the outdoors. Prefer \"lobbies\" for such spaces in larger public buildings."@en ;
  rdfs:comment "Wordt gebruikt voor ruimten direct achter de ingang van een gebouw, met soms nog een vestibule daarvoor. Voor dergelijke ruimten in openbare gebouwen wordt de voorkeur gegeven aan 'lobby's'."@nl ;
  rdfs:isDefinedBy <https://w3id.org/con-tax/zones/aat-spaces> ;
  rdfs:label "entrance halls"@en ;
  rdfs:label "hal (entree)"@nl ;
  rdfs:label "hal"@nl ;
  rdfs:label "hallen (entree)"@nl ;
  rdfs:label "hallen"@nl ;
  rdfs:label "ingangshal"@nl ;
  rdfs:label "ingangshallen"@nl ;
  rdfs:seeAlso <http://vocab.getty.edu/aat/300004263> ;
  rdfs:seeAlso wd:Q38382224 ;
  rdfs:subClassOf <https://w3id.org/con-tax/zones/aat-spaces#300004259> ;
.
<https://w3id.org/con-tax/zones/aat-spaces#300004264>
  rdf:type owl:Class ;
  rdfs:comment "Grote toegangsruimten, met name in hotels. Voor toegangsruimten in privéwoningen wordt 'hallen' gebruikt."@nl ;
  rdfs:comment "Large halls serving as entrance spaces in public buildings or as anterooms, especially to legislative chambers. For entrance spaces in private houses, use \"entrance halls.\""@en ;
  rdfs:isDefinedBy <https://w3id.org/con-tax/zones/aat-spaces> ;
  rdfs:label "lobbies"@en ;
  rdfs:label "lobby"@nl ;
  rdfs:label "lobby's"@nl ;
  rdfs:seeAlso <http://vocab.getty.edu/aat/300004264> ;
  rdfs:seeAlso wd:Q31948 ;
  rdfs:subClassOf <https://w3id.org/con-tax/zones/aat-spaces#300004259> ;
.
<https://w3id.org/con-tax/zones/aat-spaces#300004279>
  rdf:type owl:Class ;
  rdfs:comment "Areas specially equipped for loading and receiving items onto and from motor vehicles or railroad cars parked adjacent."@en ;
  rdfs:comment "Ingangsruimten, bedoeld voor het laden en lossen van goederen op en van motorvoertuigen of treinwagons die er voorgereden zijn."@nl ;
  rdfs:isDefinedBy <https://w3id.org/con-tax/zones/aat-spaces> ;
  rdfs:label "laadbordes"@nl ;
  rdfs:label "laadbordessen"@nl ;
  rdfs:label "laadperron"@nl ;
  rdfs:label "laadperrons"@nl ;
  rdfs:label "laadplatforms"@nl ;
  rdfs:label "loading docks"@en ;
  rdfs:seeAlso <http://vocab.getty.edu/aat/300004279> ;
  rdfs:seeAlso wd:Q1799919 ;
  rdfs:subClassOf <https://w3id.org/con-tax/zones/aat-spaces#300004259> ;
.
<https://w3id.org/con-tax/zones/aat-spaces#300004281>
  rdf:type owl:Class ;
  rdfs:comment "Vestibules of andere ingangsruimten waar natte en modderige kleding of schoeisel kan worden uitgetrokken alvorens het huis te betreden. Geen Nederlands equivalent, gebruik 'vestibules'."@nl ;
  rdfs:comment "Vestibules or other peripheral spaces of houses in which wet and muddy clothes or footwear can be removed prior to entering the house."@en ;
  rdfs:isDefinedBy <https://w3id.org/con-tax/zones/aat-spaces> ;
  rdfs:label "mud room"@nl ;
  rdfs:label "mud rooms"@en ;
  rdfs:label "mud rooms"@nl ;
  rdfs:seeAlso <http://vocab.getty.edu/aat/300004281> ;
  rdfs:subClassOf <https://w3id.org/con-tax/zones/aat-spaces#300004259> ;
.
<https://w3id.org/con-tax/zones/aat-spaces#300004283>
  rdf:type owl:Class ;
  rdfs:comment "Relatief smalle binnenruimten die zijn ontworpen om toegang te verschaffen tot andere ruimten."@nl ;
  rdfs:comment "Relatively narrow spaces designed to provide access; usually interior spaces."@en ;
  rdfs:isDefinedBy <https://w3id.org/con-tax/zones/aat-spaces> ;
  rdfs:label "doorgang"@nl ;
  rdfs:label "doorgangen"@nl ;
  rdfs:label "passages (circulation spaces)"@en ;
  rdfs:seeAlso <http://vocab.getty.edu/aat/300004283> ;
  rdfs:subClassOf <https://w3id.org/con-tax/zones/aat-spaces#300004241> ;
.
<https://w3id.org/con-tax/zones/aat-spaces#300004284>
  rdf:type owl:Class ;
  rdfs:comment "Doorgangen tussen groepen zitplaatsen."@nl ;
  rdfs:comment "Includes both passages between sections of seats and the side divisions of buildings where the interior is divided into parts by columns or piers."@en ;
  rdfs:isDefinedBy <https://w3id.org/con-tax/zones/aat-spaces> ;
  rdfs:label "aisles"@en ;
  rdfs:label "gangpad"@nl ;
  rdfs:label "gangpaden"@nl ;
  rdfs:seeAlso <http://vocab.getty.edu/aat/300004284> ;
  rdfs:seeAlso wd:Q939723 ;
  rdfs:subClassOf <https://w3id.org/con-tax/zones/aat-spaces#300004241> ;
  rdfs:subClassOf <https://w3id.org/con-tax/zones/aat-spaces#300004560> ;
.
<https://w3id.org/con-tax/zones/aat-spaces#300004294>
  rdf:type owl:Class ;
  rdfs:comment "Doorgangen die toegang verschaffen tot de kamers van een gebouw."@nl ;
  rdfs:comment "Passages affording access and entrance to the rooms of a building."@en ;
  rdfs:isDefinedBy <https://w3id.org/con-tax/zones/aat-spaces> ;
  rdfs:label "corridors"@en ;
  rdfs:label "gang"@nl ;
  rdfs:label "gangen"@nl ;
  rdfs:seeAlso <http://vocab.getty.edu/aat/300004294> ;
  rdfs:seeAlso wd:Q1135449 ;
  rdfs:subClassOf <https://w3id.org/con-tax/zones/aat-spaces#300004283> ;
.
<https://w3id.org/con-tax/zones/aat-spaces#300004295>
  rdf:type owl:Class ;
  rdfs:comment "Corridors or galleries in Roman architecture with windowlike openings, whether subterranean or above ground."@en ;
  rdfs:comment "Overdekte gangen of galerijen in de Romeinse architectuur."@nl ;
  rdfs:isDefinedBy <https://w3id.org/con-tax/zones/aat-spaces> ;
  rdfs:label "cryptoportici"@en ;
  rdfs:label "cryptoportici"@nl ;
  rdfs:label "cryptoporticus"@nl ;
  rdfs:seeAlso <http://vocab.getty.edu/aat/300004295> ;
  rdfs:seeAlso wd:Q660398 ;
  rdfs:subClassOf <https://w3id.org/con-tax/zones/aat-spaces#300004283> ;
.
<https://w3id.org/con-tax/zones/aat-spaces#300004296>
  rdf:type owl:Class ;
  rdfs:comment "Lage booggangen onder langs daken van hoge gebouwen, bestaande uit een reeks van bogen op korte vrijstaande zuiltjes. Wordt aangetroffen in de Romaanse architectuur in Noord-Italië en het Rijnland."@nl ;
  rdfs:comment "Passageways through the exterior walls of buildings and open to the outside through small-scale or slender arcades; found in Italian and German Romanesque architecture."@en ;
  rdfs:isDefinedBy <https://w3id.org/con-tax/zones/aat-spaces> ;
  rdfs:label "dwarf galleries"@en ;
  rdfs:label "dwerggalerij"@nl ;
  rdfs:label "dwerggalerijen"@nl ;
  rdfs:seeAlso <http://vocab.getty.edu/aat/300004296> ;
  rdfs:seeAlso wd:Q244148 ;
  rdfs:subClassOf <https://w3id.org/con-tax/zones/aat-spaces#300004283> ;
.
<https://w3id.org/con-tax/zones/aat-spaces#300004298>
  rdf:type owl:Class ;
  rdfs:comment "Ancient Roman entrance passages leading from the street into buildings, usually houses."@en ;
  rdfs:comment "Doorgangen die van de straat in gebouwen (meestal huizen) leiden in de Romeinse architectuur."@nl ;
  rdfs:isDefinedBy <https://w3id.org/con-tax/zones/aat-spaces> ;
  rdfs:label "fauces"@en ;
  rdfs:label "fauces"@nl ;
  rdfs:seeAlso <http://vocab.getty.edu/aat/300004298> ;
  rdfs:seeAlso wd:Q1398341 ;
  rdfs:subClassOf <https://w3id.org/con-tax/zones/aat-spaces#300004283> ;
.
<https://w3id.org/con-tax/zones/aat-spaces#300004307>
  rdf:type owl:Class ;
  rdfs:comment "Passageways between the walls of the cella of a classical temple and the columns of the peristyle."@en ;
  rdfs:comment "Zuilengangen langs de zijkanten van antieke tempels. DEB"@nl ;
  rdfs:isDefinedBy <https://w3id.org/con-tax/zones/aat-spaces> ;
  rdfs:label "pteroma"@nl ;
  rdfs:label "pteromata"@en ;
  rdfs:label "pteron"@nl ;
  rdfs:seeAlso <http://vocab.getty.edu/aat/300004307> ;
  rdfs:subClassOf <https://w3id.org/con-tax/zones/aat-spaces#300004651> ;
.
<https://w3id.org/con-tax/zones/aat-spaces#300004314>
  rdf:type owl:Class ;
  rdfs:comment "In Medieval halls, the spaces between the screens (which act as visual barriers) and the doors to the service rooms (buttery, kitchen, pantry)."@en ;
  rdfs:comment "Ruimten tussen de kamerschermen (die als visuele obstakels dienen) en de deuren naar de dienstvertrekken (provisiekamer, keuken, voorraadkamer) in Middeleeuwse zalen."@nl ;
  rdfs:isDefinedBy <https://w3id.org/con-tax/zones/aat-spaces> ;
  rdfs:label "screens passage"@nl ;
  rdfs:label "screens passages"@en ;
  rdfs:label "screens passages"@nl ;
  rdfs:seeAlso <http://vocab.getty.edu/aat/300004314> ;
  rdfs:subClassOf <https://w3id.org/con-tax/zones/aat-spaces#300004283> ;
.
<https://w3id.org/con-tax/zones/aat-spaces#300004315>
  rdf:type owl:Class ;
  rdfs:comment "Areas rising through the centers of buildings, devoted to such service functions as pipe chases, air ducts, elevators, fire stairs, and rest rooms."@en ;
  rdfs:comment "Wordt gebruikt voor centrale ruimten voor nutsvoorzieningen zoals leidingen, liften, brandtrappen en toiletten in gebouwen met meerdere verdiepingen."@nl ;
  rdfs:isDefinedBy <https://w3id.org/con-tax/zones/aat-spaces> ;
  rdfs:label "installatiekern"@nl ;
  rdfs:label "installatiekernen"@nl ;
  rdfs:label "service cores"@en ;
  rdfs:seeAlso <http://vocab.getty.edu/aat/300004315> ;
  rdfs:subClassOf <https://w3id.org/con-tax/zones/aat-spaces#300133704> ;
.
<https://w3id.org/con-tax/zones/aat-spaces#300004316>
  rdf:type owl:Class ;
  rdfs:comment "Kokervormige ruimten."@nl ;
  rdfs:comment "Well-like passages or enclosed vertical spaces in a building."@en ;
  rdfs:isDefinedBy <https://w3id.org/con-tax/zones/aat-spaces> ;
  rdfs:label "schacht (binnenruimte)"@nl ;
  rdfs:label "schacht"@nl ;
  rdfs:label "schachten (binnenruimten)"@nl ;
  rdfs:label "schachten"@nl ;
  rdfs:label "shafts (spaces)"@en ;
  rdfs:seeAlso <http://vocab.getty.edu/aat/300004316> ;
  rdfs:subClassOf <https://w3id.org/con-tax/zones/aat-spaces#300078790> ;
.
<https://w3id.org/con-tax/zones/aat-spaces#300004317>
  rdf:type owl:Class ;
  rdfs:comment "Very small courts that are enclosed within the walls of a building and supply ventilation to windows. Prefer \"light courts\" for somewhat larger courts supplying significant light as well as ventilation, or courts supplying only light."@en ;
  rdfs:comment "Zeer kleine binnenplaatsen in de vorm van verticale schachten ten behoeve van de ventilatie van de aangrenzende ruimten. Gebruik 'lichtschachten' voor wat grotere binnenplaatsen die naast ventilatie ook een aanmerkelijke hoeveelheid licht toelaten."@nl ;
  rdfs:isDefinedBy <https://w3id.org/con-tax/zones/aat-spaces> ;
  rdfs:label "air shafts"@en ;
  rdfs:label "luchtschacht"@nl ;
  rdfs:label "luchtschachten"@nl ;
  rdfs:seeAlso <http://vocab.getty.edu/aat/300004317> ;
  rdfs:seeAlso wd:Q1459897 ;
  rdfs:subClassOf <https://w3id.org/con-tax/zones/aat-spaces#300004316> ;
.
<https://w3id.org/con-tax/zones/aat-spaces#300004321>
  rdf:type owl:Class ;
  rdfs:comment "Kokers om licht door te laten voor lagere ruimten in een gebouw. Gebruik voor relatief kleine binnenplaatsen 'lichtschachten'."@nl ;
  rdfs:comment "Shafts designed to admit light to the interior rooms of a building."@en ;
  rdfs:isDefinedBy <https://w3id.org/con-tax/zones/aat-spaces> ;
  rdfs:label "lichtkoker"@nl ;
  rdfs:label "lichtkokers"@nl ;
  rdfs:label "light wells"@en ;
  rdfs:seeAlso <http://vocab.getty.edu/aat/300004321> ;
  rdfs:subClassOf <https://w3id.org/con-tax/zones/aat-spaces#300004316> ;
.
<https://w3id.org/con-tax/zones/aat-spaces#300004323>
  rdf:type owl:Class ;
  rdfs:comment "Open spaces in a structure intended to allow placement and operation of an escalator."@en ;
  rdfs:isDefinedBy <https://w3id.org/con-tax/zones/aat-spaces> ;
  rdfs:label "escalator wells"@en ;
  rdfs:label "roltrapschacht"@nl ;
  rdfs:label "roltrapschachten"@nl ;
  rdfs:seeAlso <http://vocab.getty.edu/aat/300004323> ;
  rdfs:subClassOf <https://w3id.org/con-tax/zones/aat-spaces#300004241> ;
.
<https://w3id.org/con-tax/zones/aat-spaces#300004324>
  rdf:type owl:Class ;
  rdfs:comment "Ruimten die een of meer verdiepingen bestrijken en die trappen bevatten."@nl ;
  rdfs:comment "Spaces, extending through one or more floors, that contain staircases."@en ;
  rdfs:isDefinedBy <https://w3id.org/con-tax/zones/aat-spaces> ;
  rdfs:label "stairwells"@en ;
  rdfs:label "trappenhuis"@nl ;
  rdfs:label "trappenhuizen"@nl ;
  rdfs:label "trapzalen"@nl ;
  rdfs:seeAlso <http://vocab.getty.edu/aat/300004324> ;
  rdfs:seeAlso wd:Q2451751 ;
  rdfs:subClassOf <https://w3id.org/con-tax/zones/aat-spaces#300004241> ;
.
<https://w3id.org/con-tax/zones/aat-spaces#300004326>
  rdf:type owl:Class ;
  rdfs:comment "Cilindervormige of rechthoekige ruimten waarin de trappen van huizen zijn gebouwd, minder ruim van opzet dan 'trappenhuizen' (VWB)."@nl ;
  rdfs:comment "Stairwells equipped with a system that prevents stairwells in highrise buildings from becoming smoke-filled in case of fire. Stairwells are pressurized by using fans or otherwise forcing fresh outside air through air ducts in the building's exterior walls and down the stairwell shafts. As the system pumps increasingly more air into the stairwells, the air pressure rises until it is greater than the air pressure on the building's floors. Given that stairwell doors must open into stairwells in the direction of egress from the building interior, standards are typically in place to regulate the pressure so that it is not too great to prevent ease of opening."@en ;
  rdfs:isDefinedBy <https://w3id.org/con-tax/zones/aat-spaces> ;
  rdfs:label "pressurized stairwells"@en ;
  rdfs:label "trapkoker"@nl ;
  rdfs:label "trapkokers"@nl ;
  rdfs:label "trapkooi"@nl ;
  rdfs:label "trapkooien"@nl ;
  rdfs:seeAlso <http://vocab.getty.edu/aat/300004326> ;
  rdfs:subClassOf <https://w3id.org/con-tax/zones/aat-spaces#300004324> ;
.
<https://w3id.org/con-tax/zones/aat-spaces#300004328>
  rdf:type gvp:GuideTerm ;
  rdfs:isDefinedBy <https://w3id.org/con-tax/zones/aat-spaces> ;
  rdfs:label "<display rooms and spaces>"@en ;
  rdfs:label "<expositieruimten>"@nl ;
  rdfs:label "<expositiezalen en -ruimten>"@nl ;
  rdfs:label "expositieruimten"@nl ;
  rdfs:label "expositiezalen en -ruimten"@nl ;
  rdfs:seeAlso <http://vocab.getty.edu/aat/300004328> ;
  contax:containsConcept <https://w3id.org/con-tax/zones/aat-spaces#300004330> ;
  contax:containsConcept <https://w3id.org/con-tax/zones/aat-spaces#300004331> ;
  contax:containsConcept <https://w3id.org/con-tax/zones/aat-spaces#300004415> ;
  contax:containsConcept <https://w3id.org/con-tax/zones/aat-spaces#300005814> ;
  contax:containsConcept <https://w3id.org/con-tax/zones/aat-spaces#300025978> ;
  contax:containsConcept <https://w3id.org/con-tax/zones/aat-spaces#300192556> ;
  contax:containsConcept <https://w3id.org/con-tax/zones/aat-spaces#300240057> ;
  contax:containsConcept <https://w3id.org/con-tax/zones/aat-spaces#300419455> ;
.
<https://w3id.org/con-tax/zones/aat-spaces#300004330>
  rdf:type owl:Class ;
  rdfs:comment "Rooms in museums in which furnishings are displayed within a historically accurate architectural setting."@en ;
  rdfs:comment "Ruimten in musea waarin met originele objecten historische interieurs zijn gereconstrueerd."@nl ;
  rdfs:isDefinedBy <https://w3id.org/con-tax/zones/aat-spaces> ;
  rdfs:label "period rooms"@en ;
  rdfs:label "stijlkamer"@nl ;
  rdfs:label "stijlkamers"@nl ;
  rdfs:seeAlso <http://vocab.getty.edu/aat/300004330> ;
  rdfs:seeAlso wd:Q2071002 ;
  rdfs:subClassOf <https://w3id.org/con-tax/zones/aat-spaces#300133704> ;
.
<https://w3id.org/con-tax/zones/aat-spaces#300004331>
  rdf:type owl:Class ;
  rdfs:comment "Rooms devoted to the display of merchandise for sale."@en ;
  rdfs:comment "Ruimten bedoeld om produkten te tonen en te verkopen."@nl ;
  rdfs:isDefinedBy <https://w3id.org/con-tax/zones/aat-spaces> ;
  rdfs:label "showrooms"@en ;
  rdfs:label "showrooms"@nl ;
  rdfs:label "toonkamers"@nl ;
  rdfs:label "toonzaal"@nl ;
  rdfs:label "toonzalen"@nl ;
  rdfs:seeAlso <http://vocab.getty.edu/aat/300004331> ;
  rdfs:seeAlso wd:Q2094773 ;
  rdfs:subClassOf <https://w3id.org/con-tax/zones/aat-spaces#300133704> ;
.
<https://w3id.org/con-tax/zones/aat-spaces#300004332>
  rdf:type gvp:GuideTerm ;
  rdfs:isDefinedBy <https://w3id.org/con-tax/zones/aat-spaces> ;
  rdfs:label "<eating and drinking spaces>"@en ;
  rdfs:label "<eet- en drinkruimte>"@nl ;
  rdfs:label "<eet- en drinkruimten>"@nl ;
  rdfs:label "eet- en drinkruimte"@nl ;
  rdfs:label "eet- en drinkruimten"@nl ;
  rdfs:seeAlso <http://vocab.getty.edu/aat/300004332> ;
  contax:containsConcept <https://w3id.org/con-tax/zones/aat-spaces#300004333> ;
  contax:containsConcept <https://w3id.org/con-tax/zones/aat-spaces#300004339> ;
  contax:containsConcept <https://w3id.org/con-tax/zones/aat-spaces#300004340> ;
  contax:containsConcept <https://w3id.org/con-tax/zones/aat-spaces#300004342> ;
  contax:containsConcept <https://w3id.org/con-tax/zones/aat-spaces#300004344> ;
  contax:containsConcept <https://w3id.org/con-tax/zones/aat-spaces#300004346> ;
  contax:containsConcept <https://w3id.org/con-tax/zones/aat-spaces#300004349> ;
  contax:containsConcept <https://w3id.org/con-tax/zones/aat-spaces#300005162> ;
  contax:containsConcept <https://w3id.org/con-tax/zones/aat-spaces#300005172> ;
  contax:containsConcept <https://w3id.org/con-tax/zones/aat-spaces#300065035> ;
  contax:containsConcept <https://w3id.org/con-tax/zones/aat-spaces#300081842> ;
  contax:containsConcept <https://w3id.org/con-tax/zones/aat-spaces#300082888> ;
  contax:containsConcept <https://w3id.org/con-tax/zones/aat-spaces#300111871> ;
  contax:containsConcept <https://w3id.org/con-tax/zones/aat-spaces#300312219> ;
  contax:containsConcept <https://w3id.org/con-tax/zones/aat-spaces#300312220> ;
.
<https://w3id.org/con-tax/zones/aat-spaces#300004333>
  rdf:type owl:Class ;
  rdfs:comment "Large rooms, halls, or apartments designed or used for festive or state functions."@en ;
  rdfs:comment "Zalen of andere grote ruimten voor feestelijke en plechtige aangelegenheden."@nl ;
  rdfs:isDefinedBy <https://w3id.org/con-tax/zones/aat-spaces> ;
  rdfs:label "banketzaal"@nl ;
  rdfs:label "banketzalen"@nl ;
  rdfs:label "banquet halls"@en ;
  rdfs:seeAlso <http://vocab.getty.edu/aat/300004333> ;
  rdfs:subClassOf <https://w3id.org/con-tax/zones/aat-spaces#300133704> ;
.
<https://w3id.org/con-tax/zones/aat-spaces#300004339>
  rdf:type owl:Class ;
  rdfs:comment "Alcoves where light meals are taken; usually containing a built-in table and seating."@en ;
  rdfs:comment "Zitnissen waar lichte maaltijden worden genuttigd, meestal met een ingebouwde tafel en zitplaatsen."@nl ;
  rdfs:isDefinedBy <https://w3id.org/con-tax/zones/aat-spaces> ;
  rdfs:label "breakfast nooks"@en ;
  rdfs:label "ontbijthoekje"@nl ;
  rdfs:label "ontbijthoekjes"@nl ;
  rdfs:seeAlso <http://vocab.getty.edu/aat/300004339> ;
  rdfs:subClassOf <https://w3id.org/con-tax/zones/aat-spaces#300133704> ;
.
<https://w3id.org/con-tax/zones/aat-spaces#300004340>
  rdf:type owl:Class ;
  rdfs:comment "Kleine kamers voor het ochtendmaal. Ze liggen meestal, maar niet altijd, naast de eetzaal. In noordelijke klimaten liggen ze vaak op het oosten om het ochtendlicht op te vangen."@nl ;
  rdfs:comment "Small rooms for the morning meal; usually, but not always, adjoining the chief dining room; in northern climates often specially arranged with an eastern exposure to catch the morning sun."@en ;
  rdfs:isDefinedBy <https://w3id.org/con-tax/zones/aat-spaces> ;
  rdfs:label "breakfast rooms"@en ;
  rdfs:label "ontbijtkamer"@nl ;
  rdfs:label "ontbijtkamers"@nl ;
  rdfs:seeAlso <http://vocab.getty.edu/aat/300004340> ;
  rdfs:subClassOf <https://w3id.org/con-tax/zones/aat-spaces#300133704> ;
.
<https://w3id.org/con-tax/zones/aat-spaces#300004342>
  rdf:type owl:Class ;
  rdfs:comment "Ruimten waar men zichzelf kan bedienen van op lange toonbanden gereedstaand eten en drinken om het ter plekke op te eten."@nl ;
  rdfs:comment "Self-service establishments providing prepared food and drinks from long counters for on-premise or immediate consumption."@en ;
  rdfs:isDefinedBy <https://w3id.org/con-tax/zones/aat-spaces> ;
  rdfs:label "cafeterias (eating and drinking spaces)"@en ;
  rdfs:label "snelbuffet"@nl ;
  rdfs:label "snelbuffetten"@nl ;
  rdfs:label "zelfbedieningsrestaurant"@nl ;
  rdfs:label "zelfbedieningsrestaurants"@nl ;
  rdfs:seeAlso <http://vocab.getty.edu/aat/300004342> ;
  rdfs:seeAlso wd:Q8463304 ;
  rdfs:subClassOf <https://w3id.org/con-tax/zones/aat-spaces#300133704> ;
.
<https://w3id.org/con-tax/zones/aat-spaces#300004344>
  rdf:type owl:Class ;
  rdfs:comment "Small dining areas when they are extensions of living rooms. Use \"dinettes\" when referring to similar spaces that are extensions of kitchens or pantries."@en ;
  rdfs:comment "Zitnissen aan woonkamers, bestemd om maaltijden te gebruiken. Geen Nederlands equivalent. Zie 'eethoeken'."@nl ;
  rdfs:isDefinedBy <https://w3id.org/con-tax/zones/aat-spaces> ;
  rdfs:label "dining alcove"@nl ;
  rdfs:label "dining alcoves"@en ;
  rdfs:label "dining alcoves"@nl ;
  rdfs:seeAlso <http://vocab.getty.edu/aat/300004344> ;
  rdfs:subClassOf <https://w3id.org/con-tax/zones/aat-spaces#300133704> ;
.
<https://w3id.org/con-tax/zones/aat-spaces#300004346>
  rdf:type owl:Class ;
  rdfs:comment "Grote eetruimten. Gebruik voor eetzalen van universiteiten 'mensa's'."@nl ;
  rdfs:comment "Use both for large dining rooms, as in a college, and for buildings containing a dining hall."@en ;
  rdfs:isDefinedBy <https://w3id.org/con-tax/zones/aat-spaces> ;
  rdfs:label "dining halls"@en ;
  rdfs:label "eetzaal"@nl ;
  rdfs:label "eetzalen"@nl ;
  rdfs:seeAlso <http://vocab.getty.edu/aat/300004346> ;
  rdfs:subClassOf <https://w3id.org/con-tax/zones/aat-spaces#300133704> ;
.
<https://w3id.org/con-tax/zones/aat-spaces#300004347>
  rdf:type owl:Class ;
  rdfs:comment "Dining halls of monasteries or other religious institutions."@en ;
  rdfs:comment "Eetzalen van kloosters en andere religieuze instellingen."@nl ;
  rdfs:isDefinedBy <https://w3id.org/con-tax/zones/aat-spaces> ;
  rdfs:label "refectories"@en ;
  rdfs:label "refectorium"@nl ;
  rdfs:label "refectoriums"@nl ;
  rdfs:label "refters"@nl ;
  rdfs:seeAlso <http://vocab.getty.edu/aat/300004347> ;
  rdfs:seeAlso wd:Q568225 ;
  rdfs:subClassOf <https://w3id.org/con-tax/zones/aat-spaces#300004346> ;
.
<https://w3id.org/con-tax/zones/aat-spaces#300004348>
  rdf:type owl:Class ;
  rdfs:comment "Areas on military bases that serve chiefly as dining halls, rooms or separate buildings."@en ;
  rdfs:comment "Ruimten waar personeels- of clubleden tegen matige prijzen kunnen eten of meegebracht eten kunnen nuttigen. Gebruik 'messes' voor kantines van legerofficieren."@nl ;
  rdfs:isDefinedBy <https://w3id.org/con-tax/zones/aat-spaces> ;
  rdfs:label "kantine"@nl ;
  rdfs:label "kantines"@nl ;
  rdfs:label "mess halls"@en ;
  rdfs:seeAlso <http://vocab.getty.edu/aat/300004348> ;
  rdfs:seeAlso wd:Q443767 ;
  rdfs:subClassOf <https://w3id.org/con-tax/zones/aat-spaces#300004346> ;
.
<https://w3id.org/con-tax/zones/aat-spaces#300004349>
  rdf:type owl:Class ;
  rdfs:comment "Kamers in privéwoningen of openbare etablissementen waar het avondmaal en andere hoofdmaaltijden worden genuttigd en die voor dit doel zijn ingericht."@nl ;
  rdfs:comment "Rooms in private houses or public establishments in which dinner and other principal meals are taken and which are furnished for this purpose."@en ;
  rdfs:isDefinedBy <https://w3id.org/con-tax/zones/aat-spaces> ;
  rdfs:label "dining rooms"@en ;
  rdfs:label "eetkamer"@nl ;
  rdfs:label "eetkamers"@nl ;
  rdfs:seeAlso <http://vocab.getty.edu/aat/300004349> ;
  rdfs:seeAlso wd:Q661199 ;
  rdfs:subClassOf <https://w3id.org/con-tax/zones/aat-spaces#300133704> ;
.
<https://w3id.org/con-tax/zones/aat-spaces#300004359>
  rdf:type owl:Class ;
  rdfs:comment "Dining rooms in Roman houses; were usually furnished with a low table and surrounded on three sides by couches."@en ;
  rdfs:comment "Eetkamers in Romeinse huizen, die meestal waren uitgerust met een lage tafel die aan drie kanten werd omringd door banken."@nl ;
  rdfs:isDefinedBy <https://w3id.org/con-tax/zones/aat-spaces> ;
  rdfs:label "triclinia (kamers)"@nl ;
  rdfs:label "triclinia (rooms)"@en ;
  rdfs:label "triclinia"@nl ;
  rdfs:label "triclinium (kamer)"@nl ;
  rdfs:label "triclinium"@nl ;
  rdfs:seeAlso <http://vocab.getty.edu/aat/300004359> ;
  rdfs:seeAlso wd:Q914598 ;
  rdfs:subClassOf <https://w3id.org/con-tax/zones/aat-spaces#300004349> ;
.
<https://w3id.org/con-tax/zones/aat-spaces#300004362>
  rdf:type owl:Class ;
  rdfs:comment "Rooms or spaces in buildings that are used for sleeping. "@en ;
  rdfs:isDefinedBy <https://w3id.org/con-tax/zones/aat-spaces> ;
  rdfs:label "slaapruimte"@nl ;
  rdfs:label "slaapruimten"@nl ;
  rdfs:label "sleeping spaces"@en ;
  rdfs:seeAlso <http://vocab.getty.edu/aat/300004362> ;
  rdfs:subClassOf <https://w3id.org/con-tax/zones/aat-spaces#300133704> ;
.
<https://w3id.org/con-tax/zones/aat-spaces#300004364>
  rdf:type owl:Class ;
  rdfs:comment "Rooms designed for or used to contain a bed or beds for sleeping."@en ;
  rdfs:isDefinedBy <https://w3id.org/con-tax/zones/aat-spaces> ;
  rdfs:label "bedrooms"@en ;
  rdfs:label "slaapkamer"@nl ;
  rdfs:label "slaapkamers"@nl ;
  rdfs:label "slaapvertrekken"@nl ;
  rdfs:seeAlso <http://vocab.getty.edu/aat/300004364> ;
  rdfs:seeAlso wd:Q193837 ;
  rdfs:subClassOf <https://w3id.org/con-tax/zones/aat-spaces#300004362> ;
.
<https://w3id.org/con-tax/zones/aat-spaces#300004367>
  rdf:type owl:Class ;
  rdfs:comment "Ancient Roman domestic spaces often considered sleeping chambers, but that may also have functioned as social spaces for more private activities such as polytheistic worship, study, or other personal or intimate uses of the householder."@en ;
  rdfs:comment "Slaapkamers in Romeinse huizen."@nl ;
  rdfs:isDefinedBy <https://w3id.org/con-tax/zones/aat-spaces> ;
  rdfs:label "cubicula (domestic spaces)"@en ;
  rdfs:label "cubicula"@nl ;
  rdfs:label "cubiculum"@nl ;
  rdfs:seeAlso <http://vocab.getty.edu/aat/300004367> ;
  rdfs:subClassOf <https://w3id.org/con-tax/zones/aat-spaces#300004364> ;
.
<https://w3id.org/con-tax/zones/aat-spaces#300004369>
  rdf:type owl:Class ;
  rdfs:comment "Kamers om zich te verkleden, zowel in woonhuizen als in theaters, sportaccomodaties en clubhuizen."@nl ;
  rdfs:comment "Rooms for dressing and the toilet, usually opening from a bedroom."@en ;
  rdfs:isDefinedBy <https://w3id.org/con-tax/zones/aat-spaces> ;
  rdfs:label "dressing rooms"@en ;
  rdfs:label "kleedkamer"@nl ;
  rdfs:label "kleedkamers"@nl ;
  rdfs:seeAlso <http://vocab.getty.edu/aat/300004369> ;
  rdfs:seeAlso wd:Q7140850 ;
  rdfs:subClassOf <https://w3id.org/con-tax/zones/aat-spaces#300133704> ;
.
<https://w3id.org/con-tax/zones/aat-spaces#300004373>
  rdf:type owl:Class ;
  rdfs:comment "Delen van Griekse en Romeinde huizen in de Oudheid die alleen door vrouwen werden gebruikt."@nl ;
  rdfs:comment "Women's apartments in ancient Greek or Roman houses. For the sections of Greek houses set aside for men, use \"andra.\""@en ;
  rdfs:isDefinedBy <https://w3id.org/con-tax/zones/aat-spaces> ;
  rdfs:label "gynaecea"@en ;
  rdfs:label "gynaecea"@nl ;
  rdfs:label "gynaeceum"@nl ;
  rdfs:seeAlso <http://vocab.getty.edu/aat/300004373> ;
  rdfs:subClassOf <https://w3id.org/con-tax/zones/aat-spaces#300260517> ;
.
<https://w3id.org/con-tax/zones/aat-spaces#300004376>
  rdf:type owl:Class ;
  rdfs:comment "De voor vrouwen bestemde, afgezonderde gedeelten in de woningen van (aanzienlijke) mohammedanen."@nl ;
  rdfs:comment "Women's quarters of Islamic houses. For the portions of Islamic houses reserved for men, use \"selamliks.\""@en ;
  rdfs:isDefinedBy <https://w3id.org/con-tax/zones/aat-spaces> ;
  rdfs:label "harem"@nl ;
  rdfs:label "harems"@en ;
  rdfs:label "harems"@nl ;
  rdfs:seeAlso <http://vocab.getty.edu/aat/300004376> ;
  rdfs:seeAlso wd:Q1170287 ;
  rdfs:seeAlso wd:Q165853 ;
  rdfs:subClassOf <https://w3id.org/con-tax/zones/aat-spaces#300260517> ;
.
<https://w3id.org/con-tax/zones/aat-spaces#300004380>
  rdf:type owl:Class ;
  rdfs:comment "Kamers bestemd voor jonge kinderen."@nl ;
  rdfs:comment "Rooms or areas set aside and furnished for babies and young children, especially those located in a house and serving as a bedroom or playroom. A nursery differs from a nursery school or day care in that the latter house private or public institutions for the instruction of young children, while a nursery is typically in a private home or an orphanage and facilitates the care of babies in addition to young children."@en ;
  rdfs:isDefinedBy <https://w3id.org/con-tax/zones/aat-spaces> ;
  rdfs:label "kinderkamer"@nl ;
  rdfs:label "kinderkamers"@nl ;
  rdfs:label "nurseries (rooms)"@en ;
  rdfs:seeAlso <http://vocab.getty.edu/aat/300004380> ;
  rdfs:seeAlso wd:Q1741939 ;
  rdfs:subClassOf <https://w3id.org/con-tax/zones/aat-spaces#300133704> ;
.
<https://w3id.org/con-tax/zones/aat-spaces#300004382>
  rdf:type owl:Class ;
  rdfs:comment "Certain upper floor rooms in Medieval houses that are smaller than halls and reserved for private family use. The form grew out of the Greek and Roman \"solariums (building spaces).\""@en ;
  rdfs:comment "Verwarmbare woonvertrekken in de Middeleeuwen. VWB"@nl ;
  rdfs:isDefinedBy <https://w3id.org/con-tax/zones/aat-spaces> ;
  rdfs:label "kemenade"@nl ;
  rdfs:label "kemenaden"@nl ;
  rdfs:label "solars (building spaces)"@en ;
  rdfs:seeAlso <http://vocab.getty.edu/aat/300004382> ;
  rdfs:subClassOf <https://w3id.org/con-tax/zones/aat-spaces#300078790> ;
.
<https://w3id.org/con-tax/zones/aat-spaces#300004388>
  rdf:type gvp:GuideTerm ;
  rdfs:isDefinedBy <https://w3id.org/con-tax/zones/aat-spaces> ;
  rdfs:label "<social and sitting spaces>"@en ;
  rdfs:label "<sociale en zitruimten>"@nl ;
  rdfs:label "sociale en zitruimten"@nl ;
  rdfs:seeAlso <http://vocab.getty.edu/aat/300004388> ;
  contax:containsConcept <https://w3id.org/con-tax/zones/aat-spaces#300004414> ;
  contax:containsConcept <https://w3id.org/con-tax/zones/aat-spaces#300004416> ;
  contax:containsConcept <https://w3id.org/con-tax/zones/aat-spaces#300004417> ;
  contax:containsConcept <https://w3id.org/con-tax/zones/aat-spaces#300004419> ;
  contax:containsConcept <https://w3id.org/con-tax/zones/aat-spaces#300004435> ;
  contax:containsConcept <https://w3id.org/con-tax/zones/aat-spaces#300004436> ;
  contax:containsConcept <https://w3id.org/con-tax/zones/aat-spaces#300004440> ;
  contax:containsConcept <https://w3id.org/con-tax/zones/aat-spaces#300004441> ;
  contax:containsConcept <https://w3id.org/con-tax/zones/aat-spaces#300004450> ;
  contax:containsConcept <https://w3id.org/con-tax/zones/aat-spaces#300004459> ;
  contax:containsConcept <https://w3id.org/con-tax/zones/aat-spaces#300004503> ;
  contax:containsConcept <https://w3id.org/con-tax/zones/aat-spaces#300004520> ;
  contax:containsConcept <https://w3id.org/con-tax/zones/aat-spaces#300007427> ;
  contax:containsConcept <https://w3id.org/con-tax/zones/aat-spaces#300078138> ;
  contax:containsConcept <https://w3id.org/con-tax/zones/aat-spaces#300081958> ;
  contax:containsConcept <https://w3id.org/con-tax/zones/aat-spaces#300082083> ;
.
<https://w3id.org/con-tax/zones/aat-spaces#300004391>
  rdf:type owl:Class ;
  rdfs:comment "Delen van Griekse huizen in de Oudheid die alleen door mannen werden gebruikt."@nl ;
  rdfs:comment "Parts of ancient Greek houses used only by men. For those sections set aside for women, use \"gynaecea.\""@en ;
  rdfs:isDefinedBy <https://w3id.org/con-tax/zones/aat-spaces> ;
  rdfs:label "andra"@en ;
  rdfs:label "andra"@nl ;
  rdfs:label "andron"@nl ;
  rdfs:seeAlso <http://vocab.getty.edu/aat/300004391> ;
  rdfs:subClassOf <https://w3id.org/con-tax/zones/aat-spaces#300260516> ;
.
<https://w3id.org/con-tax/zones/aat-spaces#300004393>
  rdf:type owl:Class ;
  rdfs:comment "Grote ruimten voor vergaderingen, ook wel gebruikt voor sociale bijeenkomsten, zoals bals en ontvangsten, voornamelijk 18e-eeuws. Geen Nederlands equivalent. Gebruik 'balzalen' of 'vergaderzalen'."@nl ;
  rdfs:comment "Rooms, primarily of the 18th century, in which social gatherings and balls (commonly referred to as assemblies) were held."@en ;
  rdfs:isDefinedBy <https://w3id.org/con-tax/zones/aat-spaces> ;
  rdfs:label "assembly room (amerikaans)"@nl ;
  rdfs:label "assembly room"@nl ;
  rdfs:label "assembly rooms (amerikaans)"@nl ;
  rdfs:label "assembly rooms"@en ;
  rdfs:label "assembly rooms"@nl ;
  rdfs:seeAlso <http://vocab.getty.edu/aat/300004393> ;
  rdfs:seeAlso wd:Q4808723 ;
  rdfs:subClassOf <https://w3id.org/con-tax/zones/aat-spaces#300133704> ;
.
<https://w3id.org/con-tax/zones/aat-spaces#300004394>
  rdf:type owl:Class ;
  rdfs:comment "Rooms or entire buildings designed for a variety of activities such as would occur on a stage before a seated audience; for rooms or buildings used only for theatrical performances, use \"theaters;\" for rooms with fixed seating designed for lectures, use \"lecture halls.\""@en ;
  rdfs:comment "Wordt gebruikt voor zowel ruimten als hele gebouwen bestemd voor een verscheidenheid aan activiteiten die op een podium voor een zittend publiek plaatsvinden. Voor ruimten en gebouwen die alleen voor theatervoorstellingen dienen wordt 'theaters' gebruikt; voor ruimten met vaste zitplaatsen, bestemd voor lezingen, wordt 'voordracht- of lezingenzalen' gebruikt."@nl ;
  rdfs:isDefinedBy <https://w3id.org/con-tax/zones/aat-spaces> ;
  rdfs:label "auditorium"@nl ;
  rdfs:label "auditoriums"@en ;
  rdfs:label "auditoriums"@nl ;
  rdfs:label "gehoorzalen"@nl ;
  rdfs:seeAlso <http://vocab.getty.edu/aat/300004394> ;
  rdfs:seeAlso wd:Q230752 ;
  rdfs:subClassOf <https://w3id.org/con-tax/zones/aat-spaces#300075881> ;
.
<https://w3id.org/con-tax/zones/aat-spaces#300004398>
  rdf:type owl:Class ;
  rdfs:comment "Rooms designed or adapted for the holding of conferences, with the room usually focused around a large table and chairs."@en ;
  rdfs:isDefinedBy <https://w3id.org/con-tax/zones/aat-spaces> ;
  rdfs:label "conference rooms"@en ;
  rdfs:label "conferentiekamers"@nl ;
  rdfs:label "conferentiezalen"@nl ;
  rdfs:label "vergaderzaal"@nl ;
  rdfs:label "vergaderzalen"@nl ;
  rdfs:seeAlso <http://vocab.getty.edu/aat/300004398> ;
  rdfs:seeAlso wd:Q1207465 ;
  rdfs:subClassOf <https://w3id.org/con-tax/zones/aat-spaces#300075881> ;
.
<https://w3id.org/con-tax/zones/aat-spaces#300004408>
  rdf:type owl:Class ;
  rdfs:comment "Refers to rooms, usually in courthouses, where sessions of a court of law are held."@en ;
  rdfs:comment "Ruimten voor de openbare zittingen van een rechtscollege. Gebruik 'raadkamers' voor ruimten voor besloten bijeenkomsten van een rechtscollege."@nl ;
  rdfs:isDefinedBy <https://w3id.org/con-tax/zones/aat-spaces> ;
  rdfs:label "courtrooms"@en-us ;
  rdfs:label "rechtszaal"@nl ;
  rdfs:label "rechtszalen"@nl ;
  rdfs:seeAlso <http://vocab.getty.edu/aat/300004408> ;
  rdfs:subClassOf <https://w3id.org/con-tax/zones/aat-spaces#300075881> ;
.
<https://w3id.org/con-tax/zones/aat-spaces#300004409>
  rdf:type owl:Class ;
  rdfs:comment "Large rooms with fixed seating, designed for lectures. For large rooms designed for activities such as concerts or plays and requiring a large stage, see \"auditoriums.\""@en ;
  rdfs:comment "Wordt gebruikt voor grote ruimten met vaste zitplaatsen bestemd voor lezingen. Gebruik voor grote ruimten bestemd voor een verscheidenheid aan activiteiten op een podium 'auditoriums'."@nl ;
  rdfs:isDefinedBy <https://w3id.org/con-tax/zones/aat-spaces> ;
  rdfs:label "lecture halls"@en-us ;
  rdfs:label "lezingenzalen"@nl ;
  rdfs:label "voordrachtzaal"@nl ;
  rdfs:label "voordrachtzalen"@nl ;
  rdfs:seeAlso <http://vocab.getty.edu/aat/300004409> ;
  rdfs:subClassOf <https://w3id.org/con-tax/zones/aat-spaces#300075881> ;
.
<https://w3id.org/con-tax/zones/aat-spaces#300004413>
  rdf:type owl:Class ;
  rdfs:comment "Large rooms designed for formal dancing or any room in which balls are routinely held."@en ;
  rdfs:isDefinedBy <https://w3id.org/con-tax/zones/aat-spaces> ;
  rdfs:label "ballrooms"@en ;
  rdfs:label "balzaal"@nl ;
  rdfs:label "balzalen"@nl ;
  rdfs:seeAlso <http://vocab.getty.edu/aat/300004413> ;
  rdfs:seeAlso wd:Q805353 ;
  rdfs:subClassOf <https://w3id.org/con-tax/zones/aat-spaces#300133704> ;
.
<https://w3id.org/con-tax/zones/aat-spaces#300004414>
  rdf:type owl:Class ;
  rdfs:comment "Kamers in bijvoorbeeld hotels en universiteiten voor informele samenkomst."@nl ;
  rdfs:comment "Public lounges or similar rooms in such places as hotels and colleges."@en ;
  rdfs:isDefinedBy <https://w3id.org/con-tax/zones/aat-spaces> ;
  rdfs:label "common rooms"@en ;
  rdfs:label "gemeenschappelijke vertrek"@nl ;
  rdfs:label "gemeenschappelijke vertrekken"@nl ;
  rdfs:seeAlso <http://vocab.getty.edu/aat/300004414> ;
  rdfs:seeAlso wd:Q3660943 ;
  rdfs:subClassOf <https://w3id.org/con-tax/zones/aat-spaces#300133704> ;
.
<https://w3id.org/con-tax/zones/aat-spaces#300004415>
  rdf:type owl:Class ;
  rdfs:comment "In current usage, attached rooms in dwellings or other buildings, having glass wall panels and roofs, often constructed on the back or side of the building and used as a sun room or for growing indoor plants. Usage overlaps with “solariums,” which are typically rooms with large windows. In historical usage, meaning overlaps with \"greenhouses,\" which are typically larger glazed structures devoted to growing and displaying plants."@en ;
  rdfs:comment "Kassen of beglaasde kamers aangebouwd aan woningen, qom van de zon te genieten, maar ook als kas om planten te houden."@nl ;
  rdfs:isDefinedBy <https://w3id.org/con-tax/zones/aat-spaces> ;
  rdfs:label "conservatories (building spaces)"@en ;
  rdfs:label "serre (aanbouw)"@nl ;
  rdfs:label "serre"@nl ;
  rdfs:label "serres (aanbouwen)"@nl ;
  rdfs:label "serres"@nl ;
  rdfs:seeAlso <http://vocab.getty.edu/aat/300004415> ;
  rdfs:subClassOf <https://w3id.org/con-tax/zones/aat-spaces#300133704> ;
.
<https://w3id.org/con-tax/zones/aat-spaces#300004416>
  rdf:type owl:Class ;
  rdfs:comment "Kleine, informele privévertrekken in huizen of appartementen die worden gebruikt om in te werken, te lezen of te ontspannen."@nl ;
  rdfs:comment "Small, private, informal rooms in houses or apartments used for work, reading, or relaxation."@en ;
  rdfs:isDefinedBy <https://w3id.org/con-tax/zones/aat-spaces> ;
  rdfs:label "den"@nl ;
  rdfs:label "dens (rooms)"@en ;
  rdfs:label "dens"@nl ;
  rdfs:seeAlso <http://vocab.getty.edu/aat/300004416> ;
  rdfs:subClassOf <https://w3id.org/con-tax/zones/aat-spaces#300133704> ;
.
<https://w3id.org/con-tax/zones/aat-spaces#300004417>
  rdf:type owl:Class ;
  rdfs:comment "Formal reception rooms, as in a home or hotel, or rooms to which one may retire for privacy or rest."@en ;
  rdfs:comment "Kamers met een privé-karakter, bedoeld om in te zitten, gasten te ontvangen en te verpozen. Gebruik 'salons' voor grotere en officiëlere zitruimten."@nl ;
  rdfs:isDefinedBy <https://w3id.org/con-tax/zones/aat-spaces> ;
  rdfs:label "drawing rooms"@en ;
  rdfs:label "zitkamer"@nl ;
  rdfs:label "zitkamers"@nl ;
  rdfs:seeAlso <http://vocab.getty.edu/aat/300004417> ;
  rdfs:seeAlso wd:Q11166097 ;
  rdfs:subClassOf <https://w3id.org/con-tax/zones/aat-spaces#300133704> ;
.
<https://w3id.org/con-tax/zones/aat-spaces#300004419>
  rdf:type owl:Class ;
  rdfs:comment "Informal living rooms, often adjacent to the kitchen, where a family may gather."@en ;
  rdfs:comment "Kamers in woonhuizen, vaak naast de keuken gelegen, die gebruikt worden om te eten en te drinken, te verpozen en voor andere dagelijkse bezigheden. Doorgaans in combinatie met een 'nette kamer'. Zie voor soortgelijke vertrekken in woonhuizen na 1945 'woonkamers'."@nl ;
  rdfs:isDefinedBy <https://w3id.org/con-tax/zones/aat-spaces> ;
  rdfs:label "family rooms"@en ;
  rdfs:label "huiskamer"@nl ;
  rdfs:label "huiskamers"@nl ;
  rdfs:seeAlso <http://vocab.getty.edu/aat/300004419> ;
  rdfs:seeAlso wd:Q5433389 ;
  rdfs:subClassOf <https://w3id.org/con-tax/zones/aat-spaces#300133704> ;
.
<https://w3id.org/con-tax/zones/aat-spaces#300004420>
  rdf:type owl:Class ;
  rdfs:comment "In general refers to rooms large in proportion to rooms for domestic functions, circulation, or storage; may be used specifically for the principal rooms of a Medieval house and for large central rooms from the 19th century onward in certain English and American houses."@en ;
  rdfs:comment "Ruimten die groter zijn dan kamers, in gebouwen van allerlei aard. Wordt ook gebruikt voor de belangrijkste ruimten van middeleeuwse huizen en voor grote ruimten in aanzienlijke huizen."@nl ;
  rdfs:isDefinedBy <https://w3id.org/con-tax/zones/aat-spaces> ;
  rdfs:label "halls (interior spaces)"@en ;
  rdfs:label "zaal"@nl ;
  rdfs:label "zalen"@nl ;
  rdfs:seeAlso <http://vocab.getty.edu/aat/300004420> ;
  rdfs:subClassOf <https://w3id.org/con-tax/zones/aat-spaces#300078790> ;
.
<https://w3id.org/con-tax/zones/aat-spaces#300004425>
  rdf:type owl:Class ;
  rdfs:comment "Halls whose roof is supported by rows of columns giving a forestlike appearance."@en ;
  rdfs:comment "Zalen waarvan het dak wordt gedragen door rijen zuilen."@nl ;
  rdfs:isDefinedBy <https://w3id.org/con-tax/zones/aat-spaces> ;
  rdfs:label "hypostyle halls"@en ;
  rdfs:label "zuilenhal"@nl ;
  rdfs:label "zuilenhallen"@nl ;
  rdfs:seeAlso <http://vocab.getty.edu/aat/300004425> ;
  rdfs:seeAlso wd:Q1324228 ;
  rdfs:subClassOf <https://w3id.org/con-tax/zones/aat-spaces#300004420> ;
.
<https://w3id.org/con-tax/zones/aat-spaces#300004433>
  rdf:type owl:Class ;
  rdfs:comment "Rooms located in homes or other buildings and containing books for reading, study, or reference, typically with shelves for the books and a desk or table for users of the library."@en ;
  rdfs:comment "Ruimten voor het bewaren, toegankelijk maken en lezen van publicaties."@nl ;
  rdfs:isDefinedBy <https://w3id.org/con-tax/zones/aat-spaces> ;
  rdfs:label "bibliotheek (ruimte)"@nl ;
  rdfs:label "bibliotheek"@nl ;
  rdfs:label "bibliotheken (ruimten)"@nl ;
  rdfs:label "bibliotheken"@nl ;
  rdfs:label "libraries (rooms)"@en ;
  rdfs:seeAlso <http://vocab.getty.edu/aat/300004433> ;
  rdfs:seeAlso wd:Q7075 ;
  rdfs:subClassOf <https://w3id.org/con-tax/zones/aat-spaces#300133704> ;
.
<https://w3id.org/con-tax/zones/aat-spaces#300004434>
  rdf:type owl:Class ;
  rdfs:comment "Rooms in clubs, libraries, hotels, or public institutions especially adapted and appropriate to reading and study."@en ;
  rdfs:comment "Ruimten in clubs, bibliotheken, hotels of openbare instellingen die bedoeld zijn om in te lezen."@nl ;
  rdfs:isDefinedBy <https://w3id.org/con-tax/zones/aat-spaces> ;
  rdfs:label "leeskamer"@nl ;
  rdfs:label "leeskamers"@nl ;
  rdfs:label "leeszaal (ruimte)"@nl ;
  rdfs:label "leeszaal"@nl ;
  rdfs:label "leeszalen (ruimten)"@nl ;
  rdfs:label "leeszalen"@nl ;
  rdfs:label "reading rooms"@en ;
  rdfs:label "studiezaal"@nl ;
  rdfs:label "studiezalen"@nl ;
  rdfs:seeAlso <http://vocab.getty.edu/aat/300004434> ;
  rdfs:seeAlso wd:Q1753764 ;
  rdfs:subClassOf <https://w3id.org/con-tax/zones/aat-spaces#300133704> ;
.
<https://w3id.org/con-tax/zones/aat-spaces#300004435>
  rdf:type owl:Class ;
  rdfs:comment "Rooms in contemporary residences used for entertaining guests, reading, watching television, or other activities, generally more formal than a den but serving a wider range of activities than a 19th-century parlor."@en ;
  rdfs:comment "Ruimten in hedendaagse woningen waarin men gasten ontvangt, leest, televisie kijkt of andere activiteiten bedrijft, doorgaans iets formeler van karakter dan een ‘den’ maar bedoeld voor een breder scala van activiteiten dan een 19de-eeuwse ontvangstzaal."@nl ;
  rdfs:isDefinedBy <https://w3id.org/con-tax/zones/aat-spaces> ;
  rdfs:label "living rooms"@en ;
  rdfs:label "woonkamer"@nl ;
  rdfs:label "woonkamers"@nl ;
  rdfs:label "woonvertrekken"@nl ;
  rdfs:seeAlso <http://vocab.getty.edu/aat/300004435> ;
  rdfs:seeAlso wd:Q475018 ;
  rdfs:subClassOf <https://w3id.org/con-tax/zones/aat-spaces#300133704> ;
.
<https://w3id.org/con-tax/zones/aat-spaces#300004436>
  rdf:type owl:Class ;
  rdfs:comment "Informal sitting rooms, as in hotels, theaters, airports, and institutional buildings."@en ;
  rdfs:comment "Informele zitruimten, zoals bijvoorbeeld in hotels en theaters."@nl ;
  rdfs:isDefinedBy <https://w3id.org/con-tax/zones/aat-spaces> ;
  rdfs:label "lounge"@nl ;
  rdfs:label "lounges (sitting rooms)"@en ;
  rdfs:label "lounges"@nl ;
  rdfs:seeAlso <http://vocab.getty.edu/aat/300004436> ;
  rdfs:subClassOf <https://w3id.org/con-tax/zones/aat-spaces#300133704> ;
.
<https://w3id.org/con-tax/zones/aat-spaces#300004440>
  rdf:type owl:Class ;
  rdfs:comment "Sitting rooms, sometimes reserved for women, used during the early part of the day; popular from the early 19th century to the early 20th century, especially in England."@en ;
  rdfs:comment "Wordt gebruikt voor zitkamers, soms gereserveerd voor vrouwen, die 's ochtends gebruikt worden. Ze waren populair van begin 19e- tot begin 20e eeuw, vooral in Engeland."@nl ;
  rdfs:isDefinedBy <https://w3id.org/con-tax/zones/aat-spaces> ;
  rdfs:label "morning room"@nl ;
  rdfs:label "morning rooms"@en ;
  rdfs:label "morning rooms"@nl ;
  rdfs:seeAlso <http://vocab.getty.edu/aat/300004440> ;
  rdfs:subClassOf <https://w3id.org/con-tax/zones/aat-spaces#300133704> ;
.
<https://w3id.org/con-tax/zones/aat-spaces#300004441>
  rdf:type owl:Class ;
  rdfs:comment "Rooms intended for conversation and the reception of guests in residences, hotels, monasteries, or churches, particularly common in the 19th century. The contemporary living room is similar to the parlor in that often another room is provided for daily family relaxation."@en ;
  rdfs:comment "Wordt gebruikt voor kamers die zijn bedoeld voor conversatie en de ontvangst van gasten in residenties, hotels, kloosters of kerken. De laat 20e-eeuwse woonkamer lijkt op de 19e of vroeg 20e -eeuwse salon in die zin dat vaak een andere kamer dient voor de dagelijkse ontspanning met het gezin."@nl ;
  rdfs:isDefinedBy <https://w3id.org/con-tax/zones/aat-spaces> ;
  rdfs:label "ontvangstzalen"@nl ;
  rdfs:label "ontvangszaal"@nl ;
  rdfs:label "parloir"@nl ;
  rdfs:label "parloirs"@nl ;
  rdfs:label "parlors"@en-us ;
  rdfs:seeAlso <http://vocab.getty.edu/aat/300004441> ;
  rdfs:subClassOf <https://w3id.org/con-tax/zones/aat-spaces#300133704> ;
.
<https://w3id.org/con-tax/zones/aat-spaces#300004445>
  rdf:type owl:Class ;
  rdfs:comment "Rooms where great personages formally receive company."@en ;
  rdfs:comment "Ruimten waar belangrijke personen formele ontvangsten houden."@nl ;
  rdfs:isDefinedBy <https://w3id.org/con-tax/zones/aat-spaces> ;
  rdfs:label "audiëntievertrek"@nl ;
  rdfs:label "audiëntievertrekken"@nl ;
  rdfs:label "audiëntiezalen"@nl ;
  rdfs:label "presence chambers"@en ;
  rdfs:seeAlso <http://vocab.getty.edu/aat/300004445> ;
  rdfs:subClassOf <https://w3id.org/con-tax/zones/aat-spaces#300075880> ;
.
<https://w3id.org/con-tax/zones/aat-spaces#300004449>
  rdf:type owl:Class ;
  rdfs:comment "Chief rooms of state containing the throne."@en ;
  rdfs:comment "De belangrijkste staatsievertrekken, waarin de troon staat."@nl ;
  rdfs:isDefinedBy <https://w3id.org/con-tax/zones/aat-spaces> ;
  rdfs:label "throne rooms"@en ;
  rdfs:label "troonzaal"@nl ;
  rdfs:label "troonzalen"@nl ;
  rdfs:seeAlso <http://vocab.getty.edu/aat/300004449> ;
  rdfs:seeAlso wd:Q1251792 ;
  rdfs:subClassOf <https://w3id.org/con-tax/zones/aat-spaces#300075880> ;
.
<https://w3id.org/con-tax/zones/aat-spaces#300004450>
  rdf:type owl:Class ;
  rdfs:comment "Kamers bedoeld voor gebruik door wachtenden, zoals in treinstations of ziekenhuizen."@nl ;
  rdfs:comment "Rooms furnished for the use of persons waiting, as in railroad stations or medical offices."@en ;
  rdfs:isDefinedBy <https://w3id.org/con-tax/zones/aat-spaces> ;
  rdfs:label "wachtkamer (zitkamer)"@nl ;
  rdfs:label "wachtkamer"@nl ;
  rdfs:label "wachtkamers (zitkamers)"@nl ;
  rdfs:label "wachtkamers"@nl ;
  rdfs:label "wachtlokaal"@nl ;
  rdfs:label "wachtlokalen"@nl ;
  rdfs:label "waiting rooms"@en ;
  rdfs:seeAlso <http://vocab.getty.edu/aat/300004450> ;
  rdfs:seeAlso wd:Q674251 ;
  rdfs:subClassOf <https://w3id.org/con-tax/zones/aat-spaces#300133704> ;
.
<https://w3id.org/con-tax/zones/aat-spaces#300004451>
  rdf:type owl:Class ;
  rdfs:comment "Rooms in homes or public buildings furnished and reserved for recreation and informal entertaining."@en ;
  rdfs:comment "Wordt gebruikt voor ruimten in huizen of openbare gebouwen die zijn bestemd voor recreatie en informeel amusement."@nl ;
  rdfs:isDefinedBy <https://w3id.org/con-tax/zones/aat-spaces> ;
  rdfs:label "recreatieruimte"@nl ;
  rdfs:label "recreatieruimten"@nl ;
  rdfs:label "recreatiezaal"@nl ;
  rdfs:label "recreatiezalen"@nl ;
  rdfs:label "recreation rooms"@en ;
  rdfs:seeAlso <http://vocab.getty.edu/aat/300004451> ;
  rdfs:seeAlso wd:Q2911974 ;
  rdfs:subClassOf <https://w3id.org/con-tax/zones/aat-spaces#300133704> ;
.
<https://w3id.org/con-tax/zones/aat-spaces#300004452>
  rdf:type owl:Class ;
  rdfs:comment "Recreation rooms devoted entirely to table games."@en ;
  rdfs:comment "Wordt gebruikt voor recreatiekamers die volledig gewijd zijn aan tafelspelen."@nl ;
  rdfs:isDefinedBy <https://w3id.org/con-tax/zones/aat-spaces> ;
  rdfs:label "game rooms"@en ;
  rdfs:label "tafelspelkamer"@nl ;
  rdfs:label "tafelspelkamers"@nl ;
  rdfs:seeAlso <http://vocab.getty.edu/aat/300004452> ;
  rdfs:subClassOf <https://w3id.org/con-tax/zones/aat-spaces#300004451> ;
.
<https://w3id.org/con-tax/zones/aat-spaces#300004455>
  rdf:type owl:Class ;
  rdfs:comment "Kamers voornamelijk in particuliere huizen waarin een biljarttafel staat."@nl ;
  rdfs:comment "Rooms intended primarily for playing billiards."@en ;
  rdfs:isDefinedBy <https://w3id.org/con-tax/zones/aat-spaces> ;
  rdfs:label "biljartkamer"@nl ;
  rdfs:label "biljartkamers"@nl ;
  rdfs:label "billiard rooms"@en-us ;
  rdfs:seeAlso <http://vocab.getty.edu/aat/300004455> ;
  rdfs:seeAlso wd:Q4911823 ;
  rdfs:subClassOf <https://w3id.org/con-tax/zones/aat-spaces#300004452> ;
.
<https://w3id.org/con-tax/zones/aat-spaces#300004457>
  rdf:type owl:Class ;
  rdfs:comment "Rooms fitted out or reserved for children to play in."@en ;
  rdfs:comment "Wordt gebruikt voor kamers die zijn bestemd voor kinderen om in te spelen."@nl ;
  rdfs:isDefinedBy <https://w3id.org/con-tax/zones/aat-spaces> ;
  rdfs:label "playrooms"@en-us ;
  rdfs:label "speelkamer"@nl ;
  rdfs:label "speelkamers"@nl ;
  rdfs:seeAlso <http://vocab.getty.edu/aat/300004457> ;
  rdfs:subClassOf <https://w3id.org/con-tax/zones/aat-spaces#300004451> ;
.
<https://w3id.org/con-tax/zones/aat-spaces#300004459>
  rdf:type owl:Class ;
  rdfs:comment "Spacious, usually formal and elegantly furnished rooms, used primarily for entertaining."@en ;
  rdfs:comment "Wordt gebruikt voor ruime, officiële en elegant ingerichte kamers die voornamelijk worden gebruikt voor ontvangst en amusement. Gebruik 'zitkamers' voor soortgelijke, maar meestal kleinere vertrekken met een privé-karakter."@nl ;
  rdfs:isDefinedBy <https://w3id.org/con-tax/zones/aat-spaces> ;
  rdfs:label "pronkkamers"@nl ;
  rdfs:label "salon"@nl ;
  rdfs:label "salons (rooms for entertaining)"@en ;
  rdfs:label "salons"@nl ;
  rdfs:seeAlso <http://vocab.getty.edu/aat/300004459> ;
  rdfs:subClassOf <https://w3id.org/con-tax/zones/aat-spaces#300133704> ;
.
<https://w3id.org/con-tax/zones/aat-spaces#300004465>
  rdf:type owl:Class ;
  rdfs:comment "Kamers of ruimten in een gebouw die zijn bestemd voor opslag."@nl ;
  rdfs:comment "Rooms or areas in a structure that are allocated for storage. "@en ;
  rdfs:isDefinedBy <https://w3id.org/con-tax/zones/aat-spaces> ;
  rdfs:label "bergruimte"@nl ;
  rdfs:label "bergruimten"@nl ;
  rdfs:label "bewaar- en opslagruimte"@nl ;
  rdfs:label "bewaar- en opslagruimten"@nl ;
  rdfs:label "storage spaces"@en ;
  rdfs:seeAlso <http://vocab.getty.edu/aat/300004465> ;
  rdfs:seeAlso wd:Q21551014 ;
  rdfs:subClassOf <https://w3id.org/con-tax/zones/aat-spaces#300133704> ;
.
<https://w3id.org/con-tax/zones/aat-spaces#300004467>
  rdf:type owl:Class ;
  rdfs:comment "Kleine zijkamers of uitsparingen in een gebouw met meestal een deur. Gebouwd of gebruikt voor het bergen van kleding, gereedschappen of voorraden."@nl ;
  rdfs:comment "Small side-rooms or recesses in a structure, usually having a door, built or used for storing clothing, utensils, or provisions."@en ;
  rdfs:isDefinedBy <https://w3id.org/con-tax/zones/aat-spaces> ;
  rdfs:label "bergkast"@nl ;
  rdfs:label "bergkasten"@nl ;
  rdfs:label "closets (storage spaces)"@en ;
  rdfs:label "vaste kast"@nl ;
  rdfs:label "vaste kasten"@nl ;
  rdfs:seeAlso <http://vocab.getty.edu/aat/300004467> ;
  rdfs:seeAlso wd:Q1723368 ;
  rdfs:subClassOf <https://w3id.org/con-tax/zones/aat-spaces#300004465> ;
.
<https://w3id.org/con-tax/zones/aat-spaces#300004468>
  rdf:type owl:Class ;
  rdfs:comment "Small rooms in homes or public buildings used for storing brooms and other cleaning equipment."@en ;
  rdfs:isDefinedBy <https://w3id.org/con-tax/zones/aat-spaces> ;
  rdfs:label "bezemkast"@nl ;
  rdfs:label "bezemkasten"@nl ;
  rdfs:label "broom closets"@en-us ;
  rdfs:seeAlso <http://vocab.getty.edu/aat/300004468> ;
  rdfs:subClassOf <https://w3id.org/con-tax/zones/aat-spaces#300004467> ;
.
<https://w3id.org/con-tax/zones/aat-spaces#300004471>
  rdf:type owl:Class ;
  rdfs:comment "Kamers waar jassen of andere kledingstukken gedurende iemands bezoek kunnen worden achtergelaten."@nl ;
  rdfs:comment "Rooms in which cloaks, coats, hats, or other outerwear garments may be placed, usually located near the entrance of a place of assembly and intended for short-term placement of the garments. The term may also refer to a space located in railway-stations, other transportation stations, or hotel, where luggage of any description is temporarily taken charge of."@en ;
  rdfs:isDefinedBy <https://w3id.org/con-tax/zones/aat-spaces> ;
  rdfs:label "cloakrooms"@en-us ;
  rdfs:label "vestiaire"@nl ;
  rdfs:label "vestiaires"@nl ;
  rdfs:seeAlso <http://vocab.getty.edu/aat/300004471> ;
  rdfs:subClassOf <https://w3id.org/con-tax/zones/aat-spaces#300004465> ;
.
<https://w3id.org/con-tax/zones/aat-spaces#300004472>
  rdf:type owl:Class ;
  rdfs:comment "Kleine kamers, meestal in een huis, gebouwd en gebruikt voor het opslaan van kleding."@nl ;
  rdfs:comment "Small rooms, usually in a home, built or used for storing clothing."@en ;
  rdfs:isDefinedBy <https://w3id.org/con-tax/zones/aat-spaces> ;
  rdfs:label "clothes closets"@en-us ;
  rdfs:label "inloopkast"@nl ;
  rdfs:label "inloopkasten"@nl ;
  rdfs:seeAlso <http://vocab.getty.edu/aat/300004472> ;
  rdfs:subClassOf <https://w3id.org/con-tax/zones/aat-spaces#300004467> ;
.
<https://w3id.org/con-tax/zones/aat-spaces#300004473>
  rdf:type owl:Class ;
  rdfs:comment "Kamers voor opslag, en soms verzorging, van kledingstukken."@nl ;
  rdfs:comment "Rooms devoted to the storage, and sometimes the care, of clothes."@en ;
  rdfs:isDefinedBy <https://w3id.org/con-tax/zones/aat-spaces> ;
  rdfs:label "garderobe (kamer)"@nl ;
  rdfs:label "garderobe"@nl ;
  rdfs:label "garderobes (kamers)"@nl ;
  rdfs:label "garderobes"@nl ;
  rdfs:label "kleerkamers"@nl ;
  rdfs:label "wardrobes (rooms)"@en ;
  rdfs:seeAlso <http://vocab.getty.edu/aat/300004473> ;
  rdfs:subClassOf <https://w3id.org/con-tax/zones/aat-spaces#300004465> ;
.
<https://w3id.org/con-tax/zones/aat-spaces#300004476>
  rdf:type owl:Class ;
  rdfs:comment "Afgesloten, met schappen ingerichte kasten of kleine kamers voor het opslaan van bedlinnen en handdoeken etc."@nl ;
  rdfs:comment "Enclosed, shelved spaces or small rooms for storing bed linens and towels."@en ;
  rdfs:isDefinedBy <https://w3id.org/con-tax/zones/aat-spaces> ;
  rdfs:label "linen closets"@en-us ;
  rdfs:label "linnenkamer"@nl ;
  rdfs:label "linnenkamers"@nl ;
  rdfs:label "linnenkast"@nl ;
  rdfs:label "linnenkasten"@nl ;
  rdfs:seeAlso <http://vocab.getty.edu/aat/300004476> ;
  rdfs:subClassOf <https://w3id.org/con-tax/zones/aat-spaces#300004467> ;
.
<https://w3id.org/con-tax/zones/aat-spaces#300004479>
  rdf:type owl:Class ;
  rdfs:comment "Rooms set apart for the storing of goods or supplies in a home, public building, or ship."@en ;
  rdfs:isDefinedBy <https://w3id.org/con-tax/zones/aat-spaces> ;
  rdfs:label "opslagkamer"@nl ;
  rdfs:label "opslagkamers"@nl ;
  rdfs:label "rommelkamer"@nl ;
  rdfs:label "rommelkamers"@nl ;
  rdfs:label "storerooms"@en ;
  rdfs:seeAlso <http://vocab.getty.edu/aat/300004479> ;
  rdfs:seeAlso wd:Q7902854 ;
  rdfs:subClassOf <https://w3id.org/con-tax/zones/aat-spaces#300004465> ;
.
<https://w3id.org/con-tax/zones/aat-spaces#300004482>
  rdf:type owl:Class ;
  rdfs:comment "Rooms or sets of rooms for the systematic maintenance and storage of records and documents."@en ;
  rdfs:comment "Ruimten bedoeld voor opslag en beheer van archieven en documenten."@nl ;
  rdfs:isDefinedBy <https://w3id.org/con-tax/zones/aat-spaces> ;
  rdfs:label "archief (ruimte)"@nl ;
  rdfs:label "archief"@nl ;
  rdfs:label "archieven (ruimten)"@nl ;
  rdfs:label "archieven"@nl ;
  rdfs:label "archives (rooms)"@en ;
  rdfs:seeAlso <http://vocab.getty.edu/aat/300004482> ;
  rdfs:subClassOf <https://w3id.org/con-tax/zones/aat-spaces#300004465> ;
.
<https://w3id.org/con-tax/zones/aat-spaces#300004483>
  rdf:type owl:Class ;
  rdfs:comment "Kamers voor het ontvangen, controleren en verwerken van bagage."@nl ;
  rdfs:comment "Rooms for receiving, checking, and handling luggage."@en ;
  rdfs:isDefinedBy <https://w3id.org/con-tax/zones/aat-spaces> ;
  rdfs:label "bagagedepot"@nl ;
  rdfs:label "bagagedepots"@nl ;
  rdfs:label "baggage rooms"@en ;
  rdfs:seeAlso <http://vocab.getty.edu/aat/300004483> ;
  rdfs:subClassOf <https://w3id.org/con-tax/zones/aat-spaces#300004465> ;
.
<https://w3id.org/con-tax/zones/aat-spaces#300004488>
  rdf:type owl:Class ;
  rdfs:comment "Opslagruimten voor kaarsen en andere verlichtingsmiddelen."@nl ;
  rdfs:comment "Storage places for candles and other lighting devices."@en ;
  rdfs:isDefinedBy <https://w3id.org/con-tax/zones/aat-spaces> ;
  rdfs:label "chandleries (rooms)"@en ;
  rdfs:label "kaarsenopslagplaats"@nl ;
  rdfs:label "kaarsenopslagplaatsen"@nl ;
  rdfs:seeAlso <http://vocab.getty.edu/aat/300004488> ;
  rdfs:seeAlso wd:Q5071215 ;
  rdfs:subClassOf <https://w3id.org/con-tax/zones/aat-spaces#300004465> ;
.
<https://w3id.org/con-tax/zones/aat-spaces#300004490>
  rdf:type owl:Class ;
  rdfs:comment "Rooms kept at low temperatures for the storage of perishable items, such as food, or other items prone to deterioration or pests, such as film or archival materials."@en ;
  rdfs:comment "Ruimten die op een lage temperatuur worden gehouden voor de opslag van bederflijke waren."@nl ;
  rdfs:isDefinedBy <https://w3id.org/con-tax/zones/aat-spaces> ;
  rdfs:label "cold storage rooms"@en ;
  rdfs:label "koelcel"@nl ;
  rdfs:label "koelcellen"@nl ;
  rdfs:label "koelkamer"@nl ;
  rdfs:label "koelkamers"@nl ;
  rdfs:label "koelruimte"@nl ;
  rdfs:label "koelruimten"@nl ;
  rdfs:seeAlso <http://vocab.getty.edu/aat/300004490> ;
  rdfs:subClassOf <https://w3id.org/con-tax/zones/aat-spaces#300004465> ;
.
<https://w3id.org/con-tax/zones/aat-spaces#300004498>
  rdf:type owl:Class ;
  rdfs:comment "Kamers waar voedsel wordt opgeslagen."@nl ;
  rdfs:comment "Rooms or closets where food is stored; originally storage spaces primarily used for meat, particularly bacon, from which the term is probably derived (\"lard room\")."@en ;
  rdfs:isDefinedBy <https://w3id.org/con-tax/zones/aat-spaces> ;
  rdfs:label "larders"@en ;
  rdfs:label "provisiekamer"@nl ;
  rdfs:label "provisiekamers"@nl ;
  rdfs:seeAlso <http://vocab.getty.edu/aat/300004498> ;
  rdfs:seeAlso wd:Q4899148 ;
  rdfs:subClassOf <https://w3id.org/con-tax/zones/aat-spaces#300004465> ;
.
<https://w3id.org/con-tax/zones/aat-spaces#300004499>
  rdf:type owl:Class ;
  rdfs:comment "Kamers waarin voedsel en eet- en drinkgerei worden bewaard en vanwaar uit wordt uitgeserveerd."@nl ;
  rdfs:comment "Rooms or closets in which food, groceries, and other provisions, or silverware, dishes, and other items are kept."@en ;
  rdfs:isDefinedBy <https://w3id.org/con-tax/zones/aat-spaces> ;
  rdfs:label "pantries"@en ;
  rdfs:label "pantry"@nl ;
  rdfs:label "pantry's"@nl ;
  rdfs:label "voorraadkamer"@nl ;
  rdfs:label "voorraadkamers"@nl ;
  rdfs:seeAlso <http://vocab.getty.edu/aat/300004499> ;
  rdfs:seeAlso wd:Q258313 ;
  rdfs:subClassOf <https://w3id.org/con-tax/zones/aat-spaces#300004465> ;
.
<https://w3id.org/con-tax/zones/aat-spaces#300004503>
  rdf:type owl:Class ;
  rdfs:comment "Kamers (vaak rechthoekig) die zich aan de achterkant bevinden van koloniale huizen in New England en die dienden als een combinatie van keuken, woonkamer, en werkkamer."@nl ;
  rdfs:comment "Rooms (often rectangular) at the back of colonial houses in the United States, especially in the Northeast, which served as a combination kitchen, living room, and workroom."@en ;
  rdfs:isDefinedBy <https://w3id.org/con-tax/zones/aat-spaces> ;
  rdfs:label "keeping room"@nl ;
  rdfs:label "keeping rooms"@en-us ;
  rdfs:label "keeping rooms"@nl ;
  rdfs:seeAlso <http://vocab.getty.edu/aat/300004503> ;
  rdfs:subClassOf <https://w3id.org/con-tax/zones/aat-spaces#300133704> ;
.
<https://w3id.org/con-tax/zones/aat-spaces#300004505>
  rdf:type gvp:GuideTerm ;
  rdfs:isDefinedBy <https://w3id.org/con-tax/zones/aat-spaces> ;
  rdfs:label "<werk- en instructieruimte>"@nl ;
  rdfs:label "<werk- en instructieruimten>"@nl ;
  rdfs:label "<work and instructional spaces>"@en ;
  rdfs:label "werk- en instructieruimte"@nl ;
  rdfs:label "werk- en instructieruimten"@nl ;
  rdfs:seeAlso <http://vocab.getty.edu/aat/300004505> ;
  contax:containsConcept <https://w3id.org/con-tax/zones/aat-spaces#300004507> ;
  contax:containsConcept <https://w3id.org/con-tax/zones/aat-spaces#300004511> ;
  contax:containsConcept <https://w3id.org/con-tax/zones/aat-spaces#300004514> ;
  contax:containsConcept <https://w3id.org/con-tax/zones/aat-spaces#300004519> ;
  contax:containsConcept <https://w3id.org/con-tax/zones/aat-spaces#300004521> ;
  contax:containsConcept <https://w3id.org/con-tax/zones/aat-spaces#300004523> ;
  contax:containsConcept <https://w3id.org/con-tax/zones/aat-spaces#300004530> ;
  contax:containsConcept <https://w3id.org/con-tax/zones/aat-spaces#300004531> ;
  contax:containsConcept <https://w3id.org/con-tax/zones/aat-spaces#300005391> ;
  contax:containsConcept <https://w3id.org/con-tax/zones/aat-spaces#300005396> ;
  contax:containsConcept <https://w3id.org/con-tax/zones/aat-spaces#300006262> ;
  contax:containsConcept <https://w3id.org/con-tax/zones/aat-spaces#300007725> ;
  contax:containsConcept <https://w3id.org/con-tax/zones/aat-spaces#300065050> ;
  contax:containsConcept <https://w3id.org/con-tax/zones/aat-spaces#300122189> ;
  contax:containsConcept <https://w3id.org/con-tax/zones/aat-spaces#300124785> ;
  contax:containsConcept <https://w3id.org/con-tax/zones/aat-spaces#300179437> ;
  contax:containsConcept <https://w3id.org/con-tax/zones/aat-spaces#300256426> ;
  contax:containsConcept <https://w3id.org/con-tax/zones/aat-spaces#300411346> ;
.
<https://w3id.org/con-tax/zones/aat-spaces#300004506>
  rdf:type owl:Class ;
  rdfs:comment "Kamers met geluiddempende muren, speciaal ontworpen voor akoestische experimenten."@nl ;
  rdfs:comment "Specially constructed rooms with walls desgined with such sound-absorbency that the interior is as close to total silence as possible. They are generally used for scientific experiments."@en ;
  rdfs:isDefinedBy <https://w3id.org/con-tax/zones/aat-spaces> ;
  rdfs:label "anechoic rooms"@en ;
  rdfs:label "echovrije kamer"@nl ;
  rdfs:label "echovrije kamers"@nl ;
  rdfs:seeAlso <http://vocab.getty.edu/aat/300004506> ;
  rdfs:subClassOf <https://w3id.org/con-tax/zones/aat-spaces#300133704> ;
.
<https://w3id.org/con-tax/zones/aat-spaces#300004507>
  rdf:type owl:Class ;
  rdfs:comment "Rooms devoted to formal instruction in schools."@en ;
  rdfs:comment "Ruimten in scholen, bestemd voor het geven van onderwijs. Gebruik 'leslokalen' voor lesruimten in het algemeen."@nl ;
  rdfs:isDefinedBy <https://w3id.org/con-tax/zones/aat-spaces> ;
  rdfs:label "classrooms"@en ;
  rdfs:label "klaslokaal"@nl ;
  rdfs:label "klaslokalen"@nl ;
  rdfs:label "schoollokaal"@nl ;
  rdfs:label "schoollokalen"@nl ;
  rdfs:seeAlso <http://vocab.getty.edu/aat/300004507> ;
  rdfs:seeAlso wd:Q621114 ;
  rdfs:subClassOf <https://w3id.org/con-tax/zones/aat-spaces#300133704> ;
.
<https://w3id.org/con-tax/zones/aat-spaces#300004509>
  rdf:type owl:Class ;
  rdfs:comment "Kamers waarin moeite wordt gedaan om verontreiniging buiten te houden, inclusief luchtverontreiniging, door middel van  luchtfilters, matten of andere middelen, zoals in  computerkamers of ruimten waar precisie-instrumenten in elkaar worden gezet."@nl ;
  rdfs:comment "Rooms in which efforts are made to keep contamination out, including atmospheric pollutants, by the use of air filters, mats, or other devices, as in assembly rooms for precision products or computer rooms."@en ;
  rdfs:isDefinedBy <https://w3id.org/con-tax/zones/aat-spaces> ;
  rdfs:label "clean rooms"@en ;
  rdfs:label "steriele kamer"@nl ;
  rdfs:label "steriele kamers"@nl ;
  rdfs:seeAlso <http://vocab.getty.edu/aat/300004509> ;
  rdfs:seeAlso wd:Q794827 ;
  rdfs:subClassOf <https://w3id.org/con-tax/zones/aat-spaces#300133704> ;
.
<https://w3id.org/con-tax/zones/aat-spaces#300004510>
  rdf:type owl:Class ;
  rdfs:comment "In current usage, usually refers to rooms, located in offices or other public or commercial buildings, that are reserved for computer servers and have regulated temperature and humidity suited for the optimum operation and storage of computer equipment. In the recent past, before the advent of networked environments, the term often referred to rooms reserved for a number of stand-alone computers, often in a school or other facility offering training in the use of computers or computer applications; the term may occasionally have this meaning in the present."@en ;
  rdfs:isDefinedBy <https://w3id.org/con-tax/zones/aat-spaces> ;
  rdfs:label "computer rooms"@en ;
  rdfs:label "computerruimte"@nl ;
  rdfs:label "computerruimten"@nl ;
  rdfs:seeAlso <http://vocab.getty.edu/aat/300004510> ;
  rdfs:subClassOf <https://w3id.org/con-tax/zones/aat-spaces#300103941> ;
.
<https://w3id.org/con-tax/zones/aat-spaces#300004511>
  rdf:type owl:Class ;
  rdfs:comment "Rooms containing control equipment, common examples being in broadcasting stations, auditoriums, and theaters."@en ;
  rdfs:comment "Wordt gebruikt voor ruimten waarin zich aflees- en bedieningsapparatuur bevindt, zoals bijvoorbeeld in radio- en televisiestations, gehoorzalen en theaters, maar ook in ziekenhuizen en fabrieken."@nl ;
  rdfs:isDefinedBy <https://w3id.org/con-tax/zones/aat-spaces> ;
  rdfs:label "control rooms"@en ;
  rdfs:label "controlekamer"@nl ;
  rdfs:label "controlekamers"@nl ;
  rdfs:seeAlso <http://vocab.getty.edu/aat/300004511> ;
  rdfs:seeAlso wd:Q390516 ;
  rdfs:subClassOf <https://w3id.org/con-tax/zones/aat-spaces#300133704> ;
.
<https://w3id.org/con-tax/zones/aat-spaces#300004512>
  rdf:type owl:Class ;
  rdfs:comment "Kamers die zijn afgeschermd van licht of die verlicht worden door een dokalamp voor het bewerken en verwerken van lichtgevoelig materiaal."@nl ;
  rdfs:comment "Rooms freed from light or lighted by a safelight for handling and processing light-sensitive materials."@en ;
  rdfs:isDefinedBy <https://w3id.org/con-tax/zones/aat-spaces> ;
  rdfs:label "darkrooms"@en-us ;
  rdfs:label "doka"@nl ;
  rdfs:label "doka's"@nl ;
  rdfs:label "donkere kamer"@nl ;
  rdfs:label "donkere kamers"@nl ;
  rdfs:seeAlso <http://vocab.getty.edu/aat/300004512> ;
  rdfs:seeAlso wd:Q601413 ;
  rdfs:subClassOf <https://w3id.org/con-tax/zones/aat-spaces#300133704> ;
.
<https://w3id.org/con-tax/zones/aat-spaces#300004514>
  rdf:type owl:Class ;
  rdfs:comment "Rooms intended for the preparation and cooking of food."@en ;
  rdfs:comment "Ruimten bestemd voor de bereiding van voedsel."@nl ;
  rdfs:isDefinedBy <https://w3id.org/con-tax/zones/aat-spaces> ;
  rdfs:label "keuken"@nl ;
  rdfs:label "keukens"@nl ;
  rdfs:label "kitchens"@en ;
  rdfs:seeAlso <http://vocab.getty.edu/aat/300004514> ;
  rdfs:seeAlso wd:Q43164 ;
  rdfs:subClassOf <https://w3id.org/con-tax/zones/aat-spaces#300133704> ;
.
<https://w3id.org/con-tax/zones/aat-spaces#300004517>
  rdf:type owl:Class ;
  rdfs:comment "Kleine ruimten of gedeelten van grotere ruimten met de meest essentiële keukenuitrusting."@nl ;
  rdfs:comment "Small rooms or alcoves fitted with the essential conveniences of a kitchen."@en ;
  rdfs:isDefinedBy <https://w3id.org/con-tax/zones/aat-spaces> ;
  rdfs:label "kitchenette"@nl ;
  rdfs:label "kitchenettes"@en ;
  rdfs:label "kitchenettes"@nl ;
  rdfs:seeAlso <http://vocab.getty.edu/aat/300004517> ;
  rdfs:seeAlso wd:Q1804676 ;
  rdfs:subClassOf <https://w3id.org/con-tax/zones/aat-spaces#300004514> ;
.
<https://w3id.org/con-tax/zones/aat-spaces#300004519>
  rdf:type owl:Class ;
  rdfs:comment "Ruimten voor praktisch onderwijs en zelfstudie in vreemde talen met behulp van opname- en luisterapparatuur."@nl ;
  rdfs:comment "Special rooms with sound recording and reproducing equipment for use by students studying languages."@en ;
  rdfs:isDefinedBy <https://w3id.org/con-tax/zones/aat-spaces> ;
  rdfs:label "language laboratories"@en ;
  rdfs:label "talenpracticum"@nl ;
  rdfs:label "talenpracticums"@nl ;
  rdfs:seeAlso <http://vocab.getty.edu/aat/300004519> ;
  rdfs:seeAlso wd:Q958035 ;
  rdfs:subClassOf <https://w3id.org/con-tax/zones/aat-spaces#300133704> ;
.
<https://w3id.org/con-tax/zones/aat-spaces#300004520>
  rdf:type owl:Class ;
  rdfs:comment "Rooms devoted primarily to the playing of musical instruments or the giving of recitals, as in houses and hotels."@en ;
  rdfs:comment "Wordt gebruikt voor kamers die zijn bedoeld om muziek te maken of recitals te geven, bijvoorbeeld in huizen en hotels."@nl ;
  rdfs:isDefinedBy <https://w3id.org/con-tax/zones/aat-spaces> ;
  rdfs:label "music rooms"@en ;
  rdfs:label "muziekkamer"@nl ;
  rdfs:label "muziekkamers"@nl ;
  rdfs:seeAlso <http://vocab.getty.edu/aat/300004520> ;
  rdfs:seeAlso wd:Q21550795 ;
  rdfs:subClassOf <https://w3id.org/con-tax/zones/aat-spaces#300133704> ;
.
<https://w3id.org/con-tax/zones/aat-spaces#300004521>
  rdf:type owl:Class ;
  rdfs:comment "Rooms where business, administrative, or professional activities are conducted."@en ;
  rdfs:comment "Ruimten bestemd voor zakelijke, administratieve of financiële activiteiten. Gebruik 'praktijkruimten' voor ruimten bestemd voor medische of paramedische activiteiten."@nl ;
  rdfs:isDefinedBy <https://w3id.org/con-tax/zones/aat-spaces> ;
  rdfs:label "kantoor (kamer)"@nl ;
  rdfs:label "kantoor"@nl ;
  rdfs:label "kantoorruimten"@nl ;
  rdfs:label "kantoren (kamers)"@nl ;
  rdfs:label "kantoren"@nl ;
  rdfs:label "offices (work spaces)"@en ;
  rdfs:label "werkruimte"@nl ;
  rdfs:label "werkruimten"@nl ;
  rdfs:seeAlso <http://vocab.getty.edu/aat/300004521> ;
  rdfs:seeAlso wd:Q182060 ;
  rdfs:subClassOf <https://w3id.org/con-tax/zones/aat-spaces#300133704> ;
.
<https://w3id.org/con-tax/zones/aat-spaces#300004523>
  rdf:type owl:Class ;
  rdfs:comment "Rooms off the kitchen for storing and washing dishes and food."@en ;
  rdfs:comment "Ruimten naast keukens die worden gebruikt voor het afwassen en opbergen van serviesgoed en voor het wassen van etenswaren."@nl ;
  rdfs:isDefinedBy <https://w3id.org/con-tax/zones/aat-spaces> ;
  rdfs:label "afwaskeuken"@nl ;
  rdfs:label "afwaskeukens"@nl ;
  rdfs:label "sculleries"@en ;
  rdfs:seeAlso <http://vocab.getty.edu/aat/300004523> ;
  rdfs:seeAlso wd:Q2669066 ;
  rdfs:subClassOf <https://w3id.org/con-tax/zones/aat-spaces#300133704> ;
.
<https://w3id.org/con-tax/zones/aat-spaces#300004526>
  rdf:type owl:Class ;
  rdfs:comment "Rooms designed or used to house heating, laundry, or general maintenance equipment."@en ;
  rdfs:comment "Ruimten voor centrale verwarmingsinstallaties, soms ook om te wassen en was te drogen en voor materiaal voor algemeen onderhoud."@nl ;
  rdfs:isDefinedBy <https://w3id.org/con-tax/zones/aat-spaces> ;
  rdfs:label "bijkeuken"@nl ;
  rdfs:label "bijkeukens"@nl ;
  rdfs:label "utility rooms"@en ;
  rdfs:seeAlso <http://vocab.getty.edu/aat/300004526> ;
  rdfs:seeAlso wd:Q7902854 ;
  rdfs:subClassOf <https://w3id.org/con-tax/zones/aat-spaces#300133704> ;
.
<https://w3id.org/con-tax/zones/aat-spaces#300004527>
  rdf:type owl:Class ;
  rdfs:comment "Ruimten voor de boilers die worden gebruikt voor verwarming, ventilatie of energieopwekking."@nl ;
  rdfs:comment "Spaces provided for the boilers used for heating, ventilation, or power generation."@en ;
  rdfs:isDefinedBy <https://w3id.org/con-tax/zones/aat-spaces> ;
  rdfs:label "boiler rooms"@en ;
  rdfs:label "ketelruimte"@nl ;
  rdfs:label "ketelruimten"@nl ;
  rdfs:seeAlso <http://vocab.getty.edu/aat/300004527> ;
  rdfs:subClassOf <https://w3id.org/con-tax/zones/aat-spaces#300004526> ;
.
<https://w3id.org/con-tax/zones/aat-spaces#300004530>
  rdf:type owl:Class ;
  rdfs:comment "Rooms or groups of rooms equipped for washing, drying, and ironing clothes."@en ;
  rdfs:comment "Ruimten bedoeld voor het wassen, drogen en strijken van wasgoed."@nl ;
  rdfs:isDefinedBy <https://w3id.org/con-tax/zones/aat-spaces> ;
  rdfs:label "laundry rooms"@en ;
  rdfs:label "waskeuken"@nl ;
  rdfs:label "waskeukens"@nl ;
  rdfs:seeAlso <http://vocab.getty.edu/aat/300004530> ;
  rdfs:seeAlso wd:Q267734 ;
  rdfs:subClassOf <https://w3id.org/con-tax/zones/aat-spaces#300133704> ;
.
<https://w3id.org/con-tax/zones/aat-spaces#300004531>
  rdf:type owl:Class ;
  rdfs:comment "Refers to public or private spaces set aside for manual or light industrial work. It may be used to refer to spaces in which fine art was created, particularly regarding art dating prior to the 16th century. It may also refer to spaces in which woodworkers, furniture makers, pottery makers, glass makers, and other craftspeople work. In the most general sense, it refers to spaces where goods of any type are made, prepared for sale, or sold. In modern usage, the term \"studios\" is generally used to refer to spaces for creating fine art dating from the 16th century to the present. "@en ;
  rdfs:comment "Verwijst naar openbare of particuliere ruimten die bedoeld zijn voor de uitvoering van handwerk of lichte industriële arbeid. De term kan verwijzen naar ruimten waarin kunst werd vervaardigd, met name in relatie tot kunstvoorwerpen van voor de 16de eeuw. Ook kan de term verwijzen naar ruimten waarin houtbewerkers, schrijnwerkers, pottenbakkers, glasblazers en andere ambachtslieden werkzaam zijn. In de meest algemene betekenis verwijst de term naar ruimten waarin goederen van allerlei aard worden vervaardigd, voor verkoop worden gereedgemaakt of verkocht. In het moderne taalgebruik wordt doorgaans de term 'ateliers' gebruikt om te verwijzen naar ruimten waarin kunst wordt vervaardigd, in de periode vanaf de 16de eeuw tot heden."@nl ;
  rdfs:isDefinedBy <https://w3id.org/con-tax/zones/aat-spaces> ;
  rdfs:label "werkplaats (werk- en instructieruimte)"@nl ;
  rdfs:label "werkplaats"@nl ;
  rdfs:label "werkplaatsen (werk- en instructieruimten)"@nl ;
  rdfs:label "werkplaatsen"@nl ;
  rdfs:label "workshops (work spaces)"@en ;
  rdfs:seeAlso <http://vocab.getty.edu/aat/300004531> ;
  rdfs:seeAlso wd:Q656720 ;
  rdfs:subClassOf <https://w3id.org/con-tax/zones/aat-spaces#300133704> ;
.
<https://w3id.org/con-tax/zones/aat-spaces#300004536>
  rdf:type owl:Class ;
  rdfs:comment "Rooms or spaces in buildings that are used for health facilities."@en ;
  rdfs:isDefinedBy <https://w3id.org/con-tax/zones/aat-spaces> ;
  rdfs:label "health facility spaces"@en ;
  rdfs:label "ruimte voor gezondheidszorg"@nl ;
  rdfs:label "ruimten voor gezondheidszorg"@nl ;
  rdfs:seeAlso <http://vocab.getty.edu/aat/300004536> ;
  rdfs:subClassOf <https://w3id.org/con-tax/zones/aat-spaces#300133704> ;
.
<https://w3id.org/con-tax/zones/aat-spaces#300004540>
  rdf:type owl:Class ;
  rdfs:comment "Hospital areas equipped and staffed for the prompt treatment of acute illness, trauma, or other medical emergencies."@en ;
  rdfs:comment "Ziekenhuisafdelingen of gebouwen bemand en ingericht voor de onmiddellijke behandeling van acute ziekten of ongevaltrauma's."@nl ;
  rdfs:isDefinedBy <https://w3id.org/con-tax/zones/aat-spaces> ;
  rdfs:label "eerstehulpafdeling"@nl ;
  rdfs:label "eerstehulpafdelingen"@nl ;
  rdfs:label "emergency rooms"@en ;
  rdfs:seeAlso <http://vocab.getty.edu/aat/300004540> ;
  rdfs:seeAlso wd:Q1295316 ;
  rdfs:subClassOf <https://w3id.org/con-tax/zones/aat-spaces#300004536> ;
.
<https://w3id.org/con-tax/zones/aat-spaces#300004543>
  rdf:type owl:Class ;
  rdfs:comment "Divisions, floors, or rooms of hospitals for a particular type or group of patients."@en ;
  rdfs:comment "Groepen ruimten, verdiepingen of afzonderlijke ruimten in (medische) zorginstellingen voor een bepaald type of een bepaalde groep patiënten."@nl ;
  rdfs:isDefinedBy <https://w3id.org/con-tax/zones/aat-spaces> ;
  rdfs:label "hospital wards"@en ;
  rdfs:label "ziekenzaal"@nl ;
  rdfs:label "ziekenzalen"@nl ;
  rdfs:seeAlso <http://vocab.getty.edu/aat/300004543> ;
  rdfs:subClassOf <https://w3id.org/con-tax/zones/aat-spaces#300004536> ;
.
<https://w3id.org/con-tax/zones/aat-spaces#300004552>
  rdf:type owl:Class ;
  rdfs:comment "Areas in hospitals for critically ill patients requiring especially close surveillance and special life-support equipment."@en ;
  rdfs:comment "Ruimten in ziekenhuizen voor ernstig zieke patiënten die speciale zorg en aandacht behoeven."@nl ;
  rdfs:isDefinedBy <https://w3id.org/con-tax/zones/aat-spaces> ;
  rdfs:label "bewakingsafdeling"@nl ;
  rdfs:label "bewakingsafdelingen"@nl ;
  rdfs:label "intensive care units"@en ;
  rdfs:label "intensivecareafdeling"@nl ;
  rdfs:label "intensivecareafdelingen"@nl ;
  rdfs:seeAlso <http://vocab.getty.edu/aat/300004552> ;
  rdfs:seeAlso wd:Q5094647 ;
  rdfs:subClassOf <https://w3id.org/con-tax/zones/aat-spaces#300004543> ;
.
<https://w3id.org/con-tax/zones/aat-spaces#300004554>
  rdf:type owl:Class ;
  rdfs:comment "Intensive care units devoted to the treatment of burn victims."@en ;
  rdfs:comment "Ruimten in ziekenhuizen of ook wel afzonderlijke gebouwen voor de verpleging van brandwondenpatiënten."@nl ;
  rdfs:isDefinedBy <https://w3id.org/con-tax/zones/aat-spaces> ;
  rdfs:label "brandwondencentra"@nl ;
  rdfs:label "brandwondencentrum"@nl ;
  rdfs:label "burn units"@en ;
  rdfs:seeAlso <http://vocab.getty.edu/aat/300004554> ;
  rdfs:seeAlso wd:Q2151257 ;
  rdfs:subClassOf <https://w3id.org/con-tax/zones/aat-spaces#300004552> ;
.
<https://w3id.org/con-tax/zones/aat-spaces#300004555>
  rdf:type owl:Class ;
  rdfs:comment "Areas located in a hospital or other health care facility and containing beds and specialized equipment for the care of patients with coronary disease or recovering from heart surgery."@en ;
  rdfs:isDefinedBy <https://w3id.org/con-tax/zones/aat-spaces> ;
  rdfs:label "coronary care units"@en ;
  rdfs:label "hartbewakingsafdeling"@nl ;
  rdfs:label "hartbewakingsafdelingen"@nl ;
  rdfs:seeAlso <http://vocab.getty.edu/aat/300004555> ;
  rdfs:seeAlso wd:Q2604639 ;
  rdfs:subClassOf <https://w3id.org/con-tax/zones/aat-spaces#300004552> ;
.
<https://w3id.org/con-tax/zones/aat-spaces#300004556>
  rdf:type owl:Class ;
  rdfs:comment "Hospital rooms which are equipped with apparatus for meeting post-operative emergencies and in which surgical patients are kept during the immediate post-operative period for care and recovery from anesthesia."@en ;
  rdfs:comment "Ruimten in ziekenhuizen uitgerust met apparaten om postoperatieve noodsituaties op te vangen en waarin geopereerde patiënten verblijven gedurende de periode vlak na de operatie tot het ontwaken uit de verdoving."@nl ;
  rdfs:isDefinedBy <https://w3id.org/con-tax/zones/aat-spaces> ;
  rdfs:label "recoverkamer"@nl ;
  rdfs:label "recoverkamers"@nl ;
  rdfs:label "recovery rooms"@en ;
  rdfs:label "uitslaapkamer"@nl ;
  rdfs:label "uitslaapkamers"@nl ;
  rdfs:label "verkoeverkamer"@nl ;
  rdfs:label "verkoeverkamers"@nl ;
  rdfs:seeAlso <http://vocab.getty.edu/aat/300004556> ;
  rdfs:seeAlso wd:Q760111 ;
  rdfs:subClassOf <https://w3id.org/con-tax/zones/aat-spaces#300004536> ;
.
<https://w3id.org/con-tax/zones/aat-spaces#300004557>
  rdf:type owl:Class ;
  rdfs:comment "Ruimten, meestal in ziekenhuizen, waar chirurgische handelingen worden verricht."@nl ;
  rdfs:comment "Specially equipped rooms, usually in hospitals, where surgical procedures are performed."@en ;
  rdfs:isDefinedBy <https://w3id.org/con-tax/zones/aat-spaces> ;
  rdfs:label "operatiekamer"@nl ;
  rdfs:label "operatiekamers"@nl ;
  rdfs:label "operating rooms"@en-us ;
  rdfs:seeAlso <http://vocab.getty.edu/aat/300004557> ;
  rdfs:seeAlso wd:Q1060822 ;
  rdfs:subClassOf <https://w3id.org/con-tax/zones/aat-spaces#300004536> ;
.
<https://w3id.org/con-tax/zones/aat-spaces#300004559>
  rdf:type owl:Class ;
  rdfs:comment "Rooms and other spaces within churches, temples, synagogues, mosques, and other religious buildings."@en ;
  rdfs:isDefinedBy <https://w3id.org/con-tax/zones/aat-spaces> ;
  rdfs:label "religious building spaces"@en ;
  rdfs:label "ruimte in religieus gebouw"@nl ;
  rdfs:label "ruimten in religieuze gebouwen"@nl ;
  rdfs:seeAlso <http://vocab.getty.edu/aat/300004559> ;
  rdfs:subClassOf <https://w3id.org/con-tax/zones/aat-spaces#300133704> ;
.
<https://w3id.org/con-tax/zones/aat-spaces#300004560>
  rdf:type owl:Class ;
  rdfs:comment "Spaces or rooms located in Christian religious buildings. "@en ;
  rdfs:isDefinedBy <https://w3id.org/con-tax/zones/aat-spaces> ;
  rdfs:label "Christian religious building spaces"@en ;
  rdfs:label "ruimte in Christelijk religieus gebouw"@nl ;
  rdfs:label "ruimten in Christelijke religieuze gebouwen"@nl ;
  rdfs:seeAlso <http://vocab.getty.edu/aat/300004560> ;
  rdfs:subClassOf <https://w3id.org/con-tax/zones/aat-spaces#300004559> ;
.
<https://w3id.org/con-tax/zones/aat-spaces#300004565>
  rdf:type owl:Class ;
  rdfs:comment "Ruimten in christelijke kerken waarin zich het hoogaltaar bevindt en die gereserveerd zijn voor gebruik door geestelijken. Behelst ook het zangkoor wanneer dat aanwezig is. Gebruik 'zangkoren' voor de ruimten in christelijke kerken die zich doorgaans tussen de altaarruimte en het schip bevinden en die zijn gereserveerd voor koorzangers."@nl ;
  rdfs:comment "Spaces in Christian churches containing the high altar and reserved for the use of the clergy. Includes the choir when present. Use \"choirs\" for the spaces in Christian churches, generally between the altar area and the nave, reserved for choristers."@en ;
  rdfs:isDefinedBy <https://w3id.org/con-tax/zones/aat-spaces> ;
  rdfs:label "chancels"@en ;
  rdfs:label "koor"@nl ;
  rdfs:label "koren"@nl ;
  rdfs:seeAlso <http://vocab.getty.edu/aat/300004565> ;
  rdfs:seeAlso wd:Q14616641 ;
  rdfs:subClassOf <https://w3id.org/con-tax/zones/aat-spaces#300004560> ;
.
<https://w3id.org/con-tax/zones/aat-spaces#300004566>
  rdf:type owl:Class ;
  rdfs:comment "Ruimten van een opgedeeld koor die het verst van het sanctuarium verwijderd liggen."@nl ;
  rdfs:comment "Spaces of a divided choir farthest from the sanctuary, or the enclosed spaces between the inner and outer gates of deep choir screens."@en ;
  rdfs:isDefinedBy <https://w3id.org/con-tax/zones/aat-spaces> ;
  rdfs:label "antechoirs"@en-us ;
  rdfs:label "voorkoor"@nl ;
  rdfs:label "voorkoren"@nl ;
  rdfs:seeAlso <http://vocab.getty.edu/aat/300004566> ;
  rdfs:subClassOf <https://w3id.org/con-tax/zones/aat-spaces#300004560> ;
.
<https://w3id.org/con-tax/zones/aat-spaces#300004573>
  rdf:type owl:Class ;
  rdfs:comment "Refers to those areas of a church situated behind the high altar; often found in English Medieval architecture."@en ;
  rdfs:comment "Ruimten in hoofdzakelijk middeleeuwse kerken in Engeland die zich achter het hoogaltaar bevinden."@nl ;
  rdfs:isDefinedBy <https://w3id.org/con-tax/zones/aat-spaces> ;
  rdfs:label "achterkoor"@nl ;
  rdfs:label "achterkoren"@nl ;
  rdfs:label "retrochoirs"@en ;
  rdfs:seeAlso <http://vocab.getty.edu/aat/300004573> ;
  rdfs:seeAlso wd:Q5638212 ;
  rdfs:subClassOf <https://w3id.org/con-tax/zones/aat-spaces#300004560> ;
.
<https://w3id.org/con-tax/zones/aat-spaces#300004575>
  rdf:type owl:Class ;
  rdfs:comment "De meest gewijde plaatsen in religieuze gebouwen. In een christelijke kerk is het de ruimte waarin zich het hoofdaltaar bevindt."@nl ;
  rdfs:comment "Refers to the most sacred spaces of religious buildings; in a Christian church, the area containing the main altar."@en ;
  rdfs:isDefinedBy <https://w3id.org/con-tax/zones/aat-spaces> ;
  rdfs:label "sanctuaria"@nl ;
  rdfs:label "sanctuaries (religious building spaces)"@en ;
  rdfs:label "sanctuarium"@nl ;
  rdfs:seeAlso <http://vocab.getty.edu/aat/300004575> ;
  rdfs:seeAlso wd:Q47848 ;
  rdfs:subClassOf <https://w3id.org/con-tax/zones/aat-spaces#300004559> ;
.
<https://w3id.org/con-tax/zones/aat-spaces#300004590>
  rdf:type owl:Class ;
  rdfs:comment "Rooms or small buildings that serve as sanctuaries or places of Christian worship; often having an altar. A chapel may be used for private worship in or attached to a church, palace, house, prison, monastery, or school. It may alternatively be used for public worship of the established Church, subordinate to or dependent upon the parish church, the accommodation supplied by which it in some way supplements. The concept includes both freestanding chapels and rooms or recesses serving as chapels in churches or other buildings. The Latin \"cappella\" or the French-derived \"chappelle\" or \"chapelle\" are occasionally used for \"chapel\" in English texts. In its original meaning, the term referred specifically to the shrine in which the kings of France preserved the cape (cloak) of St. Martin."@en ;
  rdfs:comment "Ruimten of kleine gebouwen die dienst doen als sanctuarium of christelijke gebedsplaats. Een kapel kan worden gebruikt voor besloten erediensten in of verbonden aan een kerk, paleis, huis, gevangenis, klooster of school. De kapel kan ook worden gebruikt voor openbare erediensten van de staatskerk, ondergeschikt aan of afhankelijk van de parochiekerk, waarvan de accommodatie op een bepaalde manier wordt aangevuld door de kapel. Het concept omvat zowel vrijstaande kapellen als ruimten die dienst doen als kapel in kerken of overige gebouwen. Het Latijnse 'cappella' wordt soms ook gebruikt voor 'kapel'. De term wordt soms ook gebruikt in de oorspronkelijke betekenis, waarbij specifiek werd verwezen naar het heiligdom waarin de koningen van Frankrijk de mantel van St. Martin bewaarden."@nl ;
  rdfs:isDefinedBy <https://w3id.org/con-tax/zones/aat-spaces> ;
  rdfs:label "chapels (rooms or structures)"@en ;
  rdfs:label "kapel"@nl ;
  rdfs:label "kapellen (ruimten of constructies)"@nl ;
  rdfs:label "kapellen"@nl ;
  rdfs:seeAlso <http://vocab.getty.edu/aat/300004590> ;
  rdfs:seeAlso wd:Q108325 ;
  rdfs:subClassOf <https://w3id.org/con-tax/zones/aat-spaces#300004560> ;
.
<https://w3id.org/con-tax/zones/aat-spaces#300004591>
  rdf:type owl:Class ;
  rdfs:comment "Chapels at the west end of Byzantine churches, especially of the Armenian type."@en ;
  rdfs:comment "Kapellen aan de westkant van Byzantijnse kerken, vooral van het Armeense type."@nl ;
  rdfs:isDefinedBy <https://w3id.org/con-tax/zones/aat-spaces> ;
  rdfs:label "antiparabema"@nl ;
  rdfs:label "antiparabemata"@en ;
  rdfs:label "antiparabemata"@nl ;
  rdfs:seeAlso <http://vocab.getty.edu/aat/300004591> ;
  rdfs:subClassOf <https://w3id.org/con-tax/zones/aat-spaces#300004590> ;
.
<https://w3id.org/con-tax/zones/aat-spaces#300004593>
  rdf:type owl:Class ;
  rdfs:comment "Kleine apsissen, vooral die aan grotere apsissen of kooromgangen zijn gebouwd."@nl ;
  rdfs:comment "Small apses, especially those which project from a larger apse."@en ;
  rdfs:isDefinedBy <https://w3id.org/con-tax/zones/aat-spaces> ;
  rdfs:label "apsidiolen"@nl ;
  rdfs:label "apsidioles"@en ;
  rdfs:label "apsidiool"@nl ;
  rdfs:seeAlso <http://vocab.getty.edu/aat/300004593> ;
  rdfs:subClassOf <https://w3id.org/con-tax/zones/aat-spaces#300004607> ;
.
<https://w3id.org/con-tax/zones/aat-spaces#300004599>
  rdf:type owl:Class ;
  rdfs:comment "Major chapels dedicated to the Virgin Mary, usually located in the axis of a church at its east end."@en ;
  rdfs:comment "Op zichzelf staande kapelletjes of deel van kerken gewijd aan Maria."@nl ;
  rdfs:isDefinedBy <https://w3id.org/con-tax/zones/aat-spaces> ;
  rdfs:label "Mariakapel"@nl ;
  rdfs:label "Mariakapellen"@nl ;
  rdfs:label "lady chapels"@en ;
  rdfs:seeAlso <http://vocab.getty.edu/aat/300004599> ;
  rdfs:seeAlso wd:Q1800075 ;
  rdfs:subClassOf <https://w3id.org/con-tax/zones/aat-spaces#300004590> ;
.
<https://w3id.org/con-tax/zones/aat-spaces#300004606>
  rdf:type owl:Class ;
  rdfs:comment "Combination of apse, ambulatory, and usually radial chapels of a church, especially French Gothic."@en ;
  rdfs:comment "Gedeelten van christelijke kerken aan de oostzijde van het koor, vaak bestaande uit apsis, kooromgang en straalkapellen."@nl ;
  rdfs:isDefinedBy <https://w3id.org/con-tax/zones/aat-spaces> ;
  rdfs:label "chevets (building spaces)"@en ;
  rdfs:label "koorsluiting"@nl ;
  rdfs:label "koorsluitingen"@nl ;
  rdfs:seeAlso <http://vocab.getty.edu/aat/300004606> ;
  rdfs:subClassOf <https://w3id.org/con-tax/zones/aat-spaces#300004560> ;
.
<https://w3id.org/con-tax/zones/aat-spaces#300004607>
  rdf:type owl:Class ;
  rdfs:comment "Halfronde of polygonale aanbouwen aan een grotere ruimte. Gebruikelijk in Romeinse basilieken en christelijke kerken."@nl ;
  rdfs:comment "Semicircular or polygonal extensions off of a larger space; common in Roman basilicas and Christian churches."@en ;
  rdfs:isDefinedBy <https://w3id.org/con-tax/zones/aat-spaces> ;
  rdfs:label "absis"@nl ;
  rdfs:label "absissen"@nl ;
  rdfs:label "apses"@en ;
  rdfs:label "apsis"@nl ;
  rdfs:label "apsissen"@nl ;
  rdfs:seeAlso <http://vocab.getty.edu/aat/300004607> ;
  rdfs:subClassOf <https://w3id.org/con-tax/zones/aat-spaces#300078790> ;
.
<https://w3id.org/con-tax/zones/aat-spaces#300004608>
  rdf:type owl:Class ;
  rdfs:comment "Apsissen die tegenover andere apsissen zijn geplaatst."@nl ;
  rdfs:comment "Refers to apses situated opposite other apses."@en ;
  rdfs:isDefinedBy <https://w3id.org/con-tax/zones/aat-spaces> ;
  rdfs:label "contra-apsis"@nl ;
  rdfs:label "contra-apsissen"@nl ;
  rdfs:label "counter apses"@en ;
  rdfs:seeAlso <http://vocab.getty.edu/aat/300004608> ;
  rdfs:subClassOf <https://w3id.org/con-tax/zones/aat-spaces#300004607> ;
.
<https://w3id.org/con-tax/zones/aat-spaces#300004614>
  rdf:type owl:Class ;
  rdfs:comment "Kamers of gebouwen die worden gebruikt voor geheime en non-conformistische erediensten."@nl ;
  rdfs:comment "Rooms or buildings used for secret or nonconformist worship."@en ;
  rdfs:isDefinedBy <https://w3id.org/con-tax/zones/aat-spaces> ;
  rdfs:label "conventicles"@en ;
  rdfs:label "conventikels"@nl ;
  rdfs:label "schuilkerk"@nl ;
  rdfs:label "schuilkerken"@nl ;
  rdfs:seeAlso <http://vocab.getty.edu/aat/300004614> ;
  rdfs:subClassOf <https://w3id.org/con-tax/zones/aat-spaces#300004560> ;
.
<https://w3id.org/con-tax/zones/aat-spaces#300004615>
  rdf:type owl:Class ;
  rdfs:comment "Plaatsen in christelijke kerken waar een transept het schip kruist."@nl ;
  rdfs:comment "Places in churches where a transept crosses the nave."@en ;
  rdfs:isDefinedBy <https://w3id.org/con-tax/zones/aat-spaces> ;
  rdfs:label "crossings (building spaces)"@en ;
  rdfs:label "kruising"@nl ;
  rdfs:label "kruisingen"@nl ;
  rdfs:label "viering (ruimte)"@nl ;
  rdfs:label "viering"@nl ;
  rdfs:label "vieringen (ruimten)"@nl ;
  rdfs:label "vieringen"@nl ;
  rdfs:seeAlso <http://vocab.getty.edu/aat/300004615> ;
  rdfs:subClassOf <https://w3id.org/con-tax/zones/aat-spaces#300004560> ;
.
<https://w3id.org/con-tax/zones/aat-spaces#300004618>
  rdf:type owl:Class ;
  rdfs:comment "Subterranean rooms or entire stories in churches, often serving as places of burial."@en ;
  rdfs:comment "Wordt gebruikt voor ondergrondse ruimten onder het altaarhuis of volledige verdiepingen onder kerken, die vaak als begraafplaatsen dienen."@nl ;
  rdfs:isDefinedBy <https://w3id.org/con-tax/zones/aat-spaces> ;
  rdfs:label "crypte"@nl ;
  rdfs:label "crypten"@nl ;
  rdfs:label "crypts"@en ;
  rdfs:seeAlso <http://vocab.getty.edu/aat/300004618> ;
  rdfs:seeAlso wd:Q192619 ;
  rdfs:subClassOf <https://w3id.org/con-tax/zones/aat-spaces#300004560> ;
.
<https://w3id.org/con-tax/zones/aat-spaces#300004624>
  rdf:type owl:Class ;
  rdfs:comment "Entrance porches in early basilican churches, and for interior vestibules across the western end of later churches. For narthexlike spaces at the west end of some English and French Romanesque and Gothic churches, often used as chapels, prefer \"galilees.\""@en ;
  rdfs:comment "Westportalen van vroeg-christelijke basilica's, en westelijke ingangsportalen van latere kerken. Gebruik 'galilea's' voor voorkerken aan de westkant van sommige grote kloosterkerken uit de 10e tot 12e eeuw."@nl ;
  rdfs:isDefinedBy <https://w3id.org/con-tax/zones/aat-spaces> ;
  rdfs:label "narthex"@nl ;
  rdfs:label "narthexen"@nl ;
  rdfs:label "narthexes"@en ;
  rdfs:seeAlso <http://vocab.getty.edu/aat/300004624> ;
  rdfs:seeAlso wd:Q208576 ;
  rdfs:subClassOf <https://w3id.org/con-tax/zones/aat-spaces#300004259> ;
  rdfs:subClassOf <https://w3id.org/con-tax/zones/aat-spaces#300004560> ;
.
<https://w3id.org/con-tax/zones/aat-spaces#300004625>
  rdf:type owl:Class ;
  rdfs:comment "Inner narthexes where there is also an outer narthex (the exonarthex)."@en ;
  rdfs:comment "Naar binnen geopende narthexen. Zie ook 'exonarthexen': narthexen die naar buiten geopend zijn."@nl ;
  rdfs:isDefinedBy <https://w3id.org/con-tax/zones/aat-spaces> ;
  rdfs:label "esonarthex"@nl ;
  rdfs:label "esonarthexen"@nl ;
  rdfs:label "esonarthexes"@en ;
  rdfs:seeAlso <http://vocab.getty.edu/aat/300004625> ;
  rdfs:subClassOf <https://w3id.org/con-tax/zones/aat-spaces#300004624> ;
.
<https://w3id.org/con-tax/zones/aat-spaces#300004626>
  rdf:type owl:Class ;
  rdfs:comment "Naar buiten geopende narthexen. Zie ook 'esonarthexen': narthexen die naar binnen geopend zijn."@nl ;
  rdfs:comment "The outer narthexes where there is also an inner narthex (the esonarthex)."@en ;
  rdfs:isDefinedBy <https://w3id.org/con-tax/zones/aat-spaces> ;
  rdfs:label "exonarthex"@nl ;
  rdfs:label "exonarthexen"@nl ;
  rdfs:label "exonarthexes"@en ;
  rdfs:seeAlso <http://vocab.getty.edu/aat/300004626> ;
  rdfs:subClassOf <https://w3id.org/con-tax/zones/aat-spaces#300004624> ;
.
<https://w3id.org/con-tax/zones/aat-spaces#300004627>
  rdf:type owl:Class ;
  rdfs:comment "Refers to the main central part of an interior divided into a high center with lower side portions divided by columns or piers, usually but not always in a church. Use also for the main part of a church without aisles but with a distinct chancel."@en ;
  rdfs:comment "Rompen van kerken, onderscheiden van het koor en eventuele voorbouwsels aan de tegenovergestelde zijde (torens, westwerk). Het schip is eenbeukig of onderverdeeld in middenbeuk of -schip en zijbeuken of -schepen. VWB"@nl ;
  rdfs:isDefinedBy <https://w3id.org/con-tax/zones/aat-spaces> ;
  rdfs:label "naves"@en ;
  rdfs:label "schepen (kerkruimten)"@nl ;
  rdfs:label "schepen"@nl ;
  rdfs:label "schip (binnenruimte)"@nl ;
  rdfs:label "schip"@nl ;
  rdfs:seeAlso <http://vocab.getty.edu/aat/300004627> ;
  rdfs:seeAlso wd:Q188714 ;
  rdfs:subClassOf <https://w3id.org/con-tax/zones/aat-spaces#300078790> ;
.
<https://w3id.org/con-tax/zones/aat-spaces#300004631>
  rdf:type owl:Class ;
  rdfs:comment "Rooms in or attached to churches where the sacred vessels and other treasures are kept. Vestments may also be stored here and the space used by the celebrants to dress for the services. For rooms used primarily for dressing for the services, use \"vestries (dressing rooms),\" although in modern usage, particularly for newer and smaller churches, the vestry and the sacristy are often the same room."@en ;
  rdfs:comment "Ruimten in of aan kerken waar de liturgische voorwerpen en misgewaden worden bewaard."@nl ;
  rdfs:isDefinedBy <https://w3id.org/con-tax/zones/aat-spaces> ;
  rdfs:label "sacristie"@nl ;
  rdfs:label "sacristies (religious spaces)"@en ;
  rdfs:label "sacristieën"@nl ;
  rdfs:seeAlso <http://vocab.getty.edu/aat/300004631> ;
  rdfs:seeAlso wd:Q468939 ;
  rdfs:subClassOf <https://w3id.org/con-tax/zones/aat-spaces#300004560> ;
.
<https://w3id.org/con-tax/zones/aat-spaces#300004635>
  rdf:type owl:Class ;
  rdfs:comment "Rooms for keeping the valuables of a church."@en ;
  rdfs:comment "Ruimten om de kostbaarheden van een kerk te bewaren."@nl ;
  rdfs:isDefinedBy <https://w3id.org/con-tax/zones/aat-spaces> ;
  rdfs:label "cimeliarch"@nl ;
  rdfs:label "cimeliarchs"@en ;
  rdfs:label "cimeliarchs"@nl ;
  rdfs:seeAlso <http://vocab.getty.edu/aat/300004635> ;
  rdfs:subClassOf <https://w3id.org/con-tax/zones/aat-spaces#300006050> ;
.
<https://w3id.org/con-tax/zones/aat-spaces#300004636>
  rdf:type owl:Class ;
  rdfs:comment "Sacristies in Orthodox Eastern and Byzantine churches."@en ;
  rdfs:comment "Sacristieën in oosters-orthodoxe en Byzantijnse kerken."@nl ;
  rdfs:isDefinedBy <https://w3id.org/con-tax/zones/aat-spaces> ;
  rdfs:label "diaconica"@en ;
  rdfs:label "diakonie"@nl ;
  rdfs:label "diakonieën"@nl ;
  rdfs:seeAlso <http://vocab.getty.edu/aat/300004636> ;
  rdfs:seeAlso wd:Q1283862 ;
  rdfs:subClassOf <https://w3id.org/con-tax/zones/aat-spaces#300004631> ;
.
<https://w3id.org/con-tax/zones/aat-spaces#300004645>
  rdf:type owl:Class ;
  rdfs:comment "Dwarsarmen van kruisvormige kerken."@nl ;
  rdfs:comment "Transverse arms of cruciform buildings, usually churches."@en ;
  rdfs:isDefinedBy <https://w3id.org/con-tax/zones/aat-spaces> ;
  rdfs:label "dwarsbeuken"@nl ;
  rdfs:label "transept"@nl ;
  rdfs:label "transepten"@nl ;
  rdfs:label "transepts"@en ;
  rdfs:seeAlso <http://vocab.getty.edu/aat/300004645> ;
  rdfs:seeAlso wd:Q202949 ;
  rdfs:subClassOf <https://w3id.org/con-tax/zones/aat-spaces#300004560> ;
.
<https://w3id.org/con-tax/zones/aat-spaces#300004651>
  rdf:type owl:Class ;
  rdfs:comment "Spaces or rooms located in temples. "@en ;
  rdfs:isDefinedBy <https://w3id.org/con-tax/zones/aat-spaces> ;
  rdfs:label "tempelruimte"@nl ;
  rdfs:label "tempelruimten"@nl ;
  rdfs:label "temple spaces"@en ;
  rdfs:seeAlso <http://vocab.getty.edu/aat/300004651> ;
  rdfs:subClassOf <https://w3id.org/con-tax/zones/aat-spaces#300004559> ;
.
<https://w3id.org/con-tax/zones/aat-spaces#300004652>
  rdf:type owl:Class ;
  rdfs:comment "Kleine binnenkamers grenzend aan of binnenin de naos, te vinden in sommige oude Griekse tempels."@nl ;
  rdfs:comment "Small inner rooms adjacent to or within the naos, found in some ancient temples."@en ;
  rdfs:isDefinedBy <https://w3id.org/con-tax/zones/aat-spaces> ;
  rdfs:label "adyta"@en ;
  rdfs:label "adyton"@nl ;
  rdfs:label "adytons"@nl ;
  rdfs:seeAlso <http://vocab.getty.edu/aat/300004652> ;
  rdfs:subClassOf <https://w3id.org/con-tax/zones/aat-spaces#300004651> ;
.
<https://w3id.org/con-tax/zones/aat-spaces#300004658>
  rdf:type owl:Class ;
  rdfs:comment "Meestal gebruikt om te verwijzen naar de belangrijkste inwendige ruimte van een Griekse tempel, met daarin het beeld van een godheid, hoewel het woord soms ook als synoniem van 'cella' wordt gebruikt."@nl ;
  rdfs:comment "Principal interior chambers or architectural cores of certain religious buildings or sanctuaries. Among examples are ancient Greek architecture, where the naos was the main sanctuary of a temple; in Byzantine architecture, where the naos was typically the area of a centrally planned church reserved for the liturgy; and in Egyptian architecture and art, where the naos was a shrine housing the god or carried in miniature by the god."@en ;
  rdfs:isDefinedBy <https://w3id.org/con-tax/zones/aat-spaces> ;
  rdfs:label "naoi (chambers)"@en ;
  rdfs:label "naoi"@nl ;
  rdfs:label "naos"@nl ;
  rdfs:seeAlso <http://vocab.getty.edu/aat/300004658> ;
  rdfs:subClassOf <https://w3id.org/con-tax/zones/aat-spaces#300004559> ;
.
<https://w3id.org/con-tax/zones/aat-spaces#300004662>
  rdf:type owl:Class ;
  rdfs:comment "Ruimten aan de achterzijden van Griekse tempels. VWB"@nl ;
  rdfs:comment "The recessed porch in the rear of a Greek temple."@en ;
  rdfs:isDefinedBy <https://w3id.org/con-tax/zones/aat-spaces> ;
  rdfs:label "opisthodomoi"@en ;
  rdfs:label "opisthodomoi"@nl ;
  rdfs:label "opisthodomos"@nl ;
  rdfs:seeAlso <http://vocab.getty.edu/aat/300004662> ;
  rdfs:subClassOf <https://w3id.org/con-tax/zones/aat-spaces#300004651> ;
.
<https://w3id.org/con-tax/zones/aat-spaces#300004670>
  rdf:type owl:Class ;
  rdfs:comment "Ruimten aan de voorzijden van Griekse tempels. VWB"@nl ;
  rdfs:comment "The open vestibule in front of the naos or cella of a temple."@en ;
  rdfs:isDefinedBy <https://w3id.org/con-tax/zones/aat-spaces> ;
  rdfs:label "pronaoi"@en ;
  rdfs:label "pronaoi"@nl ;
  rdfs:label "pronaos"@nl ;
  rdfs:seeAlso <http://vocab.getty.edu/aat/300004670> ;
  rdfs:subClassOf <https://w3id.org/con-tax/zones/aat-spaces#300004651> ;
.
<https://w3id.org/con-tax/zones/aat-spaces#300004677>
  rdf:type owl:Class ;
  rdfs:comment "Spaces and rooms located in theaters."@en ;
  rdfs:isDefinedBy <https://w3id.org/con-tax/zones/aat-spaces> ;
  rdfs:label "theater spaces"@en ;
  rdfs:label "theaterruimte"@nl ;
  rdfs:label "theaterruimten"@nl ;
  rdfs:seeAlso <http://vocab.getty.edu/aat/300004677> ;
  rdfs:seeAlso wd:Q42679632 ;
  rdfs:subClassOf <https://w3id.org/con-tax/zones/aat-spaces#300133704> ;
  contax:containsGuideTerm <https://w3id.org/con-tax/zones/aat-spaces#300104772> ;
.
<https://w3id.org/con-tax/zones/aat-spaces#300004678>
  rdf:type owl:Class ;
  rdfs:comment "In modern theaters, the entire main-floor space for spectators."@en ;
  rdfs:comment "In moderne theaters, de volledige hoofdvloerruimte voor toeschouwers."@nl ;
  rdfs:isDefinedBy <https://w3id.org/con-tax/zones/aat-spaces> ;
  rdfs:label "orchestras (audience spaces)"@en ;
  rdfs:label "parterre"@nl ;
  rdfs:seeAlso <http://vocab.getty.edu/aat/300004678> ;
  rdfs:subClassOf <https://w3id.org/con-tax/zones/aat-spaces#300104771> ;
.
<https://w3id.org/con-tax/zones/aat-spaces#300004708>
  rdf:type owl:Class ;
  rdfs:comment "Stages of ancient Greek and Roman theaters. For the stage podiums of ancient Roman theaters, use \"pulpita.\" For the areas of modern theaters nearest the audience, use \"forestages.\""@en ;
  rdfs:comment "Tonelen van oude Romeinse theaters."@nl ;
  rdfs:isDefinedBy <https://w3id.org/con-tax/zones/aat-spaces> ;
  rdfs:label "proscaenium"@nl ;
  rdfs:label "proscaeniums"@nl ;
  rdfs:label "proscenia"@en ;
  rdfs:seeAlso <http://vocab.getty.edu/aat/300004708> ;
  rdfs:seeAlso wd:Q21550903 ;
  rdfs:subClassOf <https://w3id.org/con-tax/zones/aat-spaces#300004751> ;
.
<https://w3id.org/con-tax/zones/aat-spaces#300004717>
  rdf:type owl:Class ;
  rdfs:comment "Stage podiums of ancient Roman theaters, especially the areas rising above the orchestra. For the stages of ancient Roman theaters, use \"proscenia.\""@en ;
  rdfs:comment "Tonelen van oude Griekse theaters."@nl ;
  rdfs:isDefinedBy <https://w3id.org/con-tax/zones/aat-spaces> ;
  rdfs:label "pulpita"@en ;
  rdfs:label "pulpita"@nl ;
  rdfs:seeAlso <http://vocab.getty.edu/aat/300004717> ;
  rdfs:subClassOf <https://w3id.org/con-tax/zones/aat-spaces#300100082> ;
.
<https://w3id.org/con-tax/zones/aat-spaces#300004734>
  rdf:type owl:Class ;
  rdfs:comment "De in rijen oplopende, halfcirkelvormige zitruimten in antieke theaters en amfitheaters."@nl ;
  rdfs:comment "Tiered, semicircular seating areas in ancient, especially Roman, theaters and amphitheaters."@en ;
  rdfs:isDefinedBy <https://w3id.org/con-tax/zones/aat-spaces> ;
  rdfs:label "cavea"@nl ;
  rdfs:label "caveae"@en ;
  rdfs:label "caveae"@nl ;
  rdfs:seeAlso <http://vocab.getty.edu/aat/300004734> ;
  rdfs:subClassOf <https://w3id.org/con-tax/zones/aat-spaces#300104771> ;
.
<https://w3id.org/con-tax/zones/aat-spaces#300004736>
  rdf:type owl:Class ;
  rdfs:comment "Refers to the wedgeshaped sections of seats in ancient theaters."@en ;
  rdfs:comment "Wordt gebruikt voor wigvormige gedeelten met zitplaatsen in antieke theaters."@nl ;
  rdfs:isDefinedBy <https://w3id.org/con-tax/zones/aat-spaces> ;
  rdfs:label "cunei"@en ;
  rdfs:label "segment (toeschouwersruimte)"@nl ;
  rdfs:label "segment"@nl ;
  rdfs:label "segmenten (toeschouwersruimten)"@nl ;
  rdfs:label "segmenten"@nl ;
  rdfs:seeAlso <http://vocab.getty.edu/aat/300004736> ;
  rdfs:subClassOf <https://w3id.org/con-tax/zones/aat-spaces#300104771> ;
.
<https://w3id.org/con-tax/zones/aat-spaces#300004740>
  rdf:type owl:Class ;
  rdfs:comment "Side entrances in ancient Greek theaters between the audience and scaena affording access for spectators."@en ;
  rdfs:comment "Zij-ingangen in antieke Griekse theaters, tussen het publiek en scaena, die toegang verschaffen aan de toeschouwers."@nl ;
  rdfs:isDefinedBy <https://w3id.org/con-tax/zones/aat-spaces> ;
  rdfs:label "parodoi"@en ;
  rdfs:label "parodoi"@nl ;
  rdfs:label "parodos"@nl ;
  rdfs:seeAlso <http://vocab.getty.edu/aat/300004740> ;
  rdfs:seeAlso wd:Q2627815 ;
  rdfs:subClassOf <https://w3id.org/con-tax/zones/aat-spaces#300104771> ;
.
<https://w3id.org/con-tax/zones/aat-spaces#300004744>
  rdf:type owl:Class ;
  rdfs:comment "Doorgangen tussen hoger en lager gelegen rijen zitplaatsen in Romeinse theaters. Gebruik 'diazomata' voor soortgelijke doorgangen in Griekse theaters."@nl ;
  rdfs:comment "Walkways, concentric with the rows of seats, between the upper and lower seating tiers in a Roman theater.  For similar features in Greek theaters, use \"diazomata.\""@en ;
  rdfs:isDefinedBy <https://w3id.org/con-tax/zones/aat-spaces> ;
  rdfs:label "praecinctio"@nl ;
  rdfs:label "praecinctiones"@en ;
  rdfs:label "praecinctiones"@nl ;
  rdfs:seeAlso <http://vocab.getty.edu/aat/300004744> ;
  rdfs:seeAlso wd:Q1209251 ;
  rdfs:subClassOf <https://w3id.org/con-tax/zones/aat-spaces#300104771> ;
.
<https://w3id.org/con-tax/zones/aat-spaces#300004748>
  rdf:type owl:Class ;
  rdfs:comment "Entrances piercing the banks of seats of theaters or amphitheaters."@en ;
  rdfs:comment "Toegangen tussen de rijen stoelen van theaters of amfitheaters."@nl ;
  rdfs:isDefinedBy <https://w3id.org/con-tax/zones/aat-spaces> ;
  rdfs:label "vomitories"@en-us ;
  rdfs:label "vomitorium"@nl ;
  rdfs:label "vomitoriums"@nl ;
  rdfs:seeAlso <http://vocab.getty.edu/aat/300004748> ;
  rdfs:subClassOf <https://w3id.org/con-tax/zones/aat-spaces#300104771> ;
.
<https://w3id.org/con-tax/zones/aat-spaces#300004751>
  rdf:type owl:Class ;
  rdfs:comment "Podia in theaters, waarop voorstellingen worden gegeven."@nl ;
  rdfs:comment "Theatrical platforms, visible to an audience and commonly framed by a proscenium arch, on which performances are carried out."@en ;
  rdfs:isDefinedBy <https://w3id.org/con-tax/zones/aat-spaces> ;
  rdfs:label "bühnen"@nl ;
  rdfs:label "stages (performance spaces)"@en ;
  rdfs:label "toneel"@nl ;
  rdfs:label "tonelen"@nl ;
  rdfs:seeAlso <http://vocab.getty.edu/aat/300004751> ;
  rdfs:seeAlso wd:Q194428 ;
  rdfs:subClassOf <https://w3id.org/con-tax/zones/aat-spaces#300004677> ;
.
<https://w3id.org/con-tax/zones/aat-spaces#300004753>
  rdf:type owl:Class ;
  rdfs:comment "Areas located on the roof of a building, usually flat areas that are accessible to inhabitants of the building."@en ;
  rdfs:comment "Hoogste horizontale delen van daken. VWB"@nl ;
  rdfs:isDefinedBy <https://w3id.org/con-tax/zones/aat-spaces> ;
  rdfs:label "rooftops"@en-us ;
  rdfs:label "vorst (dak)"@nl ;
  rdfs:label "vorst"@nl ;
  rdfs:label "vorsten (daken)"@nl ;
  rdfs:label "vorsten"@nl ;
  rdfs:seeAlso <http://vocab.getty.edu/aat/300004753> ;
  rdfs:subClassOf <https://w3id.org/con-tax/zones/aat-spaces#300075460> ;
.
<https://w3id.org/con-tax/zones/aat-spaces#300004759>
  rdf:type owl:Class ;
  rdfs:comment "Rooms, often wholly or mostly below ground level, used for storage of food and often other items; for similar areas serving utility purposes or as living spaces, use \"basements.\""@en ;
  rdfs:comment "Wordt gebruikt voor ruimten die geheel of voor het grootste deel ondergronds liggen en die worden gebruikt voor opslag, vooral van voedsel. Voor soortgelijke ruimten die als woonruimte dienen of voor andere gebruiksdoeleinden wordt 'souterrains (verdiepingen)' gebruikt."@nl ;
  rdfs:isDefinedBy <https://w3id.org/con-tax/zones/aat-spaces> ;
  rdfs:label "cellars (storerooms)"@en ;
  rdfs:label "kelder"@nl ;
  rdfs:label "kelders"@nl ;
  rdfs:seeAlso <http://vocab.getty.edu/aat/300004759> ;
  rdfs:seeAlso wd:Q43275450 ;
  rdfs:subClassOf <https://w3id.org/con-tax/zones/aat-spaces#300004465> ;
.
<https://w3id.org/con-tax/zones/aat-spaces#300004760>
  rdf:type owl:Class ;
  rdfs:comment "Cellars in which beer is stored."@en ;
  rdfs:comment "Wordt gebruikt voor kelders waarin bier wordt opgeslagen."@nl ;
  rdfs:isDefinedBy <https://w3id.org/con-tax/zones/aat-spaces> ;
  rdfs:label "beer cellars"@en ;
  rdfs:label "bierkelder"@nl ;
  rdfs:label "bierkelders"@nl ;
  rdfs:seeAlso <http://vocab.getty.edu/aat/300004760> ;
  rdfs:subClassOf <https://w3id.org/con-tax/zones/aat-spaces#300004759> ;
.
<https://w3id.org/con-tax/zones/aat-spaces#300004761>
  rdf:type owl:Class ;
  rdfs:comment "Cellars, partially or wholly underground and usually covered with dirt, where root crops and other crops are stored."@en ;
  rdfs:comment "Kelders die geheel of gedeeltelijk ondergronds liggen, waarin aardappels en andere wortel- en knolgewassen kunnen worden opgeslagen."@nl ;
  rdfs:isDefinedBy <https://w3id.org/con-tax/zones/aat-spaces> ;
  rdfs:label "aardappelkelder"@nl ;
  rdfs:label "aardappelkelders"@nl ;
  rdfs:label "root cellars"@en ;
  rdfs:seeAlso <http://vocab.getty.edu/aat/300004761> ;
  rdfs:seeAlso wd:Q1349300 ;
  rdfs:subClassOf <https://w3id.org/con-tax/zones/aat-spaces#300004759> ;
.
<https://w3id.org/con-tax/zones/aat-spaces#300004762>
  rdf:type owl:Class ;
  rdfs:comment "Rooms in which wine is stored, in bottles or barrels, usually fully or partially below ground level."@en ;
  rdfs:comment "Wordt gebruikt voor ruimten waarin wijn wordt opgeslagen, zowel onder- als bovengronds."@nl ;
  rdfs:isDefinedBy <https://w3id.org/con-tax/zones/aat-spaces> ;
  rdfs:label "wijnkelder"@nl ;
  rdfs:label "wijnkelders"@nl ;
  rdfs:label "wine cellars"@en ;
  rdfs:seeAlso <http://vocab.getty.edu/aat/300004762> ;
  rdfs:seeAlso wd:Q22995 ;
  rdfs:subClassOf <https://w3id.org/con-tax/zones/aat-spaces#300004759> ;
.
<https://w3id.org/con-tax/zones/aat-spaces#300004772>
  rdf:type owl:Class ;
  rdfs:comment "Lange, nauwe doorgangen die naar grafkamers en tholoi leiden."@nl ;
  rdfs:comment "Long, narrow passages leading into chamber tombs and tholoi."@en ;
  rdfs:isDefinedBy <https://w3id.org/con-tax/zones/aat-spaces> ;
  rdfs:label "dromoi"@en ;
  rdfs:label "dromoi"@nl ;
  rdfs:label "dromos"@nl ;
  rdfs:seeAlso <http://vocab.getty.edu/aat/300004772> ;
  rdfs:seeAlso wd:Q9212100 ;
  rdfs:subClassOf <https://w3id.org/con-tax/zones/aat-spaces#300075882> ;
.
<https://w3id.org/con-tax/zones/aat-spaces#300004777>
  rdf:type owl:Class ;
  rdfs:comment "Onderaardse kerkers."@nl ;
  rdfs:comment "Prison cells generally in the form of shafts with openings only at the top; often concealed pits below the floor."@en ;
  rdfs:isDefinedBy <https://w3id.org/con-tax/zones/aat-spaces> ;
  rdfs:label "oubliettes"@en ;
  rdfs:label "oubliëtte"@nl ;
  rdfs:label "oubliëttes"@nl ;
  rdfs:label "verliezen"@nl ;
  rdfs:seeAlso <http://vocab.getty.edu/aat/300004777> ;
  rdfs:subClassOf <https://w3id.org/con-tax/zones/aat-spaces#300004026> ;
.
<https://w3id.org/con-tax/zones/aat-spaces#300004779>
  rdf:type owl:Class ;
  rdfs:comment "Ondergrondse doorgangen of vertrekken."@nl ;
  rdfs:comment "Underground passages or chambers."@en ;
  rdfs:isDefinedBy <https://w3id.org/con-tax/zones/aat-spaces> ;
  rdfs:label "souterrain (passage)"@nl ;
  rdfs:label "souterrain"@nl ;
  rdfs:label "souterrains (passages)"@en ;
  rdfs:label "souterrains (passages)"@nl ;
  rdfs:label "souterrains"@nl ;
  rdfs:seeAlso <http://vocab.getty.edu/aat/300004779> ;
  rdfs:seeAlso wd:Q137937 ;
  rdfs:subClassOf <https://w3id.org/con-tax/zones/aat-spaces#300004283> ;
.
<https://w3id.org/con-tax/zones/aat-spaces#300005162>
  rdf:type owl:Class ;
  rdfs:comment "Public rooms, as in hotels, clubs, or restaurants, where cocktails and other drinks are served."@en ;
  rdfs:comment "Ruimten in bijvoorbeeld hotels, clubs of restaurants, waar cocktails en andere dranken worden geserveerd."@nl ;
  rdfs:isDefinedBy <https://w3id.org/con-tax/zones/aat-spaces> ;
  rdfs:label "cocktail lounges"@en-us ;
  rdfs:label "cocktailbar"@nl ;
  rdfs:label "cocktailbars"@nl ;
  rdfs:seeAlso <http://vocab.getty.edu/aat/300005162> ;
  rdfs:subClassOf <https://w3id.org/con-tax/zones/aat-spaces#300133704> ;
.
<https://w3id.org/con-tax/zones/aat-spaces#300005165>
  rdf:type owl:Class ;
  rdfs:comment "Publieke gelegenheden om melk en melkdranken te gebruiken."@nl ;
  rdfs:comment "Snack bars that sell milk drinks and other refreshments."@en ;
  rdfs:isDefinedBy <https://w3id.org/con-tax/zones/aat-spaces> ;
  rdfs:label "melksalon"@nl ;
  rdfs:label "melksalons"@nl ;
  rdfs:label "milk bars"@en-us ;
  rdfs:seeAlso <http://vocab.getty.edu/aat/300005165> ;
  rdfs:seeAlso wd:Q1750272 ;
  rdfs:subClassOf <https://w3id.org/con-tax/zones/aat-spaces#300005172> ;
.
<https://w3id.org/con-tax/zones/aat-spaces#300005172>
  rdf:type owl:Class ;
  rdfs:comment "Eating facilities where quick, light meals, refreshments, or snacks are served, usually at a counter."@en ;
  rdfs:comment "Eetgelegenheden waar snelle lichte maaltijden, dranken of tussendoortjes worden geserveerd, meestal aan een toog."@nl ;
  rdfs:isDefinedBy <https://w3id.org/con-tax/zones/aat-spaces> ;
  rdfs:label "cafetaria's"@nl ;
  rdfs:label "patatzaken"@nl ;
  rdfs:label "snack bars"@en ;
  rdfs:label "snackbar"@nl ;
  rdfs:label "snackbars"@nl ;
  rdfs:seeAlso <http://vocab.getty.edu/aat/300005172> ;
  rdfs:seeAlso wd:Q1318768 ;
  rdfs:subClassOf <https://w3id.org/con-tax/zones/aat-spaces#300133704> ;
.
<https://w3id.org/con-tax/zones/aat-spaces#300005391>
  rdf:type owl:Class ;
  rdfs:comment "Rooms and spaces designed for the origination or recording of radio or television programs; for telecommunications buildings containing facilities for sending and receiving microwave transmissions, use \"broadcasting stations.\""@en ;
  rdfs:comment "Wordt gebruikt voor ruimten bestemd voor het opnemen van radio- of televisieprogramma's. Gebruik 'omroepstations' voor de gebouwen waarin zich omroepstudio's bevinden."@nl ;
  rdfs:isDefinedBy <https://w3id.org/con-tax/zones/aat-spaces> ;
  rdfs:label "broadcasting studios"@en ;
  rdfs:label "omroepstudio"@nl ;
  rdfs:label "omroepstudio's"@nl ;
  rdfs:seeAlso <http://vocab.getty.edu/aat/300005391> ;
  rdfs:subClassOf <https://w3id.org/con-tax/zones/aat-spaces#300133704> ;
.
<https://w3id.org/con-tax/zones/aat-spaces#300005392>
  rdf:type owl:Class ;
  rdfs:comment "Broadcasting studios designed for radio programs; for larger facilities, including offices and equipment, from which the transmissions are sent and received, use \"radio stations.\""@en ;
  rdfs:comment "Studio's bedoeld voor het opnemen van radioprogramma's. Gebruik 'radiostations' voor de gebouwen waarin zich dergelijke studio's bevinden."@nl ;
  rdfs:isDefinedBy <https://w3id.org/con-tax/zones/aat-spaces> ;
  rdfs:label "radio studios"@en ;
  rdfs:label "radio-opnamestudio"@nl ;
  rdfs:label "radio-opnamestudio's"@nl ;
  rdfs:label "radiostudio"@nl ;
  rdfs:label "radiostudio's"@nl ;
  rdfs:seeAlso <http://vocab.getty.edu/aat/300005392> ;
  rdfs:seeAlso wd:Q2470835 ;
  rdfs:subClassOf <https://w3id.org/con-tax/zones/aat-spaces#300005391> ;
.
<https://w3id.org/con-tax/zones/aat-spaces#300005394>
  rdf:type owl:Class ;
  rdfs:comment "A series of rooms specifically designed for the origination of live or taped television programs;(MHDSTT) for the larger facilities, including offices and equipment, from where the transmissions are sent and received, use \"television stations.\""@en ;
  rdfs:comment "Studio's bedoeld voor het opnemen van televisieprogramma's. Gebruik 'televisiestations' voor de gebouwen waarin zich dergelijke studio's bevinden."@nl ;
  rdfs:isDefinedBy <https://w3id.org/con-tax/zones/aat-spaces> ;
  rdfs:label "teeveestudio's"@nl ;
  rdfs:label "televisiestudio"@nl ;
  rdfs:label "televisiestudio's"@nl ;
  rdfs:label "television studios"@en ;
  rdfs:label "tv-studio's"@nl ;
  rdfs:seeAlso <http://vocab.getty.edu/aat/300005394> ;
  rdfs:seeAlso wd:Q511355 ;
  rdfs:subClassOf <https://w3id.org/con-tax/zones/aat-spaces#300005391> ;
.
<https://w3id.org/con-tax/zones/aat-spaces#300005396>
  rdf:type owl:Class ;
  rdfs:comment "Buildings or spaces designed or used for audio recording, typically conforming to special acoustical requirements and having specialized equipment."@en ;
  rdfs:isDefinedBy <https://w3id.org/con-tax/zones/aat-spaces> ;
  rdfs:label "geluidsstudio"@nl ;
  rdfs:label "geluidsstudio's"@nl ;
  rdfs:label "sound studios"@en ;
  rdfs:seeAlso <http://vocab.getty.edu/aat/300005396> ;
  rdfs:subClassOf <https://w3id.org/con-tax/zones/aat-spaces#300133704> ;
.
<https://w3id.org/con-tax/zones/aat-spaces#300005397>
  rdf:type owl:Class ;
  rdfs:comment "Studios designed or used for creating audio recordings, such as tape and electronic recordings."@en ;
  rdfs:isDefinedBy <https://w3id.org/con-tax/zones/aat-spaces> ;
  rdfs:label "opnamestudio"@nl ;
  rdfs:label "opnamestudio's"@nl ;
  rdfs:label "recording studios"@en ;
  rdfs:seeAlso <http://vocab.getty.edu/aat/300005397> ;
  rdfs:seeAlso wd:Q746369 ;
  rdfs:subClassOf <https://w3id.org/con-tax/zones/aat-spaces#300005396> ;
.
<https://w3id.org/con-tax/zones/aat-spaces#300005398>
  rdf:type owl:Class ;
  rdfs:comment "Rooms or studios made acoustically suitable (as by soundproofing) for producing sound motion pictures."@en ;
  rdfs:comment "Studio's die, door ze geluiddicht te maken, akoestisch geschikt zijn om geluid aan films toe te voegen."@nl ;
  rdfs:isDefinedBy <https://w3id.org/con-tax/zones/aat-spaces> ;
  rdfs:label "geluiddichte opnamestudio"@nl ;
  rdfs:label "geluiddichte opnamestudio's"@nl ;
  rdfs:label "sound stages"@en ;
  rdfs:seeAlso <http://vocab.getty.edu/aat/300005398> ;
  rdfs:seeAlso wd:Q6497985 ;
  rdfs:subClassOf <https://w3id.org/con-tax/zones/aat-spaces#300005396> ;
.
<https://w3id.org/con-tax/zones/aat-spaces#300005422>
  rdf:type owl:Class ;
  rdfs:comment "Small structures, typically large enough for a single person to comfortably enter and furnished with a payphone for public use. They are typically characterized by having a door for privacy and windows to alert others that the booth is in use."@en ;
  rdfs:isDefinedBy <https://w3id.org/con-tax/zones/aat-spaces> ;
  rdfs:label "telefooncel"@nl ;
  rdfs:label "telefooncellen"@nl ;
  rdfs:label "telefoongidsen"@nl ;
  rdfs:label "telephone booths"@en-us ;
  rdfs:seeAlso <http://vocab.getty.edu/aat/300005422> ;
  rdfs:seeAlso wd:Q1143785 ;
  rdfs:subClassOf <https://w3id.org/con-tax/zones/aat-spaces#300004086> ;
.
<https://w3id.org/con-tax/zones/aat-spaces#300005479>
  rdf:type owl:Class ;
  rdfs:comment "Refers to passages, sharing a roof common with the rest of the building, connecting two parts of a log house of the American folk architecture tradition. Distinguished from \"breezeways\" by its folk architecture and log house context and its common roof."@en ;
  rdfs:comment "Wordt gebruikt voor overdekte doorgangen die twee delen van een blokhut met elkaar verbinden in de traditionele Amerikaanse volksarchitectuur. Geen Nederlands equivalent. Gebruik 'overdekte doorgangen'."@nl ;
  rdfs:isDefinedBy <https://w3id.org/con-tax/zones/aat-spaces> ;
  rdfs:label "dogtrot"@nl ;
  rdfs:label "dogtrots"@en-us ;
  rdfs:label "dogtrots"@nl ;
  rdfs:seeAlso <http://vocab.getty.edu/aat/300005479> ;
  rdfs:subClassOf <https://w3id.org/con-tax/zones/aat-spaces#300075459> ;
.
<https://w3id.org/con-tax/zones/aat-spaces#300005648>
  rdf:type owl:Class ;
  rdfs:comment "Ruimten in christelijke kerken tussen het zangkoor en het sanctuarium, meestal gereserveerd voor geestelijken."@nl ;
  rdfs:comment "That part in the eastern arm of a church between the choir and the sanctuary, usually reserved for the clergy."@en ;
  rdfs:isDefinedBy <https://w3id.org/con-tax/zones/aat-spaces> ;
  rdfs:label "presbyteria"@nl ;
  rdfs:label "presbyteries"@en ;
  rdfs:label "priesterkoor"@nl ;
  rdfs:label "priesterkoren"@nl ;
  rdfs:seeAlso <http://vocab.getty.edu/aat/300005648> ;
  rdfs:subClassOf <https://w3id.org/con-tax/zones/aat-spaces#300004560> ;
.
<https://w3id.org/con-tax/zones/aat-spaces#300005715>
  rdf:type owl:Class ;
  rdfs:comment "Apartments serving as an example of others in the same building or complex for prospective renters."@en ;
  rdfs:comment "Wooneenheden die als voorbeeld dienen voor toekomstige huurders van dergelijke wooneenheden in hetzelfde gebouw of complex."@nl ;
  rdfs:isDefinedBy <https://w3id.org/con-tax/zones/aat-spaces> ;
  rdfs:label "model apartments"@en-us ;
  rdfs:label "modelappartement"@nl ;
  rdfs:label "modelappartementen"@nl ;
  rdfs:label "modelflats"@nl ;
  rdfs:seeAlso <http://vocab.getty.edu/aat/300005715> ;
  rdfs:subClassOf <https://w3id.org/con-tax/zones/aat-spaces#300004063> ;
.
<https://w3id.org/con-tax/zones/aat-spaces#300005814>
  rdf:type owl:Class ;
  rdfs:comment "Rooms or buildings containing a systematically ordered collection of preserved plants; for gardens of herbs, use \"herb gardens.\""@en ;
  rdfs:comment "Wordt gebruikt voor kamers of gebouwen waarin zich een systematisch geordende collectie beschermde planten bevindt. Voor tuinen met kruiden wordt 'kruidentuin' gebruikt."@nl ;
  rdfs:isDefinedBy <https://w3id.org/con-tax/zones/aat-spaces> ;
  rdfs:label "herbaria"@en ;
  rdfs:label "herbaria"@nl ;
  rdfs:label "herbarium"@nl ;
  rdfs:seeAlso <http://vocab.getty.edu/aat/300005814> ;
  rdfs:subClassOf <https://w3id.org/con-tax/zones/aat-spaces#300133704> ;
.
<https://w3id.org/con-tax/zones/aat-spaces#300006013>
  rdf:type owl:Class ;
  rdfs:comment "Government offices or office buildings for examining claims to patents and for granting patents."@en ;
  rdfs:comment "Overheidsinstellingen waar octrooiaanvragen worden onderzocht en waar octrooien worden verleend."@nl ;
  rdfs:isDefinedBy <https://w3id.org/con-tax/zones/aat-spaces> ;
  rdfs:label "octrooibureau"@nl ;
  rdfs:label "octrooibureaus"@nl ;
  rdfs:label "octrooikantoor"@nl ;
  rdfs:label "octrooikantoren"@nl ;
  rdfs:label "patent offices"@en ;
  rdfs:label "patentbureaus"@nl ;
  rdfs:seeAlso <http://vocab.getty.edu/aat/300006013> ;
  rdfs:subClassOf <https://w3id.org/con-tax/zones/aat-spaces#300004521> ;
.
<https://w3id.org/con-tax/zones/aat-spaces#300006050>
  rdf:type owl:Class ;
  rdfs:comment "Opslagruimten voor waardevolle voorwerpen. Gebruik voor gebouwen met dezelfde functie 'schathuizen'."@nl ;
  rdfs:comment "Rooms or spaces that serve as storage places for valuable objects. For buildings designed for this purpose use 'treasuries (buildings).'"@en ;
  rdfs:isDefinedBy <https://w3id.org/con-tax/zones/aat-spaces> ;
  rdfs:label "schatkamer"@nl ;
  rdfs:label "schatkamers"@nl ;
  rdfs:label "treasuries (rooms)"@en ;
  rdfs:seeAlso <http://vocab.getty.edu/aat/300006050> ;
  rdfs:subClassOf <https://w3id.org/con-tax/zones/aat-spaces#300004465> ;
.
<https://w3id.org/con-tax/zones/aat-spaces#300006262>
  rdf:type owl:Class ;
  rdfs:comment "Large rooms where sails are cut out, fabricated, and maintained."@en ;
  rdfs:comment "Ruimten waar zeilen worden vervaardigd en onderhouden."@nl ;
  rdfs:isDefinedBy <https://w3id.org/con-tax/zones/aat-spaces> ;
  rdfs:label "sail lofts"@en ;
  rdfs:label "zeilmakerij"@nl ;
  rdfs:label "zeilmakerijen"@nl ;
  rdfs:seeAlso <http://vocab.getty.edu/aat/300006262> ;
  rdfs:subClassOf <https://w3id.org/con-tax/zones/aat-spaces#300133704> ;
.
<https://w3id.org/con-tax/zones/aat-spaces#300007053>
  rdf:type owl:Class ;
  rdfs:comment "Spaces where teeth are examined, X-rayed, cleaned, extracted, cavities filled, and other minor surgeries are performed on teeth by or under the supervision of a dentist; they typically include a waiting room and a room or rooms with a chair and other equipment for the examination of patients."@en ;
  rdfs:isDefinedBy <https://w3id.org/con-tax/zones/aat-spaces> ;
  rdfs:label "dental offices"@en ;
  rdfs:label "tandartsenkabinetten"@nl ;
  rdfs:label "tandartskabinet"@nl ;
  rdfs:label "tandartspraktijk"@nl ;
  rdfs:label "tandartspraktijken"@nl ;
  rdfs:seeAlso <http://vocab.getty.edu/aat/300007053> ;
  rdfs:subClassOf <https://w3id.org/con-tax/zones/aat-spaces#300004521> ;
.
<https://w3id.org/con-tax/zones/aat-spaces#300007306>
  rdf:type owl:Class ;
  rdfs:comment "Indoor spaces, usually oval in plan and having special floor surfacing, designed for running or jogging; for similar recreation spaces outdoors, use \"running tracks.\""@en ;
  rdfs:comment "Wordt gebruikt voor binnenruimten, waarin meestal een langgerekt ovaal met een speciale vloerbedekking, voornamelijk voor hardlopen. Voor soortgelijk recreatieruimten buiten wordt 'atletiekbanen' gebruikt."@nl ;
  rdfs:isDefinedBy <https://w3id.org/con-tax/zones/aat-spaces> ;
  rdfs:label "indoor tracks"@en ;
  rdfs:label "indoorbaan"@nl ;
  rdfs:label "indoorbanen"@nl ;
  rdfs:seeAlso <http://vocab.getty.edu/aat/300007306> ;
  rdfs:subClassOf <https://w3id.org/con-tax/zones/aat-spaces#300133704> ;
.
<https://w3id.org/con-tax/zones/aat-spaces#300007423>
  rdf:type owl:Class ;
  rdfs:comment "Enclosed spaces composed of a garth and surrounding walkways, which are generally arcaded on the courtyard side and walled on the other; usually found in Christian religious building complexes. Use for such features in secular buildings only when closely resembling the prototype."@en ;
  rdfs:comment "Galerijen die doorgaans in drie of vier armen of panden rechthoekig de kloosterhof omzomen. Kloostergangen zijn omgeven door de belangrijkste kloostergebouwen, waardoor zij als verbindingsgangen dienst doen. Hier werd de kloosterlingen een plaats van verpozing en voor meditatie geboden, beschut tegen weer en wind, respectievelijk zonnehitte."@nl ;
  rdfs:isDefinedBy <https://w3id.org/con-tax/zones/aat-spaces> ;
  rdfs:label "cloisters"@en ;
  rdfs:label "kloostergang"@nl ;
  rdfs:label "kloostergangen"@nl ;
  rdfs:seeAlso <http://vocab.getty.edu/aat/300007423> ;
  rdfs:seeAlso wd:Q1430154 ;
  rdfs:subClassOf <https://w3id.org/con-tax/zones/aat-spaces#300004560> ;
.
<https://w3id.org/con-tax/zones/aat-spaces#300007424>
  rdf:type owl:Class ;
  rdfs:comment "Binnenplaatsen van kloosters, omgeven door kloostergangen."@nl ;
  rdfs:comment "Open courtyards surrounded by walkways, especially in a group of buildings of a monastery or college."@en ;
  rdfs:isDefinedBy <https://w3id.org/con-tax/zones/aat-spaces> ;
  rdfs:label "cloister garths"@en ;
  rdfs:label "kloosterhof"@nl ;
  rdfs:label "kloosterhoven"@nl ;
  rdfs:label "pandhof"@nl ;
  rdfs:label "pandhoven"@nl ;
  rdfs:seeAlso <http://vocab.getty.edu/aat/300007424> ;
  rdfs:subClassOf <https://w3id.org/con-tax/zones/aat-spaces#300004095> ;
.
<https://w3id.org/con-tax/zones/aat-spaces#300007427>
  rdf:type owl:Class ;
  rdfs:comment "Heated parlors or sitting rooms in monasteries."@en ;
  rdfs:comment "Verwarmde zalen in kloosters. VWB"@nl ;
  rdfs:isDefinedBy <https://w3id.org/con-tax/zones/aat-spaces> ;
  rdfs:label "calefactoria"@nl ;
  rdfs:label "calefactories"@en ;
  rdfs:label "calefactorium"@nl ;
  rdfs:label "stoof (ruimte)"@nl ;
  rdfs:label "stoof"@nl ;
  rdfs:label "stoven (ruimten)"@nl ;
  rdfs:label "stoven"@nl ;
  rdfs:seeAlso <http://vocab.getty.edu/aat/300007427> ;
  rdfs:seeAlso wd:Q2596189 ;
  rdfs:subClassOf <https://w3id.org/con-tax/zones/aat-spaces#300133704> ;
.
<https://w3id.org/con-tax/zones/aat-spaces#300007431>
  rdf:type owl:Class ;
  rdfs:comment "In monastic architecture, rooms, groups of rooms, or separate buildings where monastic rule was relaxed."@en ;
  rdfs:comment "Ruimten in kloosters of aparte gebouwen bij kloosters waar de kloosterregels minder streng toegepast werden."@nl ;
  rdfs:isDefinedBy <https://w3id.org/con-tax/zones/aat-spaces> ;
  rdfs:label "misericorden"@nl ;
  rdfs:label "misericordes"@nl ;
  rdfs:label "misericords (building spaces)"@en ;
  rdfs:seeAlso <http://vocab.getty.edu/aat/300007431> ;
  rdfs:subClassOf <https://w3id.org/con-tax/zones/aat-spaces#300004560> ;
.
<https://w3id.org/con-tax/zones/aat-spaces#300007432>
  rdf:type owl:Class ;
  rdfs:comment "Kamers in kloosters en nonnenkloosters waar bezoek mag worden ontvangen."@nl ;
  rdfs:comment "Rooms in monasteries or convents where visitors may be received."@en ;
  rdfs:isDefinedBy <https://w3id.org/con-tax/zones/aat-spaces> ;
  rdfs:label "auditoria hospitum"@nl ;
  rdfs:label "auditorium hospitum"@nl ;
  rdfs:label "parlatories"@en ;
  rdfs:label "spreekkamer (kloosters)"@nl ;
  rdfs:label "spreekkamer"@nl ;
  rdfs:label "spreekkamers (kloosters)"@nl ;
  rdfs:label "spreekkamers"@nl ;
  rdfs:seeAlso <http://vocab.getty.edu/aat/300007432> ;
  rdfs:subClassOf <https://w3id.org/con-tax/zones/aat-spaces#300004560> ;
.
<https://w3id.org/con-tax/zones/aat-spaces#300007450>
  rdf:type owl:Class ;
  rdfs:comment "Chapels of a church endowed for chanting of masses and other services."@en ;
  rdfs:comment "Wordt gebruikt voor kapellen, altaren of andere delen van een kerk die zijn bedoeld voor het zingen van missen, gewoonlijk voor de stichter."@nl ;
  rdfs:isDefinedBy <https://w3id.org/con-tax/zones/aat-spaces> ;
  rdfs:label "chantries"@en ;
  rdfs:label "fundatiekapel"@nl ;
  rdfs:label "fundatiekapellen"@nl ;
  rdfs:seeAlso <http://vocab.getty.edu/aat/300007450> ;
  rdfs:seeAlso wd:Q575842 ;
  rdfs:subClassOf <https://w3id.org/con-tax/zones/aat-spaces#300004590> ;
.
<https://w3id.org/con-tax/zones/aat-spaces#300007454>
  rdf:type owl:Class ;
  rdfs:comment "Kapellen voor privé- of familiegraftomben. Gebruik 'rouwkapellen' voor ruimten waarin rouwdiensten worden gehouden."@nl ;
  rdfs:comment "Rooms or relatively small freesanding structures containing tombs or sarcophagi, usually for individuals, families, or members of a particular community. For rooms or structures adjacent to a tomb, used by the mourners or for offerings to the dead, prefer \"tomb chapels.\""@en ;
  rdfs:isDefinedBy <https://w3id.org/con-tax/zones/aat-spaces> ;
  rdfs:label "grafkapel"@nl ;
  rdfs:label "grafkapellen"@nl ;
  rdfs:label "sepulchral chapels"@en ;
  rdfs:seeAlso <http://vocab.getty.edu/aat/300007454> ;
  rdfs:seeAlso wd:Q1424583 ;
  rdfs:subClassOf <https://w3id.org/con-tax/zones/aat-spaces#300004590> ;
.
<https://w3id.org/con-tax/zones/aat-spaces#300007459>
  rdf:type owl:Class ;
  rdfs:comment "Places for prayer comprising a room or building for private worship; typically located in a church, madrasa, house, monastery, guild hall, or other locations associated with various religions or rites. In the Roman Catholic church, the usage and number of services allowed in an oratory are defined by canon law. In Christian architecture, oratories seem to have originated from the chapels erected over the tombs of the early martyrs where the faithful gathered to pray, combined with the necessity of having a place of worship for the people in rural districts at a time when churches proper were restricted to cathedral cities."@en ;
  rdfs:comment "Privé-bidkapellen."@nl ;
  rdfs:isDefinedBy <https://w3id.org/con-tax/zones/aat-spaces> ;
  rdfs:label "oratories"@en ;
  rdfs:label "oratorium"@nl ;
  rdfs:label "oratoriums"@nl ;
  rdfs:seeAlso <http://vocab.getty.edu/aat/300007459> ;
  rdfs:subClassOf <https://w3id.org/con-tax/zones/aat-spaces#300004559> ;
.
<https://w3id.org/con-tax/zones/aat-spaces#300007461>
  rdf:type owl:Class ;
  rdfs:comment "Rooms or other relatively small places set aside for worship by an individual, family, or small group, where no public services are provided. A private chapel may be within the confines of a larger church, home, or other larger building; it may also be a free standing structure."@en ;
  rdfs:isDefinedBy <https://w3id.org/con-tax/zones/aat-spaces> ;
  rdfs:label "private chapels"@en ;
  rdfs:label "privé-kapel"@nl ;
  rdfs:label "privé-kapellen"@nl ;
  rdfs:seeAlso <http://vocab.getty.edu/aat/300007461> ;
  rdfs:seeAlso wd:Q3657724 ;
  rdfs:subClassOf <https://w3id.org/con-tax/zones/aat-spaces#300004590> ;
.
<https://w3id.org/con-tax/zones/aat-spaces#300007462>
  rdf:type owl:Class ;
  rdfs:comment "Private chapels for a royal court."@en ;
  rdfs:comment "Privé-kapellen aan een koninklijk hof."@nl ;
  rdfs:isDefinedBy <https://w3id.org/con-tax/zones/aat-spaces> ;
  rdfs:label "hofkapel"@nl ;
  rdfs:label "hofkapellen"@nl ;
  rdfs:label "royal chapels"@en ;
  rdfs:seeAlso <http://vocab.getty.edu/aat/300007462> ;
  rdfs:seeAlso wd:Q16147981 ;
  rdfs:subClassOf <https://w3id.org/con-tax/zones/aat-spaces#300004590> ;
.
<https://w3id.org/con-tax/zones/aat-spaces#300007572>
  rdf:type owl:Class ;
  rdfs:comment "May be used broadly for any consecrated place in ancient Roman or Christian architecture, but more specific terms are preferred, such as \"chapels,\" \"shrines,\" \"sacristies,\" or \"sanctuaries.\""@en ;
  rdfs:comment "Oud-Romeinse of christelijke gewijde plaatsen. Gebruik bij voorkeur meer specifieke termen."@nl ;
  rdfs:isDefinedBy <https://w3id.org/con-tax/zones/aat-spaces> ;
  rdfs:label "sacraria"@en ;
  rdfs:label "sacraria"@nl ;
  rdfs:label "sacrarium"@nl ;
  rdfs:seeAlso <http://vocab.getty.edu/aat/300007572> ;
  rdfs:subClassOf <https://w3id.org/con-tax/zones/aat-spaces#300004559> ;
.
<https://w3id.org/con-tax/zones/aat-spaces#300007689>
  rdf:type owl:Class ;
  rdfs:comment "Reinforced underground shelters, either specifically designed or improvised, to give the civil population or military personnel protection against enemy bombing attacks by aircraft, particularly shelters dating from World War II or the inter-war years."@en ;
  rdfs:isDefinedBy <https://w3id.org/con-tax/zones/aat-spaces> ;
  rdfs:label "air raid shelters"@en ;
  rdfs:label "bomvrije schuilkelder"@nl ;
  rdfs:label "bomvrije schuilkelders"@nl ;
  rdfs:seeAlso <http://vocab.getty.edu/aat/300007689> ;
  rdfs:seeAlso wd:Q389959 ;
  rdfs:subClassOf <https://w3id.org/con-tax/zones/aat-spaces#300312256> ;
.
<https://w3id.org/con-tax/zones/aat-spaces#300007691>
  rdf:type owl:Class ;
  rdfs:comment "Shelters, typically underground or in caves, intended to provide reasonable protection against the radiation and fallout of atomic bombs, typically having thicker walls and other features beyond those required in shelters for protection against conventional bombs."@en ;
  rdfs:isDefinedBy <https://w3id.org/con-tax/zones/aat-spaces> ;
  rdfs:label "atoomschuilkelder"@nl ;
  rdfs:label "atoomschuilkelders"@nl ;
  rdfs:label "nuclear bomb shelters"@en ;
  rdfs:seeAlso <http://vocab.getty.edu/aat/300007691> ;
  rdfs:subClassOf <https://w3id.org/con-tax/zones/aat-spaces#300312256> ;
.
<https://w3id.org/con-tax/zones/aat-spaces#300007725>
  rdf:type owl:Class ;
  rdfs:comment "Verwijst naar ruimten die zijn bedoeld voor kunstenaars om in te werken. De term wordt in algemene zin gebruikt voor werkruimten voor kunstenaars vanaf de 16de eeuw tot heden. De kenmerken van een atelier komen vaak voort uit praktische vereisten zoals voldoende licht en voldoende ruimte om het kunstwerk te maken en materialen op te slaan. Het atelier kan ook dienstdoen als locatie voor het tentoonstellen van afgeronde kunstwerken of het geven van trainingen. Bij het tot stand brengen van een kunstwerk kunnen meerdere artistieke processen een rol spelen; het atelier kan dan ook zijn onderverdeeld voor verschillende activiteiten. De term 'werkplaatsen' verwijst in het algemeen naar ruimten die werden gebruikt door ambachtslieden, kunstenaars die vóór de 16de eeuw actief waren en door fabrieksmedewerkers."@nl ;
  rdfs:comment "Working places set aside for artists to work. The term is generally applied to workspaces used by artists creating fine art, particularly art dating from the 16th century to the present. The characteristics of a studio may be dictated by the practical requirements of adequate light, ample space in which to create the work of art, and storage of materials. Display of the finished art works and training may also be accommodated in a studio. Creation of an art work may require a range of artistic processes; therefore, separate areas of work may be delegated in the studio. The term may also refer to spaces used by dancers, singers, musicians, and other performing artists to create or practice. The term \"workshops\" is generally refers to spaces used by craftspeople, artists working prior to the 16th century, and industrial workers. For studios that are larger spaces or complexes, and are used to create films, television or radio programs, or other large scale productions, use \"motion picture studios,\" \"broadcasting studios,\" \"sound studios,\" \"recording studios,\" \"radio studios,\" or \"television studios.\" "@en ;
  rdfs:isDefinedBy <https://w3id.org/con-tax/zones/aat-spaces> ;
  rdfs:label "atelier (werkruimten)"@nl ;
  rdfs:label "atelier"@nl ;
  rdfs:label "ateliers (werkruimten)"@nl ;
  rdfs:label "ateliers"@nl ;
  rdfs:label "studio's (werkplaatsen)"@nl ;
  rdfs:label "studio's"@nl ;
  rdfs:label "studios (work spaces)"@en ;
  rdfs:seeAlso <http://vocab.getty.edu/aat/300007725> ;
  rdfs:subClassOf <https://w3id.org/con-tax/zones/aat-spaces#300133704> ;
.
<https://w3id.org/con-tax/zones/aat-spaces#300007794>
  rdf:type owl:Class ;
  rdfs:comment "Delen van treinstations die onderdak verschaffen aan mensen die op hun trein wachten."@nl ;
  rdfs:comment "Parts of railroad passenger terminals providing accommodations for persons waiting for trains."@en ;
  rdfs:isDefinedBy <https://w3id.org/con-tax/zones/aat-spaces> ;
  rdfs:label "headhouses"@en-us ;
  rdfs:label "stationsgebouw"@nl ;
  rdfs:label "stationsgebouwen"@nl ;
  rdfs:seeAlso <http://vocab.getty.edu/aat/300007794> ;
  rdfs:subClassOf <https://w3id.org/con-tax/zones/aat-spaces#300004450> ;
.
<https://w3id.org/con-tax/zones/aat-spaces#300007795>
  rdf:type owl:Class ;
  rdfs:comment "De delen van spoorwegstations die de perrons en rails overkappen."@nl ;
  rdfs:comment "The parts of railroad stations that cover the tracks."@en ;
  rdfs:isDefinedBy <https://w3id.org/con-tax/zones/aat-spaces> ;
  rdfs:label "stationsoverkapping"@nl ;
  rdfs:label "stationsoverkappingen"@nl ;
  rdfs:label "train sheds"@en ;
  rdfs:seeAlso <http://vocab.getty.edu/aat/300007795> ;
  rdfs:subClassOf <https://w3id.org/con-tax/zones/aat-spaces#300103935> ;
.
<https://w3id.org/con-tax/zones/aat-spaces#300007821>
  rdf:type owl:Class ;
  rdfs:comment "Booth, stalls, or offices at which tolls, duties, or customs are collected, particularly booths at which the toll for the right of passage across a bridge or along a road are collected."@en ;
  rdfs:comment "Kantoor waar tol moet worden betaald."@nl ;
  rdfs:isDefinedBy <https://w3id.org/con-tax/zones/aat-spaces> ;
  rdfs:label "commiezenhuizen"@nl ;
  rdfs:label "tolkantoor"@nl ;
  rdfs:label "tolkantoren"@nl ;
  rdfs:label "tollbooths"@en ;
  rdfs:seeAlso <http://vocab.getty.edu/aat/300007821> ;
  rdfs:subClassOf <https://w3id.org/con-tax/zones/aat-spaces#300004086> ;
.
<https://w3id.org/con-tax/zones/aat-spaces#300008006>
  rdf:type owl:Class ;
  rdfs:comment "Rooms or spaces that are within buildings and have one or more seats and a pit used as toilets which lack plumbing facilities, distinguished from \"outhouses\" which are separate structures in domestic contexts containing similar arrangements of toilet facilities. For rooms or spaces with toilets having plumbing, use \"bathrooms\" or \"lavatories (rooms).\""@en ;
  rdfs:comment "Ruimten in gebouwen, met een of meer zitplaatsen en een put, en die worden gebruikt als toilet zonder riolering. Te onderscheiden van 'privaathuisjes', losstaande gebouwtjes bij woonhuizen die gelijksoortige toiletfaciliteiten bieden. Voor ruimten met toiletten die wel riolering hebben gebruik: 'toiletten'."@nl ;
  rdfs:isDefinedBy <https://w3id.org/con-tax/zones/aat-spaces> ;
  rdfs:label "bestekamers"@nl ;
  rdfs:label "heimelijkheden"@nl ;
  rdfs:label "plee"@nl ;
  rdfs:label "plees"@nl ;
  rdfs:label "privaat"@nl ;
  rdfs:label "privaten"@nl ;
  rdfs:label "privies"@en ;
  rdfs:label "schijthuizen"@nl ;
  rdfs:label "sekreet"@nl ;
  rdfs:label "sekreten"@nl ;
  rdfs:label "stil"@nl ;
  rdfs:label "stillen"@nl ;
  rdfs:seeAlso <http://vocab.getty.edu/aat/300008006> ;
  rdfs:subClassOf <https://w3id.org/con-tax/zones/aat-spaces#300133704> ;
.
<https://w3id.org/con-tax/zones/aat-spaces#300008014>
  rdf:type owl:Class ;
  rdfs:comment "Wholly or partially underground refuges from tornadoes or other violent storms."@en ;
  rdfs:comment "Wordt gebruikt voor geheel of gedeeltelijk ondergrondse schuilplaatsen in geval van tornado's of andere zware stormen."@nl ;
  rdfs:isDefinedBy <https://w3id.org/con-tax/zones/aat-spaces> ;
  rdfs:label "schuilkelder"@nl ;
  rdfs:label "schuilkelders"@nl ;
  rdfs:label "storm cellars"@en ;
  rdfs:seeAlso <http://vocab.getty.edu/aat/300008014> ;
  rdfs:seeAlso wd:Q7620195 ;
  rdfs:subClassOf <https://w3id.org/con-tax/zones/aat-spaces#300103935> ;
.
<https://w3id.org/con-tax/zones/aat-spaces#300025978>
  rdf:type owl:Class ;
  rdfs:comment "Kleine kamers of studeerkamers in privéwoningen, waarin collecties kunstwerken en/of biologische of geologische monsters worden tentoongesteld; populair tijdens de Italiaanse Renaissance."@nl ;
  rdfs:comment "Small chambers or studies in private homes housing collections of art works or biological or geological specimens, popular during the Italian Renaissance."@en ;
  rdfs:isDefinedBy <https://w3id.org/con-tax/zones/aat-spaces> ;
  rdfs:label "studiolo"@nl ;
  rdfs:label "studiolos"@en ;
  rdfs:label "studiolos"@nl ;
  rdfs:seeAlso <http://vocab.getty.edu/aat/300025978> ;
  rdfs:seeAlso wd:Q672603 ;
  rdfs:subClassOf <https://w3id.org/con-tax/zones/aat-spaces#300133704> ;
.
<https://w3id.org/con-tax/zones/aat-spaces#300049869>
  rdf:type owl:Class ;
  rdfs:comment "Any of the equipment effecting movement on the stage, including groove systems, devices for flying figures, etc."@en ;
  rdfs:comment "Geheel van apparaten, waarmee het beweegbare decor en de licht- en geluidsinstallaties worden bediend."@nl ;
  rdfs:isDefinedBy <https://w3id.org/con-tax/zones/aat-spaces> ;
  rdfs:label "stage machinery"@en ;
  rdfs:label "toneelmachinerie"@nl ;
  rdfs:label "toneelmachinerieën"@nl ;
  rdfs:seeAlso <http://vocab.getty.edu/aat/300049869> ;
  rdfs:subClassOf <https://w3id.org/con-tax/zones/aat-spaces#300100082> ;
.
<https://w3id.org/con-tax/zones/aat-spaces#300051413>
  rdf:type owl:Class ;
  rdfs:comment "Vertical passages through which dumbwaiters, lifts, or similar contrivances move from level to level."@en ;
  rdfs:comment "Verticale schachten waardoor etensliften, liften of gelijksoortige toestellen van de ene verdieping naar de andere kunnen bewegen."@nl ;
  rdfs:isDefinedBy <https://w3id.org/con-tax/zones/aat-spaces> ;
  rdfs:label "hoistways"@en ;
  rdfs:label "liftkoker"@nl ;
  rdfs:label "liftkokers"@nl ;
  rdfs:label "liftschacht"@nl ;
  rdfs:label "liftschachten"@nl ;
  rdfs:seeAlso <http://vocab.getty.edu/aat/300051413> ;
  rdfs:subClassOf <https://w3id.org/con-tax/zones/aat-spaces#300004316> ;
.
<https://w3id.org/con-tax/zones/aat-spaces#300065028>
  rdf:type owl:Class ;
  rdfs:comment "Open ruimten onder straatniveau rond een kelderraam of -deur, die grenzen aan de funderingsmuren."@nl ;
  rdfs:comment "Open subsurface spaces around a basement window or doorway, adjacent to the foundation walls."@en ;
  rdfs:isDefinedBy <https://w3id.org/con-tax/zones/aat-spaces> ;
  rdfs:label "areaways"@en-us ;
  rdfs:label "keldergat"@nl ;
  rdfs:label "keldergaten"@nl ;
  rdfs:seeAlso <http://vocab.getty.edu/aat/300065028> ;
  rdfs:subClassOf <https://w3id.org/con-tax/zones/aat-spaces#300075460> ;
.
<https://w3id.org/con-tax/zones/aat-spaces#300065035>
  rdf:type owl:Class ;
  rdfs:comment "Rooms at a spa designed for drinking mineral waters, as at Bath, England."@en ;
  rdfs:comment "Ruimten bij minerale bronnen, voor het drinken van bronwater, zoals in Bath, Engeland."@nl ;
  rdfs:isDefinedBy <https://w3id.org/con-tax/zones/aat-spaces> ;
  rdfs:label "drinkhal"@nl ;
  rdfs:label "drinkhallen"@nl ;
  rdfs:label "koerzaal"@nl ;
  rdfs:label "koerzalen"@nl ;
  rdfs:label "kursaal"@nl ;
  rdfs:label "kursalen"@nl ;
  rdfs:label "pump rooms"@en ;
  rdfs:seeAlso <http://vocab.getty.edu/aat/300065035> ;
  rdfs:subClassOf <https://w3id.org/con-tax/zones/aat-spaces#300133704> ;
.
<https://w3id.org/con-tax/zones/aat-spaces#300065045>
  rdf:type owl:Class ;
  rdfs:comment "Porches or rooms having open sides or many windows arranged to permit sleeping in the open air."@en ;
  rdfs:comment "Veranda's, om in de buitenlucht te slapen."@nl ;
  rdfs:isDefinedBy <https://w3id.org/con-tax/zones/aat-spaces> ;
  rdfs:label "slaapveranda"@nl ;
  rdfs:label "slaapveranda's"@nl ;
  rdfs:label "sleeping porches"@en ;
  rdfs:seeAlso <http://vocab.getty.edu/aat/300065045> ;
  rdfs:subClassOf <https://w3id.org/con-tax/zones/aat-spaces#300004132> ;
.
<https://w3id.org/con-tax/zones/aat-spaces#300065050>
  rdf:type owl:Class ;
  rdfs:isDefinedBy <https://w3id.org/con-tax/zones/aat-spaces> ;
  rdfs:label "naaikamer"@nl ;
  rdfs:label "naaikamers"@nl ;
  rdfs:label "sewing rooms"@en ;
  rdfs:seeAlso <http://vocab.getty.edu/aat/300065050> ;
  rdfs:subClassOf <https://w3id.org/con-tax/zones/aat-spaces#300133704> ;
.
<https://w3id.org/con-tax/zones/aat-spaces#300065054>
  rdf:type owl:Class ;
  rdfs:comment "Spaces designed for viewing a landscape, or observing wildlife. These may be open spaces at the tops of tall buildings or constructed in natural environments."@en ;
  rdfs:isDefinedBy <https://w3id.org/con-tax/zones/aat-spaces> ;
  rdfs:label "observatieplatform"@nl ;
  rdfs:label "observatieplatforms"@nl ;
  rdfs:label "observation decks"@en ;
  rdfs:seeAlso <http://vocab.getty.edu/aat/300065054> ;
  rdfs:seeAlso wd:Q29898766 ;
  rdfs:subClassOf <https://w3id.org/con-tax/zones/aat-spaces#300004113> ;
.
<https://w3id.org/con-tax/zones/aat-spaces#300065059>
  rdf:type owl:Class ;
  rdfs:comment "Apartments with rooms on two levels."@en ;
  rdfs:comment "Wooneenheden met een eigen toegang, waarbij woon- en slaapverdieping boven elkaar liggen, deel uitmakend van een flatgebouw."@nl ;
  rdfs:isDefinedBy <https://w3id.org/con-tax/zones/aat-spaces> ;
  rdfs:label "duplex apartments"@en-us ;
  rdfs:label "duplexappartement"@nl ;
  rdfs:label "duplexappartementen"@nl ;
  rdfs:seeAlso <http://vocab.getty.edu/aat/300065059> ;
  rdfs:subClassOf <https://w3id.org/con-tax/zones/aat-spaces#300004063> ;
.
<https://w3id.org/con-tax/zones/aat-spaces#300069805>
  rdf:type gvp:GuideTerm ;
  rdfs:isDefinedBy <https://w3id.org/con-tax/zones/aat-spaces> ;
  rdfs:label "<stable and barn spaces>"@en ;
  rdfs:label "<stal- en schuurruimte>"@nl ;
  rdfs:label "<stal- en schuurruimten>"@nl ;
  rdfs:label "stal- en schuurruimte"@nl ;
  rdfs:label "stal- en schuurruimten"@nl ;
  rdfs:seeAlso <http://vocab.getty.edu/aat/300069805> ;
  contax:containsConcept <https://w3id.org/con-tax/zones/aat-spaces#300004042> ;
  contax:containsConcept <https://w3id.org/con-tax/zones/aat-spaces#300004172> ;
  contax:containsConcept <https://w3id.org/con-tax/zones/aat-spaces#300069806> ;
  contax:containsConcept <https://w3id.org/con-tax/zones/aat-spaces#300080603> ;
  contax:containsConcept <https://w3id.org/con-tax/zones/aat-spaces#300411496> ;
.
<https://w3id.org/con-tax/zones/aat-spaces#300069806>
  rdf:type owl:Class ;
  rdfs:comment "Rooms in or attached to a horse barn or stable for the storage and maintenance of riding tack and often of stud records or for the display of prizes or other honors of the stable."@en ;
  rdfs:comment "Ruimten in of aan paardenstallen, voor de opslag en het onderhoud van zadels en tuig en waar vaak ook stoeterijgegevens, prijzen en ander eerbetoon aan de stoeterij worden bewaard."@nl ;
  rdfs:isDefinedBy <https://w3id.org/con-tax/zones/aat-spaces> ;
  rdfs:label "tack rooms"@en ;
  rdfs:label "zadelkamer"@nl ;
  rdfs:label "zadelkamers"@nl ;
  rdfs:seeAlso <http://vocab.getty.edu/aat/300069806> ;
  rdfs:subClassOf <https://w3id.org/con-tax/zones/aat-spaces#300133704> ;
.
<https://w3id.org/con-tax/zones/aat-spaces#300075338>
  rdf:type owl:Class ;
  rdfs:isDefinedBy <https://w3id.org/con-tax/zones/aat-spaces> ;
  rdfs:label "filmzaal"@nl ;
  rdfs:label "filmzalen"@nl ;
  rdfs:label "screening rooms"@en ;
  rdfs:seeAlso <http://vocab.getty.edu/aat/300075338> ;
  rdfs:subClassOf <https://w3id.org/con-tax/zones/aat-spaces#300133704> ;
.
<https://w3id.org/con-tax/zones/aat-spaces#300075405>
  rdf:type owl:Class ;
  rdfs:comment "Lounges die zijn gereserveerd voor belangrijke en bevoorrechte personen, zoals bijvoorbeeld op schepen en op luchthavens."@nl ;
  rdfs:comment "Lounges reserved for privileged and important individuals."@en ;
  rdfs:isDefinedBy <https://w3id.org/con-tax/zones/aat-spaces> ;
  rdfs:label "V.I.P. lounges"@en ;
  rdfs:label "VIP-lounge"@nl ;
  rdfs:label "VIP-lounges"@nl ;
  rdfs:seeAlso <http://vocab.getty.edu/aat/300075405> ;
  rdfs:subClassOf <https://w3id.org/con-tax/zones/aat-spaces#300004436> ;
.
<https://w3id.org/con-tax/zones/aat-spaces#300075458>
  rdf:type owl:Class ;
  rdfs:comment "Rooms that are connected or combined, such as apartments or suites. "@en ;
  rdfs:isDefinedBy <https://w3id.org/con-tax/zones/aat-spaces> ;
  rdfs:label "combinations of rooms"@en ;
  rdfs:label "samenstel van kamers"@nl ;
  rdfs:seeAlso <http://vocab.getty.edu/aat/300075458> ;
  rdfs:subClassOf <https://w3id.org/con-tax/zones/aat-spaces#300078790> ;
.
<https://w3id.org/con-tax/zones/aat-spaces#300075459>
  rdf:type owl:Class ;
  rdfs:comment "Building spaces that are covered, and located on the exterior of the buildings. "@en ;
  rdfs:isDefinedBy <https://w3id.org/con-tax/zones/aat-spaces> ;
  rdfs:label "exterior covered spaces"@en ;
  rdfs:label "overdekte buitenruimte"@nl ;
  rdfs:label "overdekte buitenruimten"@nl ;
  rdfs:seeAlso <http://vocab.getty.edu/aat/300075459> ;
  rdfs:seeAlso wd:Q21550596 ;
  rdfs:subClassOf <https://w3id.org/con-tax/zones/aat-spaces#300133704> ;
.
<https://w3id.org/con-tax/zones/aat-spaces#300075460>
  rdf:type owl:Class ;
  rdfs:comment "Spaces attached to buildings that are uncovered. "@en ;
  rdfs:isDefinedBy <https://w3id.org/con-tax/zones/aat-spaces> ;
  rdfs:label "niet-overdekte ruimte"@nl ;
  rdfs:label "niet-overdekte ruimten"@nl ;
  rdfs:label "uncovered spaces"@en ;
  rdfs:seeAlso <http://vocab.getty.edu/aat/300075460> ;
  rdfs:subClassOf <https://w3id.org/con-tax/zones/aat-spaces#300133704> ;
.
<https://w3id.org/con-tax/zones/aat-spaces#300075767>
  rdf:type owl:Class ;
  rdfs:comment "Use to designate large rooms that are much longer than they are wide, such as the long galleries of Elizabethan country houses."@en ;
  rdfs:comment "Zalen die veel langer zijn dan dat ze breed zijn, belangrijk onderdeel in de paleisbouw van Renaissance en Barok, bijvoorbeeld de 'long galleries' in Engelse landhuizen uit de tijd van Jacobus I en Elizabeth I."@nl ;
  rdfs:isDefinedBy <https://w3id.org/con-tax/zones/aat-spaces> ;
  rdfs:label "long galleries"@en ;
  rdfs:label "wandelzaal"@nl ;
  rdfs:label "wandelzalen"@nl ;
  rdfs:seeAlso <http://vocab.getty.edu/aat/300075767> ;
  rdfs:seeAlso wd:Q164419 ;
  rdfs:subClassOf <https://w3id.org/con-tax/zones/aat-spaces#300078790> ;
.
<https://w3id.org/con-tax/zones/aat-spaces#300075769>
  rdf:type gvp:GuideTerm ;
  rdfs:isDefinedBy <https://w3id.org/con-tax/zones/aat-spaces> ;
  rdfs:label "<nuts- en toegangsruimten>"@nl ;
  rdfs:label "<utility and access spaces>"@en ;
  rdfs:label "nuts- en toegangsruimten"@nl ;
  rdfs:seeAlso <http://vocab.getty.edu/aat/300075769> ;
  contax:containsConcept <https://w3id.org/con-tax/zones/aat-spaces#300004245> ;
  contax:containsConcept <https://w3id.org/con-tax/zones/aat-spaces#300004246> ;
  contax:containsConcept <https://w3id.org/con-tax/zones/aat-spaces#300004249> ;
  contax:containsConcept <https://w3id.org/con-tax/zones/aat-spaces#300004257> ;
  contax:containsConcept <https://w3id.org/con-tax/zones/aat-spaces#300004315> ;
  contax:containsConcept <https://w3id.org/con-tax/zones/aat-spaces#300004526> ;
.
<https://w3id.org/con-tax/zones/aat-spaces#300075770>
  rdf:type gvp:GuideTerm ;
  rdfs:isDefinedBy <https://w3id.org/con-tax/zones/aat-spaces> ;
  rdfs:label "<kamers en ruimten naar gebruikers>"@nl ;
  rdfs:label "<rooms and spaces by occupants>"@en ;
  rdfs:label "kamers en ruimten naar gebruikers"@nl ;
  rdfs:seeAlso <http://vocab.getty.edu/aat/300075770> ;
  contax:containsConcept <https://w3id.org/con-tax/zones/aat-spaces#300004380> ;
  contax:containsConcept <https://w3id.org/con-tax/zones/aat-spaces#300082094> ;
  contax:containsConcept <https://w3id.org/con-tax/zones/aat-spaces#300255752> ;
  contax:containsConcept <https://w3id.org/con-tax/zones/aat-spaces#300260516> ;
  contax:containsConcept <https://w3id.org/con-tax/zones/aat-spaces#300260517> ;
.
<https://w3id.org/con-tax/zones/aat-spaces#300075809>
  rdf:type gvp:GuideTerm ;
  rdfs:isDefinedBy <https://w3id.org/con-tax/zones/aat-spaces> ;
  rdfs:label "<entertainment and recreation spaces>"@en ;
  rdfs:label "<sport- en recreatieruimte>"@nl ;
  rdfs:label "<sport- en recreatieruimten>"@nl ;
  rdfs:label "sport- en recreatieruimte"@nl ;
  rdfs:label "sport- en recreatieruimten"@nl ;
  rdfs:seeAlso <http://vocab.getty.edu/aat/300075809> ;
  contax:containsConcept <https://w3id.org/con-tax/zones/aat-spaces#300004393> ;
  contax:containsConcept <https://w3id.org/con-tax/zones/aat-spaces#300004413> ;
  contax:containsConcept <https://w3id.org/con-tax/zones/aat-spaces#300004451> ;
  contax:containsConcept <https://w3id.org/con-tax/zones/aat-spaces#300004520> ;
  contax:containsConcept <https://w3id.org/con-tax/zones/aat-spaces#300007306> ;
  contax:containsConcept <https://w3id.org/con-tax/zones/aat-spaces#300075338> ;
  contax:containsConcept <https://w3id.org/con-tax/zones/aat-spaces#300081184> ;
  contax:containsConcept <https://w3id.org/con-tax/zones/aat-spaces#300179305> ;
  contax:containsConcept <https://w3id.org/con-tax/zones/aat-spaces#300249326> ;
  contax:containsConcept <https://w3id.org/con-tax/zones/aat-spaces#300263175> ;
.
<https://w3id.org/con-tax/zones/aat-spaces#300075830>
  rdf:type owl:Class ;
  rdfs:comment "Grote, overwelfde zalen waarvan één kant op een binnenplaats uitkomt. Gebruikelijk in de Parthische, de Sassanidische en Islamitische architectuur."@nl ;
  rdfs:comment "Large vaulted halls having one side open to a court; prevalent in Parthian, Sassanian, and Islamic architecture."@en ;
  rdfs:isDefinedBy <https://w3id.org/con-tax/zones/aat-spaces> ;
  rdfs:label "iwan"@nl ;
  rdfs:label "iwans"@en ;
  rdfs:label "iwans"@nl ;
  rdfs:seeAlso <http://vocab.getty.edu/aat/300075830> ;
  rdfs:subClassOf <https://w3id.org/con-tax/zones/aat-spaces#300075459> ;
.
<https://w3id.org/con-tax/zones/aat-spaces#300075880>
  rdf:type owl:Class ;
  rdfs:comment "Spaces in buildings used specifically for receptions. "@en ;
  rdfs:isDefinedBy <https://w3id.org/con-tax/zones/aat-spaces> ;
  rdfs:label "ontvangstruimten"@nl ;
  rdfs:label "reception spaces"@en ;
  rdfs:seeAlso <http://vocab.getty.edu/aat/300075880> ;
  rdfs:subClassOf <https://w3id.org/con-tax/zones/aat-spaces#300133704> ;
.
<https://w3id.org/con-tax/zones/aat-spaces#300075881>
  rdf:type owl:Class ;
  rdfs:comment "Rooms in buildings specifcally used for gatherings or meetings."@en ;
  rdfs:isDefinedBy <https://w3id.org/con-tax/zones/aat-spaces> ;
  rdfs:label "assembly spaces"@en ;
  rdfs:label "ruimten voor samenkomst"@nl ;
  rdfs:seeAlso <http://vocab.getty.edu/aat/300075881> ;
  rdfs:subClassOf <https://w3id.org/con-tax/zones/aat-spaces#300133704> ;
.
<https://w3id.org/con-tax/zones/aat-spaces#300075882>
  rdf:type owl:Class ;
  rdfs:comment "Rooms and spaces located in places of burial."@en ;
  rdfs:isDefinedBy <https://w3id.org/con-tax/zones/aat-spaces> ;
  rdfs:label "graftomberuimten"@nl ;
  rdfs:label "tomb spaces"@en ;
  rdfs:seeAlso <http://vocab.getty.edu/aat/300075882> ;
  rdfs:subClassOf <https://w3id.org/con-tax/zones/aat-spaces#300133704> ;
.
<https://w3id.org/con-tax/zones/aat-spaces#300075884>
  rdf:type owl:Class ;
  rdfs:comment "Halfronde of polygonale omloopruimten die een apsis of een rechtgesloten koor omsluiten."@nl ;
  rdfs:comment "Semicircular or polygonal circulation spaces enclosing an apse or a straight-ended sanctuary."@en ;
  rdfs:isDefinedBy <https://w3id.org/con-tax/zones/aat-spaces> ;
  rdfs:label "ambulatoria"@nl ;
  rdfs:label "ambulatories"@en ;
  rdfs:label "ambulatorium"@nl ;
  rdfs:label "ambulatoriums"@nl ;
  rdfs:label "deambulatoria"@nl ;
  rdfs:label "deambulatorium"@nl ;
  rdfs:label "trans"@nl ;
  rdfs:label "transen"@nl ;
  rdfs:seeAlso <http://vocab.getty.edu/aat/300075884> ;
  rdfs:seeAlso wd:Q756720 ;
  rdfs:subClassOf <https://w3id.org/con-tax/zones/aat-spaces#300004284> ;
  rdfs:subClassOf <https://w3id.org/con-tax/zones/aat-spaces#300004560> ;
.
<https://w3id.org/con-tax/zones/aat-spaces#300076663>
  rdf:type owl:Class ;
  rdfs:comment "Rooms adjacent to a lady's bedroom, serving as private sitting rooms and dressing rooms."@en ;
  rdfs:comment "Wordt gebruikt voor kamers voor dames die dienen als privé-zitkamers en kleedkamers en die naast hun slaapkamers liggen."@nl ;
  rdfs:isDefinedBy <https://w3id.org/con-tax/zones/aat-spaces> ;
  rdfs:label "boudoir (kamer)"@nl ;
  rdfs:label "boudoir"@nl ;
  rdfs:label "boudoirs (kamers)"@nl ;
  rdfs:label "boudoirs (rooms)"@en ;
  rdfs:label "boudoirs"@nl ;
  rdfs:seeAlso <http://vocab.getty.edu/aat/300076663> ;
  rdfs:seeAlso wd:Q62238 ;
  rdfs:subClassOf <https://w3id.org/con-tax/zones/aat-spaces#300078138> ;
.
<https://w3id.org/con-tax/zones/aat-spaces#300076669>
  rdf:type owl:Class ;
  rdfs:comment "Rooms at which baggage, parcels, clothing, or other personal articles are deposited with a clerk for temporary storage."@en ;
  rdfs:comment "Ruimten waar bagage, pakjes, kleding of andere persoonlijke artikelen tijdelijk in bewaring worden gegeven aan een toezichthouder. Gebruik voor ruimten in openbare gebouwen waar jassen en dergelijke kunnen worden opgehangen 'vestiaires', voor ruimten om kleding te bewaren in de huiselijke sfeer 'kleerkamers'."@nl ;
  rdfs:isDefinedBy <https://w3id.org/con-tax/zones/aat-spaces> ;
  rdfs:label "checkrooms"@en-us ;
  rdfs:label "garderobe"@nl ;
  rdfs:label "garderobes"@nl ;
  rdfs:seeAlso <http://vocab.getty.edu/aat/300076669> ;
  rdfs:subClassOf <https://w3id.org/con-tax/zones/aat-spaces#300004465> ;
.
<https://w3id.org/con-tax/zones/aat-spaces#300077176>
  rdf:type owl:Class ;
  rdfs:comment "Kamers voor de formele ontvangst van gasten, vertegenwoordigers en ander bezoek."@nl ;
  rdfs:comment "Rooms whose purpose is the formal reception of guests, tradesmen, and other visitors."@en ;
  rdfs:isDefinedBy <https://w3id.org/con-tax/zones/aat-spaces> ;
  rdfs:label "ontvangkamer"@nl ;
  rdfs:label "ontvangkamers"@nl ;
  rdfs:label "ontvangstkamer"@nl ;
  rdfs:label "ontvangstkamers"@nl ;
  rdfs:label "receptiekamer"@nl ;
  rdfs:label "receptiekamers"@nl ;
  rdfs:label "reception rooms"@en ;
  rdfs:seeAlso <http://vocab.getty.edu/aat/300077176> ;
  rdfs:subClassOf <https://w3id.org/con-tax/zones/aat-spaces#300075880> ;
.
<https://w3id.org/con-tax/zones/aat-spaces#300078138>
  rdf:type owl:Class ;
  rdfs:comment "Relatively small, private rooms, often adjacent to bedrooms in great houses, serving as sitting rooms, rooms for dressing, study, devotion, or private meetings, and, during certain periods, often containing collections of curiosities and art objects."@en ;
  rdfs:comment "Wordt gebruikt voor kleine privévertrekken die meestal naast slaapkamers in landhuizen liggen en dienen als zit- en kleedkamer, en waarin zich vaak collecties van kunstobjecten bevinden."@nl ;
  rdfs:isDefinedBy <https://w3id.org/con-tax/zones/aat-spaces> ;
  rdfs:label "cabinets (rooms)"@en ;
  rdfs:label "kabinet (kamer)"@nl ;
  rdfs:label "kabinet"@nl ;
  rdfs:label "kabinetten (kamers)"@nl ;
  rdfs:label "kabinetten"@nl ;
  rdfs:seeAlso <http://vocab.getty.edu/aat/300078138> ;
  rdfs:subClassOf <https://w3id.org/con-tax/zones/aat-spaces#300133704> ;
.
<https://w3id.org/con-tax/zones/aat-spaces#300078146>
  rdf:type owl:Class ;
  rdfs:comment "Refers to the ground floors of theaters, especially those at the rear; most appropriate in an English and historical rather than a modern American context."@en ;
  rdfs:comment "Wordt gebruikt om de begane grond van theaters aan te duiden, vooral het gedeelte aan de achterzijde. Eerder in een Engelse en historische context dan een moderne Amerikaanse."@nl ;
  rdfs:isDefinedBy <https://w3id.org/con-tax/zones/aat-spaces> ;
  rdfs:label "pit (theaterruimte)"@nl ;
  rdfs:label "pit"@nl ;
  rdfs:label "pits (theater spaces)"@en ;
  rdfs:label "pits (theaterruimten)"@nl ;
  rdfs:label "pits"@nl ;
  rdfs:seeAlso <http://vocab.getty.edu/aat/300078146> ;
  rdfs:subClassOf <https://w3id.org/con-tax/zones/aat-spaces#300104771> ;
.
<https://w3id.org/con-tax/zones/aat-spaces#300078790>
  rdf:type owl:Class ;
  rdfs:comment "Spaces located in the interior of structures. "@en ;
  rdfs:isDefinedBy <https://w3id.org/con-tax/zones/aat-spaces> ;
  rdfs:label "binnenruimte"@nl ;
  rdfs:label "binnenruimten"@nl ;
  rdfs:label "interior spaces (spaces by location)"@en ;
  rdfs:seeAlso <http://vocab.getty.edu/aat/300078790> ;
  rdfs:subClassOf <https://w3id.org/con-tax/zones/aat-spaces#300133704> ;
.
<https://w3id.org/con-tax/zones/aat-spaces#300080054>
  rdf:type owl:Class ;
  rdfs:comment "Areas or spaces located in ancient Roman baths. "@en ;
  rdfs:isDefinedBy <https://w3id.org/con-tax/zones/aat-spaces> ;
  rdfs:label "Roman bath spaces"@en ;
  rdfs:label "Romeinse badruimte"@nl ;
  rdfs:label "Romeinse badruimten"@nl ;
  rdfs:seeAlso <http://vocab.getty.edu/aat/300080054> ;
  rdfs:subClassOf <https://w3id.org/con-tax/zones/aat-spaces#300133704> ;
.
<https://w3id.org/con-tax/zones/aat-spaces#300080603>
  rdf:type owl:Class ;
  rdfs:comment "Rooms in barns or stables with provisions for feeding horses or other animals."@en ;
  rdfs:comment "Ruimten in schuren of stallen met voorzieningen voor het voederen van paarden of andere dieren. Geen Nederlands equivalent."@nl ;
  rdfs:isDefinedBy <https://w3id.org/con-tax/zones/aat-spaces> ;
  rdfs:label "feed rooms"@en ;
  rdfs:label "voedingsruimte"@nl ;
  rdfs:label "voedingsruimten"@nl ;
  rdfs:seeAlso <http://vocab.getty.edu/aat/300080603> ;
  rdfs:subClassOf <https://w3id.org/con-tax/zones/aat-spaces#300133704> ;
.
<https://w3id.org/con-tax/zones/aat-spaces#300080610>
  rdf:type owl:Class ;
  rdfs:comment "Afzonderlijke compartimenten in schuren of stallen, waarin dieren enigszins vrij kunnen rondlopen. Met name gebruikt met betrekking tot paarden."@nl ;
  rdfs:comment "In barns or stables, individual compartments in which an animal may move about freely."@en ;
  rdfs:isDefinedBy <https://w3id.org/con-tax/zones/aat-spaces> ;
  rdfs:label "box (stalruimte)"@nl ;
  rdfs:label "box stalls"@en ;
  rdfs:label "box"@nl ;
  rdfs:label "boxen (stalruimten)"@nl ;
  rdfs:label "boxen"@nl ;
  rdfs:seeAlso <http://vocab.getty.edu/aat/300080610> ;
  rdfs:subClassOf <https://w3id.org/con-tax/zones/aat-spaces#300004172> ;
.
<https://w3id.org/con-tax/zones/aat-spaces#300080791>
  rdf:type owl:Class ;
  rdfs:comment "De belangrijkste kamers van oude Griekse huizen en soortgelijke kamers in oude Romeinse huizen, meestal gebruikt om in te dineren."@nl ;
  rdfs:comment "Refers to the main rooms of ancient Greek houses and for similar rooms in ancient Roman houses used as reception areas."@en ;
  rdfs:isDefinedBy <https://w3id.org/con-tax/zones/aat-spaces> ;
  rdfs:label "oeci"@en ;
  rdfs:label "oeci"@nl ;
  rdfs:label "oecus"@nl ;
  rdfs:seeAlso <http://vocab.getty.edu/aat/300080791> ;
  rdfs:subClassOf <https://w3id.org/con-tax/zones/aat-spaces#300078790> ;
.
<https://w3id.org/con-tax/zones/aat-spaces#300080798>
  rdf:type owl:Class ;
  rdfs:comment "Overdekte binnenplaatsen met direct daglicht in of tussen gebouwen van meerdere verdiepingen; vanaf ongeveer 1960."@nl ;
  rdfs:comment "Refers to many-storied, skylit spaces in or between high-rise buildings, common since 1960."@en ;
  rdfs:isDefinedBy <https://w3id.org/con-tax/zones/aat-spaces> ;
  rdfs:label "atrium (binnenruimte)"@nl ;
  rdfs:label "atrium"@nl ;
  rdfs:label "atriums (binnenruimten)"@nl ;
  rdfs:label "atriums (interior spaces)"@en ;
  rdfs:label "atriums"@nl ;
  rdfs:seeAlso <http://vocab.getty.edu/aat/300080798> ;
  rdfs:subClassOf <https://w3id.org/con-tax/zones/aat-spaces#300078790> ;
.
<https://w3id.org/con-tax/zones/aat-spaces#300080805>
  rdf:type owl:Class ;
  rdfs:comment "Overdekte buitenruimten die twee delen van een huis, of een huis en een garage met elkaar verbinden."@nl ;
  rdfs:comment "Roofed passages connecting two parts of a house or a house and garage; common after 1930. Distinct from \"dogtrots,\" which occur in folk architecture and log houses."@en ;
  rdfs:isDefinedBy <https://w3id.org/con-tax/zones/aat-spaces> ;
  rdfs:label "breezeways"@en-us ;
  rdfs:label "overdekte doorgang"@nl ;
  rdfs:label "overdekte doorgangen"@nl ;
  rdfs:seeAlso <http://vocab.getty.edu/aat/300080805> ;
  rdfs:subClassOf <https://w3id.org/con-tax/zones/aat-spaces#300075459> ;
.
<https://w3id.org/con-tax/zones/aat-spaces#300080971>
  rdf:type owl:Class ;
  rdfs:comment "Binnenplaatsen aan de achterzijde van antieke Romeinse huizen, gewoonlijk een tuin omgeven door een zuilengang."@nl ;
  rdfs:comment "Refers to the court toward the back of a Roman house, commonly with a small garden surrounded by a colonnade."@en ;
  rdfs:isDefinedBy <https://w3id.org/con-tax/zones/aat-spaces> ;
  rdfs:label "peristilia"@nl ;
  rdfs:label "peristilium"@nl ;
  rdfs:label "peristyle (Romeinse binnenplaats)"@nl ;
  rdfs:label "peristyle"@nl ;
  rdfs:label "peristylen (Romeinse binnenplaatsen)"@nl ;
  rdfs:label "peristylen"@nl ;
  rdfs:label "peristyles (Roman courtyards)"@en ;
  rdfs:seeAlso <http://vocab.getty.edu/aat/300080971> ;
  rdfs:seeAlso wd:Q725453 ;
  rdfs:subClassOf <https://w3id.org/con-tax/zones/aat-spaces#300004095> ;
.
<https://w3id.org/con-tax/zones/aat-spaces#300081124>
  rdf:type owl:Class ;
  rdfs:comment "Rooms containing a sink and toilet, but neither tub nor shower."@en ;
  rdfs:comment "Wordt gebruikt voor kamers waarin zich een wastafel en een w.c. bevinden."@nl ;
  rdfs:isDefinedBy <https://w3id.org/con-tax/zones/aat-spaces> ;
  rdfs:label "lavatories (rooms)"@en ;
  rdfs:label "toiletblok"@nl ;
  rdfs:label "toiletblokken"@nl ;
  rdfs:label "toiletruimte"@nl ;
  rdfs:label "toiletruimten"@nl ;
  rdfs:seeAlso <http://vocab.getty.edu/aat/300081124> ;
  rdfs:subClassOf <https://w3id.org/con-tax/zones/aat-spaces#300133704> ;
.
<https://w3id.org/con-tax/zones/aat-spaces#300081126>
  rdf:type owl:Class ;
  rdfs:comment "Refers to enclosures erected around toilets for privacy."@en ;
  rdfs:comment "Wordt gebruikt voor afsluitbare kamers, waarin zich een afzonderlijk toilet bevindt."@nl ;
  rdfs:isDefinedBy <https://w3id.org/con-tax/zones/aat-spaces> ;
  rdfs:label "toilet compartments"@en ;
  rdfs:label "toiletkamer"@nl ;
  rdfs:label "toiletkamers"@nl ;
  rdfs:seeAlso <http://vocab.getty.edu/aat/300081126> ;
  rdfs:subClassOf <https://w3id.org/con-tax/zones/aat-spaces#300133704> ;
.
<https://w3id.org/con-tax/zones/aat-spaces#300081128>
  rdf:type owl:Class ;
  rdfs:comment "Showrooms in hotels specially arranged for the display of merchandise by traveling salesmen."@en ;
  rdfs:comment "Showrooms, bijvoorbeeld in hotels, bedoeld voor het tonen van monsters van produkten door vertegenwoordigers."@nl ;
  rdfs:isDefinedBy <https://w3id.org/con-tax/zones/aat-spaces> ;
  rdfs:label "sample rooms"@en ;
  rdfs:label "verkoopvitrine"@nl ;
  rdfs:label "verkoopvitrines"@nl ;
  rdfs:seeAlso <http://vocab.getty.edu/aat/300081128> ;
  rdfs:subClassOf <https://w3id.org/con-tax/zones/aat-spaces#300004331> ;
.
<https://w3id.org/con-tax/zones/aat-spaces#300081159>
  rdf:type owl:Class ;
  rdfs:comment "Kamers bestemd voor bijeenkomsten van een bestuur, doorgaans voorzien van een vergadertafel."@nl ;
  rdfs:comment "Rooms that are designated for meetings of a board and usually contain a large conference table."@en ;
  rdfs:isDefinedBy <https://w3id.org/con-tax/zones/aat-spaces> ;
  rdfs:label "bestuurskamer"@nl ;
  rdfs:label "bestuurskamers"@nl ;
  rdfs:label "boardrooms"@en-us ;
  rdfs:label "directiekamer"@nl ;
  rdfs:label "directiekamers"@nl ;
  rdfs:seeAlso <http://vocab.getty.edu/aat/300081159> ;
  rdfs:subClassOf <https://w3id.org/con-tax/zones/aat-spaces#300004398> ;
.
<https://w3id.org/con-tax/zones/aat-spaces#300081177>
  rdf:type owl:Class ;
  rdfs:comment "Rooms equipped for card playing."@en ;
  rdfs:comment "Wordt gebruikt voor kamers die zijn bestemd voor het kaartspelen."@nl ;
  rdfs:isDefinedBy <https://w3id.org/con-tax/zones/aat-spaces> ;
  rdfs:label "cardrooms"@en-us ;
  rdfs:label "kaartkamer"@nl ;
  rdfs:label "kaartkamers"@nl ;
  rdfs:seeAlso <http://vocab.getty.edu/aat/300081177> ;
  rdfs:seeAlso wd:Q5038786 ;
  rdfs:subClassOf <https://w3id.org/con-tax/zones/aat-spaces#300004452> ;
.
<https://w3id.org/con-tax/zones/aat-spaces#300081184>
  rdf:type owl:Class ;
  rdfs:comment "Rooms devoted to gambling."@en ;
  rdfs:comment "Wordt gebruikt voor ruimten die gebruikt worden om te gokken."@nl ;
  rdfs:isDefinedBy <https://w3id.org/con-tax/zones/aat-spaces> ;
  rdfs:label "gaming rooms"@en ;
  rdfs:label "speelzaal"@nl ;
  rdfs:label "speelzalen"@nl ;
  rdfs:seeAlso <http://vocab.getty.edu/aat/300081184> ;
  rdfs:subClassOf <https://w3id.org/con-tax/zones/aat-spaces#300133704> ;
.
<https://w3id.org/con-tax/zones/aat-spaces#300081620>
  rdf:type owl:Class ;
  rdfs:comment "Kamers, bedoeld als ingang naar en wachtruimte bij een andere, belangrijkere kamer."@nl ;
  rdfs:comment "Rooms preceding or serving as a lobby or means of access to another and more important room."@en ;
  rdfs:isDefinedBy <https://w3id.org/con-tax/zones/aat-spaces> ;
  rdfs:label "antechambres"@nl ;
  rdfs:label "anterooms"@en-us ;
  rdfs:label "antichambre"@nl ;
  rdfs:label "antichambres"@nl ;
  rdfs:label "voorvertrekken"@nl ;
  rdfs:seeAlso <http://vocab.getty.edu/aat/300081620> ;
  rdfs:seeAlso wd:Q4771130 ;
  rdfs:subClassOf <https://w3id.org/con-tax/zones/aat-spaces#300004259> ;
.
<https://w3id.org/con-tax/zones/aat-spaces#300081731>
  rdf:type owl:Class ;
  rdfs:comment "De buitenste of minder belangrijke binnenplaatsen van landhuizen of kastelen."@nl ;
  rdfs:comment "Refers to the outer or lesser courts of mansions or castles."@en ;
  rdfs:isDefinedBy <https://w3id.org/con-tax/zones/aat-spaces> ;
  rdfs:label "base-courts"@en ;
  rdfs:label "basse-cours"@nl ;
  rdfs:label "buitenhof"@nl ;
  rdfs:label "buitenhoven"@nl ;
  rdfs:label "hoerderhoven"@nl ;
  rdfs:seeAlso <http://vocab.getty.edu/aat/300081731> ;
  rdfs:subClassOf <https://w3id.org/con-tax/zones/aat-spaces#300004095> ;
.
<https://w3id.org/con-tax/zones/aat-spaces#300081780>
  rdf:type gvp:GuideTerm ;
  rdfs:isDefinedBy <https://w3id.org/con-tax/zones/aat-spaces> ;
  rdfs:label "<lees- en schrijfruimten>"@nl ;
  rdfs:label "<reading and writing spaces>"@en ;
  rdfs:label "lees- en schrijfruimten"@nl ;
  rdfs:seeAlso <http://vocab.getty.edu/aat/300081780> ;
  contax:containsConcept <https://w3id.org/con-tax/zones/aat-spaces#300004173> ;
  contax:containsConcept <https://w3id.org/con-tax/zones/aat-spaces#300004433> ;
  contax:containsConcept <https://w3id.org/con-tax/zones/aat-spaces#300004434> ;
  contax:containsConcept <https://w3id.org/con-tax/zones/aat-spaces#300081781> ;
  contax:containsConcept <https://w3id.org/con-tax/zones/aat-spaces#300081784> ;
  contax:containsConcept <https://w3id.org/con-tax/zones/aat-spaces#300132308> ;
  contax:containsConcept <https://w3id.org/con-tax/zones/aat-spaces#300386040> ;
.
<https://w3id.org/con-tax/zones/aat-spaces#300081781>
  rdf:type owl:Class ;
  rdfs:comment "Kamers of ruimten in huiselijke omgeving die worden gebruikt om in te lezen, te schrijven en te studeren."@nl ;
  rdfs:comment "Rooms or spaces in domestic contexts used for reading, writing, and study."@en ;
  rdfs:isDefinedBy <https://w3id.org/con-tax/zones/aat-spaces> ;
  rdfs:label "studeerkamer"@nl ;
  rdfs:label "studeerkamers"@nl ;
  rdfs:label "studeervertrek"@nl ;
  rdfs:label "studeervertrekken"@nl ;
  rdfs:label "studies (rooms)"@en ;
  rdfs:seeAlso <http://vocab.getty.edu/aat/300081781> ;
  rdfs:seeAlso wd:Q1759167 ;
  rdfs:subClassOf <https://w3id.org/con-tax/zones/aat-spaces#300133704> ;
.
<https://w3id.org/con-tax/zones/aat-spaces#300081784>
  rdf:type owl:Class ;
  rdfs:comment "Kamers die bestemd zijn om in te schrijven, zoals in een residentie, hotel of club."@nl ;
  rdfs:comment "Rooms set aside for writing, as in a residence, hotel, or club."@en ;
  rdfs:isDefinedBy <https://w3id.org/con-tax/zones/aat-spaces> ;
  rdfs:label "schrijfkamer"@nl ;
  rdfs:label "schrijfkamers"@nl ;
  rdfs:label "writing rooms"@en ;
  rdfs:seeAlso <http://vocab.getty.edu/aat/300081784> ;
  rdfs:subClassOf <https://w3id.org/con-tax/zones/aat-spaces#300133704> ;
.
<https://w3id.org/con-tax/zones/aat-spaces#300081842>
  rdf:type owl:Class ;
  rdfs:comment "Eetruimten die onderdeel vormen van andere ruimten, zoals keukens en woonkamers."@nl ;
  rdfs:comment "Small dining areas, usually extensions of kitchens or pantries; for such areas when they are extensions of living rooms, use \"dining alcoves.\""@en ;
  rdfs:isDefinedBy <https://w3id.org/con-tax/zones/aat-spaces> ;
  rdfs:label "dinettes"@en ;
  rdfs:label "eethoek"@nl ;
  rdfs:label "eethoeken"@nl ;
  rdfs:seeAlso <http://vocab.getty.edu/aat/300081842> ;
  rdfs:subClassOf <https://w3id.org/con-tax/zones/aat-spaces#300133704> ;
.
<https://w3id.org/con-tax/zones/aat-spaces#300081956>
  rdf:type owl:Class ;
  rdfs:comment "Rooms containing a number of beds and serving as communal sleeping quarters, as in an institution, fraternity house, or passenger ship."@en ;
  rdfs:comment "Zalen met bedden die dienen als gemeenschappelijke slaapruimte, b.v. in internaten, jeugdherbergen of kazernes. Gebruik voor slaapzalen in kloosters 'dormitoria'."@nl ;
  rdfs:isDefinedBy <https://w3id.org/con-tax/zones/aat-spaces> ;
  rdfs:label "dormitories (rooms)"@en ;
  rdfs:label "slaapzaal"@nl ;
  rdfs:label "slaapzalen"@nl ;
  rdfs:seeAlso <http://vocab.getty.edu/aat/300081956> ;
  rdfs:subClassOf <https://w3id.org/con-tax/zones/aat-spaces#300004362> ;
.
<https://w3id.org/con-tax/zones/aat-spaces#300081958>
  rdf:type owl:Class ;
  rdfs:comment "Rooms for sitting and relaxation, often located adjacent to bedrooms and generally more private than living rooms or parlors."@en ;
  rdfs:comment "Wordt gebruikt voor kamers die zijn bedoeld om in te zitten en ontspannen; meestal gelegen naast slaapkamers en over het algemeen meer privé dan woonkamers of salons."@nl ;
  rdfs:isDefinedBy <https://w3id.org/con-tax/zones/aat-spaces> ;
  rdfs:label "sitting room"@nl ;
  rdfs:label "sitting rooms"@en ;
  rdfs:label "sitting rooms"@nl ;
  rdfs:seeAlso <http://vocab.getty.edu/aat/300081958> ;
  rdfs:seeAlso wd:Q10550521 ;
  rdfs:seeAlso wd:Q475018 ;
  rdfs:subClassOf <https://w3id.org/con-tax/zones/aat-spaces#300133704> ;
.
<https://w3id.org/con-tax/zones/aat-spaces#300082014>
  rdf:type owl:Class ;
  rdfs:comment "Dienstvertrekken tussen keukens en eetkamers, die zijn uitgerust met toonbanken, wasbakken en bergruimte voor porselein en zilver."@nl ;
  rdfs:comment "Service rooms between kitchens and dining rooms, typically equipped with counters, a sink, and storage space for china and silver."@en ;
  rdfs:isDefinedBy <https://w3id.org/con-tax/zones/aat-spaces> ;
  rdfs:label "butlers' pantries"@en ;
  rdfs:label "butlerskeuken"@nl ;
  rdfs:label "butlerskeukens"@nl ;
  rdfs:seeAlso <http://vocab.getty.edu/aat/300082014> ;
  rdfs:subClassOf <https://w3id.org/con-tax/zones/aat-spaces#300004499> ;
.
<https://w3id.org/con-tax/zones/aat-spaces#300082023>
  rdf:type owl:Class ;
  rdfs:comment "Certain rooms or spaces in large houses, usually connected to kitchens, where liquors, preserves, and cakes are kept."@en ;
  rdfs:comment "Wordt gebruikt voor kamers of ruimten in grote huizen, die meestal in verbinding staan met de keuken en waarin drank, confituren en taarten worden bewaard."@nl ;
  rdfs:isDefinedBy <https://w3id.org/con-tax/zones/aat-spaces> ;
  rdfs:label "destilleerkamer"@nl ;
  rdfs:label "destilleerkamers"@nl ;
  rdfs:label "stillrooms"@en-us ;
  rdfs:seeAlso <http://vocab.getty.edu/aat/300082023> ;
  rdfs:seeAlso wd:Q17130650 ;
  rdfs:subClassOf <https://w3id.org/con-tax/zones/aat-spaces#300004465> ;
.
<https://w3id.org/con-tax/zones/aat-spaces#300082039>
  rdf:type gvp:GuideTerm ;
  rdfs:isDefinedBy <https://w3id.org/con-tax/zones/aat-spaces> ;
  rdfs:label "<kamers en ruimten naar eigenschap>"@nl ;
  rdfs:label "<rooms and spaces by property>"@en ;
  rdfs:label "kamers en ruimten naar eigenschap"@nl ;
  rdfs:seeAlso <http://vocab.getty.edu/aat/300082039> ;
  contax:containsConcept <https://w3id.org/con-tax/zones/aat-spaces#300004506> ;
  contax:containsConcept <https://w3id.org/con-tax/zones/aat-spaces#300004509> ;
  contax:containsConcept <https://w3id.org/con-tax/zones/aat-spaces#300004512> ;
  contax:containsConcept <https://w3id.org/con-tax/zones/aat-spaces#300379866> ;
.
<https://w3id.org/con-tax/zones/aat-spaces#300082083>
  rdf:type owl:Class ;
  rdfs:comment "Kamers die bestemd zijn om te roken, zoals in hotels of clubhuizen en op schepen. Gebruik voor rookruimten in woonhuizen 'rookkamers'."@nl ;
  rdfs:comment "Rooms set apart for smoking, as in hotels or clubhouses."@en ;
  rdfs:isDefinedBy <https://w3id.org/con-tax/zones/aat-spaces> ;
  rdfs:label "rooksalon"@nl ;
  rdfs:label "rooksalons"@nl ;
  rdfs:label "smoking rooms"@en-us ;
  rdfs:seeAlso <http://vocab.getty.edu/aat/300082083> ;
  rdfs:seeAlso wd:Q1052631 ;
  rdfs:subClassOf <https://w3id.org/con-tax/zones/aat-spaces#300133704> ;
.
<https://w3id.org/con-tax/zones/aat-spaces#300082087>
  rdf:type owl:Class ;
  rdfs:isDefinedBy <https://w3id.org/con-tax/zones/aat-spaces> ;
  rdfs:label "gun rooms"@en ;
  rdfs:label "wapenkamer"@nl ;
  rdfs:label "wapenkamers"@nl ;
  rdfs:seeAlso <http://vocab.getty.edu/aat/300082087> ;
  rdfs:seeAlso wd:Q17118025 ;
  rdfs:subClassOf <https://w3id.org/con-tax/zones/aat-spaces#300004465> ;
.
<https://w3id.org/con-tax/zones/aat-spaces#300082091>
  rdf:type owl:Class ;
  rdfs:comment "Rooms in houses set aside for the care of babies and young children during the night, typically having little furniture beyond bedding for the children, a chair and sometimes a cot or bed for the caretaker, and facilities for washing, bathing, and preparing the infant's bottle or food. Night nurseries were seldom playrooms, however, playrooms and schoolrooms were usually located nearby."@en ;
  rdfs:isDefinedBy <https://w3id.org/con-tax/zones/aat-spaces> ;
  rdfs:label "kinderslaapkamer"@nl ;
  rdfs:label "kinderslaapkamers"@nl ;
  rdfs:label "night nurseries (rooms)"@en ;
  rdfs:seeAlso <http://vocab.getty.edu/aat/300082091> ;
  rdfs:subClassOf <https://w3id.org/con-tax/zones/aat-spaces#300004380> ;
.
<https://w3id.org/con-tax/zones/aat-spaces#300082094>
  rdf:type owl:Class ;
  rdfs:comment "Rooms where servants gather and dine."@en ;
  rdfs:comment "Ruimten waar dienstpersoneel bijeenkomt en eet en drinkt."@nl ;
  rdfs:isDefinedBy <https://w3id.org/con-tax/zones/aat-spaces> ;
  rdfs:label "dienstvertrek"@nl ;
  rdfs:label "dienstvertrekken"@nl ;
  rdfs:label "servants' halls"@en ;
  rdfs:seeAlso <http://vocab.getty.edu/aat/300082094> ;
  rdfs:seeAlso wd:Q7455556 ;
  rdfs:subClassOf <https://w3id.org/con-tax/zones/aat-spaces#300133704> ;
.
<https://w3id.org/con-tax/zones/aat-spaces#300082114>
  rdf:type owl:Class ;
  rdfs:comment "Control centers for on-call nursing staff in health facilities."@en ;
  rdfs:comment "Ruimten voor oproepbaar verplegend personeel in (medische) zorginstellingen."@nl ;
  rdfs:isDefinedBy <https://w3id.org/con-tax/zones/aat-spaces> ;
  rdfs:label "medische wacht"@nl ;
  rdfs:label "medische wachten"@nl ;
  rdfs:label "nurses' stations"@en ;
  rdfs:seeAlso <http://vocab.getty.edu/aat/300082114> ;
  rdfs:subClassOf <https://w3id.org/con-tax/zones/aat-spaces#300004536> ;
.
<https://w3id.org/con-tax/zones/aat-spaces#300082243>
  rdf:type owl:Class ;
  rdfs:comment "Kamers in het Romeinse badhuis of de gymnastiekschool tussen het laconicum, sudatorium en het caldarium, waar atleten zich terugtrokken om het zweet van hun lichamen te verwijderen."@nl ;
  rdfs:comment "Rooms in the Roman bath or gymnasium between the laconicum, sudatorium, or stove, and the caldarium or warm bath where athletes retired to remove sweat from their bodies."@en ;
  rdfs:isDefinedBy <https://w3id.org/con-tax/zones/aat-spaces> ;
  rdfs:label "sudatione"@nl ;
  rdfs:label "sudationes"@en ;
  rdfs:seeAlso <http://vocab.getty.edu/aat/300082243> ;
  rdfs:subClassOf <https://w3id.org/con-tax/zones/aat-spaces#300080054> ;
.
<https://w3id.org/con-tax/zones/aat-spaces#300082254>
  rdf:type owl:Class ;
  rdfs:comment "Rooms or separate structures devoted to funeral services in funeral homes. For chapels intended to permanently contain individual or family tombs, use \"sepulchral chapels.\""@en ;
  rdfs:comment "Ruimten voor rouwdiensten in rouwcentra. Gebruik 'grafkapellen' voor kapellen waarin zich privé- of familiegraftomben bevinden."@nl ;
  rdfs:isDefinedBy <https://w3id.org/con-tax/zones/aat-spaces> ;
  rdfs:label "funeral chapels"@en ;
  rdfs:label "rouwkapel"@nl ;
  rdfs:label "rouwkapellen"@nl ;
  rdfs:seeAlso <http://vocab.getty.edu/aat/300082254> ;
  rdfs:seeAlso wd:Q1466031 ;
  rdfs:subClassOf <https://w3id.org/con-tax/zones/aat-spaces#300004590> ;
.
<https://w3id.org/con-tax/zones/aat-spaces#300082888>
  rdf:type owl:Class ;
  rdfs:comment "Rooms found in large houses and hotels intended for meals that are part of late evening entertainments."@en ;
  rdfs:comment "Ruimten in grote huizen en hotels die zijn bestemd voor maaltijden die deel uitmaken van amusement op de late avond. Zie ook 'eetzalen'."@nl ;
  rdfs:isDefinedBy <https://w3id.org/con-tax/zones/aat-spaces> ;
  rdfs:label "supper room"@nl ;
  rdfs:label "supper rooms"@en ;
  rdfs:label "supper rooms"@nl ;
  rdfs:seeAlso <http://vocab.getty.edu/aat/300082888> ;
  rdfs:subClassOf <https://w3id.org/con-tax/zones/aat-spaces#300133704> ;
.
<https://w3id.org/con-tax/zones/aat-spaces#300082978>
  rdf:type owl:Class ;
  rdfs:comment "Afsluitbare ruimten om waardevolle voorwerpen veilig in te bewaren. Ze zijn gewoonlijk gemaakt van staal."@nl ;
  rdfs:comment "Spaces constructed and used for containing and safekeeping valuables from theft or damage; may be climate controlled."@en ;
  rdfs:isDefinedBy <https://w3id.org/con-tax/zones/aat-spaces> ;
  rdfs:label "kluis"@nl ;
  rdfs:label "kluizen"@nl ;
  rdfs:label "vaults (protective spaces)"@en ;
  rdfs:seeAlso <http://vocab.getty.edu/aat/300082978> ;
  rdfs:subClassOf <https://w3id.org/con-tax/zones/aat-spaces#300103935> ;
.
<https://w3id.org/con-tax/zones/aat-spaces#300083039>
  rdf:type owl:Class ;
  rdfs:comment "Doorgangen tussen de hoger en lager gelegen rijen zitplaatsen in Griekse theaters. Gebruik 'praecinctiones' voor gelijksoortige doorgangen in Romeinse theaters."@nl ;
  rdfs:comment "Passages or aisles in Greek theaters concentric with the outer wall. For similar features in Roman theaters, use \"praecinctiones.\""@en ;
  rdfs:isDefinedBy <https://w3id.org/con-tax/zones/aat-spaces> ;
  rdfs:label "diazoma"@nl ;
  rdfs:label "diazomata"@en ;
  rdfs:label "diazomata"@nl ;
  rdfs:seeAlso <http://vocab.getty.edu/aat/300083039> ;
  rdfs:seeAlso wd:Q11694134 ;
  rdfs:subClassOf <https://w3id.org/con-tax/zones/aat-spaces#300104771> ;
.
<https://w3id.org/con-tax/zones/aat-spaces#300083042>
  rdf:type owl:Class ;
  rdfs:comment "Halfcirkelvormige ruimten vóór de scaena in antieke theaters."@nl ;
  rdfs:comment "The semicircular spaces before the scaena in ancient theaters."@en ;
  rdfs:isDefinedBy <https://w3id.org/con-tax/zones/aat-spaces> ;
  rdfs:label "orchestras (stage spaces)"@en ;
  rdfs:label "orkest (toneelruimte)"@nl ;
  rdfs:label "orkest"@nl ;
  rdfs:label "orkesten (toneelruimten)"@nl ;
  rdfs:label "orkesten"@nl ;
  rdfs:seeAlso <http://vocab.getty.edu/aat/300083042> ;
  rdfs:subClassOf <https://w3id.org/con-tax/zones/aat-spaces#300004677> ;
.
<https://w3id.org/con-tax/zones/aat-spaces#300083076>
  rdf:type owl:Class ;
  rdfs:comment "Spaces between the outer and inner doors to buildings, or for sheltered spaces, recessed in the mass of the building, just outside the outer doors. For spaces just inside the outer door but not separated from the building interior by any barrier such as a door, use \"entrance halls.\""@en ;
  rdfs:comment "Wordt gebruikt voor ruimten tussen de buiten- en binnendeuren van gebouwen, of voor beschutte ruimten aan gebouwen, direct voor de buitendeuren. Gebruik 'hallen' voor ruimten die zich achter de buitendeur bevinden en niet met een binnendeur of andere barrière van de overige ruimten in het gebouw zijn gescheiden."@nl ;
  rdfs:isDefinedBy <https://w3id.org/con-tax/zones/aat-spaces> ;
  rdfs:label "portaal (binnenruimte)"@nl ;
  rdfs:label "portaal"@nl ;
  rdfs:label "portalen (binnenruimte)"@nl ;
  rdfs:label "portalen"@nl ;
  rdfs:label "vestibules"@en ;
  rdfs:label "vestibules"@nl ;
  rdfs:label "voorportalen"@nl ;
  rdfs:seeAlso <http://vocab.getty.edu/aat/300083076> ;
  rdfs:subClassOf <https://w3id.org/con-tax/zones/aat-spaces#300004259> ;
.
<https://w3id.org/con-tax/zones/aat-spaces#300100051>
  rdf:type gvp:GuideTerm ;
  rdfs:isDefinedBy <https://w3id.org/con-tax/zones/aat-spaces> ;
  rdfs:label "<kamers en ruimten naar type gebouw>"@nl ;
  rdfs:label "<rooms and spaces by building type>"@en ;
  rdfs:label "kamers en ruimten naar type gebouw"@nl ;
  rdfs:seeAlso <http://vocab.getty.edu/aat/300100051> ;
  contax:containsConcept <https://w3id.org/con-tax/zones/aat-spaces#300004536> ;
  contax:containsConcept <https://w3id.org/con-tax/zones/aat-spaces#300004559> ;
  contax:containsConcept <https://w3id.org/con-tax/zones/aat-spaces#300004677> ;
  contax:containsConcept <https://w3id.org/con-tax/zones/aat-spaces#300075882> ;
  contax:containsConcept <https://w3id.org/con-tax/zones/aat-spaces#300260522> ;
  contax:containsGuideTerm <https://w3id.org/con-tax/zones/aat-spaces#300069805> ;
.
<https://w3id.org/con-tax/zones/aat-spaces#300100078>
  rdf:type owl:Class ;
  rdfs:comment "Delen van theaters die het toneel en de ruimte erboven omvatten."@nl ;
  rdfs:comment "Parts of theaters holding the stage and the space above it."@en ;
  rdfs:isDefinedBy <https://w3id.org/con-tax/zones/aat-spaces> ;
  rdfs:label "stage houses"@en ;
  rdfs:label "toneelhuis"@nl ;
  rdfs:label "toneelhuizen"@nl ;
  rdfs:label "toneeltoren"@nl ;
  rdfs:label "toneeltorens"@nl ;
  rdfs:seeAlso <http://vocab.getty.edu/aat/300100078> ;
  rdfs:subClassOf <https://w3id.org/con-tax/zones/aat-spaces#300004677> ;
.
<https://w3id.org/con-tax/zones/aat-spaces#300100081>
  rdf:type gvp:GuideTerm ;
  rdf:type skos:OrderedCollection ;
  rdfs:isDefinedBy <https://w3id.org/con-tax/zones/aat-spaces> ;
  rdfs:label "<stages and stage components>"@en ;
  rdfs:label "<toneel en toneelonderdeel>"@nl ;
  rdfs:label "<tonelen en toneelonderdelen>"@nl ;
  rdfs:label "toneel en toneelonderdeel"@nl ;
  rdfs:label "tonelen en toneelonderdelen"@nl ;
  rdfs:seeAlso <http://vocab.getty.edu/aat/300100081> ;
  contax:containsConcept <https://w3id.org/con-tax/zones/aat-spaces#300004751> ;
  contax:containsConcept <https://w3id.org/con-tax/zones/aat-spaces#300100082> ;
.
<https://w3id.org/con-tax/zones/aat-spaces#300100082>
  rdf:type owl:Class ;
  rdfs:comment "Parts or components of stages."@en ;
  rdfs:isDefinedBy <https://w3id.org/con-tax/zones/aat-spaces> ;
  rdfs:label "stage components"@en ;
  rdfs:label "toneelonderdeel"@nl ;
  rdfs:label "toneelonderdelen"@nl ;
  rdfs:seeAlso <http://vocab.getty.edu/aat/300100082> ;
  rdfs:subClassOf <https://w3id.org/con-tax/zones/aat-spaces#300004677> ;
.
<https://w3id.org/con-tax/zones/aat-spaces#300100084>
  rdf:type owl:Class ;
  rdfs:comment "Delen van theaterpodia die dichtst bij het publiek zijn en meestal buiten het gordijn uitsteken. Voor het acteeroppervlak van oude Griekse en Romeinse theaters, gebruik \"proscaeniums\"."@nl ;
  rdfs:comment "Parts of theater stages nearest the audience and usually projecting beyond the curtain. For the acting surfaces of ancient Greek and Roman theaters, use \"proscenia.\""@en ;
  rdfs:isDefinedBy <https://w3id.org/con-tax/zones/aat-spaces> ;
  rdfs:label "forestages"@en ;
  rdfs:label "proscenium"@nl ;
  rdfs:label "prosceniums"@nl ;
  rdfs:label "voortoneel"@nl ;
  rdfs:label "voortonelen"@nl ;
  rdfs:seeAlso <http://vocab.getty.edu/aat/300100084> ;
  rdfs:subClassOf <https://w3id.org/con-tax/zones/aat-spaces#300100082> ;
.
<https://w3id.org/con-tax/zones/aat-spaces#300100093>
  rdf:type owl:Class ;
  rdfs:comment "Open stages that project into the audience."@en ;
  rdfs:comment "Tonelen die zich uitstrekken tot in het publiek."@nl ;
  rdfs:isDefinedBy <https://w3id.org/con-tax/zones/aat-spaces> ;
  rdfs:label "thrust stages"@en ;
  rdfs:label "vooruitspringend podium"@nl ;
  rdfs:label "vooruitspringende podia"@nl ;
  rdfs:seeAlso <http://vocab.getty.edu/aat/300100093> ;
  rdfs:seeAlso wd:Q641553 ;
  rdfs:subClassOf <https://w3id.org/con-tax/zones/aat-spaces#300004751> ;
.
<https://w3id.org/con-tax/zones/aat-spaces#300100100>
  rdf:type owl:Class ;
  rdfs:comment "Ruimten boven het toneel, buiten het zicht van het publiek, die tijdens een voorstelling worden gebruikt om hangende achtergronden op te slaan."@nl ;
  rdfs:comment "The spaces above the stage behind the proscenium, out of view of the audience, used during a performance for the storage of hanging scenery."@en ;
  rdfs:isDefinedBy <https://w3id.org/con-tax/zones/aat-spaces> ;
  rdfs:label "fly lofts"@en ;
  rdfs:label "toneelzolder"@nl ;
  rdfs:label "toneelzolders"@nl ;
  rdfs:seeAlso <http://vocab.getty.edu/aat/300100100> ;
  rdfs:subClassOf <https://w3id.org/con-tax/zones/aat-spaces#300004677> ;
.
<https://w3id.org/con-tax/zones/aat-spaces#300100106>
  rdf:type owl:Class ;
  rdfs:comment "Ruimten direct achter en aan weerszijden van het toneel."@nl ;
  rdfs:comment "The areas offstage and to the side of the acting area."@en ;
  rdfs:isDefinedBy <https://w3id.org/con-tax/zones/aat-spaces> ;
  rdfs:label "coulissenruimte"@nl ;
  rdfs:label "coulissenruimten"@nl ;
  rdfs:label "wings (theater spaces)"@en ;
  rdfs:seeAlso <http://vocab.getty.edu/aat/300100106> ;
  rdfs:subClassOf <https://w3id.org/con-tax/zones/aat-spaces#300004677> ;
.
<https://w3id.org/con-tax/zones/aat-spaces#300100113>
  rdf:type owl:Class ;
  rdfs:comment "Gedeeltelijk onder het toneel liggende ruimten waar het orkest zit bij opera- en balletuitvoeringen."@nl ;
  rdfs:comment "Sunken spaces in front of the forestage from which an orchestra plays."@en ;
  rdfs:isDefinedBy <https://w3id.org/con-tax/zones/aat-spaces> ;
  rdfs:label "orchestra pits"@en ;
  rdfs:label "orkestbak"@nl ;
  rdfs:label "orkestbakken"@nl ;
  rdfs:seeAlso <http://vocab.getty.edu/aat/300100113> ;
  rdfs:seeAlso wd:Q1893407 ;
  rdfs:subClassOf <https://w3id.org/con-tax/zones/aat-spaces#300004677> ;
.
<https://w3id.org/con-tax/zones/aat-spaces#300100118>
  rdf:type owl:Class ;
  rdfs:comment "Off-stage lounges for performers, also serving as a place where they may receive visitors."@en ;
  rdfs:comment "Ruimten achter de schermen voor artiesten, die ook dienen als bezoekruimte."@nl ;
  rdfs:isDefinedBy <https://w3id.org/con-tax/zones/aat-spaces> ;
  rdfs:label "artiestenfoyer"@nl ;
  rdfs:label "artiestenfoyers"@nl ;
  rdfs:label "green rooms"@en ;
  rdfs:seeAlso <http://vocab.getty.edu/aat/300100118> ;
  rdfs:subClassOf <https://w3id.org/con-tax/zones/aat-spaces#300004677> ;
.
<https://w3id.org/con-tax/zones/aat-spaces#300100120>
  rdf:type owl:Class ;
  rdfs:comment "An enclosed seating area within a theater that is either permanently or temporarily reserved for small groups of persons."@en ;
  rdfs:isDefinedBy <https://w3id.org/con-tax/zones/aat-spaces> ;
  rdfs:label "baignoire"@nl ;
  rdfs:label "baignoires"@nl ;
  rdfs:label "boxes (audience spaces)"@en ;
  rdfs:label "loge (toeschouwersruimte)"@nl ;
  rdfs:label "loge"@nl ;
  rdfs:label "loges (toeschouwersruimten)"@nl ;
  rdfs:label "loges"@nl ;
  rdfs:seeAlso <http://vocab.getty.edu/aat/300100120> ;
  rdfs:seeAlso wd:Q1868004 ;
  rdfs:subClassOf <https://w3id.org/con-tax/zones/aat-spaces#300104771> ;
.
<https://w3id.org/con-tax/zones/aat-spaces#300100143>
  rdf:type owl:Class ;
  rdfs:comment "Corridors running along the tops of counterscarps and protected by embankments whose outer slopes form glacis. Continuous path around a fortress, covered by an additional rampart such as a counterscarp or a glacis."@en ;
  rdfs:comment "Gangen die langs de bovenkanten van contrescarpen lopen en die beschermd worden door wallen waarvan de hellingen aan de buitenkant glacis vormen."@nl ;
  rdfs:isDefinedBy <https://w3id.org/con-tax/zones/aat-spaces> ;
  rdfs:label "bedekte weg"@nl ;
  rdfs:label "bedekte wegen"@nl ;
  rdfs:label "covered ways (fortification elements)"@en-us ;
  rdfs:label "gedekte weg"@nl ;
  rdfs:label "gedekte wegen"@nl ;
  rdfs:label "overdekte gang (fortificatie-element)"@nl ;
  rdfs:label "overdekte gang"@nl ;
  rdfs:label "overdekte gangen (fortificatie-elementen)"@nl ;
  rdfs:label "overdekte gangen"@nl ;
  rdfs:seeAlso <http://vocab.getty.edu/aat/300100143> ;
  rdfs:subClassOf <https://w3id.org/con-tax/zones/aat-spaces#300004283> ;
.
<https://w3id.org/con-tax/zones/aat-spaces#300101209>
  rdf:type gvp:GuideTerm ;
  rdf:type skos:OrderedCollection ;
  rdfs:isDefinedBy <https://w3id.org/con-tax/zones/aat-spaces> ;
  rdfs:label "<opper podia en opper podium componenten>"@nl ;
  rdfs:label "<upper stages and upper stage components>"@en ;
  rdfs:label "opper podia en opper podium componenten"@nl ;
  rdfs:seeAlso <http://vocab.getty.edu/aat/300101209> ;
  contax:containsConcept <https://w3id.org/con-tax/zones/aat-spaces#300101210> ;
  contax:containsConcept <https://w3id.org/con-tax/zones/aat-spaces#300101214> ;
.
<https://w3id.org/con-tax/zones/aat-spaces#300101210>
  rdf:type owl:Class ;
  rdfs:comment "Hoger gelegen tonelen in Elizabethaanse en hedendaagse Europese theaters, omvattende chamber en tarrase in Elizabethaanse theaters, hoewel er enige controverse is over hoeveel deze voorkwamen."@nl ;
  rdfs:comment "Refers to the the upper-level stages in Elizabethan and contemporary European theaters, including the chamber and tarrase in Elizabethan theaters, although the extent of its existence is controversial."@en ;
  rdfs:isDefinedBy <https://w3id.org/con-tax/zones/aat-spaces> ;
  rdfs:label "boventoneel"@nl ;
  rdfs:label "boventonelen"@nl ;
  rdfs:label "upper stages"@en ;
  rdfs:seeAlso <http://vocab.getty.edu/aat/300101210> ;
  rdfs:subClassOf <https://w3id.org/con-tax/zones/aat-spaces#300004677> ;
.
<https://w3id.org/con-tax/zones/aat-spaces#300101214>
  rdf:type owl:Class ;
  rdfs:comment "Parts or components of upper stages."@en ;
  rdfs:isDefinedBy <https://w3id.org/con-tax/zones/aat-spaces> ;
  rdfs:label "onderdelen van boventonelen"@nl ;
  rdfs:label "upper stage components"@en ;
  rdfs:seeAlso <http://vocab.getty.edu/aat/300101214> ;
  rdfs:subClassOf <https://w3id.org/con-tax/zones/aat-spaces#300004677> ;
.
<https://w3id.org/con-tax/zones/aat-spaces#300101219>
  rdf:type owl:Class ;
  rdfs:comment "De acteerruimten van upper stages, gelegen voor de chambers van Elizabethaanse theaters."@nl ;
  rdfs:comment "Upper stage acting areas, in front of the chamber, of Elizabethan theaters."@en ;
  rdfs:isDefinedBy <https://w3id.org/con-tax/zones/aat-spaces> ;
  rdfs:label "tarrases"@en ;
  rdfs:label "toneeltribune"@nl ;
  rdfs:label "toneeltribunes"@nl ;
  rdfs:seeAlso <http://vocab.getty.edu/aat/300101219> ;
  rdfs:subClassOf <https://w3id.org/con-tax/zones/aat-spaces#300101214> ;
.
<https://w3id.org/con-tax/zones/aat-spaces#300101235>
  rdf:type owl:Class ;
  rdfs:comment "Delen van theaters achter het toneel, gebruikt als kleed- en opslagruimte, als artiestenfoyer en soms als inner stages."@nl ;
  rdfs:comment "Portions of the theater backstage used as a place for dressing and storage, for a green room, and sometimes for an inner stage."@en ;
  rdfs:isDefinedBy <https://w3id.org/con-tax/zones/aat-spaces> ;
  rdfs:label "ruimte achter de coulissen"@nl ;
  rdfs:label "ruimten achter de coulissen"@nl ;
  rdfs:label "tiring houses"@en ;
  rdfs:seeAlso <http://vocab.getty.edu/aat/300101235> ;
  rdfs:subClassOf <https://w3id.org/con-tax/zones/aat-spaces#300004677> ;
.
<https://w3id.org/con-tax/zones/aat-spaces#300101239>
  rdf:type gvp:GuideTerm ;
  rdf:type skos:OrderedCollection ;
  rdfs:isDefinedBy <https://w3id.org/con-tax/zones/aat-spaces> ;
  rdfs:label "<ruimten achter de coulissen en onderdelen daarvan>"@nl ;
  rdfs:label "<tiring houses and tiring house components>"@en ;
  rdfs:label "ruimten achter de coulissen en onderdelen daarvan"@nl ;
  rdfs:seeAlso <http://vocab.getty.edu/aat/300101239> ;
  contax:containsConcept <https://w3id.org/con-tax/zones/aat-spaces#300101235> ;
  contax:containsConcept <https://w3id.org/con-tax/zones/aat-spaces#300101241> ;
.
<https://w3id.org/con-tax/zones/aat-spaces#300101241>
  rdf:type owl:Class ;
  rdfs:comment "Parts or components of tiring houses."@en ;
  rdfs:isDefinedBy <https://w3id.org/con-tax/zones/aat-spaces> ;
  rdfs:label "onderdelen van ruimten achter de coulissen"@nl ;
  rdfs:label "tiring house components"@en ;
  rdfs:seeAlso <http://vocab.getty.edu/aat/300101241> ;
  rdfs:subClassOf <https://w3id.org/con-tax/zones/aat-spaces#300004677> ;
.
<https://w3id.org/con-tax/zones/aat-spaces#300101242>
  rdf:type owl:Class ;
  rdfs:comment "De bovenste delen van tiring houses in Elizabethaanse theaters, mogelijk gebruikt als muziekgalerijen en voor geluidseffecten."@nl ;
  rdfs:comment "Refers to the upper parts of tiring houses in Elizabethan theaters, possibly used as music galleries and for sound effects."@en ;
  rdfs:isDefinedBy <https://w3id.org/con-tax/zones/aat-spaces> ;
  rdfs:label "turret (theater component)"@nl ;
  rdfs:label "turret"@nl ;
  rdfs:label "turrets (theater components)"@en ;
  rdfs:label "turrets (theater components)"@nl ;
  rdfs:label "turrets"@nl ;
  rdfs:seeAlso <http://vocab.getty.edu/aat/300101242> ;
  rdfs:subClassOf <https://w3id.org/con-tax/zones/aat-spaces#300101241> ;
.
<https://w3id.org/con-tax/zones/aat-spaces#300103849>
  rdf:type owl:Class ;
  rdfs:comment "Apartments in a substandard building having a series of rooms arranged in a line usually with each room forming the corridor to the next."@en ;
  rdfs:comment "Wooneenheden in zeer eenvoudige flatgebouwen, waarbij de kamers achter elkaar liggen, meestal zo dat elke kamer de doorgang naar de volgende kamer vormt. Geen Nederlands equivalent."@nl ;
  rdfs:isDefinedBy <https://w3id.org/con-tax/zones/aat-spaces> ;
  rdfs:label "railroad flat"@nl ;
  rdfs:label "railroad flats"@en ;
  rdfs:label "railroad flats"@nl ;
  rdfs:seeAlso <http://vocab.getty.edu/aat/300103849> ;
  rdfs:seeAlso wd:Q7284086 ;
  rdfs:subClassOf <https://w3id.org/con-tax/zones/aat-spaces#300004064> ;
.
<https://w3id.org/con-tax/zones/aat-spaces#300103851>
  rdf:type owl:Class ;
  rdfs:comment "Apartments provided with only cold running water, often in a building with no central heating."@en ;
  rdfs:comment "Appartementen die slechts zijn voorzien van koud stromend water, vaak in een gebouw zonder centrale verwarming. Geen Nederlands equivalent."@nl ;
  rdfs:isDefinedBy <https://w3id.org/con-tax/zones/aat-spaces> ;
  rdfs:label "coldwater flat"@nl ;
  rdfs:label "coldwater flats"@en-us ;
  rdfs:label "coldwater flats"@nl ;
  rdfs:seeAlso <http://vocab.getty.edu/aat/300103851> ;
  rdfs:subClassOf <https://w3id.org/con-tax/zones/aat-spaces#300004064> ;
.
<https://w3id.org/con-tax/zones/aat-spaces#300103935>
  rdf:type owl:Class ;
  rdfs:comment "Rooms such as shelters, or other spaces specifically for protection from outside forces or elements."@en ;
  rdfs:isDefinedBy <https://w3id.org/con-tax/zones/aat-spaces> ;
  rdfs:label "beschermende ruimten"@nl ;
  rdfs:label "protective spaces"@en ;
  rdfs:seeAlso <http://vocab.getty.edu/aat/300103935> ;
  rdfs:subClassOf <https://w3id.org/con-tax/zones/aat-spaces#300133704> ;
.
<https://w3id.org/con-tax/zones/aat-spaces#300103941>
  rdf:type owl:Class ;
  rdfs:comment "Spaces or rooms used to store equipment. "@en ;
  rdfs:isDefinedBy <https://w3id.org/con-tax/zones/aat-spaces> ;
  rdfs:label "equipment spaces"@en ;
  rdfs:label "installatieruimten"@nl ;
  rdfs:seeAlso <http://vocab.getty.edu/aat/300103941> ;
  rdfs:subClassOf <https://w3id.org/con-tax/zones/aat-spaces#300133704> ;
.
<https://w3id.org/con-tax/zones/aat-spaces#300103967>
  rdf:type owl:Class ;
  rdfs:comment "Sanctuaria in laat-Indische tempels. Kan ook worden gebruikt voor vroeg-Indische tempels als geheel, bevattende het sanctuarium en de daaraan verbonden portieken."@nl ;
  rdfs:comment "The sanctuaries of later Indian temples. The term may also be used for earlier Indian temples as a whole, including sanctuary and attached porches."@en ;
  rdfs:isDefinedBy <https://w3id.org/con-tax/zones/aat-spaces> ;
  rdfs:label "vimana"@nl ;
  rdfs:label "vimana's"@nl ;
  rdfs:label "vimanas"@en ;
  rdfs:seeAlso <http://vocab.getty.edu/aat/300103967> ;
  rdfs:seeAlso wd:Q3559335 ;
  rdfs:subClassOf <https://w3id.org/con-tax/zones/aat-spaces#300004575> ;
.
<https://w3id.org/con-tax/zones/aat-spaces#300104479>
  rdf:type owl:Class ;
  rdfs:comment "Refers to spaces in Christian churches, generally between the altar area or sanctuary and the nave, reserved for choristers. For spaces containing the altar area and the choir, when present, use \"chancels.\" For elevated platforms from which a choir, often composed of laity, sings, use \"choir lofts.\""@en ;
  rdfs:comment "Ruimten in christelijke kerken, doorgaans tussen de altaarruimte of het heiligdom en het schip, gereserveerd voor koorzangers. Voor ruimten die de altaarruimte en het zangkoor, als dat aanwezig is, omvatten wordt 'koren' gebruikt. Voor verhoogde platforms van waar af een koor, vaak bestaand uit leken, zingt wordt 'koorgalerijen' gebruikt."@nl ;
  rdfs:isDefinedBy <https://w3id.org/con-tax/zones/aat-spaces> ;
  rdfs:label "choirs (church spaces)"@en ;
  rdfs:label "zangkoor"@nl ;
  rdfs:label "zangkoren"@nl ;
  rdfs:seeAlso <http://vocab.getty.edu/aat/300104479> ;
  rdfs:seeAlso wd:Q207707 ;
  rdfs:subClassOf <https://w3id.org/con-tax/zones/aat-spaces#300004560> ;
.
<https://w3id.org/con-tax/zones/aat-spaces#300104771>
  rdf:type owl:Class ;
  rdfs:comment "Spaces in theaters used to seat or contain audiences. "@en ;
  rdfs:isDefinedBy <https://w3id.org/con-tax/zones/aat-spaces> ;
  rdfs:label "audience spaces"@en ;
  rdfs:label "toeschouwersruimte"@nl ;
  rdfs:label "toeschouwersruimten"@nl ;
  rdfs:seeAlso <http://vocab.getty.edu/aat/300104771> ;
  rdfs:subClassOf <https://w3id.org/con-tax/zones/aat-spaces#300004677> ;
.
<https://w3id.org/con-tax/zones/aat-spaces#300104772>
  rdf:type gvp:GuideTerm ;
  rdfs:isDefinedBy <https://w3id.org/con-tax/zones/aat-spaces> ;
  rdfs:label "<performance and backstage spaces>"@en ;
  rdfs:label "<ruimte op en achter het toneel>"@nl ;
  rdfs:label "<ruimten op en achter het toneel>"@nl ;
  rdfs:label "ruimte op en achter het toneel"@nl ;
  rdfs:label "ruimten op en achter het toneel"@nl ;
  rdfs:seeAlso <http://vocab.getty.edu/aat/300104772> ;
  contax:containsConcept <https://w3id.org/con-tax/zones/aat-spaces#300083042> ;
  contax:containsConcept <https://w3id.org/con-tax/zones/aat-spaces#300100078> ;
  contax:containsConcept <https://w3id.org/con-tax/zones/aat-spaces#300100100> ;
  contax:containsConcept <https://w3id.org/con-tax/zones/aat-spaces#300100106> ;
  contax:containsConcept <https://w3id.org/con-tax/zones/aat-spaces#300100113> ;
  contax:containsConcept <https://w3id.org/con-tax/zones/aat-spaces#300100118> ;
  contax:containsConcept <https://w3id.org/con-tax/zones/aat-spaces#300252175> ;
  contax:containsGuideTerm <https://w3id.org/con-tax/zones/aat-spaces#300100081> ;
  contax:containsGuideTerm <https://w3id.org/con-tax/zones/aat-spaces#300101209> ;
  contax:containsGuideTerm <https://w3id.org/con-tax/zones/aat-spaces#300101239> ;
.
<https://w3id.org/con-tax/zones/aat-spaces#300105654>
  rdf:type owl:Class ;
  rdfs:comment "Includes both places where automobiles are displayed and entire dealership complexes including the sales-and-service building and surrounding lot."@en ;
  rdfs:comment "Omvat zowel zelfstandige ruimten waar auto's worden getoond als ruimten die onderdeel uitmaken van garages."@nl ;
  rdfs:isDefinedBy <https://w3id.org/con-tax/zones/aat-spaces> ;
  rdfs:label "automobile showrooms"@en ;
  rdfs:label "autoshowroom"@nl ;
  rdfs:label "autoshowrooms"@nl ;
  rdfs:seeAlso <http://vocab.getty.edu/aat/300105654> ;
  rdfs:subClassOf <https://w3id.org/con-tax/zones/aat-spaces#300004331> ;
.
<https://w3id.org/con-tax/zones/aat-spaces#300105709>
  rdf:type owl:Class ;
  rdfs:comment "Spaces in which furniture is arranged to be inspected and sold. These may be designed to resemble domestic or office environments in which the furniture would be used."@en ;
  rdfs:isDefinedBy <https://w3id.org/con-tax/zones/aat-spaces> ;
  rdfs:label "furniture showrooms"@en ;
  rdfs:label "meubeltoonzaal"@nl ;
  rdfs:label "meubeltoonzalen"@nl ;
  rdfs:seeAlso <http://vocab.getty.edu/aat/300105709> ;
  rdfs:subClassOf <https://w3id.org/con-tax/zones/aat-spaces#300004331> ;
.
<https://w3id.org/con-tax/zones/aat-spaces#300111871>
  rdf:type owl:Class ;
  rdfs:comment "Rooms provided for eating meals, particularly at a work place, school, or other such establishment where many people spend the day away from home; the the food is often brought from elsewhere, but prepared food may also be offered for sale."@en ;
  rdfs:comment "Ruimten, vaak in winkels, die zijn gespecialiseerd in lichte maaltijden of snacks, die kant en klaar zijn of snel kunnen worden klaargemaakt."@nl ;
  rdfs:isDefinedBy <https://w3id.org/con-tax/zones/aat-spaces> ;
  rdfs:label "lunchroom"@nl ;
  rdfs:label "lunchrooms"@en ;
  rdfs:label "lunchrooms"@nl ;
  rdfs:seeAlso <http://vocab.getty.edu/aat/300111871> ;
  rdfs:subClassOf <https://w3id.org/con-tax/zones/aat-spaces#300133704> ;
.
<https://w3id.org/con-tax/zones/aat-spaces#300111885>
  rdf:type owl:Class ;
  rdfs:comment "Slides, especially found in apartment blocks or offices, where mail is sent to a main repository. "@en ;
  rdfs:isDefinedBy <https://w3id.org/con-tax/zones/aat-spaces> ;
  rdfs:label "brievenkokers"@nl ;
  rdfs:label "mail chutes"@en ;
  rdfs:label "postkoker"@nl ;
  rdfs:label "postkokers"@nl ;
  rdfs:seeAlso <http://vocab.getty.edu/aat/300111885> ;
  rdfs:subClassOf <https://w3id.org/con-tax/zones/aat-spaces#300004249> ;
.
<https://w3id.org/con-tax/zones/aat-spaces#300112480>
  rdf:type owl:Class ;
  rdfs:comment "Gemetselde en meestal overwelfde graven, vaak ruimer dan gedolven graven, zodat de kelders meerdere overledenen kunnen bevatten, b.v. voor een familiegraf. VWB"@nl ;
  rdfs:comment "Spaces or containers for a casket in a burial site."@en ;
  rdfs:isDefinedBy <https://w3id.org/con-tax/zones/aat-spaces> ;
  rdfs:label "grafkelder"@nl ;
  rdfs:label "grafkelders"@nl ;
  rdfs:label "vaults (tomb spaces)"@en ;
  rdfs:seeAlso <http://vocab.getty.edu/aat/300112480> ;
  rdfs:subClassOf <https://w3id.org/con-tax/zones/aat-spaces#300075882> ;
.
<https://w3id.org/con-tax/zones/aat-spaces#300118515>
  rdf:type owl:Class ;
  rdfs:comment "Refers to the colonnaded forecourts of Early Christian churches."@en ;
  rdfs:comment "Sedert de vroegchristelijke tijd de hoven voor basilieken, omgeven door drie of vier zuilengalerijen, als bij het Romeinse atrium gedekt met naar binnen hellende daken. VWB"@nl ;
  rdfs:isDefinedBy <https://w3id.org/con-tax/zones/aat-spaces> ;
  rdfs:label "atrium (kerkvoorhof)"@nl ;
  rdfs:label "atrium"@nl ;
  rdfs:label "atriums (church courtyards)"@en ;
  rdfs:label "atriums (kerkvoorhoven)"@nl ;
  rdfs:label "atriums"@nl ;
  rdfs:seeAlso <http://vocab.getty.edu/aat/300118515> ;
  rdfs:subClassOf <https://w3id.org/con-tax/zones/aat-spaces#300004104> ;
.
<https://w3id.org/con-tax/zones/aat-spaces#300120309>
  rdf:type owl:Class ;
  rdfs:comment "De verzonken delen van upper stages in Elizabethaanse theaters."@nl ;
  rdfs:comment "Refers to the recessed part of an upper stage in an Elizabethan theater."@en ;
  rdfs:isDefinedBy <https://w3id.org/con-tax/zones/aat-spaces> ;
  rdfs:label "chamber (stage component)"@nl ;
  rdfs:label "chamber"@nl ;
  rdfs:label "chambers (stage components)"@en ;
  rdfs:label "chambers (stage components)"@nl ;
  rdfs:label "chambers"@nl ;
  rdfs:seeAlso <http://vocab.getty.edu/aat/300120309> ;
  rdfs:subClassOf <https://w3id.org/con-tax/zones/aat-spaces#300101214> ;
.
<https://w3id.org/con-tax/zones/aat-spaces#300122189>
  rdf:type owl:Class ;
  rdfs:comment "Instructional areas, or buildings, with equipment for storage and use of audiovisual aids."@en ;
  rdfs:comment "Ruimten voor het bewaren of het gebruik van audiovisuele apparatuur als hulpmiddel voor bij het onderwijs."@nl ;
  rdfs:isDefinedBy <https://w3id.org/con-tax/zones/aat-spaces> ;
  rdfs:label "audiobisueel centrum"@nl ;
  rdfs:label "audiovisual centers (spaces)"@en-us ;
  rdfs:label "audiovisuele centra"@nl ;
  rdfs:seeAlso <http://vocab.getty.edu/aat/300122189> ;
  rdfs:subClassOf <https://w3id.org/con-tax/zones/aat-spaces#300133704> ;
.
<https://w3id.org/con-tax/zones/aat-spaces#300124785>
  rdf:type owl:Class ;
  rdfs:comment "Rooms in banks open to the public for doing business and generally containing the tellers' stations, writing desks, and sometimes also officers' platforms."@en ;
  rdfs:comment "Wordt gebruikt voor ruimten in banken waar het publiek zaken kan doen, en waar zich over het algemeen de kasbediendes, bureaus en soms ook leidinggevende functionarissen bevinden. Geen Nederlands equivalent. Gebruik 'bankgebouwen' en 'kantoren (gebouwen)'."@nl ;
  rdfs:isDefinedBy <https://w3id.org/con-tax/zones/aat-spaces> ;
  rdfs:label "banking room"@nl ;
  rdfs:label "banking rooms"@en ;
  rdfs:label "banking rooms"@nl ;
  rdfs:seeAlso <http://vocab.getty.edu/aat/300124785> ;
  rdfs:subClassOf <https://w3id.org/con-tax/zones/aat-spaces#300133704> ;
.
<https://w3id.org/con-tax/zones/aat-spaces#300125571>
  rdf:type owl:Class ;
  rdfs:comment "Sections of hospitals which which provide care for women during pregnancy and childbirth, as well as care for newborn infants."@en ;
  rdfs:isDefinedBy <https://w3id.org/con-tax/zones/aat-spaces> ;
  rdfs:label "kraamafdeling"@nl ;
  rdfs:label "kraamafdelingen"@nl ;
  rdfs:label "maternity wards"@en ;
  rdfs:seeAlso <http://vocab.getty.edu/aat/300125571> ;
  rdfs:subClassOf <https://w3id.org/con-tax/zones/aat-spaces#300004543> ;
.
<https://w3id.org/con-tax/zones/aat-spaces#300126369>
  rdf:type owl:Class ;
  rdfs:comment "Includes spaces in rooms as well as rooms and buildings where blood or blood plasma is collected, processed, stored, and distributed."@en ;
  rdfs:comment "Ruimten of gebouwen waar mensen bloed afstaan en waar dit wordt verwerkt ten behoeve van de medische zorg."@nl ;
  rdfs:isDefinedBy <https://w3id.org/con-tax/zones/aat-spaces> ;
  rdfs:label "bloedbank"@nl ;
  rdfs:label "bloedbanken"@nl ;
  rdfs:label "blood banks"@en ;
  rdfs:seeAlso <http://vocab.getty.edu/aat/300126369> ;
  rdfs:seeAlso wd:Q763244 ;
  rdfs:subClassOf <https://w3id.org/con-tax/zones/aat-spaces#300004536> ;
.
<https://w3id.org/con-tax/zones/aat-spaces#300127475>
  rdf:type owl:Class ;
  rdfs:comment "Boxlike enclosures having openwork of bars, wires, or the like used to confine or protect its occupant, or to admit light or ventilation. Typically reserved for large or small enclosures of this type used for animals, or for freestanding barred enclosures for humans. For such rooms in prisons, particularly if the room is enclosed within walls and having only a limited area of bars, prefer \"prison cells.\""@en ;
  rdfs:comment "Ruimten afgeschermd met tralies, gebruikt om personen of dieren in op te sluiten, maar ze wel in het zicht te houden."@nl ;
  rdfs:isDefinedBy <https://w3id.org/con-tax/zones/aat-spaces> ;
  rdfs:label "cages (enclosures)"@en ;
  rdfs:label "kooi"@nl ;
  rdfs:label "kooien"@nl ;
  rdfs:seeAlso <http://vocab.getty.edu/aat/300127475> ;
  rdfs:subClassOf <https://w3id.org/con-tax/zones/aat-spaces#300133704> ;
.
<https://w3id.org/con-tax/zones/aat-spaces#300129867>
  rdf:type owl:Class ;
  rdfs:comment "Basins, usually rectangular, in the center of the atrium of Roman houses to receive rainwater from the surrounding roofs."@en ;
  rdfs:comment "Meestal rechthoekige bassins in het midden van het atrium van een Romeins huis, bedoeld om water op te vangen van de omringende daken."@nl ;
  rdfs:isDefinedBy <https://w3id.org/con-tax/zones/aat-spaces> ;
  rdfs:label "impluvia"@en ;
  rdfs:label "impluvia"@nl ;
  rdfs:label "impluvium"@nl ;
  rdfs:seeAlso <http://vocab.getty.edu/aat/300129867> ;
  rdfs:seeAlso wd:Q1117244 ;
  rdfs:subClassOf <https://w3id.org/con-tax/zones/aat-spaces#300004097> ;
.
<https://w3id.org/con-tax/zones/aat-spaces#300132308>
  rdf:type owl:Class ;
  rdfs:comment "Rooms used for the copying of manuscripts before the era of printing."@en ;
  rdfs:comment "Ruimten die werden gebruikt voor het kopiëren van manuscripten in de periode voor de boekdrukkunst."@nl ;
  rdfs:isDefinedBy <https://w3id.org/con-tax/zones/aat-spaces> ;
  rdfs:label "scriptoria"@en ;
  rdfs:label "scriptoria"@nl ;
  rdfs:label "scriptorium"@nl ;
  rdfs:seeAlso <http://vocab.getty.edu/aat/300132308> ;
  rdfs:seeAlso wd:Q655185 ;
  rdfs:subClassOf <https://w3id.org/con-tax/zones/aat-spaces#300133704> ;
.
<https://w3id.org/con-tax/zones/aat-spaces#300133704>
  rdf:type owl:Class ;
  rdfs:comment "Collective term referring to interior areas that are enclosed by walls or defined by other divisions. Always used in the plural. "@en ;
  rdfs:isDefinedBy <https://w3id.org/con-tax/zones/aat-spaces> ;
  rdfs:label "kamers en ruimten"@nl ;
  rdfs:label "rooms and spaces"@en ;
  rdfs:seeAlso <http://vocab.getty.edu/aat/300133704> ;
  rdfs:seeAlso wd:Q180516 ;
  rdfs:subClassOf bot:Space ;
  contax:containsGuideTerm <https://w3id.org/con-tax/zones/aat-spaces#300004011> ;
  contax:containsGuideTerm <https://w3id.org/con-tax/zones/aat-spaces#300004021> ;
  contax:containsGuideTerm <https://w3id.org/con-tax/zones/aat-spaces#300004053> ;
  contax:containsGuideTerm <https://w3id.org/con-tax/zones/aat-spaces#300075770> ;
  contax:containsGuideTerm <https://w3id.org/con-tax/zones/aat-spaces#300082039> ;
  contax:containsGuideTerm <https://w3id.org/con-tax/zones/aat-spaces#300100051> ;
  contax:containsGuideTerm <https://w3id.org/con-tax/zones/aat-spaces#300435625> ;
.
<https://w3id.org/con-tax/zones/aat-spaces#300137347>
  rdf:type owl:Class ;
  rdfs:comment "Rooms or spaces in which bells are hung in a tower; for the entire tower structure, use \"bell towers.\""@en ;
  rdfs:comment "Wordt gebruikt voor ruimten waarin luidklokken zijn opgehangen. Voor de gehele toren wordt 'klokkentorens (luidklokken)' gebruikt en voor de stellages waar de klokken in zijn opgehangen 'klokkenstoelen'."@nl ;
  rdfs:isDefinedBy <https://w3id.org/con-tax/zones/aat-spaces> ;
  rdfs:label "belfries (equipment spaces)"@en ;
  rdfs:label "klokkenzolder"@nl ;
  rdfs:label "klokkenzolders"@nl ;
  rdfs:seeAlso <http://vocab.getty.edu/aat/300137347> ;
  rdfs:subClassOf <https://w3id.org/con-tax/zones/aat-spaces#300103941> ;
.
<https://w3id.org/con-tax/zones/aat-spaces#300138214>
  rdf:type owl:Class ;
  rdfs:comment "Lage verdiepingen boven de zijkapellen en onder de kroonlijst van het middenschip in 16e- en 17e-eeuwse kerken. Ontwikkelden zich tot lange balkons en ook tot een reeks van loges, die op het middenschip uitzien. VWB"@nl ;
  rdfs:comment "Small galleries like the boxes of a theater, often inserted into the choir wall of Baroque churches."@en ;
  rdfs:isDefinedBy <https://w3id.org/con-tax/zones/aat-spaces> ;
  rdfs:label "coretti"@en ;
  rdfs:label "coretti"@nl ;
  rdfs:label "coretto"@nl ;
  rdfs:seeAlso <http://vocab.getty.edu/aat/300138214> ;
  rdfs:subClassOf <https://w3id.org/con-tax/zones/aat-spaces#300004560> ;
.
<https://w3id.org/con-tax/zones/aat-spaces#300162359>
  rdf:type owl:Class ;
  rdfs:comment "Een van de beide 'pastophoria' (nissen), waar de benodigdheden en paramenten voor het misoffer in de vroegchristelijke en Byzantijnse kerk werden klaargezet."@nl ;
  rdfs:comment "Refers to recesses, in effect chapels, used for preparation of the Eucharist by the clergy, and located on the north side of the bema in Greek churches."@en ;
  rdfs:isDefinedBy <https://w3id.org/con-tax/zones/aat-spaces> ;
  rdfs:label "protheses"@en ;
  rdfs:label "prothesis"@nl ;
  rdfs:label "prothesissen"@nl ;
  rdfs:seeAlso <http://vocab.getty.edu/aat/300162359> ;
  rdfs:seeAlso wd:Q3924264 ;
  rdfs:subClassOf <https://w3id.org/con-tax/zones/aat-spaces#300004590> ;
.
<https://w3id.org/con-tax/zones/aat-spaces#300162917>
  rdf:type owl:Class ;
  rdfs:comment "Swimming pools usually found in the palaestra of large bathhouses."@en ;
  rdfs:isDefinedBy <https://w3id.org/con-tax/zones/aat-spaces> ;
  rdfs:label "natatione"@nl ;
  rdfs:label "natationes"@en ;
  rdfs:seeAlso <http://vocab.getty.edu/aat/300162917> ;
  rdfs:subClassOf <https://w3id.org/con-tax/zones/aat-spaces#300080054> ;
.
<https://w3id.org/con-tax/zones/aat-spaces#300179305>
  rdf:type owl:Class ;
  rdfs:comment "Domestic spaces, sometimes windowless, primarily designed or used to hold home entertainment systems as their focus, especially for viewing and listening to prerecorded or computer-based materials, such as videos, music, or games. For domestic spaces designed for high-end audio-video equipment to simulate a theaterlike environment, use \"home theaters.\""@en ;
  rdfs:comment "Ruimten in woonhuizen, soms zonder ramen, voor thuisamusementssystemen, speciaal voor het kijken en luisteren naar vooraf opgenomen materiaal zoals video's, muziek of spelletjes, ook wanneer dit met de computer gebeurt. Voor ruimten die zijn ontworpen voor audio-video apparatuur van zeer hoge kwaliteit, bedoeld om een bioscoop-achtige omgeving te creëren, wordt 'huistheaters' gebruikt."@nl ;
  rdfs:isDefinedBy <https://w3id.org/con-tax/zones/aat-spaces> ;
  rdfs:label "media room"@nl ;
  rdfs:label "media rooms"@en ;
  rdfs:label "media rooms"@nl ;
  rdfs:seeAlso <http://vocab.getty.edu/aat/300179305> ;
  rdfs:subClassOf <https://w3id.org/con-tax/zones/aat-spaces#300133704> ;
.
<https://w3id.org/con-tax/zones/aat-spaces#300179437>
  rdf:type owl:Class ;
  rdfs:comment "Ruimten waar persmensen evenenten kunnen bijwonen, zoals bijvoorbeeld bij sportevenementen en politieke bijeenkomsten, en die meestal zijn uitgerust met communicatiefaciliteiten."@nl ;
  rdfs:comment "The quarters assigned as working space for media personnel, as at sporting events and political conventions, and usually equipped with communications facilities."@en ;
  rdfs:isDefinedBy <https://w3id.org/con-tax/zones/aat-spaces> ;
  rdfs:label "perstribune"@nl ;
  rdfs:label "perstribunes"@nl ;
  rdfs:label "press boxes"@en ;
  rdfs:seeAlso <http://vocab.getty.edu/aat/300179437> ;
  rdfs:seeAlso wd:Q7241635 ;
  rdfs:subClassOf <https://w3id.org/con-tax/zones/aat-spaces#300133704> ;
.
<https://w3id.org/con-tax/zones/aat-spaces#300180734>
  rdf:type owl:Class ;
  rdfs:comment "Werkruimtes in een huis die uitsluitend bestemd zijn voor  werkzaamheden die inkomen opleveren. Voor lees- en schrijfruimtes die worden gebruikt voor de huishoudboekhouding of voor ontspanning wordt 'studeerkamers' gebruikt."@nl ;
  rdfs:comment "Workspaces in the home set aside exclusively for income-producing businesses; for reading and writing spaces used for household accounting or recreational purposes, use \"studies (rooms).\""@en ;
  rdfs:isDefinedBy <https://w3id.org/con-tax/zones/aat-spaces> ;
  rdfs:label "comptoir"@nl ;
  rdfs:label "comptoirs"@nl ;
  rdfs:label "home offices (workspaces)"@en ;
  rdfs:label "kantoor (aan huis)"@nl ;
  rdfs:label "kantoor"@nl ;
  rdfs:label "kantoren (aan huis)"@nl ;
  rdfs:label "kantoren"@nl ;
  rdfs:seeAlso <http://vocab.getty.edu/aat/300180734> ;
  rdfs:subClassOf <https://w3id.org/con-tax/zones/aat-spaces#300004521> ;
.
<https://w3id.org/con-tax/zones/aat-spaces#300185263>
  rdf:type owl:Class ;
  rdfs:comment "Gewoonlijk het binnenste, besloten gedeelte van een Griekse of een Grieks-Romaanse tempel die subkamers omvat zoals de hal, het sanctuarium of de centrale ruimte en de schatkamer. Wordt soms als synoniem gebruikt voor 'naos', maar volgens sommige wetenschappers verwijst deze laatste term uitsluitend naar de centrale ruimte."@nl ;
  rdfs:comment "The interior, enclosed parts of Greek or Greco-Roman temples, usually containing the cult statue of the god and encompassing any sub-chambers within the solid wall, such as the vestibule, sanctuary or central chamber, and treasury. The term was later adopted to mean any of various small interior rooms, such as cells in a convent."@en ;
  rdfs:isDefinedBy <https://w3id.org/con-tax/zones/aat-spaces> ;
  rdfs:label "cella"@nl ;
  rdfs:label "cellae"@en ;
  rdfs:label "cellae"@nl ;
  rdfs:seeAlso <http://vocab.getty.edu/aat/300185263> ;
  rdfs:subClassOf <https://w3id.org/con-tax/zones/aat-spaces#300004651> ;
.
<https://w3id.org/con-tax/zones/aat-spaces#300190936>
  rdf:type owl:Class ;
  rdfs:comment "Rooms or areas equipped with several showerheads or shower stalls for use by a number of people at the same time."@en ;
  rdfs:comment "Wordt gebruikt voor ruimten die zijn uitgerust met meerdere douchekoppen of douchehokjes, die door een aantal mensen tegelijk kunnen worden gebruikt."@nl ;
  rdfs:isDefinedBy <https://w3id.org/con-tax/zones/aat-spaces> ;
  rdfs:label "douchekamer"@nl ;
  rdfs:label "douchekamers"@nl ;
  rdfs:label "doucheruimte"@nl ;
  rdfs:label "doucheruimten"@nl ;
  rdfs:label "shower rooms"@en ;
  rdfs:seeAlso <http://vocab.getty.edu/aat/300190936> ;
  rdfs:subClassOf <https://w3id.org/con-tax/zones/aat-spaces#300133704> ;
.
<https://w3id.org/con-tax/zones/aat-spaces#300192556>
  rdf:type owl:Class ;
  rdfs:comment "Display and study spaces providing artists, especially new, emerging artists, the opportunity to exhibit their works outside the traditional gallery and museum context. These are usually small-scale, independent areas administered by artists for the exhibition of work that is often experimental and outside mainstream art movements."@en ;
  rdfs:comment "Wordt gebruikt voor tentoonstellings- en studieruimten die vooral nieuwe, aankomende kunstenaars de mogelijkheid bieden om hun werk buiten de traditionele galerie- en museumcontext ten toon te kunnen stellen."@nl ;
  rdfs:isDefinedBy <https://w3id.org/con-tax/zones/aat-spaces> ;
  rdfs:label "alternative spaces"@en ;
  rdfs:label "kunstenaarsbroedplaats"@nl ;
  rdfs:label "kunstenaarsbroedplaatsen"@nl ;
  rdfs:seeAlso <http://vocab.getty.edu/aat/300192556> ;
  rdfs:subClassOf <https://w3id.org/con-tax/zones/aat-spaces#300133704> ;
.
<https://w3id.org/con-tax/zones/aat-spaces#300220907>
  rdf:type owl:Class ;
  rdfs:comment "Cages for confining birds."@en ;
  rdfs:comment "Getraliede ruimte om er, in woningen, vogels in te houden."@nl ;
  rdfs:isDefinedBy <https://w3id.org/con-tax/zones/aat-spaces> ;
  rdfs:label "birdcages (animal containers)"@en ;
  rdfs:label "vogelkooi"@nl ;
  rdfs:label "vogelkooien"@nl ;
  rdfs:seeAlso <http://vocab.getty.edu/aat/300220907> ;
  rdfs:subClassOf <https://w3id.org/con-tax/zones/aat-spaces#300127475> ;
.
<https://w3id.org/con-tax/zones/aat-spaces#300235020>
  rdf:type owl:Class ;
  rdfs:comment "Intensive care units designed for newborn infants under the age of one month."@en ;
  rdfs:comment "Intensivecareafdelingen voor couveusebaby's."@nl ;
  rdfs:isDefinedBy <https://w3id.org/con-tax/zones/aat-spaces> ;
  rdfs:label "couveuseafdelingen"@nl ;
  rdfs:label "neonatal intensive care units"@en ;
  rdfs:label "neonatologieafdeling"@nl ;
  rdfs:label "neonatologieafdelingen"@nl ;
  rdfs:seeAlso <http://vocab.getty.edu/aat/300235020> ;
  rdfs:seeAlso wd:Q9008292 ;
  rdfs:subClassOf <https://w3id.org/con-tax/zones/aat-spaces#300004552> ;
.
<https://w3id.org/con-tax/zones/aat-spaces#300240057>
  rdf:type owl:Class ;
  rdfs:comment "Ruimten in musea en andere gebouwen, voor het min of meer permanent tentoonstellen van collecties voorwerpen."@nl ;
  rdfs:comment "Spaces set aside, as in museums, for the display of objects in a collection."@en ;
  rdfs:isDefinedBy <https://w3id.org/con-tax/zones/aat-spaces> ;
  rdfs:label "galleries (display spaces)"@en ;
  rdfs:label "tentoonstellingszaal"@nl ;
  rdfs:label "tentoonstellingszalen"@nl ;
  rdfs:seeAlso <http://vocab.getty.edu/aat/300240057> ;
  rdfs:seeAlso wd:Q15206795 ;
  rdfs:subClassOf <https://w3id.org/con-tax/zones/aat-spaces#300133704> ;
.
<https://w3id.org/con-tax/zones/aat-spaces#300248250>
  rdf:type owl:Class ;
  rdfs:comment "Rooms or spaces from which tickets are sold, as for films, travel, or sporting events."@en ;
  rdfs:comment "Ruimten waar kaartjes worden verkocht, zoals bijvoorbeeld voor films, sportevenementen of openbaar vervoer."@nl ;
  rdfs:isDefinedBy <https://w3id.org/con-tax/zones/aat-spaces> ;
  rdfs:label "plaatskaartenbureau"@nl ;
  rdfs:label "plaatskaartenbureaus"@nl ;
  rdfs:label "ticket offices"@en ;
  rdfs:seeAlso <http://vocab.getty.edu/aat/300248250> ;
  rdfs:subClassOf <https://w3id.org/con-tax/zones/aat-spaces#300004521> ;
.
<https://w3id.org/con-tax/zones/aat-spaces#300248257>
  rdf:type owl:Class ;
  rdfs:comment "Rooms or spaces in theaters where tickets are reserved, sold, and distributed."@en ;
  rdfs:comment "Ruimten in theaters om plaatsen te bespreken."@nl ;
  rdfs:isDefinedBy <https://w3id.org/con-tax/zones/aat-spaces> ;
  rdfs:label "bespreekbureau"@nl ;
  rdfs:label "bespreekbureaus"@nl ;
  rdfs:label "box offices"@en ;
  rdfs:seeAlso <http://vocab.getty.edu/aat/300248257> ;
  rdfs:seeAlso wd:Q877435 ;
  rdfs:subClassOf <https://w3id.org/con-tax/zones/aat-spaces#300004677> ;
  rdfs:subClassOf <https://w3id.org/con-tax/zones/aat-spaces#300248250> ;
.
<https://w3id.org/con-tax/zones/aat-spaces#300248355>
  rdf:type owl:Class ;
  rdfs:comment "Kamers in woonhuizen bedoeld voor tijdelijk gebruik door gasten en doorgaans niet gebruikt door de bewoners zelf."@nl ;
  rdfs:comment "Rooms in dwellings set aside or otherwise intended for temporary use by guests and usually not regularly used by household members."@en ;
  rdfs:isDefinedBy <https://w3id.org/con-tax/zones/aat-spaces> ;
  rdfs:label "gastenkamer"@nl ;
  rdfs:label "gastenkamers"@nl ;
  rdfs:label "guest rooms"@en ;
  rdfs:label "logeerkamer"@nl ;
  rdfs:label "logeerkamers"@nl ;
  rdfs:seeAlso <http://vocab.getty.edu/aat/300248355> ;
  rdfs:subClassOf <https://w3id.org/con-tax/zones/aat-spaces#300004362> ;
.
<https://w3id.org/con-tax/zones/aat-spaces#300248512>
  rdf:type owl:Class ;
  rdfs:comment "Apartments with rooms on three levels.  For buildings comprised of three dwelling units, use either \"triplexes (multiple dwellings)\" or \"three-deckers (dwellings).\""@en ;
  rdfs:comment "Appartementen met kamers op drie verdiepingen. Voor gebouwen bestaand uit drie wooneenheden wordt of 'drie-onder-één-kap' of  'three-deckers (dwellings)' gebruikt."@nl ;
  rdfs:isDefinedBy <https://w3id.org/con-tax/zones/aat-spaces> ;
  rdfs:label "appartement met drie verdiepingen"@nl ;
  rdfs:label "appartementen met drie verdiepingen"@nl ;
  rdfs:label "triplexes (apartments)"@en ;
  rdfs:seeAlso <http://vocab.getty.edu/aat/300248512> ;
  rdfs:subClassOf <https://w3id.org/con-tax/zones/aat-spaces#300004063> ;
.
<https://w3id.org/con-tax/zones/aat-spaces#300248675>
  rdf:type owl:Class ;
  rdfs:comment "Small chapels set above and behind the high altar and usually visible from the nave of some Spanish churches of the 16th to the 18th century."@en ;
  rdfs:comment "Wordt gebruikt voor kleine kapellen die zich boven en achter het hoogaltaar bevinden, en die meestal zichtbaar zijn vanuit het schip; in sommige Spaanse kerken uit de 16e tot de 18e eeuw."@nl ;
  rdfs:isDefinedBy <https://w3id.org/con-tax/zones/aat-spaces> ;
  rdfs:label "camarines"@en ;
  rdfs:label "camarines"@nl ;
  rdfs:label "camarín"@nl ;
  rdfs:seeAlso <http://vocab.getty.edu/aat/300248675> ;
  rdfs:seeAlso wd:Q8256049 ;
  rdfs:subClassOf <https://w3id.org/con-tax/zones/aat-spaces#300004590> ;
.
<https://w3id.org/con-tax/zones/aat-spaces#300249326>
  rdf:type owl:Class ;
  rdfs:comment "Pits or enclosed areas designed for cockfighting."@en ;
  rdfs:comment "Wordt gebruikt voor kuilen of omsloten ruimten voor het houden van hanengevechten."@nl ;
  rdfs:isDefinedBy <https://w3id.org/con-tax/zones/aat-spaces> ;
  rdfs:label "cockpits (recreation spaces)"@en ;
  rdfs:label "hanenmat"@nl ;
  rdfs:label "hanenmatten"@nl ;
  rdfs:seeAlso <http://vocab.getty.edu/aat/300249326> ;
  rdfs:subClassOf <https://w3id.org/con-tax/zones/aat-spaces#300133704> ;
.
<https://w3id.org/con-tax/zones/aat-spaces#300250675>
  rdf:type owl:Class ;
  rdfs:comment "Refers to the principal bedrooms in dwellings, usually the largest and intended for the person or persons who head the household; used especially in American contexts since the 1920s."@en ;
  rdfs:comment "Wordt gebruikt voor de belangrijkste slaapkamers in woningen. Ze zijn meestal het grootst en bedoeld voor de persoon of personen die aan het hoofd van het huishouden staan."@nl ;
  rdfs:isDefinedBy <https://w3id.org/con-tax/zones/aat-spaces> ;
  rdfs:label "master bedrooms"@en ;
  rdfs:label "oudersslaapkamer"@nl ;
  rdfs:label "oudersslaapkamers"@nl ;
  rdfs:seeAlso <http://vocab.getty.edu/aat/300250675> ;
  rdfs:seeAlso wd:Q21550762 ;
  rdfs:subClassOf <https://w3id.org/con-tax/zones/aat-spaces#300004364> ;
.
<https://w3id.org/con-tax/zones/aat-spaces#300250678>
  rdf:type owl:Class ;
  rdfs:comment "Complete self-contained apartment units or extensions to a house created within, or with minor exterior additions to existing single-family homes, usually with their own separate entrances and generally for relatives of the homeowners."@en ;
  rdfs:comment "Zelfstandige wooneenheden, die gebouwd zijn in of aan een bestaande woning. Meestal hebben ze een eigen ingang en over het algemeen zijn ze bedoeld voor familieleden van de huiseigenaren."@nl ;
  rdfs:isDefinedBy <https://w3id.org/con-tax/zones/aat-spaces> ;
  rdfs:label "accessory apartments"@en ;
  rdfs:label "toegevoegd appartement"@nl ;
  rdfs:label "toegevoegde appartementen"@nl ;
  rdfs:seeAlso <http://vocab.getty.edu/aat/300250678> ;
  rdfs:subClassOf <https://w3id.org/con-tax/zones/aat-spaces#300004063> ;
.
<https://w3id.org/con-tax/zones/aat-spaces#300250966>
  rdf:type owl:Class ;
  rdfs:comment "Rooms at the rear of auditoriums or classrooms for the operation of, usually, motion-picture projectors, slide projectors, or spotlights."@en ;
  rdfs:comment "Wordt gebruikt voor ruimten achterin auditoriums, bioscopen of klaslokalen voor de bediening van filmprojectors, diaprojectors of spotlichten."@nl ;
  rdfs:isDefinedBy <https://w3id.org/con-tax/zones/aat-spaces> ;
  rdfs:label "projectiecabine"@nl ;
  rdfs:label "projectiecabines"@nl ;
  rdfs:label "projection booths"@en ;
  rdfs:seeAlso <http://vocab.getty.edu/aat/300250966> ;
  rdfs:subClassOf <https://w3id.org/con-tax/zones/aat-spaces#300004086> ;
  rdfs:subClassOf <https://w3id.org/con-tax/zones/aat-spaces#300004677> ;
  rdfs:subClassOf <https://w3id.org/con-tax/zones/aat-spaces#300103941> ;
.
<https://w3id.org/con-tax/zones/aat-spaces#300251821>
  rdf:type owl:Class ;
  rdfs:comment "Rooms appropriated to the meetings of deliberative, legislative, or judicial bodies; by extension, may also be used for the private rooms of judges."@en ;
  rdfs:comment "Wordt gebruikt voor ruimten voor bijeenkomsten van bestuurlijke, wetgevende of gerechtelijke organen. Daarnaast wordt de Amerikaanse term 'chambers' ook gebruikt voor de privévertrekken van rechters. Gebruik hiervoor in het Nederlands 'raadkamers'."@nl ;
  rdfs:isDefinedBy <https://w3id.org/con-tax/zones/aat-spaces> ;
  rdfs:label "chambers (assembly spaces)"@en ;
  rdfs:label "raadzaal"@nl ;
  rdfs:label "raadzalen"@nl ;
  rdfs:seeAlso <http://vocab.getty.edu/aat/300251821> ;
  rdfs:subClassOf <https://w3id.org/con-tax/zones/aat-spaces#300075881> ;
.
<https://w3id.org/con-tax/zones/aat-spaces#300252175>
  rdf:type owl:Class ;
  rdfs:comment "Theater spaces behind the proscenium arch or behind the back wall of the stage setting, including, for example, workshops, dressing rooms, and storage areas; in arena theaters, often includes spaces behind or under seating areas."@en ;
  rdfs:comment "Theaterruimten buiten het toneel, waar zich werkruimten, kleedkamers en opslagruimten bevinden. In amfitheaters en arenatheaters omvat het vaak ruimten achter of onder de zitruimten."@nl ;
  rdfs:isDefinedBy <https://w3id.org/con-tax/zones/aat-spaces> ;
  rdfs:label "achtertoneelruimte"@nl ;
  rdfs:label "achtertoneelruimten"@nl ;
  rdfs:label "backstageruimte"@nl ;
  rdfs:label "backstageruimten"@nl ;
  rdfs:label "backstages"@en ;
  rdfs:seeAlso <http://vocab.getty.edu/aat/300252175> ;
  rdfs:seeAlso wd:Q18696798 ;
  rdfs:subClassOf <https://w3id.org/con-tax/zones/aat-spaces#300004677> ;
.
<https://w3id.org/con-tax/zones/aat-spaces#300252423>
  rdf:type owl:Class ;
  rdfs:comment "Usually semicircular rooms with steeply rising tiers of seats in which audiences may view such events as lectures or surgery."@en ;
  rdfs:comment "Wordt gebruikt voor ronde of halfronde ruimten met steil oplopende rijen stoelen, waar het publiek bijvoorbeeld lezingen of operaties kan bijwonen."@nl ;
  rdfs:isDefinedBy <https://w3id.org/con-tax/zones/aat-spaces> ;
  rdfs:label "amfitheater (ruimte)"@nl ;
  rdfs:label "amfitheater"@nl ;
  rdfs:label "amfitheaters (ruimten)"@nl ;
  rdfs:label "amfitheaters"@nl ;
  rdfs:label "amphitheaters (rooms)"@en-us ;
  rdfs:seeAlso <http://vocab.getty.edu/aat/300252423> ;
  rdfs:subClassOf <https://w3id.org/con-tax/zones/aat-spaces#300075881> ;
.
<https://w3id.org/con-tax/zones/aat-spaces#300253484>
  rdf:type owl:Class ;
  rdfs:comment "Elaborate narthexlike spaces at the west end of some churches, especially in England and France; in some English churches, often porchlike and used as chapels or vestibules. Use normally restricted to a few examples, notably Durham, Ely, and Lincoln cathedrals, Cluny III, and St. Philibert at Tournous. Generally prefer \"narthexes\" for the entrance porches of early basilican churches and the interior vestibules across the west end of later churches."@en ;
  rdfs:comment "Voorkerken, westelijke voorgebouwen van grote kloosterkerken uit de 10e tot de 12e eeuw. Gebruik 'narthexen' voor de westportalen van vroeg-christelijke basilica's en de westelijke ingangsportalen van latere kerken."@nl ;
  rdfs:isDefinedBy <https://w3id.org/con-tax/zones/aat-spaces> ;
  rdfs:label "galilea"@nl ;
  rdfs:label "galilea's"@nl ;
  rdfs:label "galilees"@en-us ;
  rdfs:seeAlso <http://vocab.getty.edu/aat/300253484> ;
  rdfs:subClassOf <https://w3id.org/con-tax/zones/aat-spaces#300004259> ;
  rdfs:subClassOf <https://w3id.org/con-tax/zones/aat-spaces#300004560> ;
.
<https://w3id.org/con-tax/zones/aat-spaces#300254678>
  rdf:type owl:Class ;
  rdfs:comment "Kleine hokjes, waarin automatisch, na betaling, pasfoto's genomen kunnen worden."@nl ;
  rdfs:comment "Small, automatic picture-taking enclosures; usually requiring automated payment of a small fee to initiate the photographic process."@en ;
  rdfs:isDefinedBy <https://w3id.org/con-tax/zones/aat-spaces> ;
  rdfs:label "fotocabine"@nl ;
  rdfs:label "fotocabines"@nl ;
  rdfs:label "photobooths"@en ;
  rdfs:seeAlso <http://vocab.getty.edu/aat/300254678> ;
  rdfs:subClassOf <https://w3id.org/con-tax/zones/aat-spaces#300004086> ;
.
<https://w3id.org/con-tax/zones/aat-spaces#300255116>
  rdf:type owl:Class ;
  rdfs:comment "Dakverdiepingen van gebouwen, die als woning zijn ingericht. Gebruik 'penthouses' voor luxe appartementen op dakverdiepingen. Gebruik 'zolders' voor afgesloten ruimten onder schuine daken, tussen het dak en het plafond van de bovenste verdieping, vooral in huizen."@nl ;
  rdfs:comment "Large upper-level floor spaces directly below the roof of commercial buildings or warehouses, originally unpartitioned but often modified for secondary use; may also be used for domestic sleeping or storage platforms set close to ceilings or roofs and open to and overlooking a living space below. For enclosed spaces under sloping roofs, between the roof and the ceiling of the uppermost story, especially in houses, use \"attics (interior spaces).\" For substantial interior spaces at the level of an upper story, usually extending the full length or width of rooms, use \"galleries (upper level spaces).\""@en ;
  rdfs:isDefinedBy <https://w3id.org/con-tax/zones/aat-spaces> ;
  rdfs:label "loft (binnenruimte)"@nl ;
  rdfs:label "loft"@nl ;
  rdfs:label "lofts (binnenruimten)"@nl ;
  rdfs:label "lofts (upper level floors)"@en ;
  rdfs:label "lofts"@nl ;
  rdfs:seeAlso <http://vocab.getty.edu/aat/300255116> ;
  rdfs:seeAlso wd:Q620861 ;
  rdfs:subClassOf <https://w3id.org/con-tax/zones/aat-spaces#300078790> ;
.
<https://w3id.org/con-tax/zones/aat-spaces#300255133>
  rdf:type owl:Class ;
  rdfs:comment "Wordt gebruikt voor lage, niet afgewerkte zolderruimten die zich onmiddellijk onder de nokken van daken bevinden."@nl ;
  rdfs:comment "small unfinished attic spaces immediately below roof ridges."@en ;
  rdfs:isDefinedBy <https://w3id.org/con-tax/zones/aat-spaces> ;
  rdfs:label "cocklofts"@en-us ;
  rdfs:label "vliering"@nl ;
  rdfs:label "vlieringen"@nl ;
  rdfs:seeAlso <http://vocab.getty.edu/aat/300255133> ;
  rdfs:subClassOf <https://w3id.org/con-tax/zones/aat-spaces#300004076> ;
.
<https://w3id.org/con-tax/zones/aat-spaces#300255752>
  rdf:type owl:Class ;
  rdfs:comment "Kamers waar de wacht vertoeft."@nl ;
  rdfs:comment "Rooms for the accommodation of guards while on duty."@en ;
  rdfs:isDefinedBy <https://w3id.org/con-tax/zones/aat-spaces> ;
  rdfs:label "guardrooms"@en ;
  rdfs:label "wachtkamer (bewaken)"@nl ;
  rdfs:label "wachtkamer"@nl ;
  rdfs:label "wachtkamers (bewaken)"@nl ;
  rdfs:label "wachtkamers"@nl ;
  rdfs:seeAlso <http://vocab.getty.edu/aat/300255752> ;
  rdfs:subClassOf <https://w3id.org/con-tax/zones/aat-spaces#300133704> ;
.
<https://w3id.org/con-tax/zones/aat-spaces#300255760>
  rdf:type owl:Class ;
  rdfs:comment "Guardrooms in Britain in palaces, abbeys, cathedrals, and Medieval colleges."@en ;
  rdfs:comment "Wachtkamers in Engelse kastelen, abdijen, kathedralen en middeleeuwse universiteiten. Geen Nederlands equivalent."@nl ;
  rdfs:isDefinedBy <https://w3id.org/con-tax/zones/aat-spaces> ;
  rdfs:label "watching chamber"@nl ;
  rdfs:label "watching chambers"@en-us ;
  rdfs:label "watching chambers"@nl ;
  rdfs:seeAlso <http://vocab.getty.edu/aat/300255760> ;
  rdfs:subClassOf <https://w3id.org/con-tax/zones/aat-spaces#300255752> ;
.
<https://w3id.org/con-tax/zones/aat-spaces#300256426>
  rdf:type owl:Class ;
  rdfs:comment "Kamers die specifiek zijn ontworpen of worden gebruikt voor het verwerken van post."@nl ;
  rdfs:comment "Rooms specifically designed or used for the handling of postal activities."@en ;
  rdfs:isDefinedBy <https://w3id.org/con-tax/zones/aat-spaces> ;
  rdfs:label "mailrooms"@en-us ;
  rdfs:label "postkamer"@nl ;
  rdfs:label "postkamers"@nl ;
  rdfs:seeAlso <http://vocab.getty.edu/aat/300256426> ;
  rdfs:subClassOf <https://w3id.org/con-tax/zones/aat-spaces#300133704> ;
.
<https://w3id.org/con-tax/zones/aat-spaces#300259480>
  rdf:type owl:Class ;
  rdfs:comment "Te gebruiken in Griekse kerken om zijkapellen of kleine aangebouwde kerkachtige ruimten te onderscheiden van de kathedraal of hoofdkerk van een klooster."@nl ;
  rdfs:comment "Use in Greek churches to distinguish side chapels, or small added churchlike spaces, from the cathedral or principal church of a monastery."@en ;
  rdfs:isDefinedBy <https://w3id.org/con-tax/zones/aat-spaces> ;
  rdfs:label "parekklesia"@en ;
  rdfs:label "parekklesia"@nl ;
  rdfs:seeAlso <http://vocab.getty.edu/aat/300259480> ;
  rdfs:subClassOf <https://w3id.org/con-tax/zones/aat-spaces#300004590> ;
.
<https://w3id.org/con-tax/zones/aat-spaces#300260516>
  rdf:type owl:Class ;
  rdfs:comment "Enclosed spaces reserved for men of a household."@en ;
  rdfs:isDefinedBy <https://w3id.org/con-tax/zones/aat-spaces> ;
  rdfs:label "mannenverblijven"@nl ;
  rdfs:label "men's quarters"@en ;
  rdfs:seeAlso <http://vocab.getty.edu/aat/300260516> ;
  rdfs:subClassOf <https://w3id.org/con-tax/zones/aat-spaces#300133704> ;
.
<https://w3id.org/con-tax/zones/aat-spaces#300260517>
  rdf:type owl:Class ;
  rdfs:comment "Enclosed spaces reserved for women of a household."@en ;
  rdfs:isDefinedBy <https://w3id.org/con-tax/zones/aat-spaces> ;
  rdfs:label "vrouwenverblijven"@nl ;
  rdfs:label "women's quarters"@en ;
  rdfs:seeAlso <http://vocab.getty.edu/aat/300260517> ;
  rdfs:subClassOf <https://w3id.org/con-tax/zones/aat-spaces#300133704> ;
.
<https://w3id.org/con-tax/zones/aat-spaces#300260518>
  rdf:type owl:Class ;
  rdfs:comment "Portions of Islamic houses reserved for men, and in some countries, also considered the public sectors of houses. For the women's quarters of Islamic houses, use \"harems.\""@en ;
  rdfs:comment "Te gebruiken voor delen van Islamitische huizen die zijn gereserveerd voor mannen, in sommige landen ook de openbare delen van huizen. Voor de vrouwenverblijven in Islamitische huizen, gebruik 'harem'."@nl ;
  rdfs:isDefinedBy <https://w3id.org/con-tax/zones/aat-spaces> ;
  rdfs:label "selamliks"@en ;
  rdfs:label "selamliks"@nl ;
  rdfs:seeAlso <http://vocab.getty.edu/aat/300260518> ;
  rdfs:subClassOf <https://w3id.org/con-tax/zones/aat-spaces#300260516> ;
.
<https://w3id.org/con-tax/zones/aat-spaces#300260522>
  rdf:type owl:Class ;
  rdfs:comment "Rooms and other spaces within buildings that house exhibitions."@en ;
  rdfs:isDefinedBy <https://w3id.org/con-tax/zones/aat-spaces> ;
  rdfs:label "exhibition building spaces"@en ;
  rdfs:label "ruimten in tentoonstellingsgebouwen"@nl ;
  rdfs:seeAlso <http://vocab.getty.edu/aat/300260522> ;
  rdfs:subClassOf <https://w3id.org/con-tax/zones/aat-spaces#300133704> ;
.
<https://w3id.org/con-tax/zones/aat-spaces#300260523>
  rdf:type owl:Class ;
  rdfs:comment "Commercial spaces in museums or separate buildings staffed by museum personnel and selling primarily museum-specific souvenirs and related merchandise, the proceeds of which help to support the operating museum."@en ;
  rdfs:comment "Te gebruiken voor handelsruimten of aparte gebouwen, waar museumpersoneel voornamelijk museumsouvenirs en gerelateerde handelswaar verkoopt. De opbrengst komt ten goede aan het museum."@nl ;
  rdfs:isDefinedBy <https://w3id.org/con-tax/zones/aat-spaces> ;
  rdfs:label "museum shops"@en ;
  rdfs:label "museumwinkels"@nl ;
  rdfs:seeAlso <http://vocab.getty.edu/aat/300260523> ;
  rdfs:subClassOf <https://w3id.org/con-tax/zones/aat-spaces#300260522> ;
.
<https://w3id.org/con-tax/zones/aat-spaces#300260790>
  rdf:type owl:Class ;
  rdfs:comment "Arched or vaulted niches or similar recesses in Roman catacombs; usually meant to hold sarcophagi."@en ;
  rdfs:comment "Te gebruiken voor boogvormige of gewelfde nissen of andere uitsparingen in Romeinse catacomben. Meestal bestemd voor het plaatsen van sarcofagen."@nl ;
  rdfs:isDefinedBy <https://w3id.org/con-tax/zones/aat-spaces> ;
  rdfs:label "arcosolia"@en ;
  rdfs:label "arcosolia"@nl ;
  rdfs:label "arcosolium"@nl ;
  rdfs:seeAlso <http://vocab.getty.edu/aat/300260790> ;
  rdfs:subClassOf <https://w3id.org/con-tax/zones/aat-spaces#300075882> ;
.
<https://w3id.org/con-tax/zones/aat-spaces#300261995>
  rdf:type owl:Class ;
  rdfs:comment "Narrow projections of the stage extending out into the orchestra pit or the audience seating area, used by performers and fashion models."@en ;
  rdfs:comment "Te gebruiken voor smalle podiumdelen die uitsteken tot in de orkestbak of de zaal, gebruikt door uitvoerend kunstenaars en mannequins."@nl ;
  rdfs:isDefinedBy <https://w3id.org/con-tax/zones/aat-spaces> ;
  rdfs:label "plankieren (podiumonderdelen)"@nl ;
  rdfs:label "plankieren"@nl ;
  rdfs:label "runways (stage components)"@en-us ;
  rdfs:seeAlso <http://vocab.getty.edu/aat/300261995> ;
  rdfs:subClassOf <https://w3id.org/con-tax/zones/aat-spaces#300100082> ;
.
<https://w3id.org/con-tax/zones/aat-spaces#300263175>
  rdf:type owl:Class ;
  rdfs:comment "Rooms in a palace or great house, often splendidly decorated and used for official and State entertaining."@en ;
  rdfs:comment "Ruimten in een paleis of een groot huis, vaak weelderig gedecoreerd, die worden gebruikt voor officiële (staats-)ontvangsten."@nl ;
  rdfs:isDefinedBy <https://w3id.org/con-tax/zones/aat-spaces> ;
  rdfs:label "staatsiezaal"@nl ;
  rdfs:label "staatsiezalen"@nl ;
  rdfs:label "staterooms"@en ;
  rdfs:seeAlso <http://vocab.getty.edu/aat/300263175> ;
  rdfs:seeAlso wd:Q1431958 ;
  rdfs:subClassOf <https://w3id.org/con-tax/zones/aat-spaces#300133704> ;
.
<https://w3id.org/con-tax/zones/aat-spaces#300263444>
  rdf:type owl:Class ;
  rdfs:comment "Kamers met collecties van verschillende objecten, meestal fossielen, botanische rariteiten, schelpen en opgezette dieren, evenals kleine kunstwerken zoals medaillons en beeldjes, opgesteld in kabinetten, op de muren en aan het plafond. Rariteitenkabinetten waren in de 16de en 17de eeuw populair in Europa. Ze richtten zich op het vreemde en het ongewone en worden wel gezien als de voorloper van de hedendaagse musea."@nl ;
  rdfs:comment "Rooms designed to house collections of various objects, typically fossils, botanical rarities, shells, taxidermy, horns, tusks, skeletons, minerals, small artworks such as medallions and statuettes, and other items that often had been collected during exploring and trading voyages. Items were typically arranged in cabinets as well as on the walls and ceilings. Popular in 16th- and 17th-century Europe, cabinets of curiosities focused on the strange and unusual, and have been described as the forerunner to the natural history museum and other modern museums."@en ;
  rdfs:isDefinedBy <https://w3id.org/con-tax/zones/aat-spaces> ;
  rdfs:label "cabinets of curiosities (rooms)"@en ;
  rdfs:label "rariteitenkabinet"@nl ;
  rdfs:label "rariteitenkabinetten"@nl ;
  rdfs:label "rariteitenkamers"@nl ;
  rdfs:seeAlso <http://vocab.getty.edu/aat/300263444> ;
  rdfs:subClassOf <https://w3id.org/con-tax/zones/aat-spaces#300078138> ;
.
<https://w3id.org/con-tax/zones/aat-spaces#300263461>
  rdf:type owl:Class ;
  rdfs:comment "Refers to distinctive chambers in temples or churches. In ancient temples, the chambers were the apartments of the \"pastophori,\" who were an order of priests who carried the shrines of the gods in procession. According to tradition, the Temple of Jerusalem also had such chambers, thus the term is applied to apartments that imitate these chambers and are typically located on either side of the bema in ancient churches or modern Greek Orthodox churches."@en ;
  rdfs:comment "Verwijst naar onderscheiden vertrekken in tempels of kerken. In klassieke tempels waren deze vertrekken de verblijven van de 'pastophori', leden van een priesterorde die de relikwieën van de goden meedroegen in processies. Volgens de overlevering had ook de tempel in Jeruzalem zulke vertrekken, reden waarom de term ook verwijst naar ruimten die een nabootsing van deze vertrekken zijn en zich gewoonlijk bevinden aan weerszijden van de bema in klassieke kerken of moderne Grieks-orthodoxe kerken."@nl ;
  rdfs:isDefinedBy <https://w3id.org/con-tax/zones/aat-spaces> ;
  rdfs:label "pastophoria (optische instrumenten)"@nl ;
  rdfs:label "pastophoria"@en ;
  rdfs:label "pastophoria"@nl ;
  rdfs:label "pastophorium (optisch instrument)"@nl ;
  rdfs:label "pastophorium"@nl ;
  rdfs:seeAlso <http://vocab.getty.edu/aat/300263461> ;
  rdfs:seeAlso wd:Q2530842 ;
  rdfs:subClassOf <https://w3id.org/con-tax/zones/aat-spaces#300004559> ;
.
<https://w3id.org/con-tax/zones/aat-spaces#300264257>
  rdf:type owl:Class ;
  rdfs:comment "Typically refers to interior courtyards of mosques."@en ;
  rdfs:comment "Verwijst meestal naar de binnenplaats van een moskee."@nl ;
  rdfs:isDefinedBy <https://w3id.org/con-tax/zones/aat-spaces> ;
  rdfs:label "sahns"@en ;
  rdfs:label "sahns"@nl ;
  rdfs:seeAlso <http://vocab.getty.edu/aat/300264257> ;
  rdfs:subClassOf <https://w3id.org/con-tax/zones/aat-spaces#300004095> ;
.
<https://w3id.org/con-tax/zones/aat-spaces#300265733>
  rdf:type owl:Class ;
  rdfs:comment "Ruimten in een museum waar objecten zijn opgeslagen zolang ze niet worden tentoongesteld."@nl ;
  rdfs:comment "Spaces within a museum where objects are stored when not being exhibited."@en ;
  rdfs:isDefinedBy <https://w3id.org/con-tax/zones/aat-spaces> ;
  rdfs:label "museum storerooms"@en ;
  rdfs:label "museumdepots"@nl ;
  rdfs:seeAlso <http://vocab.getty.edu/aat/300265733> ;
  rdfs:subClassOf <https://w3id.org/con-tax/zones/aat-spaces#300004479> ;
.
<https://w3id.org/con-tax/zones/aat-spaces#300266115>
  rdf:type owl:Class ;
  rdfs:comment "Gemeentelijke gebouwen in bepaalde Engelse steden waar casusdiscussies worden of werden gehouden. Historisch gezien verwees de term naar stadhuizen of vergaderruimten zoals rechtszalen of raadskamers."@nl ;
  rdfs:comment "Municipal buildings in some English towns where moot cases are, or once were, discussed. Historically, the term was used to refer to town halls, or assembly spaces such as courtrooms, or council chambers."@en ;
  rdfs:isDefinedBy <https://w3id.org/con-tax/zones/aat-spaces> ;
  rdfs:label "moot halls"@en ;
  rdfs:label "studentenrechtbanken"@nl ;
  rdfs:seeAlso <http://vocab.getty.edu/aat/300266115> ;
  rdfs:seeAlso wd:Q6908719 ;
  rdfs:subClassOf <https://w3id.org/con-tax/zones/aat-spaces#300075881> ;
.
<https://w3id.org/con-tax/zones/aat-spaces#300266127>
  rdf:type owl:Class ;
  rdfs:comment "Intermediate spaces in North Indian Hindu temples; antechambers or vestibules of the sanctum."@en ;
  rdfs:comment "Tussenruimten in Noord-Indiase hindoetempels; antichambres of vestibules van het heiligdom."@nl ;
  rdfs:isDefinedBy <https://w3id.org/con-tax/zones/aat-spaces> ;
  rdfs:label "antarāla's"@nl ;
  rdfs:label "antarālas"@en ;
  rdfs:seeAlso <http://vocab.getty.edu/aat/300266127> ;
  rdfs:subClassOf <https://w3id.org/con-tax/zones/aat-spaces#300266136> ;
.
<https://w3id.org/con-tax/zones/aat-spaces#300266132>
  rdf:type owl:Class ;
  rdfs:comment "Letterlijk 'baarmoederkamers' of 'embryokamers'. Het binnenste gedeelte, het belangrijkste heiligdom van een hindoetempel, waar het object van aanbidding, een afbeelding of lingam, wordt vereerd."@nl ;
  rdfs:comment "Literally: \"womb-\" or \"embryo chambers.\" The inner, or main sanctum of a Hindu temple where the object of worship; either an image or linga, is venerated."@en ;
  rdfs:isDefinedBy <https://w3id.org/con-tax/zones/aat-spaces> ;
  rdfs:label "garbhagṛha's"@nl ;
  rdfs:label "garbhagṛhas"@en ;
  rdfs:seeAlso <http://vocab.getty.edu/aat/300266132> ;
  rdfs:subClassOf <https://w3id.org/con-tax/zones/aat-spaces#300266136> ;
.
<https://w3id.org/con-tax/zones/aat-spaces#300266136>
  rdf:type owl:Class ;
  rdfs:comment "Spaces or rooms located in Hindu religious buildings. "@en ;
  rdfs:isDefinedBy <https://w3id.org/con-tax/zones/aat-spaces> ;
  rdfs:label "Hindoetempelruimten"@nl ;
  rdfs:label "Hindu temple spaces"@en ;
  rdfs:seeAlso <http://vocab.getty.edu/aat/300266136> ;
  rdfs:seeAlso wd:Q842402 ;
  rdfs:subClassOf <https://w3id.org/con-tax/zones/aat-spaces#300004651> ;
.
<https://w3id.org/con-tax/zones/aat-spaces#300266672>
  rdf:type owl:Class ;
  rdfs:comment "In Japanese architecture, an interior space that may have evolved historically from the private altars of Zen Buddhist monks, used for the display of devotional objects; then later as elevated seating for warriors or dignitaries. The most recent use of  the space in Japanese houses is for the display of flower arrangements and scrolls that set the mood of the tea ceremony, or other art objects."@en ;
  rdfs:comment "In de Japanse architectuur een alkoof. Oorspronkelijk waarschijnlijk bedoeld voor de privéaltaren van zenboeddhistische monniken, een ruimte waar ze hun heilige objecten uitstalden. Later werden ze gebruikt voor de verhoogde zetels van krijgers en hoogwaardigheidsbekleders. Tegenwoordig is de ruimte in Japanse huizen bestemd voor het uitstallen van bloemstukken en versieringen die voor sfeer zorgen tijdens de theeceremonie, of van andere kunstvoorwerpen."@nl ;
  rdfs:isDefinedBy <https://w3id.org/con-tax/zones/aat-spaces> ;
  rdfs:label "tokonoma"@en ;
  rdfs:label "tokonoma"@nl ;
  rdfs:seeAlso <http://vocab.getty.edu/aat/300266672> ;
  rdfs:seeAlso wd:Q738760 ;
  rdfs:subClassOf <https://w3id.org/con-tax/zones/aat-spaces#300004054> ;
.
<https://w3id.org/con-tax/zones/aat-spaces#300266763>
  rdf:type owl:Class ;
  rdfs:comment "Refers generally to a cloakroom; use specifically for large rooms in monasteries or other buildings where garments are kept."@en ;
  rdfs:comment "Verwijst meestal naar een garderobe. Gebruik 'vestiaria' voor grote ruimten in kloosters waar gewaden werden bewaard."@nl ;
  rdfs:isDefinedBy <https://w3id.org/con-tax/zones/aat-spaces> ;
  rdfs:label "vestiaire"@nl ;
  rdfs:label "vestiaires"@nl ;
  rdfs:label "vestiaries"@en ;
  rdfs:seeAlso <http://vocab.getty.edu/aat/300266763> ;
  rdfs:subClassOf <https://w3id.org/con-tax/zones/aat-spaces#300004465> ;
.
<https://w3id.org/con-tax/zones/aat-spaces#300266764>
  rdf:type owl:Class ;
  rdfs:comment "In Christian churches, rooms or separate buildings in which the celebrants, other clergy, and acolytes may dress prior to the mass or other services. The room may also be used for storage of liturgical vestments, sometimes for storage of vessels, and other items, and for meetings. For rooms serving more for the storage of sacred items, use \"sacristies,\" although modern usage of the two terms broadly overlaps."@en ;
  rdfs:comment "Verwijst naar een kamer of apart gebouw waar men liturgische kledingstukken, gebruiksvoorwerpen en andere objecten bewaart en waar geestelijken zich kunnen omkleden. "@nl ;
  rdfs:isDefinedBy <https://w3id.org/con-tax/zones/aat-spaces> ;
  rdfs:label "sacristie"@nl ;
  rdfs:label "sacristieën"@nl ;
  rdfs:label "vestries (dressing rooms)"@en ;
  rdfs:seeAlso <http://vocab.getty.edu/aat/300266764> ;
  rdfs:subClassOf <https://w3id.org/con-tax/zones/aat-spaces#300004465> ;
.
<https://w3id.org/con-tax/zones/aat-spaces#300310624>
  rdf:type owl:Class ;
  rdfs:comment "In de Japanse architectuur een decoratief lessenaarsdak onder het echte dak van een gebouw, bijvoorbeeld een tempel of een ���tahōtō'. Gewoonlijk omgeven ze het hoofdgedeelte van het gebouw. Men gebruikte ze om diepte te creëren. Dit element werd op grote schaal gebruikt in de zenboeddhistische architectuur van de late twaalfde eeuw. "@nl ;
  rdfs:comment "Roofed porch or lean-to pent roofs that extend from a building, especially of a temple hall or of a \"tahōtō.\" They usually surround the main part of the building and were used as a method to increase depth. This architectural element was widely used in Zen-style architecture introduced to Japan in the late 12th century."@en ;
  rdfs:isDefinedBy <https://w3id.org/con-tax/zones/aat-spaces> ;
  rdfs:label "mokoshi"@en ;
  rdfs:label "mokoshi"@nl ;
  rdfs:seeAlso <http://vocab.getty.edu/aat/300310624> ;
  rdfs:seeAlso wd:Q3319398 ;
  rdfs:subClassOf <https://w3id.org/con-tax/zones/aat-spaces#300075459> ;
.
<https://w3id.org/con-tax/zones/aat-spaces#300310677>
  rdf:type owl:Class ;
  rdfs:comment "Cores of buildings, the parts placed directly underneath the main part of the roof; usually an odd number of bays wide and 2 bays deep. Sometimes used to refer specifically to the central part of a Buddhist temple."@en ;
  rdfs:comment "Het binnenste gedeelte van gebouwen dat zich direct onder het hoofdgedeelte van het dak bevindt. Gewoonlijk een oneven aantal vakken breed en twee vakken diep. Soms gebruikt men de term specifiek voor het centrale gedeelte van een boeddhistische tempel."@nl ;
  rdfs:isDefinedBy <https://w3id.org/con-tax/zones/aat-spaces> ;
  rdfs:label "moya"@en ;
  rdfs:label "moya"@nl ;
  rdfs:seeAlso <http://vocab.getty.edu/aat/300310677> ;
  rdfs:subClassOf <https://w3id.org/con-tax/zones/aat-spaces#300078790> ;
.
<https://w3id.org/con-tax/zones/aat-spaces#300310759>
  rdf:type owl:Class ;
  rdfs:comment "Entrance halls or porches through which one enters a Japanese building and is greeted by the host, removes one's shoes, etc. Historically, this term referred only to alcoves found in Zen temple buildings, but now the term is used to refer to any entry alcove. These areas are often decorated with screen paintings."@en ;
  rdfs:comment "Hal of veranda die men passeert bij het binnengaan van een Japans gebouw, waar men wordt begroet door de gastheer of -vrouw en waar men de schoenen kan uitdoen. Vroeger gebruikte men deze term alleen voor alkoven in zenboeddhistische tempels, maar tegenwoordig wordt de term gebruikt voor alle soorten ontvangstruimtes. Ze zijn meestal versierd met schilderingen."@nl ;
  rdfs:isDefinedBy <https://w3id.org/con-tax/zones/aat-spaces> ;
  rdfs:label "genkan"@en ;
  rdfs:label "genkan"@nl ;
  rdfs:seeAlso <http://vocab.getty.edu/aat/300310759> ;
  rdfs:seeAlso wd:Q1207721 ;
  rdfs:subClassOf <https://w3id.org/con-tax/zones/aat-spaces#300004259> ;
.
<https://w3id.org/con-tax/zones/aat-spaces#300311710>
  rdf:type owl:Class ;
  rdfs:comment "Areas where library and archival materials are housed, which are not open to users."@en ;
  rdfs:isDefinedBy <https://w3id.org/con-tax/zones/aat-spaces> ;
  rdfs:label "closed stacks"@en ;
  rdfs:label "gesloten depot"@nl ;
  rdfs:label "gesloten depots"@nl ;
  rdfs:label "gesloten opstelling"@nl ;
  rdfs:label "gesloten opstellingen"@nl ;
  rdfs:seeAlso <http://vocab.getty.edu/aat/300311710> ;
  rdfs:subClassOf <https://w3id.org/con-tax/zones/aat-spaces#300311994> ;
.
<https://w3id.org/con-tax/zones/aat-spaces#300311725>
  rdf:type owl:Class ;
  rdfs:comment "Any type of shelving which is designed to increase the storage capacity of library materials to be shelved in a given space, such as draw-out shelves, mobile ranges, and swinging-case shelves."@en ;
  rdfs:isDefinedBy <https://w3id.org/con-tax/zones/aat-spaces> ;
  rdfs:label "compact planksysteem"@nl ;
  rdfs:label "compact shelving"@en ;
  rdfs:seeAlso <http://vocab.getty.edu/aat/300311725> ;
  rdfs:subClassOf <https://w3id.org/con-tax/zones/aat-spaces#300311980> ;
.
<https://w3id.org/con-tax/zones/aat-spaces#300311980>
  rdf:type owl:Class ;
  rdfs:comment "Opslagruimte of constructie met planken waarop men boeken, dozen of andere zaken neerzet, bijvoorbeeld in bibliotheken, archieven of musea."@nl ;
  rdfs:comment "Storage area or structure containing shelves upon which books, boxes, and other materials are stored, such as in a libary, archives, or museum."@en ;
  rdfs:isDefinedBy <https://w3id.org/con-tax/zones/aat-spaces> ;
  rdfs:label "plankruimte (opslagruimte)"@nl ;
  rdfs:label "plankruimte"@nl ;
  rdfs:label "shelving (storage area)"@en ;
  rdfs:seeAlso <http://vocab.getty.edu/aat/300311980> ;
  rdfs:subClassOf <https://w3id.org/con-tax/zones/aat-spaces#300004465> ;
.
<https://w3id.org/con-tax/zones/aat-spaces#300311994>
  rdf:type owl:Class ;
  rdfs:comment "Areas of shelves in a library."@en ;
  rdfs:isDefinedBy <https://w3id.org/con-tax/zones/aat-spaces> ;
  rdfs:label "stacks (shelves)"@en ;
  rdfs:seeAlso <http://vocab.getty.edu/aat/300311994> ;
  rdfs:subClassOf <https://w3id.org/con-tax/zones/aat-spaces#300311980> ;
.
<https://w3id.org/con-tax/zones/aat-spaces#300312058>
  rdf:type owl:Class ;
  rdfs:comment "Ontvangsthallen in de paleizen van Achaemenidische heersers in Susa en Persepolis met zes rijen van zes zuilen en drie zuilengangen met elk twee rijen van zes zuilen. Deze constructies hebben mogelijk gediend als audiëntiezalen voor het hof van de koning en de ontvangst van bezoekende vazallen en ambassadeurs uit andere landen."@nl ;
  rdfs:comment "Reception halls in the palaces of Achaemenid rulers at Susa and Persepolis distinguished by six rows of six columns and three columned porticos, each with two rows of six columns. These structures may have functioned as audience halls for the king's court and visiting foreign vassals and ambassadors."@en ;
  rdfs:isDefinedBy <https://w3id.org/con-tax/zones/aat-spaces> ;
  rdfs:label "apadana"@nl ;
  rdfs:label "apadana's"@nl ;
  rdfs:label "apadanas"@en ;
  rdfs:seeAlso <http://vocab.getty.edu/aat/300312058> ;
  rdfs:seeAlso wd:Q617256 ;
  rdfs:subClassOf <https://w3id.org/con-tax/zones/aat-spaces#300004420> ;
.
<https://w3id.org/con-tax/zones/aat-spaces#300312091>
  rdf:type owl:Class ;
  rdfs:comment "Vertical shafts in buildings, ships, or dug into the earth to provide access and circulation to lower levels."@en ;
  rdfs:comment "Verticale schachten in gebouwen en schepen of uitgegraven in de grond om toegang te verschaffen tot lagere gedeelten."@nl ;
  rdfs:isDefinedBy <https://w3id.org/con-tax/zones/aat-spaces> ;
  rdfs:label "wellways"@en ;
  rdfs:label "wellways"@nl ;
  rdfs:seeAlso <http://vocab.getty.edu/aat/300312091> ;
  rdfs:subClassOf <https://w3id.org/con-tax/zones/aat-spaces#300004241> ;
.
<https://w3id.org/con-tax/zones/aat-spaces#300312219>
  rdf:type owl:Class ;
  rdfs:comment "Bars or shops where food and beverages are served, and often other provisions may be purchased, particularly such establishments located on a military base, school, factory, or other facility where many people of a particular group congregate."@en ;
  rdfs:comment "Cafés of winkels waar men voedsel en dranken serveert en vaak ook andere levensmiddelen kunnen worden gekocht, met name in militaire bases, scholen, fabrieken of andere gebouwen waarin een groot aantal mensen van een bepaalde groep bijeenkomt."@nl ;
  rdfs:isDefinedBy <https://w3id.org/con-tax/zones/aat-spaces> ;
  rdfs:label "canteens (eating and recreation spaces)"@en ;
  rdfs:label "kantine"@nl ;
  rdfs:label "kantines (eet- en recreatieruimtes)"@nl ;
  rdfs:label "kantines"@nl ;
  rdfs:seeAlso <http://vocab.getty.edu/aat/300312219> ;
  rdfs:subClassOf <https://w3id.org/con-tax/zones/aat-spaces#300133704> ;
.
<https://w3id.org/con-tax/zones/aat-spaces#300312220>
  rdf:type owl:Class ;
  rdfs:comment "Stores selling food, equipment, and other merchandise, and often serving light meals, for people employed in a particular kind of work, such as at a film studio or military installation."@en ;
  rdfs:comment "Winkels waar men voedsel en andere benodigdheden verkoopt en vaak lichte maaltijden serveert aan mensen met een bepaald soort werk, bijvoorbeeld in een filmstudio of een militaire basis."@nl ;
  rdfs:isDefinedBy <https://w3id.org/con-tax/zones/aat-spaces> ;
  rdfs:label "commissaries (store and eating spaces)"@en ;
  rdfs:label "kantine"@nl ;
  rdfs:label "kantines (winkels en eetruimtes)"@nl ;
  rdfs:label "kantines"@nl ;
  rdfs:seeAlso <http://vocab.getty.edu/aat/300312220> ;
  rdfs:subClassOf <https://w3id.org/con-tax/zones/aat-spaces#300133704> ;
.
<https://w3id.org/con-tax/zones/aat-spaces#300312256>
  rdf:type owl:Class ;
  rdfs:comment "Constructies of kamers, vaak onder de grond, die zijn versterkt om bominslagen te weerstaan en die gewoonlijk zijn voorzien van voedsel en andere eerste levensbehoeften. Bedoeld om te worden gebruikt door burgers of militair personeel tijdens vijandelijke bombardementen. "@nl ;
  rdfs:comment "Structures or chambers, often underground, that are reinforced against bombing and typically stocked with food and living essentials, intended to be used by civilians or military personnel in case of enemy bomb attack."@en ;
  rdfs:isDefinedBy <https://w3id.org/con-tax/zones/aat-spaces> ;
  rdfs:label "bomb shelters"@en ;
  rdfs:label "schuilkelder"@nl ;
  rdfs:label "schuilkelders"@nl ;
  rdfs:seeAlso <http://vocab.getty.edu/aat/300312256> ;
  rdfs:subClassOf <https://w3id.org/con-tax/zones/aat-spaces#300103935> ;
.
<https://w3id.org/con-tax/zones/aat-spaces#300312367>
  rdf:type owl:Class ;
  rdfs:comment "Kamers of kasten, gewoonlijk koel van temperatuur, waar men wijn of andere alcoholische dranken opslaat, en ook levensmiddelen zoals boter en kaas."@nl ;
  rdfs:comment "Rooms or closets, usually having a cool temperature, for storage of wine, liquors, and originally also butter and cheeses."@en ;
  rdfs:isDefinedBy <https://w3id.org/con-tax/zones/aat-spaces> ;
  rdfs:label "butteries"@en ;
  rdfs:label "provisiekamer"@nl ;
  rdfs:label "provisiekamers"@nl ;
  rdfs:seeAlso <http://vocab.getty.edu/aat/300312367> ;
  rdfs:subClassOf <https://w3id.org/con-tax/zones/aat-spaces#300004465> ;
.
<https://w3id.org/con-tax/zones/aat-spaces#300343468>
  rdf:type owl:Class ;
  rdfs:comment "Rooms or areas in domestic architecture set aside for the care of babies and young children, distinguished from \"night nurseries,\" which contain only bedding and supplies for nighttime care. Day nurseries typically serve as playrooms and schoolrooms. They are also distinguished from \"day care centers,\" which are public or private facilities for the care of groups of children, while the day nursery is in the children's home."@en ;
  rdfs:comment "Ruimtes waarin men baby's en jonge kinderen verzorgt. Te onderscheiden van nachtverblijven, die alleen bedden en voorzieningen hebben voor nachtverzorging. Dagverblijven dienen gewoonlijk als speel- en onderwijsruimtes. Kinderdagverblijven zijn publieke of particuliere instellingen voor de opvang van kinderen overdag."@nl ;
  rdfs:isDefinedBy <https://w3id.org/con-tax/zones/aat-spaces> ;
  rdfs:label "dagverblijf"@nl ;
  rdfs:label "dagverblijven (kinderopvang)"@nl ;
  rdfs:label "dagverblijven"@nl ;
  rdfs:label "day nurseries (rooms)"@en ;
  rdfs:seeAlso <http://vocab.getty.edu/aat/300343468> ;
  rdfs:subClassOf <https://w3id.org/con-tax/zones/aat-spaces#300004380> ;
.
<https://w3id.org/con-tax/zones/aat-spaces#300374884>
  rdf:type owl:Class ;
  rdfs:comment "Porches, usually attached to residential buildings, that are enclosed with small mesh screening between the columns or pillars, to permit ventilation but bar insects."@en ;
  rdfs:comment "Veranda's, gewoonlijk bij woonhuizen, waarbij horrengaas is gespannen tussen de pilaren, zodat de lucht kan circuleren, maar insecten worden buitengehouden. "@nl ;
  rdfs:isDefinedBy <https://w3id.org/con-tax/zones/aat-spaces> ;
  rdfs:label "screened porches"@en ;
  rdfs:label "veranda met horrengaas"@nl ;
  rdfs:label "veranda's met horrengaas"@nl ;
  rdfs:seeAlso <http://vocab.getty.edu/aat/300374884> ;
  rdfs:subClassOf <https://w3id.org/con-tax/zones/aat-spaces#300004132> ;
.
<https://w3id.org/con-tax/zones/aat-spaces#300375745>
  rdf:type owl:Class ;
  rdfs:comment "Balconies that are flush with or in a recess back from the surface of the exterior wall. They often have walls, sets of columns, or other supports on three sides; distinct from the general design of balconies, which are more typically set out from the surface of the wall."@en ;
  rdfs:comment "Balkons waarvan het uiteinde aan de open kant samenvalt met de buitenmuur en die dus niet uitsteken. Vaak hebben ze aan drie kanten muren, pilaren of andere dragers. Ze verschillen van de meeste andere balkons, die gewoonlijk uitsteken. "@nl ;
  rdfs:isDefinedBy <https://w3id.org/con-tax/zones/aat-spaces> ;
  rdfs:label "inspringend balkon"@nl ;
  rdfs:label "inspringende balkons"@nl ;
  rdfs:label "recessed balconies"@en ;
  rdfs:seeAlso <http://vocab.getty.edu/aat/300375745> ;
  rdfs:subClassOf <https://w3id.org/con-tax/zones/aat-spaces#300002588> ;
.
<https://w3id.org/con-tax/zones/aat-spaces#300379866>
  rdf:type owl:Class ;
  rdfs:comment "A chamber designed to create a vacuum environment by removal of air and gasses with a pump. In conservation science practice, vacuum chambers are used for such purposes as drying, degassing, fumigation, resin impregnation. "@en ;
  rdfs:isDefinedBy <https://w3id.org/con-tax/zones/aat-spaces> ;
  rdfs:label "vacuum chambers"@en ;
  rdfs:seeAlso <http://vocab.getty.edu/aat/300379866> ;
  rdfs:seeAlso wd:Q2301626 ;
  rdfs:subClassOf <https://w3id.org/con-tax/zones/aat-spaces#300133704> ;
.
<https://w3id.org/con-tax/zones/aat-spaces#300380197>
  rdf:type owl:Class ;
  rdfs:comment "A mechanically ventilated appliance to enclose use of spray paint and to confine the escape of spray vapor, exhausting it safely."@en ;
  rdfs:isDefinedBy <https://w3id.org/con-tax/zones/aat-spaces> ;
  rdfs:label "spray booths"@en ;
  rdfs:seeAlso <http://vocab.getty.edu/aat/300380197> ;
  rdfs:subClassOf <https://w3id.org/con-tax/zones/aat-spaces#300004086> ;
.
<https://w3id.org/con-tax/zones/aat-spaces#300380360>
  rdf:type owl:Class ;
  rdfs:comment "Secure, evironmentally-controlled storage spaces for photographic film. "@en ;
  rdfs:isDefinedBy <https://w3id.org/con-tax/zones/aat-spaces> ;
  rdfs:label "film vaults"@en ;
  rdfs:seeAlso <http://vocab.getty.edu/aat/300380360> ;
  rdfs:subClassOf <https://w3id.org/con-tax/zones/aat-spaces#300082978> ;
.
<https://w3id.org/con-tax/zones/aat-spaces#300386040>
  rdf:type owl:Class ;
  rdfs:comment "Libraries in Jain temple spaces."@en ;
  rdfs:isDefinedBy <https://w3id.org/con-tax/zones/aat-spaces> ;
  rdfs:label "bhandārs"@en ;
  rdfs:seeAlso <http://vocab.getty.edu/aat/300386040> ;
  rdfs:subClassOf <https://w3id.org/con-tax/zones/aat-spaces#300133704> ;
.
<https://w3id.org/con-tax/zones/aat-spaces#300386110>
  rdf:type owl:Class ;
  rdfs:comment "Drawing rooms in private houses as distinguished from a 'salon de famille;' designated as a meeting place for guests and found only in houses where the primary drawing room is so large that a more intimate space is required."@en ;
  rdfs:isDefinedBy <https://w3id.org/con-tax/zones/aat-spaces> ;
  rdfs:label "salons de compagnie"@en ;
  rdfs:seeAlso <http://vocab.getty.edu/aat/300386110> ;
  rdfs:subClassOf <https://w3id.org/con-tax/zones/aat-spaces#300004459> ;
.
<https://w3id.org/con-tax/zones/aat-spaces#300386145>
  rdf:type owl:Class ;
  rdfs:comment "In Indian temple architecture, the main shrines representing the residence or sanctum of the deity, sometimes used to describe the temple as a whole."@en ;
  rdfs:isDefinedBy <https://w3id.org/con-tax/zones/aat-spaces> ;
  rdfs:label "deuls"@en ;
  rdfs:seeAlso <http://vocab.getty.edu/aat/300386145> ;
  rdfs:seeAlso wd:Q3024819 ;
  rdfs:subClassOf <https://w3id.org/con-tax/zones/aat-spaces#300266136> ;
.
<https://w3id.org/con-tax/zones/aat-spaces#300386151>
  rdf:type owl:Class ;
  rdfs:comment "Door-like niches on the exterior walls of Hindu temples. These contain figural images, usually of deities."@en ;
  rdfs:isDefinedBy <https://w3id.org/con-tax/zones/aat-spaces> ;
  rdfs:label "devakōṣṭhas"@en ;
  rdfs:seeAlso <http://vocab.getty.edu/aat/300386151> ;
  rdfs:subClassOf <https://w3id.org/con-tax/zones/aat-spaces#300266136> ;
.
<https://w3id.org/con-tax/zones/aat-spaces#300391366>
  rdf:type owl:Class ;
  rdfs:comment "An open, single-story hall often seen in gardens, generally built at minor scenic spots."@en ;
  rdfs:isDefinedBy <https://w3id.org/con-tax/zones/aat-spaces> ;
  rdfs:label "xuan"@en ;
  rdfs:seeAlso <http://vocab.getty.edu/aat/300391366> ;
  rdfs:subClassOf <https://w3id.org/con-tax/zones/aat-spaces#300004420> ;
.
<https://w3id.org/con-tax/zones/aat-spaces#300391370>
  rdf:type owl:Class ;
  rdfs:comment "Grand reception halls. In gardens, tang are generally located in  central, public areas."@en ;
  rdfs:isDefinedBy <https://w3id.org/con-tax/zones/aat-spaces> ;
  rdfs:label "tang (halls)"@en ;
  rdfs:seeAlso <http://vocab.getty.edu/aat/300391370> ;
  rdfs:subClassOf <https://w3id.org/con-tax/zones/aat-spaces#300004420> ;
.
<https://w3id.org/con-tax/zones/aat-spaces#300400626>
  rdf:type owl:Class ;
  rdfs:comment "Graftombe ingebed in de muur van een religieus gebouw zoals een kerk of op een kerkhof."@nl ;
  rdfs:comment "Tombs embedded into the walls of religious buildings such as churches or cemeteries."@en ;
  rdfs:isDefinedBy <https://w3id.org/con-tax/zones/aat-spaces> ;
  rdfs:label "burial niches"@en ;
  rdfs:label "grafnis"@nl ;
  rdfs:label "grafnissen"@nl ;
  rdfs:seeAlso <http://vocab.getty.edu/aat/300400626> ;
  rdfs:subClassOf <https://w3id.org/con-tax/zones/aat-spaces#300075882> ;
.
<https://w3id.org/con-tax/zones/aat-spaces#300400638>
  rdf:type owl:Class ;
  rdfs:comment "Ancient Greek dining halls where important guests and visitors were invited to take a sacred meal."@en ;
  rdfs:comment "Oud-Griekse eetzaal waar belangrijke gasten en vreemdelingen ontboden werden om deel te nemen aan gewijde maaltijden."@nl ;
  rdfs:isDefinedBy <https://w3id.org/con-tax/zones/aat-spaces> ;
  rdfs:label "hestiatoria"@en ;
  rdfs:label "hestiatoria"@nl ;
  rdfs:label "hestiatorion"@nl ;
  rdfs:seeAlso <http://vocab.getty.edu/aat/300400638> ;
  rdfs:subClassOf <https://w3id.org/con-tax/zones/aat-spaces#300004349> ;
.
<https://w3id.org/con-tax/zones/aat-spaces#300400669>
  rdf:type owl:Class ;
  rdfs:comment "Heilige plaats waar men priesters of priesteressen kon raadplegen die over profetische gaven beschikten en boodschappen van de god(en) konden overbrengen."@nl ;
  rdfs:comment "Sacred places where one could consult priests or priestesses who had the prophetic gift to transfer messages from the gods."@en ;
  rdfs:isDefinedBy <https://w3id.org/con-tax/zones/aat-spaces> ;
  rdfs:label "oracular sanctuaries"@en ;
  rdfs:label "orakelheiligdom"@nl ;
  rdfs:label "orakelheiligdommen"@nl ;
  rdfs:seeAlso <http://vocab.getty.edu/aat/300400669> ;
  rdfs:subClassOf <https://w3id.org/con-tax/zones/aat-spaces#300004575> ;
.
<https://w3id.org/con-tax/zones/aat-spaces#300403946>
  rdf:type owl:Class ;
  rdfs:comment "Chapels or other room-like spaces, or small freestanding structures, adjacent to or near the tomb in a funerary site. Examples date from ancient Egypt, where offering niches developed over time into rooms, where families of the dead could visit on appropriate days of the year, to eat meals or make offerings in accordance with Egyptian funerary cults. For chapels that hold the remains of the dead, use \"sepulchral chapels.\""@en ;
  rdfs:isDefinedBy <https://w3id.org/con-tax/zones/aat-spaces> ;
  rdfs:label "tomb chapels"@en ;
  rdfs:seeAlso <http://vocab.getty.edu/aat/300403946> ;
  rdfs:subClassOf <https://w3id.org/con-tax/zones/aat-spaces#300004590> ;
.
<https://w3id.org/con-tax/zones/aat-spaces#300403955>
  rdf:type owl:Class ;
  rdfs:comment "Apartments that offer all the amenities of a normal domestic apartment but in radically reduced size. These have open space for sleeping, working, cooking, and eating. These are typically part of housing projects that are six stories high with 40 units each."@en ;
  rdfs:isDefinedBy <https://w3id.org/con-tax/zones/aat-spaces> ;
  rdfs:label "micro-units"@en ;
  rdfs:seeAlso <http://vocab.getty.edu/aat/300403955> ;
  rdfs:subClassOf <https://w3id.org/con-tax/zones/aat-spaces#300004063> ;
.
<https://w3id.org/con-tax/zones/aat-spaces#300404372>
  rdf:type owl:Class ;
  rdfs:comment "Structures that are largely open and designed to provide shade, typically comprising four posts with a roof; may be roughly roofed with brush or branches or may have tent-like canvas or roofing of another material. The structure may be temporary or more permanent. For similar small, decorative structures in gardens, prefer \"gazebos\" or \"pergolas.\""@en ;
  rdfs:isDefinedBy <https://w3id.org/con-tax/zones/aat-spaces> ;
  rdfs:label "ramadas"@en ;
  rdfs:seeAlso <http://vocab.getty.edu/aat/300404372> ;
  rdfs:subClassOf <https://w3id.org/con-tax/zones/aat-spaces#300075459> ;
.
<https://w3id.org/con-tax/zones/aat-spaces#300404896>
  rdf:type owl:Class ;
  rdfs:comment """Binnenruimten, meestal in woningen, die zo zijn ontworpen dat ze de zon binnenlaten door grote vensters. Gebruik ‘solariums' voor oude zonneveranda's of moderne zonnelounges in ziekenhuizen.
"""@nl ;
  rdfs:comment "Interior spaces, usually in dwellings, designed to allow entry of sunshine through large windows. For ancient sunporches or modern sun lounges in hospitals, use “solariums (building spaces).”"@en ;
  rdfs:isDefinedBy <https://w3id.org/con-tax/zones/aat-spaces> ;
  rdfs:label "sun rooms"@en ;
  rdfs:label "zonnekamer"@nl ;
  rdfs:label "zonnekamers"@nl ;
  rdfs:seeAlso <http://vocab.getty.edu/aat/300404896> ;
  rdfs:subClassOf <https://w3id.org/con-tax/zones/aat-spaces#300078790> ;
.
<https://w3id.org/con-tax/zones/aat-spaces#300404897>
  rdf:type owl:Class ;
  rdfs:comment "Sun rooms, usually located at the back of a dwelling, equipped with a bar or other furnishings to allow preparation of beverages and entertaining of guests. Traditionally, Florida rooms have tile floors."@en ;
  rdfs:comment """Zonnekamers, meestal aan de achterkant van een woning, uitgerust met een bar of andere elementen om drankjes te bereiden en gasten te onderhouden. Traditioneel hebben deze kamers tegelvloeren.
"""@nl ;
  rdfs:isDefinedBy <https://w3id.org/con-tax/zones/aat-spaces> ;
  rdfs:label "Florida rooms"@en ;
  rdfs:label "Floridakamers"@nl ;
  rdfs:seeAlso <http://vocab.getty.edu/aat/300404897> ;
  rdfs:subClassOf <https://w3id.org/con-tax/zones/aat-spaces#300404896> ;
.
<https://w3id.org/con-tax/zones/aat-spaces#300410329>
  rdf:type owl:Class ;
  rdfs:comment "Aisles that flank the length of the naves of religious or secular buildings, and that are often lower and smaller than the central aisle."@en ;
  rdfs:comment """Ruimten aan weerszijden van het schip van een religieus of seculier gebouw, die vaak lager en kleiner zijn dan het middenschip.
"""@nl ;
  rdfs:isDefinedBy <https://w3id.org/con-tax/zones/aat-spaces> ;
  rdfs:label "side aisles"@en ;
  rdfs:label "zijbeuk"@nl ;
  rdfs:label "zijbeuken"@nl ;
  rdfs:seeAlso <http://vocab.getty.edu/aat/300410329> ;
  rdfs:subClassOf <https://w3id.org/con-tax/zones/aat-spaces#300004284> ;
.
<https://w3id.org/con-tax/zones/aat-spaces#300410332>
  rdf:type owl:Class ;
  rdfs:comment "Circulation spaces that run the center length of religious or secular buildings that have oblong plans. Central aisles often bisect rows of pews or seating."@en ;
  rdfs:comment """Ruimten in het midden, in de lengterichting, van religieuze of seculiere gebouwen met een langwerpige indeling. Middenschepen verdelen vaak rijen stoelen in twee gedeelten
"""@nl ;
  rdfs:isDefinedBy <https://w3id.org/con-tax/zones/aat-spaces> ;
  rdfs:label "central aisles"@en ;
  rdfs:label "middenschepen"@nl ;
  rdfs:label "middenschip"@nl ;
  rdfs:seeAlso <http://vocab.getty.edu/aat/300410332> ;
  rdfs:subClassOf <https://w3id.org/con-tax/zones/aat-spaces#300004284> ;
.
<https://w3id.org/con-tax/zones/aat-spaces#300411346>
  rdf:type owl:Class ;
  rdfs:comment "Rooms for pedagogical use that do not conform to a typical school instruction structure. Use 'classrooms' for similar rooms that are located in schools."@en ;
  rdfs:comment "Ruimten waar les gegeven wordt. Gebruik voor dergelijke ruimten in scholen 'klaslokalen'."@nl ;
  rdfs:isDefinedBy <https://w3id.org/con-tax/zones/aat-spaces> ;
  rdfs:label "instructieruimte"@nl ;
  rdfs:label "instructieruimten"@nl ;
  rdfs:label "instruction rooms"@en ;
  rdfs:label "leslokaal"@nl ;
  rdfs:label "leslokalen"@nl ;
  rdfs:seeAlso <http://vocab.getty.edu/aat/300411346> ;
  rdfs:subClassOf <https://w3id.org/con-tax/zones/aat-spaces#300133704> ;
.
<https://w3id.org/con-tax/zones/aat-spaces#300411377>
  rdf:type owl:Class ;
  rdfs:comment "Instelling of afdeling, gewijd aan prent- en tekenkunst."@nl ;
  rdfs:comment "Rooms or larger areas devoted to the storage or display of fine art prints."@en ;
  rdfs:isDefinedBy <https://w3id.org/con-tax/zones/aat-spaces> ;
  rdfs:label "prentenkabinet"@nl ;
  rdfs:label "prentenkabinetten"@nl ;
  rdfs:label "print rooms"@en ;
  rdfs:seeAlso <http://vocab.getty.edu/aat/300411377> ;
  rdfs:subClassOf <https://w3id.org/con-tax/zones/aat-spaces#300004465> ;
  rdfs:subClassOf <https://w3id.org/con-tax/zones/aat-spaces#300240057> ;
.
<https://w3id.org/con-tax/zones/aat-spaces#300411381>
  rdf:type owl:Class ;
  rdfs:comment "Cellars that are accessible from wharves."@en ;
  rdfs:comment "Kelders die toegankelijk zijn vanaf een werf."@nl ;
  rdfs:isDefinedBy <https://w3id.org/con-tax/zones/aat-spaces> ;
  rdfs:label "werfkelder"@nl ;
  rdfs:label "werfkelders"@nl ;
  rdfs:label "wharf cellars"@en ;
  rdfs:seeAlso <http://vocab.getty.edu/aat/300411381> ;
  rdfs:subClassOf <https://w3id.org/con-tax/zones/aat-spaces#300004759> ;
.
<https://w3id.org/con-tax/zones/aat-spaces#300411419>
  rdf:type owl:Class ;
  rdfs:comment "Rooms or spaces on boats or in factories where machinery is housed."@en ;
  rdfs:comment "Ruimten in boten of fabrieken waar de machines zijn opgesteld."@nl ;
  rdfs:isDefinedBy <https://w3id.org/con-tax/zones/aat-spaces> ;
  rdfs:label "engine rooms"@en ;
  rdfs:label "machinekamer"@nl ;
  rdfs:label "machinekamers"@nl ;
  rdfs:label "turbinekamer"@nl ;
  rdfs:label "turbinekamers"@nl ;
  rdfs:seeAlso <http://vocab.getty.edu/aat/300411419> ;
  rdfs:subClassOf <https://w3id.org/con-tax/zones/aat-spaces#300103941> ;
.
<https://w3id.org/con-tax/zones/aat-spaces#300411421>
  rdf:type owl:Class ;
  rdfs:comment "Kapellen in of van kloosters."@nl ;
  rdfs:comment "Rooms or buildings for worship: oratories, that are attached to places of residence for a community living under religious vows."@en ;
  rdfs:isDefinedBy <https://w3id.org/con-tax/zones/aat-spaces> ;
  rdfs:label "kloosterkapel"@nl ;
  rdfs:label "kloosterkapellen"@nl ;
  rdfs:label "monastery chapels"@en ;
  rdfs:seeAlso <http://vocab.getty.edu/aat/300411421> ;
  rdfs:subClassOf <https://w3id.org/con-tax/zones/aat-spaces#300004590> ;
.
<https://w3id.org/con-tax/zones/aat-spaces#300411468>
  rdf:type owl:Class ;
  rdfs:comment "Kamers die enkele treden hoger liggen dan het voorhuis of dan de andere vertrekken op dezelfde verdieping. Bijvoorbeeld in stadshuizen of boerderijen."@nl ;
  rdfs:comment "Rooms that are a few steps higher than the front of the house or from the other rooms on the same floor. The original form is typically Dutch, seen in the Netherlands, Belgium, and in locations where the Dutch colonized."@en ;
  rdfs:isDefinedBy <https://w3id.org/con-tax/zones/aat-spaces> ;
  rdfs:label "opkamer"@nl ;
  rdfs:label "opkamers"@en ;
  rdfs:label "opkamers"@nl ;
  rdfs:seeAlso <http://vocab.getty.edu/aat/300411468> ;
  rdfs:subClassOf <https://w3id.org/con-tax/zones/aat-spaces#300078790> ;
.
<https://w3id.org/con-tax/zones/aat-spaces#300411482>
  rdf:type owl:Class ;
  rdfs:comment "Kapel terzijde van een kerkschip of koor."@nl ;
  rdfs:comment "Subsidiary chapels opening off the nave or side aisles of basilican churches. For chapels opening off the apse, prefer \"apse chapels.\""@en ;
  rdfs:isDefinedBy <https://w3id.org/con-tax/zones/aat-spaces> ;
  rdfs:label "schipkapel"@nl ;
  rdfs:label "schipkapellen"@nl ;
  rdfs:label "side chapels"@en ;
  rdfs:label "zijkapel"@nl ;
  rdfs:label "zijkapellen"@nl ;
  rdfs:seeAlso <http://vocab.getty.edu/aat/300411482> ;
  rdfs:subClassOf <https://w3id.org/con-tax/zones/aat-spaces#300004590> ;
.
<https://w3id.org/con-tax/zones/aat-spaces#300411496>
  rdf:type owl:Class ;
  rdfs:comment "Een hoefstal of travalje is een stellage of een open stal, die een hoefsmid gebruikt om paarden of ezels te beslaan."@nl ;
  rdfs:comment "Scaffolds, frames, or open sheds in which restive horses or donkeys are secured while being shod."@en ;
  rdfs:isDefinedBy <https://w3id.org/con-tax/zones/aat-spaces> ;
  rdfs:label "hoefstal"@nl ;
  rdfs:label "hoefstallen"@nl ;
  rdfs:label "travalje"@nl ;
  rdfs:label "travaljes"@nl ;
  rdfs:label "traves"@en ;
  rdfs:seeAlso <http://vocab.getty.edu/aat/300411496> ;
  rdfs:subClassOf <https://w3id.org/con-tax/zones/aat-spaces#300133704> ;
.
<https://w3id.org/con-tax/zones/aat-spaces#300411499>
  rdf:type owl:Class ;
  rdfs:comment "Entrance spaces of historic Dutch houses or farms that provide a transition from the exterior to the interior of a house. Most span the entire front width of a house, and serve as both a reception point and connection between the street, entry, stairs, and private inner rooms."@en ;
  rdfs:comment "Voorste gedeelte van historische woningen of boerderijen, namelijk de leefvertrekken waarin men van buitenaf dadelijk binnentreedt."@nl ;
  rdfs:isDefinedBy <https://w3id.org/con-tax/zones/aat-spaces> ;
  rdfs:label "voorhuis"@nl ;
  rdfs:label "voorhuises"@en ;
  rdfs:label "voorhuizen"@nl ;
  rdfs:seeAlso <http://vocab.getty.edu/aat/300411499> ;
  rdfs:subClassOf <https://w3id.org/con-tax/zones/aat-spaces#300004259> ;
.
<https://w3id.org/con-tax/zones/aat-spaces#300417303>
  rdf:type owl:Class ;
  rdfs:comment "Relatively small rooms in jails or prisons, used to confine one or more inmates; may be enclosed with bars or otherwise fortified against escape."@en ;
  rdfs:isDefinedBy <https://w3id.org/con-tax/zones/aat-spaces> ;
  rdfs:label "prison cells"@en ;
  rdfs:seeAlso <http://vocab.getty.edu/aat/300417303> ;
  rdfs:subClassOf <https://w3id.org/con-tax/zones/aat-spaces#300004026> ;
.
<https://w3id.org/con-tax/zones/aat-spaces#300417347>
  rdf:type owl:Class ;
  rdfs:comment "Subsidiary chapels opening off the apse of churches. For chapels opening off the nave or side aisles, prefer \"side chapels.\""@en ;
  rdfs:isDefinedBy <https://w3id.org/con-tax/zones/aat-spaces> ;
  rdfs:label "apse chapels"@en ;
  rdfs:seeAlso <http://vocab.getty.edu/aat/300417347> ;
  rdfs:subClassOf <https://w3id.org/con-tax/zones/aat-spaces#300004590> ;
.
<https://w3id.org/con-tax/zones/aat-spaces#300417348>
  rdf:type owl:Class ;
  rdfs:comment "Subsidiary chapels opening off the center of the apse of churches, on an axis down the center of the plan. "@en ;
  rdfs:isDefinedBy <https://w3id.org/con-tax/zones/aat-spaces> ;
  rdfs:label "axial chapels"@en ;
  rdfs:seeAlso <http://vocab.getty.edu/aat/300417348> ;
  rdfs:subClassOf <https://w3id.org/con-tax/zones/aat-spaces#300004590> ;
.
<https://w3id.org/con-tax/zones/aat-spaces#300417349>
  rdf:type owl:Class ;
  rdfs:comment "Subsidiary chapels opening off the transept of a cruciform-plan church. "@en ;
  rdfs:isDefinedBy <https://w3id.org/con-tax/zones/aat-spaces> ;
  rdfs:label "transept chapels"@en ;
  rdfs:seeAlso <http://vocab.getty.edu/aat/300417349> ;
  rdfs:subClassOf <https://w3id.org/con-tax/zones/aat-spaces#300004590> ;
.
<https://w3id.org/con-tax/zones/aat-spaces#300417350>
  rdf:type owl:Class ;
  rdfs:comment "Subsidiary chapels opening off the rounded apse of a church, having a footprint resembling petals or rays extending from the rounded apse."@en ;
  rdfs:isDefinedBy <https://w3id.org/con-tax/zones/aat-spaces> ;
  rdfs:label "radiating chapels"@en ;
  rdfs:seeAlso <http://vocab.getty.edu/aat/300417350> ;
  rdfs:subClassOf <https://w3id.org/con-tax/zones/aat-spaces#300004590> ;
.
<https://w3id.org/con-tax/zones/aat-spaces#300417374>
  rdf:type owl:Class ;
  rdfs:comment "Burial chambers, chapels, or oratories within tomb spaces such as catacombs or crypts attached to churches."@en ;
  rdfs:isDefinedBy <https://w3id.org/con-tax/zones/aat-spaces> ;
  rdfs:label "cubicula (tomb spaces)"@en ;
  rdfs:seeAlso <http://vocab.getty.edu/aat/300417374> ;
  rdfs:subClassOf <https://w3id.org/con-tax/zones/aat-spaces#300075882> ;
.
<https://w3id.org/con-tax/zones/aat-spaces#300419400>
  rdf:type owl:Class ;
  rdfs:comment "Rooms made specially secure for the custody of people or things."@en ;
  rdfs:isDefinedBy <https://w3id.org/con-tax/zones/aat-spaces> ;
  rdfs:label "strong rooms"@en ;
  rdfs:seeAlso <http://vocab.getty.edu/aat/300419400> ;
  rdfs:subClassOf <https://w3id.org/con-tax/zones/aat-spaces#300103935> ;
.
<https://w3id.org/con-tax/zones/aat-spaces#300419401>
  rdf:type owl:Class ;
  rdfs:comment "Rooms, usually above ground, intended for the protection of people from danger, such as from storms or violence. For below ground spaces for protection from tornadoes and other wind events, use \"storm cellars.\""@en ;
  rdfs:isDefinedBy <https://w3id.org/con-tax/zones/aat-spaces> ;
  rdfs:label "safe rooms"@en ;
  rdfs:seeAlso <http://vocab.getty.edu/aat/300419401> ;
  rdfs:subClassOf <https://w3id.org/con-tax/zones/aat-spaces#300103935> ;
.
<https://w3id.org/con-tax/zones/aat-spaces#300419455>
  rdf:type owl:Class ;
  rdfs:comment "Spaces where carved stone works or fragments of works of archaeological interest are displayed or stored. Lapidaria are usually part of larger museums dedicated to historical or archaeological objects, and may contain architectural elements, reliefs, sarcophagi, statues, etc."@en ;
  rdfs:isDefinedBy <https://w3id.org/con-tax/zones/aat-spaces> ;
  rdfs:label "lapidaria"@en ;
  rdfs:seeAlso <http://vocab.getty.edu/aat/300419455> ;
  rdfs:subClassOf <https://w3id.org/con-tax/zones/aat-spaces#300133704> ;
.
<https://w3id.org/con-tax/zones/aat-spaces#300420294>
  rdf:type owl:Class ;
  rdfs:isDefinedBy <https://w3id.org/con-tax/zones/aat-spaces> ;
  rdfs:label "architectural spaces"@en ;
  rdfs:seeAlso <http://vocab.getty.edu/aat/300420294> ;
  rdfs:subClassOf <https://w3id.org/con-tax/zones/aat-spaces#300133704> ;
.
<https://w3id.org/con-tax/zones/aat-spaces#300432333>
  rdf:type owl:Class ;
  rdfs:comment "Small enclosures or structures, often temporary, used for casting votes."@en ;
  rdfs:isDefinedBy <https://w3id.org/con-tax/zones/aat-spaces> ;
  rdfs:label "voting booths"@en ;
  rdfs:seeAlso <http://vocab.getty.edu/aat/300432333> ;
  rdfs:subClassOf <https://w3id.org/con-tax/zones/aat-spaces#300004086> ;
.
<https://w3id.org/con-tax/zones/aat-spaces#300432409>
  rdf:type owl:Class ;
  rdfs:comment "Booths, stalls, rooms, houses, or small buildings for the retail sale of merchandise or services. Originally referred to spaces where the goods were made or prepared for sale and also sold."@en ;
  rdfs:isDefinedBy <https://w3id.org/con-tax/zones/aat-spaces> ;
  rdfs:label "shops (retail spaces)"@en ;
  rdfs:seeAlso <http://vocab.getty.edu/aat/300432409> ;
  rdfs:subClassOf <https://w3id.org/con-tax/zones/aat-spaces#300133704> ;
.
<https://w3id.org/con-tax/zones/aat-spaces#300435625>
  rdf:type gvp:GuideTerm ;
  rdfs:isDefinedBy <https://w3id.org/con-tax/zones/aat-spaces> ;
  rdfs:label "<temporary alphabetical list: rooms and spaces>"@en ;
  rdfs:seeAlso <http://vocab.getty.edu/aat/300435625> ;
  contax:containsConcept <https://w3id.org/con-tax/zones/aat-spaces#300420294> ;
.
<https://w3id.org/con-tax/zones/aat-spaces#300438707>
  rdf:type owl:Class ;
  rdfs:comment "Rooms or sheds for the storage of ale and wine. For rooms for storing wine that are fully or partially below ground, use \"wine cellars.\""@en ;
  rdfs:isDefinedBy <https://w3id.org/con-tax/zones/aat-spaces> ;
  rdfs:label "pitcher houses"@en ;
  rdfs:seeAlso <http://vocab.getty.edu/aat/300438707> ;
  rdfs:subClassOf <https://w3id.org/con-tax/zones/aat-spaces#300004465> ;
.
<https://w3id.org/con-tax/zones/aat-spaces#300438708>
  rdf:type owl:Class ;
  rdfs:comment "Rooms or structures for storing and safekeeping bottles or barrels of wine; often climate-controlled."@en ;
  rdfs:isDefinedBy <https://w3id.org/con-tax/zones/aat-spaces> ;
  rdfs:label "wine vaults"@en ;
  rdfs:seeAlso <http://vocab.getty.edu/aat/300438708> ;
  rdfs:subClassOf <https://w3id.org/con-tax/zones/aat-spaces#300004465> ;
.
